<?xml version="1.0"?>
<rdf:RDF xmlns="https://w3id.org/demeter/crossDomain#"
     xml:base="https://w3id.org/demeter/crossDomain"
     xmlns:owl="http://www.w3.org/2002/07/owl#"
     xmlns:rdf="http://www.w3.org/1999/02/22-rdf-syntax-ns#"
     xmlns:xml="http://www.w3.org/XML/1998/namespace"
     xmlns:xsd="http://www.w3.org/2001/XMLSchema#"
     xmlns:foaf="http://xmlns.com/foaf/0.1/"
     xmlns:rdfs="http://www.w3.org/2000/01/rdf-schema#"
     xmlns:skos="http://www.w3.org/2004/02/skos/core#"
     xmlns:terms="http://purl.org/dc/terms/"
     xmlns:schema="https://schema.org/">
    <owl:Ontology rdf:about="https://w3id.org/demeter/crossDomain">
        <owl:versionIRI rdf:resource="https://w3id.org/demeter/crossDomain/1.0"/>
        <terms:contributor rdf:resource="_:genid-nodeid-node1grirlduix3"/>
        <terms:contributor rdf:resource="_:genid-nodeid-node1grirlduix5"/>
        <terms:contributor rdf:nodeID="genid1"/>
        <terms:contributor rdf:nodeID="genid3"/>
        <terms:contributor rdf:nodeID="genid5"/>
        <terms:creator rdf:nodeID="genid7"/>
        <terms:description xml:lang="en">The DEMETER cross domain ontology i) defines concepts and terms that are generic and applicable to various domains; ii) avoids conflicting or redundant definitions of the same concept in different domain specific models; iii) provides the basis for interoperability. The ontology is specified by reusing concepts and terms from a number of standard ontologies and vocabularies including OGC/W3C SOSA/SSN, OGC GeoSparql, W3C RDF data cube, QUDT, FOAF, schema.org and others. It includes alignment to ISO standards and with DEMETER core meta-model (NGSI-LD).</terms:description>
        <terms:rights xml:lang="en">This vocabulary is distributed under Creative Commons Attribution 4.0 License - http://creativecommons.org/licenses/by/4.0</terms:rights>
        <terms:title xml:lang="en">DEMETER Cross-Domain</terms:title>
        <rdfs:comment xml:lang="en">The DEMETER Agriculture Information Model (AIM) is the common vocabulary in DEMETER project providing the basis for semantic interoperability across smart farming solutions</rdfs:comment>
        <rdfs:label xml:lang="en">DEMETER Cross Domain</rdfs:label>
        <owl:versionInfo>1.0</owl:versionInfo>
        <foaf:maker rdf:nodeID="genid9"/>
    </owl:Ontology>
    <rdf:Description rdf:nodeID="genid1">
        <foaf:name>Ioanna Roussaki</foaf:name>
        <schema:affiliation>
            <rdf:Description>
                <foaf:name>ICCS</foaf:name>
            </rdf:Description>
        </schema:affiliation>
    </rdf:Description>
    <rdf:Description rdf:nodeID="genid3">
        <rdfs:seeAlso rdf:resource="http://orcid.org/0000-0003-4289-4922"/>
        <foaf:name>Raul Palma</foaf:name>
        <schema:affiliation>
            <rdf:Description>
                <foaf:name>PSNC</foaf:name>
            </rdf:Description>
        </schema:affiliation>
    </rdf:Description>
    <rdf:Description rdf:nodeID="genid5">
        <foaf:name>Rob Atkinson</foaf:name>
        <schema:affiliation>
            <rdf:Description>
                <foaf:name>OGC</foaf:name>
            </rdf:Description>
        </schema:affiliation>
    </rdf:Description>
    <rdf:Description rdf:nodeID="genid7">
        <foaf:name>Till DÃ¶hmen</foaf:name>
        <schema:affiliation>
            <rdf:Description>
                <foaf:name>Fraunhofer FIT</foaf:name>
            </rdf:Description>
        </schema:affiliation>
    </rdf:Description>
    <rdf:Description rdf:nodeID="genid9">
        <foaf:homepage rdf:resource="https://h2020-demeter.eu/"/>
        <foaf:name>DEMETER project</foaf:name>
    </rdf:Description>
    


    <!-- 
    ///////////////////////////////////////////////////////////////////////////////////////
    //
    // Annotation properties
    //
    ///////////////////////////////////////////////////////////////////////////////////////
     -->


    


    <!-- http://purl.org/dc/terms/contributor -->


    <owl:AnnotationProperty rdf:about="http://purl.org/dc/terms/contributor"/>
    


    <!-- http://purl.org/dc/terms/creator -->


    <owl:AnnotationProperty rdf:about="http://purl.org/dc/terms/creator"/>
    


    <!-- http://purl.org/dc/terms/date -->


    <owl:AnnotationProperty rdf:about="http://purl.org/dc/terms/date">
        <rdfs:comment>A date associated with an event in the life cycle of the resource</rdfs:comment>
        <rdfs:isDefinedBy rdf:resource="http://purl.org/dc/terms/"/>
        <rdfs:label>Date</rdfs:label>
    </owl:AnnotationProperty>
    


    <!-- http://purl.org/dc/terms/description -->


    <owl:AnnotationProperty rdf:about="http://purl.org/dc/terms/description"/>
    


    <!-- http://purl.org/dc/terms/identifier -->


    <owl:AnnotationProperty rdf:about="http://purl.org/dc/terms/identifier">
        <rdfs:comment>An unambiguous reference to the resource within a given context</rdfs:comment>
        <rdfs:isDefinedBy rdf:resource="http://purl.org/dc/terms/"/>
        <rdfs:label>Resource Identifier</rdfs:label>
    </owl:AnnotationProperty>
    


    <!-- http://purl.org/dc/terms/rights -->


    <owl:AnnotationProperty rdf:about="http://purl.org/dc/terms/rights"/>
    


    <!-- http://purl.org/dc/terms/title -->


    <owl:AnnotationProperty rdf:about="http://purl.org/dc/terms/title"/>
    


    <!-- http://www.w3.org/2004/02/skos/core#definition -->


    <owl:AnnotationProperty rdf:about="http://www.w3.org/2004/02/skos/core#definition">
        <rdfs:comment>A statement or formal explanation of the meaning of a concept</rdfs:comment>
        <rdfs:isDefinedBy rdf:resource="http://www.w3.org/2004/02/skos/core"/>
        <rdfs:label>definition</rdfs:label>
    </owl:AnnotationProperty>
    


    <!-- http://www.w3.org/2004/02/skos/core#editorialNote -->


    <owl:AnnotationProperty rdf:about="http://www.w3.org/2004/02/skos/core#editorialNote"/>
    


    <!-- http://www.w3.org/2004/02/skos/core#example -->


    <owl:AnnotationProperty rdf:about="http://www.w3.org/2004/02/skos/core#example">
        <rdfs:comment>An example of the use of a concept</rdfs:comment>
        <rdfs:isDefinedBy rdf:resource="http://www.w3.org/2004/02/skos/core"/>
        <rdfs:label>example</rdfs:label>
    </owl:AnnotationProperty>
    


    <!-- http://www.w3.org/2004/02/skos/core#inScheme -->


    <owl:AnnotationProperty rdf:about="http://www.w3.org/2004/02/skos/core#inScheme">
        <rdfs:comment>Relates a resource (for example a concept) to a concept scheme in which it is included</rdfs:comment>
        <rdfs:isDefinedBy rdf:resource="http://www.w3.org/2004/02/skos/core"/>
        <rdfs:label>is in scheme</rdfs:label>
    </owl:AnnotationProperty>
    


    <!-- http://www.w3.org/2004/02/skos/core#note -->


    <owl:AnnotationProperty rdf:about="http://www.w3.org/2004/02/skos/core#note"/>
    


    <!-- http://www.w3.org/2004/02/skos/core#prefLabel -->


    <owl:AnnotationProperty rdf:about="http://www.w3.org/2004/02/skos/core#prefLabel">
        <rdfs:comment>The preferred lexical label for a resource, in a given language</rdfs:comment>
        <rdfs:isDefinedBy rdf:resource="http://www.w3.org/2004/02/skos/core"/>
        <rdfs:label>preferred label</rdfs:label>
    </owl:AnnotationProperty>
    


    <!-- http://xmlns.com/foaf/0.1/depiction -->


    <owl:AnnotationProperty rdf:about="http://xmlns.com/foaf/0.1/depiction">
        <rdfs:comment>A depiction of some thing</rdfs:comment>
        <rdfs:isDefinedBy rdf:resource="http://xmlns.com/foaf/0.1/"/>
        <rdfs:label>depiction</rdfs:label>
    </owl:AnnotationProperty>
    


    <!-- http://xmlns.com/foaf/0.1/homepage -->


    <owl:AnnotationProperty rdf:about="http://xmlns.com/foaf/0.1/homepage">
        <rdfs:comment>A homepage for some thing</rdfs:comment>
        <rdfs:isDefinedBy rdf:resource="http://xmlns.com/foaf/0.1/"/>
        <rdfs:label>homepage</rdfs:label>
    </owl:AnnotationProperty>
    


    <!-- http://xmlns.com/foaf/0.1/maker -->


    <owl:AnnotationProperty rdf:about="http://xmlns.com/foaf/0.1/maker"/>
    


    <!-- http://xmlns.com/foaf/0.1/name -->


    <owl:AnnotationProperty rdf:about="http://xmlns.com/foaf/0.1/name">
        <rdfs:comment>A name for some thing</rdfs:comment>
        <rdfs:isDefinedBy rdf:resource="http://xmlns.com/foaf/0.1/"/>
        <rdfs:label>name</rdfs:label>
    </owl:AnnotationProperty>
    


    <!-- https://schema.org/affiliation -->


    <owl:AnnotationProperty rdf:about="https://schema.org/affiliation">
        <rdfs:comment xml:lang="en">An organization that this person is affiliated with. For example, a school/university, a club, or a team.</rdfs:comment>
        <rdfs:isDefinedBy rdf:resource="http://schema.org/Person"/>
        <rdfs:label xml:lang="en">Affiliation</rdfs:label>
    </owl:AnnotationProperty>
    


    <!-- https://schema.org/domainIncludes -->


    <owl:AnnotationProperty rdf:about="https://schema.org/domainIncludes">
        <rdfs:comment xml:lang="en">Relates a property to a class that is (one of) the type(s) the property is expected to be used on.</rdfs:comment>
        <rdfs:isDefinedBy rdf:resource="http://schema.org/Property"/>
        <rdfs:label xml:lang="en">Domain Includes</rdfs:label>
    </owl:AnnotationProperty>
    


    <!-- https://schema.org/rangeIncludes -->


    <owl:AnnotationProperty rdf:about="https://schema.org/rangeIncludes">
        <rdfs:comment xml:lang="en">Relates a property to a class that constitutes (one of) the expected type(s) for values of the property.</rdfs:comment>
        <rdfs:isDefinedBy rdf:resource="http://schema.org/Property"/>
        <rdfs:label xml:lang="en">Range Includes</rdfs:label>
    </owl:AnnotationProperty>
    


    <!-- 
    ///////////////////////////////////////////////////////////////////////////////////////
    //
    // Datatypes
    //
    ///////////////////////////////////////////////////////////////////////////////////////
     -->


    


    <!-- http://www.opengis.net/ont/geosparql#wktLiteral -->


    <rdfs:Datatype rdf:about="http://www.opengis.net/ont/geosparql#wktLiteral">
        <rdfs:comment xml:lang="en">A Well-known Text serialization of a geometry object.</rdfs:comment>
        <rdfs:isDefinedBy rdf:resource="http://www.opengis.net/ont/geosparql"/>
        <rdfs:isDefinedBy rdf:resource="http://www.opengis.net/spec/geosparql/1.0"/>
        <rdfs:label xml:lang="en">Well-known Text Literal</rdfs:label>
    </rdfs:Datatype>
    


    <!-- http://www.w3.org/2001/XMLSchema#date -->


    <rdfs:Datatype rdf:about="http://www.w3.org/2001/XMLSchema#date"/>
    


    <!-- 
    ///////////////////////////////////////////////////////////////////////////////////////
    //
    // Object Properties
    //
    ///////////////////////////////////////////////////////////////////////////////////////
     -->


    


    <!-- http://def.isotc211.org/iso19156/2011/SamplingFeature#SF_SamplingFeature.sampledFeature -->


    <owl:ObjectProperty rdf:about="http://def.isotc211.org/iso19156/2011/SamplingFeature#SF_SamplingFeature.sampledFeature">
        <rdfs:domain rdf:resource="http://def.isotc211.org/iso19156/2011/SamplingFeature#SF_SamplingFeature"/>
        <rdfs:range rdf:resource="http://def.isotc211.org/iso19156/2011/GeneralFeatureInstance#GFI_DomainFeature"/>
        <rdfs:range rdf:resource="http://def.isotc211.org/iso19156/2011/GeneralFeatureInstance#GFI_Feature"/>
        <rdfs:isDefinedBy rdf:resource="http://standards.iso.org/iso/19156/ed-1/en/"/>
        <rdfs:label>sampledFeature</rdfs:label>
    </owl:ObjectProperty>
    


    <!-- http://purl.oclc.org/NET/ssnx/qu/qu#unitKind -->


    <owl:ObjectProperty rdf:about="http://purl.oclc.org/NET/ssnx/qu/qu#unitKind">
        <owl:equivalentProperty rdf:resource="http://qudt.org/schema/qudt/unit"/>
        <rdfs:range rdf:resource="http://purl.oclc.org/NET/ssnx/qu/qu#Unit"/>
        <rdfs:comment>Being the qu:unitKind of something, implies being something that is a qu:Unit</rdfs:comment>
        <rdfs:isDefinedBy rdf:resource="https://www.w3.org/2005/Incubator/ssn/ssnx/qu/qu"/>
        <rdfs:label>unitKind</rdfs:label>
    </owl:ObjectProperty>
    


    <!-- http://purl.org/linked-data/cube#component -->


    <owl:ObjectProperty rdf:about="http://purl.org/linked-data/cube#component">
        <rdfs:domain rdf:resource="http://purl.org/linked-data/cube#DataStructureDefinition"/>
        <rdfs:range rdf:resource="http://purl.org/linked-data/cube#ComponentSpecification"/>
        <rdfs:comment xml:lang="en">indicates a component specification which is included in the structure of the dataset</rdfs:comment>
        <rdfs:isDefinedBy rdf:resource="http://purl.org/linked-data/cube"/>
        <rdfs:label xml:lang="en">component specification</rdfs:label>
    </owl:ObjectProperty>
    


    <!-- http://purl.org/linked-data/cube#componentAttachment -->


    <owl:ObjectProperty rdf:about="http://purl.org/linked-data/cube#componentAttachment">
        <rdfs:domain rdf:resource="http://purl.org/linked-data/cube#ComponentSpecification"/>
        <rdfs:range rdf:resource="http://www.w3.org/2000/01/rdf-schema#Class"/>
        <rdfs:comment xml:lang="en">Indicates the level at which the component property should be attached, this might an qb:DataSet, qb:Slice or qb:Observation, or a qb:MeasureProperty.</rdfs:comment>
        <rdfs:isDefinedBy rdf:resource="http://purl.org/linked-data/cube"/>
        <rdfs:label xml:lang="en">component attachment</rdfs:label>
    </owl:ObjectProperty>
    


    <!-- http://purl.org/linked-data/cube#componentProperty -->


    <owl:ObjectProperty rdf:about="http://purl.org/linked-data/cube#componentProperty">
        <rdfs:domain rdf:resource="http://purl.org/linked-data/cube#ComponentSet"/>
        <rdfs:range rdf:resource="http://purl.org/linked-data/cube#ComponentProperty"/>
        <rdfs:comment xml:lang="en">indicates a ComponentProperty (i.e. attribute/dimension) expected on a DataSet, or a dimension fixed in a SliceKey</rdfs:comment>
        <rdfs:isDefinedBy rdf:resource="http://purl.org/linked-data/cube"/>
        <rdfs:label xml:lang="en">component</rdfs:label>
    </owl:ObjectProperty>
    


    <!-- http://purl.org/linked-data/cube#concept -->


    <owl:ObjectProperty rdf:about="http://purl.org/linked-data/cube#concept">
        <rdfs:domain rdf:resource="http://purl.org/linked-data/cube#ComponentProperty"/>
        <rdfs:range rdf:resource="http://www.w3.org/2004/02/skos/core#Concept"/>
        <rdfs:comment xml:lang="en">gives the concept which is being measured or indicated by a ComponentProperty</rdfs:comment>
        <rdfs:isDefinedBy rdf:resource="http://purl.org/linked-data/cube"/>
        <rdfs:label xml:lang="en">concept</rdfs:label>
    </owl:ObjectProperty>
    


    <!-- http://purl.org/linked-data/cube#dataSet -->


    <owl:ObjectProperty rdf:about="http://purl.org/linked-data/cube#dataSet">
        <rdfs:domain rdf:resource="http://purl.org/linked-data/cube#Observation"/>
        <rdfs:range rdf:resource="http://purl.org/linked-data/cube#DataSet"/>
        <rdfs:comment xml:lang="en">indicates the data set of which this observation is a part</rdfs:comment>
        <rdfs:isDefinedBy rdf:resource="http://purl.org/linked-data/cube"/>
        <rdfs:label xml:lang="en">data set</rdfs:label>
    </owl:ObjectProperty>
    


    <!-- http://purl.org/linked-data/cube#dimension -->


    <owl:ObjectProperty rdf:about="http://purl.org/linked-data/cube#dimension">
        <rdfs:subPropertyOf rdf:resource="http://purl.org/linked-data/cube#componentProperty"/>
        <rdfs:range rdf:resource="http://purl.org/linked-data/cube#DimensionProperty"/>
        <rdfs:comment xml:lang="en">An alternative to qb:componentProperty which makes explicit that the component is a dimension</rdfs:comment>
        <rdfs:isDefinedBy rdf:resource="http://purl.org/linked-data/cube"/>
        <rdfs:label xml:lang="en">dimension</rdfs:label>
    </owl:ObjectProperty>
    


    <!-- http://purl.org/linked-data/cube#measure -->


    <owl:ObjectProperty rdf:about="http://purl.org/linked-data/cube#measure">
        <rdfs:subPropertyOf rdf:resource="http://purl.org/linked-data/cube#componentProperty"/>
        <rdfs:range rdf:resource="http://purl.org/linked-data/cube#MeasureProperty"/>
        <rdfs:comment xml:lang="en">An alternative to qb:componentProperty which makes explicit that the component is a measure</rdfs:comment>
        <rdfs:isDefinedBy rdf:resource="http://purl.org/linked-data/cube"/>
        <rdfs:label xml:lang="en">measure</rdfs:label>
    </owl:ObjectProperty>
    


    <!-- http://purl.org/linked-data/cube#observation -->


    <owl:ObjectProperty rdf:about="http://purl.org/linked-data/cube#observation">
        <rdfs:domain rdf:resource="http://purl.org/linked-data/cube#ObservationGroup"/>
        <rdfs:range rdf:resource="http://purl.org/linked-data/cube#Observation"/>
        <rdfs:comment xml:lang="en">indicates a observation contained within this slice of the data set</rdfs:comment>
        <rdfs:isDefinedBy rdf:resource="http://purl.org/linked-data/cube"/>
        <rdfs:label xml:lang="en">observation</rdfs:label>
    </owl:ObjectProperty>
    


    <!-- http://purl.org/linked-data/cube#observationGroup -->


    <owl:ObjectProperty rdf:about="http://purl.org/linked-data/cube#observationGroup">
        <rdfs:range rdf:resource="http://purl.org/linked-data/cube#ObservationGroup"/>
        <rdfs:comment xml:lang="en">Indicates a group of observations. The domain of this property is left open so that a group may be attached to different resources and need not be restricted to a single DataSet</rdfs:comment>
        <rdfs:isDefinedBy rdf:resource="http://purl.org/linked-data/cube"/>
        <rdfs:label xml:lang="en">observation group</rdfs:label>
    </owl:ObjectProperty>
    


    <!-- http://purl.org/linked-data/cube#slice -->


    <owl:ObjectProperty rdf:about="http://purl.org/linked-data/cube#slice">
        <rdfs:subPropertyOf rdf:resource="http://purl.org/linked-data/cube#observationGroup"/>
        <rdfs:domain rdf:resource="http://purl.org/linked-data/cube#DataSet"/>
        <rdfs:range rdf:resource="http://purl.org/linked-data/cube#Slice"/>
        <rdfs:comment xml:lang="en">Indicates a subset of a DataSet defined by fixing a subset of the dimensional values</rdfs:comment>
        <rdfs:isDefinedBy rdf:resource="http://purl.org/linked-data/cube"/>
        <rdfs:label xml:lang="en">slice</rdfs:label>
    </owl:ObjectProperty>
    


    <!-- http://purl.org/linked-data/cube#sliceKey -->


    <owl:ObjectProperty rdf:about="http://purl.org/linked-data/cube#sliceKey">
        <rdfs:domain rdf:resource="http://purl.org/linked-data/cube#DataStructureDefinition"/>
        <rdfs:range rdf:resource="http://purl.org/linked-data/cube#SliceKey"/>
        <rdfs:comment xml:lang="en">indicates a slice key which is used for slices in this dataset</rdfs:comment>
        <rdfs:isDefinedBy rdf:resource="http://purl.org/linked-data/cube"/>
        <rdfs:label xml:lang="en">slice key</rdfs:label>
    </owl:ObjectProperty>
    


    <!-- http://purl.org/linked-data/cube#sliceStructure -->


    <owl:ObjectProperty rdf:about="http://purl.org/linked-data/cube#sliceStructure">
        <rdfs:domain rdf:resource="http://purl.org/linked-data/cube#Slice"/>
        <rdfs:range rdf:resource="http://purl.org/linked-data/cube#SliceKey"/>
        <rdfs:comment xml:lang="en">indicates the sub-key corresponding to this slice</rdfs:comment>
        <rdfs:isDefinedBy rdf:resource="http://purl.org/linked-data/cube"/>
        <rdfs:label xml:lang="en">slice structure</rdfs:label>
    </owl:ObjectProperty>
    


    <!-- http://qudt.org/schema/qudt/hasQuantityKind -->


    <owl:ObjectProperty rdf:about="http://qudt.org/schema/qudt/hasQuantityKind">
        <rdfs:range rdf:resource="http://qudt.org/schema/qudt/QuantityKind"/>
        <rdfs:comment>A reference to the kind of a quantity</rdfs:comment>
        <rdfs:isDefinedBy rdf:resource="http://qudt.org/2.1/schema/qudt"/>
        <rdfs:label>has quantity kind</rdfs:label>
    </owl:ObjectProperty>
    


    <!-- http://qudt.org/schema/qudt/quantityValue -->


    <owl:ObjectProperty rdf:about="http://qudt.org/schema/qudt/quantityValue">
        <rdfs:range rdf:resource="http://qudt.org/schema/qudt/QuantityValue"/>
        <rdfs:comment>A reference to the value of a quantity</rdfs:comment>
        <rdfs:isDefinedBy rdf:resource="http://qudt.org/2.1/schema/qudt"/>
        <rdfs:label>quantity value</rdfs:label>
    </owl:ObjectProperty>
    


    <!-- http://qudt.org/schema/qudt/unit -->


    <owl:ObjectProperty rdf:about="http://qudt.org/schema/qudt/unit">
        <rdfs:range rdf:resource="http://qudt.org/schema/qudt/Unit"/>
        <rdfs:comment>A reference to the unit of measure of a quantity (variable or constant) of interest.</rdfs:comment>
        <rdfs:isDefinedBy rdf:resource="http://qudt.org/2.1/schema/qudt"/>
        <rdfs:label>unit</rdfs:label>
    </owl:ObjectProperty>
    


    <!-- http://www.opengis.net/ont/geosparql#hasGeometry -->


    <owl:ObjectProperty rdf:about="http://www.opengis.net/ont/geosparql#hasGeometry">
        <rdfs:domain rdf:resource="http://www.opengis.net/ont/geosparql#Feature"/>
        <rdfs:range rdf:resource="http://www.opengis.net/ont/geosparql#Geometry"/>
        <terms:contributor>Matthew Perry</terms:contributor>
        <terms:creator>OGC GeoSPARQL 1.0 Standard Working Group</terms:creator>
        <terms:date rdf:datatype="http://www.w3.org/2001/XMLSchema#date">2011-06-16</terms:date>
        <terms:description xml:lang="en">
      A spatial representation for a given feature.
    </terms:description>
        <rdfs:comment xml:lang="en">
      A spatial representation for a given feature.
    </rdfs:comment>
        <rdfs:isDefinedBy rdf:resource="http://www.opengis.net/ont/geosparql"/>
        <rdfs:isDefinedBy rdf:resource="http://www.opengis.net/spec/geosparql/1.0"/>
        <rdfs:label xml:lang="en">hasGeometry</rdfs:label>
        <skos:definition xml:lang="en">
      A spatial representation for a given feature.
    </skos:definition>
        <skos:prefLabel xml:lang="en">hasGeometry</skos:prefLabel>
    </owl:ObjectProperty>
    


    <!-- http://www.opengis.net/ont/geosparql#sfContains -->


    <owl:ObjectProperty rdf:about="http://www.opengis.net/ont/geosparql#sfContains">
        <rdfs:domain rdf:resource="http://www.opengis.net/ont/geosparql#SpatialObject"/>
        <rdfs:range rdf:resource="http://www.opengis.net/ont/geosparql#SpatialObject"/>
        <rdfs:comment xml:lang="en">Exists if the subject SpatialObject spatially contains the object SpatialObject. DE-9IM: T*****FF*</rdfs:comment>
        <rdfs:isDefinedBy rdf:resource="http://www.opengis.net/ont/geosparql"/>
        <rdfs:isDefinedBy rdf:resource="http://www.opengis.net/spec/geosparql/1.0"/>
        <rdfs:label xml:lang="en">contains</rdfs:label>
    </owl:ObjectProperty>
    


    <!-- http://www.opengis.net/ont/geosparql#sfWithin -->


    <owl:ObjectProperty rdf:about="http://www.opengis.net/ont/geosparql#sfWithin">
        <rdfs:domain rdf:resource="http://www.opengis.net/ont/geosparql#SpatialObject"/>
        <rdfs:range rdf:resource="http://www.opengis.net/ont/geosparql#SpatialObject"/>
        <rdfs:comment xml:lang="en">Exists if the subject SpatialObject is spatially within the object SpatialObject. DE-9IM: T*F**F***</rdfs:comment>
        <rdfs:isDefinedBy rdf:resource="http://www.opengis.net/ont/geosparql"/>
        <rdfs:isDefinedBy rdf:resource="http://www.opengis.net/spec/geosparql/1.0"/>
        <rdfs:label xml:lang="en">within</rdfs:label>
    </owl:ObjectProperty>
    


    <!-- http://www.w3.org/2003/01/geo/wgs84_pos#location -->


    <owl:ObjectProperty rdf:about="http://www.w3.org/2003/01/geo/wgs84_pos#location">
        <rdfs:comment>The relation between something and the point, or other geometrical thing in space, where it is.</rdfs:comment>
        <rdfs:isDefinedBy rdf:resource="http://www.w3.org/2003/01/geo/wgs84_pos#"/>
        <rdfs:label>location</rdfs:label>
    </owl:ObjectProperty>
    


    <!-- http://www.w3.org/2006/time#hasBeginning -->


    <owl:ObjectProperty rdf:about="http://www.w3.org/2006/time#hasBeginning">
        <rdfs:subPropertyOf rdf:resource="http://www.w3.org/2006/time#hasTime"/>
        <rdfs:domain rdf:resource="http://www.w3.org/2006/time#TemporalEntity"/>
        <rdfs:range rdf:resource="http://www.w3.org/2006/time#Instant"/>
        <rdfs:comment xml:lang="en">Beginning of a temporal entity</rdfs:comment>
        <rdfs:label xml:lang="en">has beginning</rdfs:label>
        <skos:definition xml:lang="en">Beginning of a temporal entity.</skos:definition>
    </owl:ObjectProperty>
    


    <!-- http://www.w3.org/2006/time#hasEnd -->


    <owl:ObjectProperty rdf:about="http://www.w3.org/2006/time#hasEnd">
        <rdfs:subPropertyOf rdf:resource="http://www.w3.org/2006/time#hasTime"/>
        <rdfs:domain rdf:resource="http://www.w3.org/2006/time#TemporalEntity"/>
        <rdfs:range rdf:resource="http://www.w3.org/2006/time#Instant"/>
        <rdfs:comment xml:lang="en">End of a temporal entity.</rdfs:comment>
        <rdfs:label xml:lang="en">has end</rdfs:label>
        <skos:definition xml:lang="en">End of a temporal entity.</skos:definition>
    </owl:ObjectProperty>
    


    <!-- http://www.w3.org/2006/time#hasTime -->


    <owl:ObjectProperty rdf:about="http://www.w3.org/2006/time#hasTime">
        <rdfs:range rdf:resource="http://www.w3.org/2006/time#TemporalEntity"/>
        <rdfs:comment xml:lang="en">Supports the association of a temporal entity (instant or interval) to any thing</rdfs:comment>
        <rdfs:label xml:lang="en">has time</rdfs:label>
        <skos:definition xml:lang="en">Supports the association of a temporal entity (instant or interval) to any thing</skos:definition>
        <skos:editorialNote xml:lang="en">Feature at risk - added in 2017 revision, and not yet widely used. </skos:editorialNote>
    </owl:ObjectProperty>
    


    <!-- http://www.w3.org/2006/time#unitType -->


    <owl:ObjectProperty rdf:about="http://www.w3.org/2006/time#unitType">
        <rdfs:range rdf:resource="http://www.w3.org/2006/time#TemporalUnit"/>
        <rdfs:comment xml:lang="en">The temporal unit which provides the precision of a date-time value or scale of a temporal extent</rdfs:comment>
        <rdfs:label xml:lang="en">temporal unit type</rdfs:label>
    </owl:ObjectProperty>
    


    <!-- http://www.w3.org/ns/sosa/hasFeatureOfInterest -->


    <owl:ObjectProperty rdf:about="http://www.w3.org/ns/sosa/hasFeatureOfInterest">
        <owl:inverseOf rdf:resource="http://www.w3.org/ns/sosa/isFeatureOfInterestOf"/>
        <rdfs:comment xml:lang="en">A relation between an Observation and the entity whose quality was observed, or between an Actuation and the entity whose property was modified, or between an act of Sampling and the entity that was sampled.</rdfs:comment>
        <rdfs:isDefinedBy rdf:resource="http://www.w3.org/ns/sosa/"/>
        <rdfs:label xml:lang="en">has feature of interest</rdfs:label>
        <skos:definition xml:lang="en">A relation between an Observation and the entity whose quality was observed, or between an Actuation and the entity whose property was modified, or between an act of Sampling and the entity that was sampled.</skos:definition>
        <skos:example xml:lang="en">For example, in an Observation of the weight of a person, the FeatureOfInterest is the person and the property is its weight.</skos:example>
        <schema:domainIncludes rdf:resource="http://www.w3.org/ns/sosa/Actuation"/>
        <schema:domainIncludes rdf:resource="http://www.w3.org/ns/sosa/Observation"/>
        <schema:domainIncludes rdf:resource="http://www.w3.org/ns/sosa/ObservationCollection"/>
        <schema:domainIncludes rdf:resource="http://www.w3.org/ns/sosa/Sampling"/>
        <schema:rangeIncludes rdf:resource="http://www.w3.org/ns/sosa/FeatureOfInterest"/>
        <schema:rangeIncludes rdf:resource="http://www.w3.org/ns/sosa/Sample"/>
    </owl:ObjectProperty>
    


    <!-- http://www.w3.org/ns/sosa/hasMember -->


    <owl:ObjectProperty rdf:about="http://www.w3.org/ns/sosa/hasMember">
        <rdfs:domain rdf:resource="http://www.w3.org/ns/sosa/ObservationCollection"/>
        <rdfs:range>
            <owl:Class>
                <owl:unionOf rdf:parseType="Collection">
                    <rdf:Description rdf:about="http://www.w3.org/ns/sosa/Observation"/>
                    <rdf:Description rdf:about="http://www.w3.org/ns/sosa/ObservationCollection"/>
                </owl:unionOf>
            </owl:Class>
        </rdfs:range>
        <rdfs:comment xml:lang="en">Link to a member within a collection of (observations) or (collections of observations) that share the same value for one or more of the characteristic properties</rdfs:comment>
        <rdfs:isDefinedBy rdf:resource="http://www.w3.org/ns/ssn/ext/"/>
        <rdfs:label xml:lang="en">member observation</rdfs:label>
        <schema:domainIncludes rdf:resource="http://www.w3.org/ns/sosa/ObservationCollection"/>
        <schema:rangeIncludes rdf:resource="http://www.w3.org/ns/sosa/Observation"/>
        <schema:rangeIncludes rdf:resource="http://www.w3.org/ns/sosa/ObservationCollection"/>
    </owl:ObjectProperty>
    


    <!-- http://www.w3.org/ns/sosa/hasResult -->


    <owl:ObjectProperty rdf:about="http://www.w3.org/ns/sosa/hasResult">
        <owl:inverseOf rdf:resource="http://www.w3.org/ns/sosa/isResultOf"/>
        <rdfs:comment xml:lang="en">Relation linking an Observation or Actuation or act of Sampling and a Result.</rdfs:comment>
        <rdfs:isDefinedBy rdf:resource="http://www.w3.org/ns/sosa/"/>
        <rdfs:label xml:lang="en">has result</rdfs:label>
        <skos:definition xml:lang="en">Relation linking an Observation or Actuation or act of Sampling and a Result.</skos:definition>
        <schema:domainIncludes rdf:resource="http://www.w3.org/ns/sosa/Actuation"/>
        <schema:domainIncludes rdf:resource="http://www.w3.org/ns/sosa/Observation"/>
        <schema:domainIncludes rdf:resource="http://www.w3.org/ns/sosa/Sampling"/>
        <schema:rangeIncludes rdf:resource="http://www.w3.org/ns/sosa/Result"/>
        <schema:rangeIncludes rdf:resource="http://www.w3.org/ns/sosa/Sample"/>
    </owl:ObjectProperty>
    


    <!-- http://www.w3.org/ns/sosa/hasUltimateFeatureOfInterest -->


    <owl:ObjectProperty rdf:about="http://www.w3.org/ns/sosa/hasUltimateFeatureOfInterest">
        <rdfs:domain>
            <owl:Class>
                <owl:unionOf rdf:parseType="Collection">
                    <rdf:Description rdf:about="http://www.w3.org/ns/sosa/Actuation"/>
                    <rdf:Description rdf:about="http://www.w3.org/ns/sosa/Observation"/>
                    <rdf:Description rdf:about="http://www.w3.org/ns/sosa/Sampling"/>
                </owl:unionOf>
            </owl:Class>
        </rdfs:domain>
        <rdfs:range rdf:resource="http://www.w3.org/ns/sosa/FeatureOfInterest"/>
        <rdfs:comment xml:lang="en">A relation to link Actuation, Observation, Sampling or FeatureOfInterest</rdfs:comment>
        <rdfs:isDefinedBy rdf:resource="http://www.w3.org/ns/ssn/ext/"/>
        <rdfs:label xml:lang="en">has ultimate feature of interest</rdfs:label>
        <schema:domainIncludes rdf:resource="http://www.w3.org/ns/sosa/Actuation"/>
        <schema:domainIncludes rdf:resource="http://www.w3.org/ns/sosa/Observation"/>
        <schema:domainIncludes rdf:resource="http://www.w3.org/ns/sosa/Sampling"/>
        <schema:rangeIncludes rdf:resource="http://www.w3.org/ns/sosa/FeatureOfInterest"/>
    </owl:ObjectProperty>
    


    <!-- http://www.w3.org/ns/sosa/hosts -->


    <owl:ObjectProperty rdf:about="http://www.w3.org/ns/sosa/hosts">
        <owl:inverseOf rdf:resource="http://www.w3.org/ns/sosa/isHostedBy"/>
        <rdfs:comment xml:lang="en">Relation between a platform and the systems it hosts.</rdfs:comment>
        <rdfs:isDefinedBy rdf:resource="http://www.w3.org/ns/sosa/"/>
        <rdfs:label xml:lang="en">host</rdfs:label>
    </owl:ObjectProperty>
    


    <!-- http://www.w3.org/ns/sosa/isFeatureOfInterestOf -->


    <owl:ObjectProperty rdf:about="http://www.w3.org/ns/sosa/isFeatureOfInterestOf">
        <rdfs:comment xml:lang="en">A relation between a FeatureOfInterest and an Observation about it, an Actuation acting on it, or an act of Sampling that sampled it.</rdfs:comment>
        <rdfs:isDefinedBy rdf:resource="http://www.w3.org/ns/sosa/"/>
        <rdfs:label xml:lang="en">is feature of interest of</rdfs:label>
        <skos:definition xml:lang="en">A relation between a FeatureOfInterest and an Observation about it, an Actuation acting on it, or an act of Sampling that sampled it.</skos:definition>
        <schema:domainIncludes rdf:resource="http://www.w3.org/ns/sosa/FeatureOfInterest"/>
        <schema:domainIncludes rdf:resource="http://www.w3.org/ns/sosa/Sample"/>
        <schema:rangeIncludes rdf:resource="http://www.w3.org/ns/sosa/Actuation"/>
        <schema:rangeIncludes rdf:resource="http://www.w3.org/ns/sosa/Observation"/>
        <schema:rangeIncludes rdf:resource="http://www.w3.org/ns/sosa/Sampling"/>
    </owl:ObjectProperty>
    


    <!-- http://www.w3.org/ns/sosa/isHostedBy -->


    <owl:ObjectProperty rdf:about="http://www.w3.org/ns/sosa/isHostedBy">
        <rdfs:comment xml:lang="en">Relation between a system and its hosting platform.</rdfs:comment>
        <rdfs:isDefinedBy rdf:resource="http://www.w3.org/ns/sosa/"/>
        <rdfs:label xml:lang="en">is hosted by</rdfs:label>
    </owl:ObjectProperty>
    


    <!-- http://www.w3.org/ns/sosa/isResultOf -->


    <owl:ObjectProperty rdf:about="http://www.w3.org/ns/sosa/isResultOf"/>
    


    <!-- http://www.w3.org/ns/sosa/madeBySensor -->


    <owl:ObjectProperty rdf:about="http://www.w3.org/ns/sosa/madeBySensor">
        <owl:inverseOf rdf:resource="http://www.w3.org/ns/sosa/madeObservation"/>
        <rdfs:comment xml:lang="en">Relation between an Observation and the Sensor which made the Observations.</rdfs:comment>
        <rdfs:isDefinedBy rdf:resource="http://www.w3.org/ns/sosa/"/>
        <rdfs:label xml:lang="en">made by sensor</rdfs:label>
        <schema:domainIncludes rdf:resource="http://www.w3.org/ns/sosa/Observation"/>
        <schema:domainIncludes rdf:resource="http://www.w3.org/ns/sosa/ObservationCollection"/>
        <schema:rangeIncludes rdf:resource="http://www.w3.org/ns/sosa/Sensor"/>
    </owl:ObjectProperty>
    


    <!-- http://www.w3.org/ns/sosa/madeObservation -->


    <owl:ObjectProperty rdf:about="http://www.w3.org/ns/sosa/madeObservation">
        <rdfs:comment xml:lang="en">Relation between a Sensor and an Observation made by the Sensor.</rdfs:comment>
        <rdfs:isDefinedBy rdf:resource="http://www.w3.org/ns/sosa/"/>
        <rdfs:label xml:lang="en">made observation</rdfs:label>
        <skos:definition xml:lang="en">Relation between a Sensor and an Observation made by the Sensor.</skos:definition>
        <schema:rangeIncludes rdf:resource="http://www.w3.org/ns/sosa/Observation"/>
    </owl:ObjectProperty>
    


    <!-- http://www.w3.org/ns/sosa/observedProperty -->


    <owl:ObjectProperty rdf:about="http://www.w3.org/ns/sosa/observedProperty">
        <terms:description xml:lang="en">Relation linking an Observation to the property that was observed. The ObservableProperty should be a property of the FeatureOfInterest (linked by hasFeatureOfInterest) of this Observation.</terms:description>
        <rdfs:comment xml:lang="en">Relation linking an Observation to the property that was observed. The ObservableProperty should be a property of the FeatureOfInterest (linked by hasFeatureOfInterest) of this Observation.</rdfs:comment>
        <rdfs:isDefinedBy rdf:resource="http://www.w3.org/ns/sosa/"/>
        <rdfs:label xml:lang="en">Observed Property</rdfs:label>
        <schema:domainIncludes rdf:resource="http://www.w3.org/ns/sosa/Observation"/>
        <schema:domainIncludes rdf:resource="http://www.w3.org/ns/sosa/ObservationCollection"/>
        <schema:rangeIncludes rdf:resource="http://www.w3.org/ns/sosa/ObservableProperty"/>
    </owl:ObjectProperty>
    


    <!-- http://www.w3.org/ns/sosa/observes -->


    <owl:ObjectProperty rdf:about="http://www.w3.org/ns/sosa/observes">
        <rdfs:comment xml:lang="en">Relation between a Sensor and an ObservableProperty that it is capable of sensing.</rdfs:comment>
        <rdfs:isDefinedBy rdf:resource="http://www.w3.org/ns/sosa/"/>
        <rdfs:label xml:lang="en">observes</rdfs:label>
        <schema:domainIncludes rdf:resource="http://www.w3.org/ns/sosa/Sensor"/>
        <schema:rangeIncludes rdf:resource="http://www.w3.org/ns/sosa/ObservableProperty"/>
    </owl:ObjectProperty>
    


    <!-- http://www.w3.org/ns/sosa/phenomenonTime -->


    <owl:ObjectProperty rdf:about="http://www.w3.org/ns/sosa/phenomenonTime">
        <rdfs:comment xml:lang="en">The time that the Result of an Observation, Actuation or Sampling applies to the FeatureOfInterest. Not necessarily the same as the resultTime. May be an Interval or an Instant, or some other compound TemporalEntity.</rdfs:comment>
        <rdfs:isDefinedBy rdf:resource="http://www.w3.org/ns/sosa/"/>
        <rdfs:label xml:lang="en">phenomenon time</rdfs:label>
        <schema:domainIncludes rdf:resource="http://www.w3.org/ns/sosa/Actuation"/>
        <schema:domainIncludes rdf:resource="http://www.w3.org/ns/sosa/Observation"/>
        <schema:domainIncludes rdf:resource="http://www.w3.org/ns/sosa/ObservationCollection"/>
        <schema:domainIncludes rdf:resource="http://www.w3.org/ns/sosa/Sampling"/>
    </owl:ObjectProperty>
    


    <!-- http://www.w3.org/ns/sosa/usedProcedure -->


    <owl:ObjectProperty rdf:about="http://www.w3.org/ns/sosa/usedProcedure">
        <rdfs:comment xml:lang="en">A relation to link to a re-usable Procedure used in making an Observation, an Actuation, or a Sample, typically through a Sensor, Actuator or Sampler.</rdfs:comment>
        <rdfs:isDefinedBy rdf:resource="http://www.w3.org/ns/sosa/"/>
        <rdfs:label xml:lang="en">used procedure</rdfs:label>
        <schema:domainIncludes rdf:resource="http://www.w3.org/ns/sosa/Actuation"/>
        <schema:domainIncludes rdf:resource="http://www.w3.org/ns/sosa/Observation"/>
        <schema:domainIncludes rdf:resource="http://www.w3.org/ns/sosa/ObservationCollection"/>
        <schema:domainIncludes rdf:resource="http://www.w3.org/ns/sosa/Sampling"/>
        <schema:rangeIncludes rdf:resource="http://www.w3.org/ns/sosa/Procedure"/>
    </owl:ObjectProperty>
    


    <!-- http://www.w3.org/ns/ssn/deployedOnPlatform -->


    <owl:ObjectProperty rdf:about="http://www.w3.org/ns/ssn/deployedOnPlatform">
        <owl:inverseOf rdf:resource="http://www.w3.org/ns/ssn/inDeployment"/>
        <rdfs:comment xml:lang="en">Relation between a deployment and the platform(s) involved in the deployment.</rdfs:comment>
        <rdfs:isDefinedBy rdf:resource="http://www.w3.org/ns/ssn/"/>
        <rdfs:label xml:lang="en">deployed on platform</rdfs:label>
    </owl:ObjectProperty>
    


    <!-- http://www.w3.org/ns/ssn/deployedSystem -->


    <owl:ObjectProperty rdf:about="http://www.w3.org/ns/ssn/deployedSystem">
        <owl:inverseOf rdf:resource="http://www.w3.org/ns/ssn/hasDeployment"/>
        <rdfs:comment xml:lang="en">Relation between a deployment and the system deployed.</rdfs:comment>
        <rdfs:isDefinedBy rdf:resource="http://www.w3.org/ns/ssn/"/>
        <rdfs:label xml:lang="en">deployed system</rdfs:label>
    </owl:ObjectProperty>
    


    <!-- http://www.w3.org/ns/ssn/hasDeployment -->


    <owl:ObjectProperty rdf:about="http://www.w3.org/ns/ssn/hasDeployment">
        <rdfs:comment xml:lang="en">Relation between a System and a Deployment, recording that the System is deployed in that Deployment.</rdfs:comment>
        <rdfs:isDefinedBy rdf:resource="http://www.w3.org/ns/ssn/"/>
        <rdfs:label xml:lang="en">has deployment</rdfs:label>
    </owl:ObjectProperty>
    


    <!-- http://www.w3.org/ns/ssn/hasInput -->


    <owl:ObjectProperty rdf:about="http://www.w3.org/ns/ssn/hasInput">
        <rdfs:comment xml:lang="en">Relation between a Procedure and an Input to it.</rdfs:comment>
        <rdfs:isDefinedBy rdf:resource="http://www.w3.org/ns/ssn/"/>
        <rdfs:label xml:lang="en">has input</rdfs:label>
    </owl:ObjectProperty>
    


    <!-- http://www.w3.org/ns/ssn/hasOutput -->


    <owl:ObjectProperty rdf:about="http://www.w3.org/ns/ssn/hasOutput">
        <rdfs:comment xml:lang="en">Relation between a Procedure and an Output of it.</rdfs:comment>
        <rdfs:isDefinedBy rdf:resource="http://www.w3.org/ns/ssn/"/>
        <rdfs:label xml:lang="en">has output</rdfs:label>
    </owl:ObjectProperty>
    


    <!-- http://www.w3.org/ns/ssn/hasProperty -->


    <owl:ObjectProperty rdf:about="http://www.w3.org/ns/ssn/hasProperty">
        <rdfs:comment>A relation between a FeatureOfInterest and a Property of that feature.</rdfs:comment>
        <rdfs:isDefinedBy rdf:resource="http://purl.oclc.org/NET/ssnx/ssn"/>
        <rdfs:label xml:lang="en">has property</rdfs:label>
    </owl:ObjectProperty>
    


    <!-- http://www.w3.org/ns/ssn/hasSubSystem -->


    <owl:ObjectProperty rdf:about="http://www.w3.org/ns/ssn/hasSubSystem">
        <rdfs:comment xml:lang="en">Relation between a system and its component parts </rdfs:comment>
        <rdfs:isDefinedBy rdf:resource="http://www.w3.org/ns/ssn/"/>
        <rdfs:label xml:lang="en">has subsystem</rdfs:label>
    </owl:ObjectProperty>
    


    <!-- http://www.w3.org/ns/ssn/implementedBy -->


    <owl:ObjectProperty rdf:about="http://www.w3.org/ns/ssn/implementedBy">
        <rdfs:comment xml:lang="en">Relation between a Procedure (an algorithm, procedure or method) and an entity that implements that Procedure in some executable way.</rdfs:comment>
        <rdfs:isDefinedBy rdf:resource="http://www.w3.org/ns/ssn/"/>
        <rdfs:label xml:lang="en">implemented by</rdfs:label>
    </owl:ObjectProperty>
    


    <!-- http://www.w3.org/ns/ssn/implements -->


    <owl:ObjectProperty rdf:about="http://www.w3.org/ns/ssn/implements">
        <rdfs:comment xml:lang="en">Relation between an entity that implements a Procedure in some executable way and the Procedure (an algorithm, procedure or method).</rdfs:comment>
        <rdfs:isDefinedBy rdf:resource="http://www.w3.org/ns/ssn/"/>
        <rdfs:label xml:lang="en">implements</rdfs:label>
    </owl:ObjectProperty>
    


    <!-- http://www.w3.org/ns/ssn/inDeployment -->


    <owl:ObjectProperty rdf:about="http://www.w3.org/ns/ssn/inDeployment">
        <rdfs:comment xml:lang="en">Relation between a platform and the deployment(s) that takes place in the platform.</rdfs:comment>
        <rdfs:isDefinedBy rdf:resource="http://www.w3.org/ns/ssn/"/>
        <rdfs:label xml:lang="en">in deployment</rdfs:label>
    </owl:ObjectProperty>
    


    <!-- http://www.w3.org/ns/ssn/isPropertyOf -->


    <owl:ObjectProperty rdf:about="http://www.w3.org/ns/ssn/isPropertyOf">
        <rdfs:comment xml:lang="en">Relation between a Property and the entity it belongs to.</rdfs:comment>
        <rdfs:isDefinedBy rdf:resource="http://www.w3.org/ns/ssn/"/>
        <rdfs:label xml:lang="en">is property of</rdfs:label>
    </owl:ObjectProperty>
    


    <!-- http://xmlns.com/foaf/0.1/member -->


    <owl:ObjectProperty rdf:about="http://xmlns.com/foaf/0.1/member">
        <rdfs:comment>The foaf:member property relates a foaf:Group to a foaf:Agent that is a member of that group.</rdfs:comment>
        <rdfs:isDefinedBy rdf:resource="http://xmlns.com/foaf/0.1/"/>
        <rdfs:label>member</rdfs:label>
    </owl:ObjectProperty>
    


    <!-- 
    ///////////////////////////////////////////////////////////////////////////////////////
    //
    // Data properties
    //
    ///////////////////////////////////////////////////////////////////////////////////////
     -->


    


    <!-- http://purl.org/linked-data/cube#order -->


    <owl:DatatypeProperty rdf:about="http://purl.org/linked-data/cube#order">
        <rdfs:domain rdf:resource="http://purl.org/linked-data/cube#ComponentSpecification"/>
        <rdfs:range rdf:resource="http://www.w3.org/2001/XMLSchema#int"/>
        <rdfs:comment xml:lang="en">indicates a priority order for the components of sets with this structure, used to guide presentations - lower order numbers come before higher numbers, un-numbered components come last</rdfs:comment>
        <rdfs:isDefinedBy rdf:resource="http://purl.org/linked-data/cube"/>
        <rdfs:label xml:lang="en">order</rdfs:label>
    </owl:DatatypeProperty>
    


    <!-- http://qudt.org/schema/qudt/numericValue -->


    <owl:DatatypeProperty rdf:about="http://qudt.org/schema/qudt/numericValue">
        <rdfs:isDefinedBy rdf:resource="http://qudt.org/2.1/schema/qudt"/>
        <rdfs:label>numeric value</rdfs:label>
    </owl:DatatypeProperty>
    


    <!-- http://www.opengis.net/ont/geosparql#asWKT -->


    <owl:DatatypeProperty rdf:about="http://www.opengis.net/ont/geosparql#asWKT">
        <rdfs:subPropertyOf rdf:resource="http://www.opengis.net/ont/geosparql#hasSerialization"/>
        <rdfs:domain rdf:resource="http://www.opengis.net/ont/geosparql#Geometry"/>
        <rdfs:range rdf:resource="http://www.opengis.net/ont/geosparql#wktLiteral"/>
        <rdfs:comment xml:lang="en">The WKT serialization of a geometry</rdfs:comment>
        <rdfs:isDefinedBy rdf:resource="http://www.opengis.net/ont/geosparql"/>
        <rdfs:isDefinedBy rdf:resource="http://www.opengis.net/spec/geosparql/1.0"/>
        <rdfs:label xml:lang="en">asWKT</rdfs:label>
    </owl:DatatypeProperty>
    


    <!-- http://www.opengis.net/ont/geosparql#hasSerialization -->


    <owl:DatatypeProperty rdf:about="http://www.opengis.net/ont/geosparql#hasSerialization">
        <rdfs:domain rdf:resource="http://www.opengis.net/ont/geosparql#Geometry"/>
        <rdfs:range rdf:resource="http://www.w3.org/2000/01/rdf-schema#Literal"/>
        <rdfs:comment xml:lang="en">Connects a geometry object with its text-based serialization</rdfs:comment>
        <rdfs:isDefinedBy rdf:resource="http://www.opengis.net/ont/geosparql"/>
        <rdfs:isDefinedBy rdf:resource="http://www.opengis.net/spec/geosparql/1.0"/>
        <rdfs:label xml:lang="en">has serialization</rdfs:label>
    </owl:DatatypeProperty>
    


    <!-- http://www.w3.org/2003/01/geo/wgs84_pos#alt -->


    <owl:DatatypeProperty rdf:about="http://www.w3.org/2003/01/geo/wgs84_pos#alt">
        <rdfs:comment>The WGS84 altitude of a SpatialThing (decimal meters above the local reference ellipsoid).</rdfs:comment>
        <rdfs:isDefinedBy rdf:resource="http://www.w3.org/2003/01/geo/wgs84_pos#"/>
        <rdfs:label>altitude</rdfs:label>
    </owl:DatatypeProperty>
    


    <!-- http://www.w3.org/2003/01/geo/wgs84_pos#lat -->


    <owl:DatatypeProperty rdf:about="http://www.w3.org/2003/01/geo/wgs84_pos#lat">
        <rdfs:comment>The WGS84 latitude of a SpatialThing (decimal degrees).</rdfs:comment>
        <rdfs:isDefinedBy rdf:resource="http://www.w3.org/2003/01/geo/wgs84_pos#"/>
        <rdfs:label>latitude</rdfs:label>
    </owl:DatatypeProperty>
    


    <!-- http://www.w3.org/2003/01/geo/wgs84_pos#long -->


    <owl:DatatypeProperty rdf:about="http://www.w3.org/2003/01/geo/wgs84_pos#long">
        <rdfs:comment>The WGS84 longitude of a SpatialThing (decimal degrees).</rdfs:comment>
        <rdfs:isDefinedBy rdf:resource="http://www.w3.org/2003/01/geo/wgs84_pos#"/>
        <rdfs:label>longitude</rdfs:label>
    </owl:DatatypeProperty>
    


    <!-- http://www.w3.org/2006/time#inXSDDate -->


    <owl:DatatypeProperty rdf:about="http://www.w3.org/2006/time#inXSDDate">
        <rdfs:domain rdf:resource="http://www.w3.org/2006/time#Instant"/>
        <rdfs:range rdf:resource="http://www.w3.org/2001/XMLSchema#date"/>
        <rdfs:comment xml:lang="en">Position of an instant, expressed using xsd:date</rdfs:comment>
        <rdfs:isDefinedBy rdf:resource="http://www.w3.org/2006/time#"/>
        <rdfs:label xml:lang="en">in XSD date</rdfs:label>
        <skos:definition xml:lang="en">Position of an instant, expressed using xsd:date</skos:definition>
    </owl:DatatypeProperty>
    


    <!-- http://www.w3.org/2006/time#inXSDDateTimeStamp -->


    <owl:DatatypeProperty rdf:about="http://www.w3.org/2006/time#inXSDDateTimeStamp">
        <rdfs:domain rdf:resource="http://www.w3.org/2006/time#Instant"/>
        <rdfs:range rdf:resource="http://www.w3.org/2001/XMLSchema#dateTimeStamp"/>
        <rdfs:comment xml:lang="en">Position of an instant, expressed using xsd:dateTimeStamp</rdfs:comment>
        <rdfs:isDefinedBy rdf:resource="http://www.w3.org/2006/time#"/>
        <rdfs:label xml:lang="en">in XSD Date-Time-Stamp</rdfs:label>
        <skos:definition xml:lang="en">Position of an instant, expressed using xsd:dateTimeStamp</skos:definition>
    </owl:DatatypeProperty>
    


    <!-- http://www.w3.org/2006/time#numericDuration -->


    <owl:DatatypeProperty rdf:about="http://www.w3.org/2006/time#numericDuration">
        <rdfs:domain rdf:resource="http://www.w3.org/2006/time#Duration"/>
        <rdfs:range rdf:resource="http://www.w3.org/2001/XMLSchema#decimal"/>
        <rdfs:comment xml:lang="en">Value of a temporal extent expressed as a decimal number scaled by a temporal unit</rdfs:comment>
        <rdfs:isDefinedBy rdf:resource="http://www.w3.org/2006/time#"/>
        <rdfs:label xml:lang="en">Numeric value of temporal duration</rdfs:label>
        <skos:definition xml:lang="en">Value of a temporal extent expressed as a decimal number scaled by a temporal unit</skos:definition>
    </owl:DatatypeProperty>
    


    <!-- http://www.w3.org/ns/prov#generatedAtTime -->


    <owl:DatatypeProperty rdf:about="http://www.w3.org/ns/prov#generatedAtTime">
        <rdfs:range rdf:resource="http://www.w3.org/2001/XMLSchema#dateTime"/>
        <rdfs:comment xml:lang="en">The time at which an entity was completely created and is available for use.</rdfs:comment>
        <rdfs:isDefinedBy rdf:resource="http://www.w3.org/ns/prov-o#"/>
        <rdfs:label>generatedAtTime</rdfs:label>
    </owl:DatatypeProperty>
    


    <!-- http://www.w3.org/ns/prov#invalidatedAtTime -->


    <owl:DatatypeProperty rdf:about="http://www.w3.org/ns/prov#invalidatedAtTime">
        <rdfs:range rdf:resource="http://www.w3.org/2001/XMLSchema#dateTime"/>
        <rdfs:comment xml:lang="en">The time at which an entity was invalidated (i.e., no longer usable).</rdfs:comment>
        <rdfs:isDefinedBy rdf:resource="http://www.w3.org/ns/prov-o#"/>
        <rdfs:label>invalidatedAtTime</rdfs:label>
    </owl:DatatypeProperty>
    


    <!-- http://www.w3.org/ns/sosa/hasSimpleResult -->


    <owl:DatatypeProperty rdf:about="http://www.w3.org/ns/sosa/hasSimpleResult">
        <rdfs:comment xml:lang="en">The simple value of an Observation or Actuation.</rdfs:comment>
        <rdfs:isDefinedBy rdf:resource="http://www.w3.org/ns/sosa/"/>
        <rdfs:label xml:lang="en">has simple result</rdfs:label>
        <skos:definition xml:lang="en">The simple value of an Observation or Actuation.</skos:definition>
        <skos:example xml:lang="en">For instance, the values 23 or true.</skos:example>
        <schema:domainIncludes rdf:resource="http://www.w3.org/ns/sosa/Actuation"/>
        <schema:domainIncludes rdf:resource="http://www.w3.org/ns/sosa/Observation"/>
    </owl:DatatypeProperty>
    


    <!-- http://www.w3.org/ns/sosa/resultTime -->


    <owl:DatatypeProperty rdf:about="http://www.w3.org/ns/sosa/resultTime">
        <rdfs:range rdf:resource="http://www.w3.org/2001/XMLSchema#dateTime"/>
        <rdfs:comment xml:lang="en">The result time is the instant of time when the Observation, Actuation or Sampling activity was completed.</rdfs:comment>
        <rdfs:isDefinedBy rdf:resource="http://www.w3.org/ns/sosa/"/>
        <rdfs:label xml:lang="en">result time</rdfs:label>
        <skos:definition xml:lang="en">The result time is the instant of time when the Observation, Actuation or Sampling activity was completed.</skos:definition>
        <schema:domainIncludes rdf:resource="http://www.w3.org/ns/sosa/Actuation"/>
        <schema:domainIncludes rdf:resource="http://www.w3.org/ns/sosa/Observation"/>
        <schema:domainIncludes rdf:resource="http://www.w3.org/ns/sosa/ObservationCollection"/>
        <schema:domainIncludes rdf:resource="http://www.w3.org/ns/sosa/Sampling"/>
    </owl:DatatypeProperty>
    


    <!-- 
    ///////////////////////////////////////////////////////////////////////////////////////
    //
    // Classes
    //
    ///////////////////////////////////////////////////////////////////////////////////////
     -->


    


    <!-- http://def.isotc211.org/iso19156/2011/GeneralFeatureInstance#GFI_DomainFeature -->


    <owl:Class rdf:about="http://def.isotc211.org/iso19156/2011/GeneralFeatureInstance#GFI_DomainFeature">
        <rdfs:subClassOf rdf:resource="http://def.isotc211.org/iso19156/2011/GeneralFeatureInstance#GFI_Feature"/>
        <rdfs:comment>The class GFI_DomainFeature represents &apos;real-world&apos; features which are the ultimate subject of an observation campaign, i.e. the features from an application domain that are .lt.i.gt.not .lt..sl.i.gt.artefacts of the observation process (sampling features). </rdfs:comment>
        <rdfs:isDefinedBy rdf:resource="http://standards.iso.org/iso/19156/ed-1/en/"/>
        <rdfs:label>GFI_DomainFeature</rdfs:label>
        <skos:definition>The class GFI_DomainFeature represents &apos;real-world&apos; features which are the ultimate subject of an observation campaign, i.e. the features from an application domain that are .lt.i.gt.not .lt..sl.i.gt.artefacts of the observation process (sampling features). </skos:definition>
    </owl:Class>
    


    <!-- http://def.isotc211.org/iso19156/2011/GeneralFeatureInstance#GFI_Feature -->


    <owl:Class rdf:about="http://def.isotc211.org/iso19156/2011/GeneralFeatureInstance#GFI_Feature">
        <owl:equivalentClass rdf:resource="http://www.opengis.net/ont/geosparql#Feature"/>
        <rdfs:comment>The class GFI_Feature (Figure 2) is an instance of the .og.metaclass.cg. GF_FeatureType (ISO 19109). It represents the set of all classes which are feature types. NOTE	GFI_Feature is implemented in GML (ISO 19136:2007) by the element gml:AbstractFeature and type gml:AbstractFeatureType. In an implementation this abstract class shall be substituted by a concrete class representing a feature type from an application schema associated with a domain of discourse (ISO 19109, ISO 19101). Sampling Features (Clause 8) are a class of feature-types whose role is primarily associated with observations.</rdfs:comment>
        <rdfs:isDefinedBy rdf:resource="http://standards.iso.org/iso/19156/ed-1/en/"/>
        <rdfs:label>GFI_Feature</rdfs:label>
        <skos:definition>The class GFI_Feature (Figure 2) is an instance of the .og.metaclass.cg. GF_FeatureType (ISO 19109). It represents the set of all classes which are feature types. NOTE	GFI_Feature is implemented in GML (ISO 19136:2007) by the element gml:AbstractFeature and type gml:AbstractFeatureType. In an implementation this abstract class shall be substituted by a concrete class representing a feature type from an application schema associated with a domain of discourse (ISO 19109, ISO 19101). Sampling Features (Clause 8) are a class of feature-types whose role is primarily associated with observations. </skos:definition>
    </owl:Class>
    


    <!-- http://def.isotc211.org/iso19156/2011/Observation#OM_Observation -->


    <owl:Class rdf:about="http://def.isotc211.org/iso19156/2011/Observation#OM_Observation">
        <owl:equivalentClass rdf:resource="http://www.w3.org/ns/sosa/Observation"/>
        <rdfs:comment>Observation process is a subtype of OM_Process. It is a process used to generate the result of the observation.</rdfs:comment>
        <rdfs:isDefinedBy rdf:resource="https://www.iso.org/standard/44595.html"/>
        <rdfs:label>Observation</rdfs:label>
        <skos:definition>Observation process is a subtype of OM_Process. It is a process used to generate the result of the observation.</skos:definition>
    </owl:Class>
    


    <!-- http://def.isotc211.org/iso19156/2011/SamplingFeature#SF_SamplingFeature -->


    <owl:Class rdf:about="http://def.isotc211.org/iso19156/2011/SamplingFeature#SF_SamplingFeature">
        <owl:equivalentClass rdf:resource="http://www.w3.org/ns/sosa/Sample"/>
        <rdfs:subClassOf rdf:resource="http://def.isotc211.org/iso19156/2011/GeneralFeatureInstance#GFI_Feature"/>
        <rdfs:comment>.lt.ul.gt.	.lt.li.gt..lt.b.gt.Role of sampling features.lt..sl.b.gt..lt..sl.li.gt..lt..sl.ul.gt.Sampling features are artefacts of an observational strategy, and have no significant function outside of their role in the observation process. The physical characteristics of the features themselves are of little interest, except perhaps to the manager of a sampling campaign.EXAMPLE	A .ldq.station.rdq. is essentially an identifiable locality where a sensor system or procedure may be deployed and an observation made. In the context of the observation model, it connotes the .ldq.world in the vicinity of the station.rdq., so the observed properties relate to the physical medium at the station, and not to any physical artefact such as a mooring, buoy, benchmark, monument, well, etc. NOTE	A transient sampling feature, such as a ships-track or flight-line, may be identified and described, but is unlikely to be revisited exactly. A sampling feature is intended to sample some feature of interest in an application domain. However, in some cases the identity, and even the exact type, of the sampled feature may not be known when observations are made using the sampling features. .lt.ul.gt.	.lt.li.gt..lt.b.gt.Classification of sampling features.lt..sl.b.gt..lt..sl.li.gt..lt..sl.ul.gt.A small number of sampling patterns are common across disciplines in observational science. These provide a basis for processing and portrayal tools which are similar across domains, and depend primarily on the geometry of the sample design. Common names for sampling features include specimen, station, profile, transect, path, swath, and scene. These are classified primarily by their topological dimension. Point-located samples are defined in this Clause, extensive samples of various dimensions in Clause 9 and specimens in Clause 10.</rdfs:comment>
        <rdfs:isDefinedBy rdf:resource="http://standards.iso.org/iso/19156/ed-1/en/"/>
        <rdfs:label>SF_SamplingFeature</rdfs:label>
        <skos:definition>.lt.ul.gt.	.lt.li.gt..lt.b.gt.Role of sampling features.lt..sl.b.gt..lt..sl.li.gt..lt..sl.ul.gt.Sampling features are artefacts of an observational strategy, and have no significant function outside of their role in the observation process. The physical characteristics of the features themselves are of little interest, except perhaps to the manager of a sampling campaign.EXAMPLE	A .ldq.station.rdq. is essentially an identifiable locality where a sensor system or procedure may be deployed and an observation made. In the context of the observation model, it connotes the .ldq.world in the vicinity of the station.rdq., so the observed properties relate to the physical medium at the station, and not to any physical artefact such as a mooring, buoy, benchmark, monument, well, etc. NOTE	A transient sampling feature, such as a ships-track or flight-line, may be identified and described, but is unlikely to be revisited exactly. A sampling feature is intended to sample some feature of interest in an application domain. However, in some cases the identity, and even the exact type, of the sampled feature may not be known when observations are made using the sampling features. .lt.ul.gt.	.lt.li.gt..lt.b.gt.Classification of sampling features.lt..sl.b.gt..lt..sl.li.gt..lt..sl.ul.gt.A small number of sampling patterns are common across disciplines in observational science. These provide a basis for processing and portrayal tools which are similar across domains, and depend primarily on the geometry of the sample design. Common names for sampling features include specimen, station, profile, transect, path, swath, and scene. These are classified primarily by their topological dimension. Point-located samples are defined in this Clause, extensive samples of various dimensions in Clause 9 and specimens in Clause 10.</skos:definition>
    </owl:Class>
    


    <!-- http://def.seegrid.csiro.au/isotc211/iso19103/2005/basic#Measure -->


    <owl:Class rdf:about="http://def.seegrid.csiro.au/isotc211/iso19103/2005/basic#Measure">
        <owl:equivalentClass rdf:resource="http://qudt.org/schema/qudt/QuantityValue"/>
        <owl:deprecated rdf:datatype="http://www.w3.org/2001/XMLSchema#boolean">true</owl:deprecated>
    </owl:Class>
    


    <!-- http://purl.oclc.org/NET/ssnx/qu/dim#Acceleration -->


    <owl:Class rdf:about="http://purl.oclc.org/NET/ssnx/qu/dim#Acceleration">
        <rdfs:subClassOf rdf:resource="http://purl.oclc.org/NET/ssnx/qu/qu#QuantityKind"/>
        <rdfs:comment>A Acceleration is something that is a QuantityKind and has a unitKind property who must be a AccelerationUnit</rdfs:comment>
        <rdfs:isDefinedBy rdf:resource="http://purl.oclc.org/NET/ssnx/qu/qu-rec20"/>
        <rdfs:label>Acceleration</rdfs:label>
    </owl:Class>
    


    <!-- http://purl.oclc.org/NET/ssnx/qu/dim#Compressibility -->


    <owl:Class rdf:about="http://purl.oclc.org/NET/ssnx/qu/dim#Compressibility">
        <rdfs:subClassOf rdf:resource="http://purl.oclc.org/NET/ssnx/qu/qu#QuantityKind"/>
        <rdfs:comment>A Compressibility is something that is a QuantityKind and has a unitKind property who must be a CompressibilityUnit</rdfs:comment>
        <rdfs:isDefinedBy rdf:resource="http://purl.oclc.org/NET/ssnx/qu/qu-rec20"/>
        <rdfs:label>Compressibility</rdfs:label>
    </owl:Class>
    


    <!-- http://purl.oclc.org/NET/ssnx/qu/dim#Concentration -->


    <owl:Class rdf:about="http://purl.oclc.org/NET/ssnx/qu/dim#Concentration">
        <rdfs:subClassOf rdf:resource="http://purl.oclc.org/NET/ssnx/qu/qu#QuantityKind"/>
        <rdfs:comment>A Concentration is something that is a QuantityKind and has a unitKind property who must be a ConcentrationUnit</rdfs:comment>
        <rdfs:isDefinedBy rdf:resource="http://purl.oclc.org/NET/ssnx/qu/qu-rec20"/>
        <rdfs:label>Concentration</rdfs:label>
    </owl:Class>
    


    <!-- http://purl.oclc.org/NET/ssnx/qu/dim#Density -->


    <owl:Class rdf:about="http://purl.oclc.org/NET/ssnx/qu/dim#Density">
        <rdfs:subClassOf rdf:resource="http://purl.oclc.org/NET/ssnx/qu/qu#QuantityKind"/>
        <rdfs:comment>A Density is something that is a QuantityKind and has a unitKind property who must be a DensityUnit</rdfs:comment>
        <rdfs:isDefinedBy rdf:resource="http://purl.oclc.org/NET/ssnx/qu/qu-rec20"/>
        <rdfs:label>Density</rdfs:label>
    </owl:Class>
    


    <!-- http://purl.oclc.org/NET/ssnx/qu/dim#Dimensionless -->


    <owl:Class rdf:about="http://purl.oclc.org/NET/ssnx/qu/dim#Dimensionless">
        <rdfs:subClassOf rdf:resource="http://purl.oclc.org/NET/ssnx/qu/qu#QuantityKind"/>
        <rdfs:comment>A Dimensionless is something that is a QuantityKind and has a unitKind property who must be a DimensionlessUnit</rdfs:comment>
        <rdfs:isDefinedBy rdf:resource="http://purl.oclc.org/NET/ssnx/qu/qu-rec20"/>
        <rdfs:label>Dimensionless</rdfs:label>
    </owl:Class>
    


    <!-- http://purl.oclc.org/NET/ssnx/qu/dim#Distance -->


    <owl:Class rdf:about="http://purl.oclc.org/NET/ssnx/qu/dim#Distance">
        <rdfs:subClassOf rdf:resource="http://purl.oclc.org/NET/ssnx/qu/qu#QuantityKind"/>
        <rdfs:comment>A dim:Distance is something that is a qu:QuantityKind and has a unitKind property who must be a dim:DistanceUnit</rdfs:comment>
        <rdfs:isDefinedBy rdf:resource="http://purl.oclc.org/NET/ssnx/qu/qu-rec20"/>
        <rdfs:label>Distance</rdfs:label>
    </owl:Class>
    


    <!-- http://purl.oclc.org/NET/ssnx/qu/dim#Energy -->


    <owl:Class rdf:about="http://purl.oclc.org/NET/ssnx/qu/dim#Energy">
        <rdfs:subClassOf rdf:resource="http://purl.oclc.org/NET/ssnx/qu/qu#QuantityKind"/>
        <rdfs:comment>A Energy is something that is a QuantityKind and has a unitKind property who must be a EnergyUnit</rdfs:comment>
        <rdfs:isDefinedBy rdf:resource="http://purl.oclc.org/NET/ssnx/qu/qu-rec20"/>
        <rdfs:label>Energy</rdfs:label>
    </owl:Class>
    


    <!-- http://purl.oclc.org/NET/ssnx/qu/dim#EnergyDensity -->


    <owl:Class rdf:about="http://purl.oclc.org/NET/ssnx/qu/dim#EnergyDensity">
        <rdfs:subClassOf rdf:resource="http://purl.oclc.org/NET/ssnx/qu/qu#QuantityKind"/>
        <rdfs:comment>A EnergyDensity is something that is a QuantityKind and has a unitKind property who must be a EnergyDensityUnit</rdfs:comment>
        <rdfs:isDefinedBy rdf:resource="http://purl.oclc.org/NET/ssnx/qu/qu-rec20"/>
        <rdfs:label>Energy Density</rdfs:label>
    </owl:Class>
    


    <!-- http://purl.oclc.org/NET/ssnx/qu/dim#EnergyFlux -->


    <owl:Class rdf:about="http://purl.oclc.org/NET/ssnx/qu/dim#EnergyFlux">
        <rdfs:subClassOf rdf:resource="http://purl.oclc.org/NET/ssnx/qu/qu#QuantityKind"/>
        <rdfs:comment>A EnergyFlux is something that is a QuantityKind and has a unitKind property who must be a EnergyFluxUnit</rdfs:comment>
        <rdfs:isDefinedBy rdf:resource="http://purl.oclc.org/NET/ssnx/qu/qu-rec20"/>
        <rdfs:label>Energy Flux</rdfs:label>
    </owl:Class>
    


    <!-- http://purl.oclc.org/NET/ssnx/qu/dim#MassPerTimePerArea -->


    <owl:Class rdf:about="http://purl.oclc.org/NET/ssnx/qu/dim#MassPerTimePerArea">
        <rdfs:subClassOf rdf:resource="http://purl.oclc.org/NET/ssnx/qu/qu#QuantityKind"/>
        <rdfs:comment>A MassPerTimePerArea is something that is a QuantityKind and has a unitKind property who must be a MassPerTimePerAreaUnit</rdfs:comment>
        <rdfs:isDefinedBy rdf:resource="http://purl.oclc.org/NET/ssnx/qu/qu-rec20"/>
        <rdfs:label>Mass Per Time Per Area</rdfs:label>
    </owl:Class>
    


    <!-- http://purl.oclc.org/NET/ssnx/qu/dim#Power -->


    <owl:Class rdf:about="http://purl.oclc.org/NET/ssnx/qu/dim#Power">
        <rdfs:subClassOf rdf:resource="http://purl.oclc.org/NET/ssnx/qu/qu#QuantityKind"/>
        <rdfs:comment>A Power is something that is of class QuantityKind and has a unitKind property who must be a PowerUnit</rdfs:comment>
        <rdfs:isDefinedBy rdf:resource="http://purl.oclc.org/NET/ssnx/qu/qu-rec20"/>
        <rdfs:label>Power</rdfs:label>
    </owl:Class>
    


    <!-- http://purl.oclc.org/NET/ssnx/qu/dim#RadianceExposure -->


    <owl:Class rdf:about="http://purl.oclc.org/NET/ssnx/qu/dim#RadianceExposure">
        <rdfs:subClassOf rdf:resource="http://purl.oclc.org/NET/ssnx/qu/qu#QuantityKind"/>
        <rdfs:comment>A RadianceExposure is something that is a QuantityKind and has a unitKind property who must be a RadianceExposureUnit</rdfs:comment>
        <rdfs:isDefinedBy rdf:resource="http://purl.oclc.org/NET/ssnx/qu/qu-rec20"/>
        <rdfs:label>Radiance Exposure</rdfs:label>
    </owl:Class>
    


    <!-- http://purl.oclc.org/NET/ssnx/qu/dim#RotationalSpeed -->


    <owl:Class rdf:about="http://purl.oclc.org/NET/ssnx/qu/dim#RotationalSpeed">
        <rdfs:subClassOf rdf:resource="http://purl.oclc.org/NET/ssnx/qu/qu#QuantityKind"/>
        <rdfs:comment>A RotationalSpeed is something that is a QuantityKind and has a unitKind property who must be a RotationalSpeedUnit</rdfs:comment>
        <rdfs:isDefinedBy rdf:resource="http://purl.oclc.org/NET/ssnx/qu/qu-rec20"/>
        <rdfs:label>Rotational Speed</rdfs:label>
    </owl:Class>
    


    <!-- http://purl.oclc.org/NET/ssnx/qu/dim#SpecificEntropy -->


    <owl:Class rdf:about="http://purl.oclc.org/NET/ssnx/qu/dim#SpecificEntropy">
        <rdfs:subClassOf rdf:resource="http://purl.oclc.org/NET/ssnx/qu/qu#QuantityKind"/>
        <rdfs:comment>A SpecificEntropy is something that is a QuantityKind and has a unitKind property who must be a SpecificEntropyUnit</rdfs:comment>
        <rdfs:isDefinedBy rdf:resource="http://purl.oclc.org/NET/ssnx/qu/qu-rec20"/>
        <rdfs:label>Specific Entropy</rdfs:label>
    </owl:Class>
    


    <!-- http://purl.oclc.org/NET/ssnx/qu/dim#StressOrPressure -->


    <owl:Class rdf:about="http://purl.oclc.org/NET/ssnx/qu/dim#StressOrPressure">
        <rdfs:subClassOf rdf:resource="http://purl.oclc.org/NET/ssnx/qu/qu#QuantityKind"/>
        <rdfs:comment>A StressOrPressure is something that is a QuantityKind and has a unitKind property who must be a StressOrPressureUnit</rdfs:comment>
        <rdfs:isDefinedBy rdf:resource="http://purl.oclc.org/NET/ssnx/qu/qu-rec20"/>
        <rdfs:label>Stress Or Pressure</rdfs:label>
    </owl:Class>
    


    <!-- http://purl.oclc.org/NET/ssnx/qu/dim#SurfaceDensity -->


    <owl:Class rdf:about="http://purl.oclc.org/NET/ssnx/qu/dim#SurfaceDensity">
        <rdfs:subClassOf rdf:resource="http://purl.oclc.org/NET/ssnx/qu/qu#QuantityKind"/>
        <rdfs:comment>A SurfaceDensity is something that is a QuantityKind and has a unitKind property who must be a SurfaceDensityUnit</rdfs:comment>
        <rdfs:isDefinedBy rdf:resource="http://purl.oclc.org/NET/ssnx/qu/qu-rec20"/>
        <rdfs:label>Surface Density</rdfs:label>
    </owl:Class>
    


    <!-- http://purl.oclc.org/NET/ssnx/qu/dim#Temperature -->


    <owl:Class rdf:about="http://purl.oclc.org/NET/ssnx/qu/dim#Temperature">
        <rdfs:subClassOf rdf:resource="http://purl.oclc.org/NET/ssnx/qu/qu#QuantityKind"/>
        <rdfs:comment>A Temperature is something that is a QuantityKind and has a unitKind property who must be a TemperatureUnit</rdfs:comment>
        <rdfs:isDefinedBy rdf:resource="http://purl.oclc.org/NET/ssnx/qu/qu-rec20"/>
        <rdfs:label>Temperature</rdfs:label>
    </owl:Class>
    


    <!-- http://purl.oclc.org/NET/ssnx/qu/dim#ThermalConductivity -->


    <owl:Class rdf:about="http://purl.oclc.org/NET/ssnx/qu/dim#ThermalConductivity">
        <rdfs:subClassOf rdf:resource="http://purl.oclc.org/NET/ssnx/qu/qu#QuantityKind"/>
        <rdfs:comment>A ThermalConductivity is something that is a QuantityKind and has a unitKind property who must be a ThermalConductivityUnit</rdfs:comment>
        <rdfs:isDefinedBy rdf:resource="http://purl.oclc.org/NET/ssnx/qu/qu-rec20"/>
        <rdfs:label>Thermal Conductivity</rdfs:label>
    </owl:Class>
    


    <!-- http://purl.oclc.org/NET/ssnx/qu/dim#VelocityOrSpeed -->


    <owl:Class rdf:about="http://purl.oclc.org/NET/ssnx/qu/dim#VelocityOrSpeed">
        <rdfs:subClassOf rdf:resource="http://purl.oclc.org/NET/ssnx/qu/qu#QuantityKind"/>
        <rdfs:comment>A VelocityOrSpeed is something that is a QuantityKind and has a unitKind property who must be a VelocityOrSpeedUnit</rdfs:comment>
        <rdfs:isDefinedBy rdf:resource="http://purl.oclc.org/NET/ssnx/qu/qu-rec20"/>
        <rdfs:label>Velocity Or Speed</rdfs:label>
    </owl:Class>
    


    <!-- http://purl.oclc.org/NET/ssnx/qu/qu#PropertyKind -->


    <owl:Class rdf:about="http://purl.oclc.org/NET/ssnx/qu/qu#PropertyKind">
        <rdfs:comment>A PropertyKind is a meta-property which helps to characterise categories of properties e.g. scalar, vector</rdfs:comment>
        <rdfs:isDefinedBy rdf:resource="http://purl.oclc.org/NET/ssnx/qu/qu-rec20"/>
        <rdfs:label>PropertyKind</rdfs:label>
    </owl:Class>
    


    <!-- http://purl.oclc.org/NET/ssnx/qu/qu#QuantityKind -->


    <owl:Class rdf:about="http://purl.oclc.org/NET/ssnx/qu/qu#QuantityKind">
        <owl:equivalentClass rdf:resource="http://qudt.org/schema/qudt/QuantityKind"/>
        <rdfs:comment>A QuantityKind is an abstract classifier that represents the [VIM] concept of kind of quantity that is defined as aspect common to mutually comparable quantities. A QuantityKind represents the essence of a quantity without any numerical value or unit. Quantities of the same kind within a given system of quantities have the same quantity dimension. However, quantities of the same dimension are not necessarily of the same kind.</rdfs:comment>
        <rdfs:isDefinedBy rdf:resource="http://purl.oclc.org/NET/ssnx/qu/qu-rec20"/>
        <rdfs:label>QuantityKind</rdfs:label>
    </owl:Class>
    


    <!-- http://purl.oclc.org/NET/ssnx/qu/qu#Unit -->


    <owl:Class rdf:about="http://purl.oclc.org/NET/ssnx/qu/qu#Unit">
        <owl:equivalentClass rdf:resource="http://qudt.org/schema/qudt/Unit"/>
    </owl:Class>
    


    <!-- http://purl.org/linked-data/cube#Attachable -->


    <owl:Class rdf:about="http://purl.org/linked-data/cube#Attachable">
        <rdfs:comment xml:lang="en">Abstract superclass for everything that can have attributes and dimensions</rdfs:comment>
        <rdfs:isDefinedBy rdf:resource="http://purl.org/linked-data/cube"/>
        <rdfs:label xml:lang="en">Attachable (abstract)</rdfs:label>
    </owl:Class>
    


    <!-- http://purl.org/linked-data/cube#AttributeProperty -->


    <owl:Class rdf:about="http://purl.org/linked-data/cube#AttributeProperty">
        <rdfs:subClassOf rdf:resource="http://purl.org/linked-data/cube#ComponentProperty"/>
        <owl:disjointWith rdf:resource="http://purl.org/linked-data/cube#MeasureProperty"/>
        <rdfs:comment xml:lang="en">The class of components which represent attributes of observations in the cube, e.g. unit of measurement</rdfs:comment>
        <rdfs:isDefinedBy rdf:resource="http://purl.org/linked-data/cube"/>
        <rdfs:label xml:lang="en">Attribute property</rdfs:label>
    </owl:Class>
    


    <!-- http://purl.org/linked-data/cube#CodedProperty -->


    <owl:Class rdf:about="http://purl.org/linked-data/cube#CodedProperty">
        <rdfs:subClassOf rdf:resource="http://purl.org/linked-data/cube#ComponentProperty"/>
        <rdfs:comment xml:lang="en">Superclass of all coded ComponentProperties</rdfs:comment>
        <rdfs:isDefinedBy rdf:resource="http://purl.org/linked-data/cube"/>
        <rdfs:label xml:lang="en">Coded property</rdfs:label>
    </owl:Class>
    


    <!-- http://purl.org/linked-data/cube#ComponentProperty -->


    <owl:Class rdf:about="http://purl.org/linked-data/cube#ComponentProperty">
        <rdfs:subClassOf rdf:resource="http://www.w3.org/1999/02/22-rdf-syntax-ns#Property"/>
        <rdfs:comment xml:lang="en">Abstract super-property of all properties representing dimensions, attributes or measures</rdfs:comment>
        <rdfs:isDefinedBy rdf:resource="http://purl.org/linked-data/cube"/>
        <rdfs:label xml:lang="en">Component property (abstract)</rdfs:label>
    </owl:Class>
    


    <!-- http://purl.org/linked-data/cube#ComponentSet -->


    <owl:Class rdf:about="http://purl.org/linked-data/cube#ComponentSet">
        <rdfs:comment xml:lang="en">Abstract class of things which reference one or more ComponentProperties</rdfs:comment>
        <rdfs:isDefinedBy rdf:resource="http://purl.org/linked-data/cube"/>
        <rdfs:label xml:lang="en">Component set</rdfs:label>
    </owl:Class>
    


    <!-- http://purl.org/linked-data/cube#ComponentSpecification -->


    <owl:Class rdf:about="http://purl.org/linked-data/cube#ComponentSpecification">
        <rdfs:subClassOf rdf:resource="http://purl.org/linked-data/cube#ComponentSet"/>
        <rdfs:comment xml:lang="en">Used to define properties of a component (attribute, dimension etc) which are specific to its usage in a DSD.</rdfs:comment>
        <rdfs:isDefinedBy rdf:resource="http://purl.org/linked-data/cube"/>
        <rdfs:label xml:lang="en">Component specification</rdfs:label>
    </owl:Class>
    


    <!-- http://purl.org/linked-data/cube#DataSet -->


    <owl:Class rdf:about="http://purl.org/linked-data/cube#DataSet">
        <rdfs:comment xml:lang="en">Represents a collection of observations, possibly organized into various slices, conforming to some common dimensional structure.</rdfs:comment>
        <rdfs:isDefinedBy rdf:resource="http://purl.org/linked-data/cube"/>
        <rdfs:label xml:lang="en">Data set</rdfs:label>
    </owl:Class>
    


    <!-- http://purl.org/linked-data/cube#DataStructureDefinition -->


    <owl:Class rdf:about="http://purl.org/linked-data/cube#DataStructureDefinition">
        <rdfs:subClassOf rdf:resource="http://purl.org/linked-data/cube#ComponentSet"/>
        <rdfs:comment xml:lang="en">Defines the structure of a DataSet or slice</rdfs:comment>
        <rdfs:isDefinedBy rdf:resource="http://purl.org/linked-data/cube"/>
        <rdfs:label xml:lang="en">Data structure definition</rdfs:label>
    </owl:Class>
    


    <!-- http://purl.org/linked-data/cube#DimensionProperty -->


    <owl:Class rdf:about="http://purl.org/linked-data/cube#DimensionProperty">
        <rdfs:subClassOf rdf:resource="http://purl.org/linked-data/cube#CodedProperty"/>
        <rdfs:subClassOf rdf:resource="http://purl.org/linked-data/cube#ComponentProperty"/>
        <owl:disjointWith rdf:resource="http://purl.org/linked-data/cube#MeasureProperty"/>
        <rdfs:comment xml:lang="en">The class of components which represent the dimensions of the cube</rdfs:comment>
        <rdfs:isDefinedBy rdf:resource="http://purl.org/linked-data/cube"/>
        <rdfs:label xml:lang="en">Dimension property</rdfs:label>
    </owl:Class>
    


    <!-- http://purl.org/linked-data/cube#MeasureProperty -->


    <owl:Class rdf:about="http://purl.org/linked-data/cube#MeasureProperty">
        <rdfs:subClassOf rdf:resource="http://purl.org/linked-data/cube#ComponentProperty"/>
        <rdfs:comment xml:lang="en">The class of components which represent the measured value of the phenomenon being observed</rdfs:comment>
        <rdfs:isDefinedBy rdf:resource="http://purl.org/linked-data/cube"/>
        <rdfs:label xml:lang="en">Measure property</rdfs:label>
    </owl:Class>
    


    <!-- http://purl.org/linked-data/cube#Observation -->


    <owl:Class rdf:about="http://purl.org/linked-data/cube#Observation">
        <rdfs:subClassOf rdf:resource="http://purl.org/linked-data/cube#Attachable"/>
        <rdfs:comment xml:lang="en">A single observation in the cube, may have one or more associated measured values</rdfs:comment>
        <rdfs:isDefinedBy rdf:resource="http://purl.org/linked-data/cube"/>
        <rdfs:label xml:lang="en">Observation</rdfs:label>
    </owl:Class>
    


    <!-- http://purl.org/linked-data/cube#ObservationGroup -->


    <owl:Class rdf:about="http://purl.org/linked-data/cube#ObservationGroup">
        <rdfs:comment xml:lang="en">A, possibly arbitrary, group of observations.</rdfs:comment>
        <rdfs:isDefinedBy rdf:resource="http://purl.org/linked-data/cube"/>
        <rdfs:label xml:lang="en">Observation Group</rdfs:label>
    </owl:Class>
    


    <!-- http://purl.org/linked-data/cube#Slice -->


    <owl:Class rdf:about="http://purl.org/linked-data/cube#Slice">
        <rdfs:subClassOf rdf:resource="http://purl.org/linked-data/cube#Attachable"/>
        <rdfs:subClassOf rdf:resource="http://purl.org/linked-data/cube#ObservationGroup"/>
        <rdfs:comment xml:lang="en">Denotes a subset of a DataSet defined by fixing a subset of the dimensional values, component properties on the Slice</rdfs:comment>
        <rdfs:isDefinedBy rdf:resource="http://purl.org/linked-data/cube"/>
        <rdfs:label xml:lang="en">Slice</rdfs:label>
    </owl:Class>
    


    <!-- http://purl.org/linked-data/cube#SliceKey -->


    <owl:Class rdf:about="http://purl.org/linked-data/cube#SliceKey">
        <rdfs:subClassOf rdf:resource="http://purl.org/linked-data/cube#ComponentSet"/>
        <rdfs:comment xml:lang="en">Denotes a subset of the component properties of a DataSet which are fixed in the corresponding slices</rdfs:comment>
        <rdfs:isDefinedBy rdf:resource="http://purl.org/linked-data/cube"/>
        <rdfs:label xml:lang="en">Slice key</rdfs:label>
    </owl:Class>
    


    <!-- http://qudt.org/schema/qudt/Quantity -->


    <owl:Class rdf:about="http://qudt.org/schema/qudt/Quantity">
        <rdfs:comment xml:lang="en">
A quantity is the measurement of an observable property of a particular object, event, or physical system. A quantity is always associated with the context of measurement (i.e. the thing measured, the measured value, the accuracy of measurement, etc.) whereas the underlying quantity kind is independent of any particular measurement. Thus, length is a quantity kind while the height of a rocket is a specific quantity of length; its magnitude that may be expressed in meters, feet, inches, etc. Examples of physical quantities include physical constants, such as the speed of light in a vacuum, Planck&apos;s constant, the electric permittivity of free space, and the fine structure constant.

In other words, quantities are quantifiable aspects of the world, such as the duration of a movie, the distance between two points, velocity of a car, the pressure of the atmosphere, and a person&apos;s weight; and units are used to describe their numerical measure.

Many quantity kinds are related to each other by various physical laws, and as a result, the associated units of some quantity kinds can be expressed as products (or ratios) of powers of other quantity kinds (e.g., momentum is mass times velocity and velocity is defined as distance divided by time). In this way, some quantities can be calculated from other measured quantities using their associations to the quantity kinds in these expressions. These quantity kind relationships are also discussed in dimensional analysis. Those that cannot be so expressed can be regarded as &quot;fundamental&quot; in this sense.

A quantity is distinguished from a &quot;quantity kind&quot; in that the former carries a value and the latter is a type specifier.
    </rdfs:comment>
        <rdfs:isDefinedBy rdf:resource="http://qudt.org/2.1/schema/qudt"/>
        <rdfs:label>Quantity</rdfs:label>
    </owl:Class>
    


    <!-- http://qudt.org/schema/qudt/QuantityKind -->


    <owl:Class rdf:about="http://qudt.org/schema/qudt/QuantityKind">
        <rdfs:comment>A Quantity Kind is any observable property that can be measured and quantified numerically. Familiar examples include physical properties such as length, mass, time, force, energy, power, electric charge, etc. Less familiar examples include currency, interest rate, price to earning ratio, and information capacity.</rdfs:comment>
        <rdfs:isDefinedBy rdf:resource="http://qudt.org/2.1/schema/qudt"/>
        <rdfs:label>Quantity Kind</rdfs:label>
    </owl:Class>
    


    <!-- http://qudt.org/schema/qudt/QuantityValue -->


    <owl:Class rdf:about="http://qudt.org/schema/qudt/QuantityValue">
        <rdfs:comment>A Quantity Value expresses the magnitude and kind of a quantity and is given by the product of a numerical value n and a unit of measure U. The number multiplying the unit is referred to as the numerical value of the quantity expressed in that unit. Refer to NIST SP 811 section 7 for more on quantity values.</rdfs:comment>
        <rdfs:isDefinedBy rdf:resource="http://qudt.org/2.1/schema/qudt"/>
        <rdfs:label>Quantity value</rdfs:label>
    </owl:Class>
    


    <!-- http://qudt.org/schema/qudt/Unit -->


    <owl:Class rdf:about="http://qudt.org/schema/qudt/Unit">
        <rdfs:comment>A unit of measure, or unit, is a particular quantity value that has been chosen as a scale for measuring other quantities the same kind (more generally of equivalent dimension). For example, the meter is a quantity of length that has been rigorously defined and standardized by the BIPM (International Board of Weights and Measures). Any measurement of the length can be expressed as a number multiplied by the unit meter. More formally, the value of a physical quantity Q with respect to a unit (U) is expressed as the scalar multiple of a real number (n)</rdfs:comment>
        <rdfs:isDefinedBy rdf:resource="http://qudt.org/2.1/schema/qudt"/>
        <rdfs:label>Unit</rdfs:label>
    </owl:Class>
    


    <!-- http://www.opengis.net/ont/geosparql#Feature -->


    <owl:Class rdf:about="http://www.opengis.net/ont/geosparql#Feature">
        <rdfs:subClassOf rdf:resource="http://www.opengis.net/ont/geosparql#SpatialObject"/>
        <rdfs:subClassOf>
            <owl:Restriction>
                <owl:onProperty rdf:resource="http://www.opengis.net/ont/geosparql#hasGeometry"/>
                <owl:allValuesFrom rdf:resource="http://www.opengis.net/ont/geosparql#Geometry"/>
            </owl:Restriction>
        </rdfs:subClassOf>
        <owl:disjointWith rdf:resource="http://www.opengis.net/ont/geosparql#Geometry"/>
        <terms:contributor>Matthew Perry</terms:contributor>
        <terms:creator>OGC GeoSPARQL 1.0 Standard Working Group</terms:creator>
        <terms:date rdf:datatype="http://www.w3.org/2001/XMLSchema#date">2011-06-16</terms:date>
        <terms:description xml:lang="en">
      This class represents the top-level feature type. This class is 
      equivalent to GFI_Feature defined in ISO 19156:2011, and it is 
      superclass of all feature types.
    </terms:description>
        <rdfs:comment xml:lang="en">
      This class represents the top-level feature type. This class is 
      equivalent to GFI_Feature defined in ISO 19156:2011, and it is 
      superclass of all feature types.
    </rdfs:comment>
        <rdfs:isDefinedBy rdf:resource="http://www.opengis.net/ont/geosparql"/>
        <rdfs:isDefinedBy rdf:resource="http://www.opengis.net/spec/geosparql/1.0"/>
        <rdfs:label xml:lang="en">Feature</rdfs:label>
        <skos:definition xml:lang="en">
      This class represents the top-level feature type. This class is 
      equivalent to GFI_Feature defined in ISO 19156:2011, and it is 
      superclass of all feature types.
    </skos:definition>
        <skos:prefLabel xml:lang="en">Feature</skos:prefLabel>
    </owl:Class>
    


    <!-- http://www.opengis.net/ont/geosparql#Geometry -->


    <owl:Class rdf:about="http://www.opengis.net/ont/geosparql#Geometry">
        <rdfs:subClassOf rdf:resource="http://www.opengis.net/ont/geosparql#SpatialObject"/>
        <terms:contributor>Matthew Perry</terms:contributor>
        <terms:creator>OGC GeoSPARQL 1.0 Standard Working Group</terms:creator>
        <terms:date rdf:datatype="http://www.w3.org/2001/XMLSchema#date">2011-06-16</terms:date>
        <terms:description xml:lang="en">
      The class represents the top-level geometry type. This class is 
      equivalent to the UML class GM_Object defined in ISO 19107, and 
      it is superclass of all geometry types.
    </terms:description>
        <rdfs:comment xml:lang="en">
      The class represents the top-level geometry type. This class is 
      equivalent to the UML class GM_Object defined in ISO 19107, and 
      it is superclass of all geometry types.
    </rdfs:comment>
        <rdfs:isDefinedBy rdf:resource="http://www.opengis.net/ont/geosparql"/>
        <rdfs:isDefinedBy rdf:resource="http://www.opengis.net/spec/geosparql/1.0"/>
        <rdfs:label xml:lang="en">Geometry</rdfs:label>
        <skos:definition xml:lang="en">
      The class represents the top-level geometry type. This class is 
      equivalent to the UML class GM_Object defined in ISO 19107, and 
      it is superclass of all geometry types.
    </skos:definition>
        <skos:prefLabel xml:lang="en">Geometry</skos:prefLabel>
    </owl:Class>
    


    <!-- http://www.opengis.net/ont/geosparql#SpatialObject -->


    <owl:Class rdf:about="http://www.opengis.net/ont/geosparql#SpatialObject">
        <rdfs:subClassOf>
            <owl:Restriction>
                <owl:onProperty rdf:resource="http://www.opengis.net/ont/geosparql#hasGeometry"/>
                <owl:allValuesFrom rdf:resource="http://www.opengis.net/ont/geosparql#Geometry"/>
            </owl:Restriction>
        </rdfs:subClassOf>
        <rdfs:subClassOf>
            <owl:Restriction>
                <owl:onProperty rdf:resource="http://www.opengis.net/ont/geosparql#sfContains"/>
                <owl:allValuesFrom rdf:resource="http://www.opengis.net/ont/geosparql#SpatialObject"/>
            </owl:Restriction>
        </rdfs:subClassOf>
        <rdfs:subClassOf>
            <owl:Restriction>
                <owl:onProperty rdf:resource="http://www.opengis.net/ont/geosparql#sfWithin"/>
                <owl:allValuesFrom rdf:resource="http://www.opengis.net/ont/geosparql#SpatialObject"/>
            </owl:Restriction>
        </rdfs:subClassOf>
        <rdfs:comment xml:lang="en">The class spatial-object represents everything that can have a spatial representation. It is superclass of feature and geometry.</rdfs:comment>
        <rdfs:isDefinedBy rdf:resource="http://www.opengis.net/ont/geosparql"/>
        <rdfs:label xml:lang="en">SpatialObject</rdfs:label>
    </owl:Class>
    


    <!-- http://www.opengis.net/ont/sf#Curve -->


    <owl:Class rdf:about="http://www.opengis.net/ont/sf#Curve">
        <rdfs:subClassOf rdf:resource="http://www.opengis.net/ont/sf#Geometry"/>
        <rdfs:comment xml:lang="en">
A Curve is a 1-dimensional geometric object usually stored as a sequence of Points, with the subtype of Curve specifying the form of the interpolation between Points. This specification defines only one subclass of Curve, LineString, which uses linear interpolation between Points.
A Curve is a 1-dimensional geometric object that is the homeomorphic image of a real, closed, interval.
A Curve is simple if it does not pass through the same Point twice with the possible exception of the two end
points.
A Curve is closed if its start Point is equal to its end Point.
The boundary of a closed Curve is empty.
A Curve that is simple and closed is a Ring.
The boundary of a non-closed Curve consists of its two end Points.
A Curve is defined as topologically closed, that is, it contains its endpoints f(a) and f(b).
    </rdfs:comment>
        <rdfs:isDefinedBy rdf:resource="http://www.opengis.net/ont/sf"/>
        <rdfs:label xml:lang="en">Curve</rdfs:label>
    </owl:Class>
    


    <!-- http://www.opengis.net/ont/sf#Geometry -->


    <owl:Class rdf:about="http://www.opengis.net/ont/sf#Geometry">
        <rdfs:subClassOf rdf:resource="http://www.opengis.net/ont/geosparql#Geometry"/>
        <rdfs:comment xml:lang="en">
Geometry is the root class of the hierarchy.
The instantiable subclasses of Geometry are restricted to 0, 1 and 2-dimensional geometric objects that exist in 2, 3 or 4-dimensional coordinate space (R2, R3 or R4). Geometry values in R2 have points with coordinate values for x and y. Geometry values in R3 have points with coordinate values for x, y and z or for x, y and m. Geometry values in R4 have points with coordinate values for x, y, z and m.
The interpretation of the coordinates is subject to the coordinate reference systems associated to the point. All coordinates within a geometry object should be in the same coordinate reference systems. Each coordinate shall be unambiguously associated to a coordinate reference system either directly or through its containing geometry. The z coordinate of a point is typically, but not necessarily, represents altitude or elevation. The m coordinate represents a measurement.
All Geometry classes described in this specification are defined so that instances of Geometry are topologically closed, i.e. all represented geometries include their boundary as point sets. This does not affect their representation, and open version of the same classes may be used in other circumstances, such as topological representations.
    </rdfs:comment>
        <rdfs:isDefinedBy rdf:resource="http://www.opengis.net/ont/sf"/>
        <rdfs:label xml:lang="en">Geometry</rdfs:label>
    </owl:Class>
    


    <!-- http://www.opengis.net/ont/sf#GeometryCollection -->


    <owl:Class rdf:about="http://www.opengis.net/ont/sf#GeometryCollection">
        <rdfs:subClassOf rdf:resource="http://www.opengis.net/ont/sf#Geometry"/>
        <rdfs:comment xml:lang="en">
A GeometryCollection is a geometric object that is a collection of some number of geometric objects.
All the elements in a GeometryCollection shall be in the same Spatial Reference System. This is also the Spatial Reference System for the GeometryCollection.
GeometryCollection places no other constraints on its elements. Subclasses of GeometryCollection may restrict membership based on dimension and may also place other constraints on the degree of spatial overlap between elements.
    </rdfs:comment>
        <rdfs:isDefinedBy rdf:resource="http://www.opengis.net/ont/sf"/>
        <rdfs:label xml:lang="en">Geometry Collection</rdfs:label>
    </owl:Class>
    


    <!-- http://www.opengis.net/ont/sf#Line -->


    <owl:Class rdf:about="http://www.opengis.net/ont/sf#Line">
        <rdfs:subClassOf rdf:resource="http://www.opengis.net/ont/sf#LineString"/>
        <rdfs:comment xml:lang="en">
A Line is a LineString with exactly 2 Points.
    </rdfs:comment>
        <rdfs:isDefinedBy rdf:resource="http://www.opengis.net/ont/sf"/>
        <rdfs:label xml:lang="en">Line</rdfs:label>
    </owl:Class>
    


    <!-- http://www.opengis.net/ont/sf#LineString -->


    <owl:Class rdf:about="http://www.opengis.net/ont/sf#LineString">
        <rdfs:subClassOf rdf:resource="http://www.opengis.net/ont/sf#Curve"/>
        <rdfs:comment xml:lang="en">
A LineString is a Curve with linear interpolation between Points. Each consecutive pair of Points defines a Line segment.
    </rdfs:comment>
        <rdfs:isDefinedBy rdf:resource="http://www.opengis.net/ont/sf"/>
        <rdfs:label xml:lang="en">Line String</rdfs:label>
    </owl:Class>
    


    <!-- http://www.opengis.net/ont/sf#LinearRing -->


    <owl:Class rdf:about="http://www.opengis.net/ont/sf#LinearRing">
        <rdfs:subClassOf rdf:resource="http://www.opengis.net/ont/sf#LineString"/>
        <rdfs:comment xml:lang="en">
A LinearRing is a LineString that is both closed and simple.
    </rdfs:comment>
        <rdfs:isDefinedBy rdf:resource="http://www.opengis.net/ont/sf"/>
        <rdfs:label xml:lang="en">Linear Ring</rdfs:label>
    </owl:Class>
    


    <!-- http://www.opengis.net/ont/sf#MultiCurve -->


    <owl:Class rdf:about="http://www.opengis.net/ont/sf#MultiCurve">
        <rdfs:subClassOf rdf:resource="http://www.opengis.net/ont/sf#GeometryCollection"/>
        <rdfs:comment xml:lang="en">
A MultiCurve is a 1-dimensional GeometryCollection whose elements are Curves.
A MultiCurve defines a set of methods for its subclasses and is included for reasons of extensibility.
A MultiCurve is simple if and only if all of its elements are simple and the only intersections between any two elements occur at Points that are on the boundaries of both elements.
The boundary of a MultiCurve is obtained by applying the mod 2 union rule: A Point is in the boundary of a MultiCurve if it is in the boundaries of an odd number of elements of the MultiCurve.
A MultiCurve is closed if all of its elements are closed. The boundary of a closed MultiCurve is always empty.
A MultiCurve is defined as topologically closed.
    </rdfs:comment>
        <rdfs:isDefinedBy rdf:resource="http://www.opengis.net/ont/sf"/>
        <rdfs:label xml:lang="en">Multi Curve</rdfs:label>
    </owl:Class>
    


    <!-- http://www.opengis.net/ont/sf#MultiLineString -->


    <owl:Class rdf:about="http://www.opengis.net/ont/sf#MultiLineString">
        <rdfs:subClassOf rdf:resource="http://www.opengis.net/ont/sf#MultiCurve"/>
        <rdfs:comment xml:lang="en">
A MultiLineString is a MultiCurve whose elements are LineStrings.
    </rdfs:comment>
        <rdfs:isDefinedBy rdf:resource="http://www.opengis.net/ont/sf"/>
        <rdfs:label xml:lang="en">Multi Line String</rdfs:label>
    </owl:Class>
    


    <!-- http://www.opengis.net/ont/sf#MultiPoint -->


    <owl:Class rdf:about="http://www.opengis.net/ont/sf#MultiPoint">
        <rdfs:subClassOf rdf:resource="http://www.opengis.net/ont/sf#GeometryCollection"/>
        <rdfs:comment xml:lang="en">
A MultiPoint is a 0-dimensional GeometryCollection. The elements of a MultiPoint are restricted to Points. ThePoints are not connected or ordered in any semantically important way.
A MultiPoint is simple if no two Points in the MultiPoint are equal (have identical coordinate values in X and Y).
Every MultiPoint is spatially equal to a simple Multipoint.
The boundary of a MultiPoint is the empty set.
    </rdfs:comment>
        <rdfs:isDefinedBy rdf:resource="http://www.opengis.net/ont/sf"/>
        <rdfs:label xml:lang="en">Multi Point</rdfs:label>
    </owl:Class>
    


    <!-- http://www.opengis.net/ont/sf#MultiPolygon -->


    <owl:Class rdf:about="http://www.opengis.net/ont/sf#MultiPolygon">
        <rdfs:subClassOf rdf:resource="http://www.opengis.net/ont/sf#MultiSurface"/>
        <rdfs:comment xml:lang="en">
A MultiPolygon is a MultiSurface whose elements are Polygons.
The assertions for MultiPolygons are as follows.
a) The interiors of 2 Polygons that are elements of a MultiPolygon may not intersect.
b) The boundaries of any 2 Polygons that are elements of a MultiPolygon may not cross and may touch at only a finite number of Points.
c) A MultiPolygon is defined as topologically closed.
d) A MultiPolygon may not have cut lines, spikes or punctures, a MultiPolygon is a regular closed Point set,
e) The interior of a MultiPolygon with more than 1 Polygon is not connected; the number of connected components of the interior of a MultiPolygon is equal to the number of Polygons in the MultiPolygon. 
The boundary of a MultiPolygon is a set of closed Curves (LineStrings) corresponding to the boundaries of its element Polygons. Each Curve in the boundary of the MultiPolygon is in the boundary of exactly 1 element Polygon, and every Curve in the boundary of an element Polygon is in the boundary of the MultiPolygon.
    </rdfs:comment>
        <rdfs:isDefinedBy rdf:resource="http://www.opengis.net/ont/sf"/>
        <rdfs:label xml:lang="en">Multi Polygon</rdfs:label>
    </owl:Class>
    


    <!-- http://www.opengis.net/ont/sf#MultiSurface -->


    <owl:Class rdf:about="http://www.opengis.net/ont/sf#MultiSurface">
        <rdfs:subClassOf rdf:resource="http://www.opengis.net/ont/sf#GeometryCollection"/>
        <rdfs:comment xml:lang="en">
A MultiSurface is a 2-dimensional GeometryCollection whose elements are Surfaces, all using coordinates from the same coordinate reference system. The geometric interiors of any two Surfaces in a MultiSurface may not intersect in the full coordinate system. The boundaries of any two coplanar elements in a MultiSurface may intersect, at most, at a finite number of Points. If they were to meet along a curve, they could be merged into a single surface.
A MultiSurface may be used to represent heterogeneous surfaces collections of polygons and polyhedral surfaces. It defines a set of methods for its subclasses. The subclass of MultiSurface is MultiPolygon corresponding to a collection of Polygons only. Other collections shall use MultiSurface.
    </rdfs:comment>
        <rdfs:isDefinedBy rdf:resource="http://www.opengis.net/ont/sf"/>
        <rdfs:label xml:lang="en">Multi Surface</rdfs:label>
    </owl:Class>
    


    <!-- http://www.opengis.net/ont/sf#Point -->


    <owl:Class rdf:about="http://www.opengis.net/ont/sf#Point">
        <rdfs:subClassOf rdf:resource="http://www.opengis.net/ont/sf#Geometry"/>
        <rdfs:comment xml:lang="en">
A Point is a 0-dimensional geometric object and represents a single location in coordinate space. 
A Point has an x-coordinate value, a y-coordinate value. If called for by the associated Spatial Reference System, it may also have coordinate values for z and m.
The boundary of a Point is the empty set.
    </rdfs:comment>
        <rdfs:isDefinedBy rdf:resource="http://www.opengis.net/ont/sf"/>
        <rdfs:label xml:lang="en">Point</rdfs:label>
    </owl:Class>
    


    <!-- http://www.opengis.net/ont/sf#Polygon -->


    <owl:Class rdf:about="http://www.opengis.net/ont/sf#Polygon">
        <rdfs:subClassOf rdf:resource="http://www.opengis.net/ont/sf#Surface"/>
        <rdfs:comment xml:lang="en">
A Polygon is a planar Surface defined by 1 exterior boundary and 0 or more interior boundaries. Each interior boundary defines a hole in the Polygon.
The exterior boundary LinearRing defines the top of the surface which is the side of the surface from which the exterior boundary appears to traverse the boundary in a counter clockwise direction. The interior LinearRings will have the opposite orientation, and appear as clockwise when viewed from the top,
The assertions for Polygons (the rules that define valid Polygons) are as follows:
a) Polygons are topologically closed;
b) The boundary of a Polygon consists of a set of LinearRings that make up its exterior and interior boundaries;
c) No two Rings in the boundary cross and the Rings in the boundary of a Polygon may intersect at a Point but only as a tangent.
d) A Polygon may not have cut lines, spikes or punctures.
e) The interior of every Polygon is a connected point set;
f) The exterior of a Polygon with 1 or more holes is not connected. Each hole defines a connected component of the exterior.
    </rdfs:comment>
        <rdfs:isDefinedBy rdf:resource="http://www.opengis.net/ont/sf"/>
        <rdfs:label xml:lang="en">Polygon</rdfs:label>
    </owl:Class>
    


    <!-- http://www.opengis.net/ont/sf#PolyhedralSurface -->


    <owl:Class rdf:about="http://www.opengis.net/ont/sf#PolyhedralSurface">
        <rdfs:subClassOf rdf:resource="http://www.opengis.net/ont/sf#Surface"/>
        <rdfs:comment xml:lang="en">
A PolyhedralSurface is a contiguous collection of polygons, which share common boundary segments. For each pair of polygons that touch, the common boundary shall be expressible as a finite collection of LineStrings. Each such LineString shall be part of the boundary of at most 2 Polygon patches. 
For any two polygons that share a common boundary, the top of the polygon shall be consistent. This means that when two LinearRings from these two Polygons traverse the common boundary segment, they do so in opposite directions. Since the Polyhedral surface is contiguous, all polygons will be thus consistently oriented. This means that a non-oriented surface (such as Mbius band) shall not have single surface representations. They may be represented by a MultiSurface.
If each such LineString is the boundary of exactly 2 Polygon patches, then the PolyhedralSurface is a simple, closed polyhedron and is topologically isomorphic to the surface of a sphere. By the Jordan Surface Theorem (Jordans Theorem for 2-spheres), such polyhedrons enclose a solid topologically isomorphic to the interior of a sphere; the ball. In this case, the top of the surface will either point inward or outward of the enclosed finite solid. If outward, the surface is the exterior boundary of the enclosed surface. If inward, the surface is the interior of the infinite complement of the enclosed solid. A Ball with some number of voids (holes) inside can thus be presented as one exterior boundary shell, and some number in interior boundary shells.
    </rdfs:comment>
        <rdfs:isDefinedBy rdf:resource="http://www.opengis.net/ont/sf"/>
        <rdfs:label xml:lang="en">Polyhedral Surface</rdfs:label>
    </owl:Class>
    


    <!-- http://www.opengis.net/ont/sf#Surface -->


    <owl:Class rdf:about="http://www.opengis.net/ont/sf#Surface">
        <rdfs:subClassOf rdf:resource="http://www.opengis.net/ont/sf#Geometry"/>
        <rdfs:comment xml:lang="en">
A Surface is a 2-dimensional geometric object.
A simple Surface may consists of a single patch that is associated with one exterior boundary and 0 or more interior boundaries. A single such Surface patch in 3-dimensional space is isometric to planar Surfaces, by a simple affine rotation matrix that rotates the patch onto the plane z = 0. If the patch is not vertical, the projection onto the same plane is an isomorphism, and can be represented as a linear transformation, i.e. an affine.
Polyhedral Surfaces are formed by stitching together such simple Surfaces patches along their common boundaries. Such polyhedral Surfaces in a 3-dimensional space may not be planar as a whole, depending on the orientation of their planar normals. If all the patches are in alignment (their normals are parallel), then the whole stitched polyhedral surface is co-planar and can be represented as a single patch if it is connected.
The boundary of a simple Surface is the set of closed Curves corresponding to its exterior and interior boundaries.
A Polygon is a simple Surface that is planar. A PolyhedralSurface is a simple surface, consisting of some number of Polygon patches or facets. If a PolyhedralSurface is closed, then it bounds a solid. A MultiSurface containing a set of closed PolyhedralSurfaces can be used to represent a Solid object with holes.
    </rdfs:comment>
        <rdfs:isDefinedBy rdf:resource="http://www.opengis.net/ont/sf"/>
        <rdfs:label xml:lang="en">Surface</rdfs:label>
    </owl:Class>
    


    <!-- http://www.opengis.net/ont/sf#TIN -->


    <owl:Class rdf:about="http://www.opengis.net/ont/sf#TIN">
        <rdfs:subClassOf rdf:resource="http://www.opengis.net/ont/sf#PolyhedralSurface"/>
        <rdfs:comment xml:lang="en">
A TIN (triangulated irregular network) is a PolyhedralSurface consisting only of Triangle patches.
    </rdfs:comment>
        <rdfs:isDefinedBy rdf:resource="http://www.opengis.net/ont/sf"/>
        <rdfs:label xml:lang="en">Triangulated Irregular Network</rdfs:label>
    </owl:Class>
    


    <!-- http://www.opengis.net/ont/sf#Triangle -->


    <owl:Class rdf:about="http://www.opengis.net/ont/sf#Triangle">
        <rdfs:subClassOf rdf:resource="http://www.opengis.net/ont/sf#Polygon"/>
        <rdfs:comment xml:lang="en">
 A Triangle is a polygon with 3 distinct, non-collinear vertices and no interior boundary.
    </rdfs:comment>
        <rdfs:isDefinedBy rdf:resource="http://www.opengis.net/ont/sf"/>
        <rdfs:label xml:lang="en">Triangle</rdfs:label>
    </owl:Class>
    


    <!-- http://www.w3.org/1999/02/22-rdf-syntax-ns#Property -->


    <owl:Class rdf:about="http://www.w3.org/1999/02/22-rdf-syntax-ns#Property"/>
    


    <!-- http://www.w3.org/2000/01/rdf-schema#Class -->


    <owl:Class rdf:about="http://www.w3.org/2000/01/rdf-schema#Class"/>
    


    <!-- http://www.w3.org/2003/01/geo/wgs84_pos#Point -->


    <owl:Class rdf:about="http://www.w3.org/2003/01/geo/wgs84_pos#Point">
        <rdfs:subClassOf rdf:resource="http://www.opengis.net/ont/geosparql#Geometry"/>
        <rdfs:comment> 
Uniquely identified by lat/long/alt. i.e.

spaciallyIntersects(P1, P2) :- lat(P1, LAT), long(P1, LONG), alt(P1, ALT),
  lat(P2, LAT), long(P2, LONG), alt(P2, ALT).

sameThing(P1, P2) :- type(P1, Point), type(P2, Point), spaciallyIntersects(P1, P2).
  </rdfs:comment>
        <rdfs:comment>A point, typically described using a coordinate system relative to Earth, such as WGS84.</rdfs:comment>
        <rdfs:isDefinedBy rdf:resource="http://www.w3.org/2003/01/geo/wgs84_pos#"/>
        <rdfs:label xml:lang="en">Point</rdfs:label>
    </owl:Class>
    


    <!-- http://www.w3.org/2004/02/skos/core#Concept -->


    <owl:Class rdf:about="http://www.w3.org/2004/02/skos/core#Concept"/>
    


    <!-- http://www.w3.org/2004/02/skos/core#Scheme -->


    <owl:Class rdf:about="http://www.w3.org/2004/02/skos/core#Scheme">
        <rdfs:comment>The Scheme class of SKOS Vocabulary</rdfs:comment>
        <rdfs:isDefinedBy rdf:resource="http://www.w3.org/2004/02/skos/core#"/>
        <rdfs:label>Scheme</rdfs:label>
    </owl:Class>
    


    <!-- http://www.w3.org/2006/time#Duration -->


    <owl:Class rdf:about="http://www.w3.org/2006/time#Duration">
        <rdfs:subClassOf rdf:resource="http://www.w3.org/2006/time#TemporalDuration"/>
        <rdfs:comment xml:lang="en">Duration of a temporal extent expressed as a number scaled by a temporal unit</rdfs:comment>
        <rdfs:isDefinedBy rdf:resource="http://www.w3.org/2006/time#"/>
        <rdfs:label xml:lang="en">Time duration</rdfs:label>
        <skos:definition xml:lang="en">Duration of a temporal extent expressed as a number scaled by a temporal unit</skos:definition>
        <skos:note xml:lang="en">Alternative to time:DurationDescription to support description of a temporal duration other than using a calendar/clock system.</skos:note>
    </owl:Class>
    


    <!-- http://www.w3.org/2006/time#Instant -->


    <owl:Class rdf:about="http://www.w3.org/2006/time#Instant">
        <rdfs:subClassOf rdf:resource="http://www.w3.org/2006/time#TemporalEntity"/>
        <rdfs:comment xml:lang="en">A temporal entity with zero extent or duration</rdfs:comment>
        <rdfs:isDefinedBy rdf:resource="http://www.w3.org/2006/time#"/>
        <rdfs:label xml:lang="en">Time instant</rdfs:label>
        <skos:definition xml:lang="en">A temporal entity with zero extent or duration</skos:definition>
    </owl:Class>
    


    <!-- http://www.w3.org/2006/time#Interval -->


    <owl:Class rdf:about="http://www.w3.org/2006/time#Interval">
        <rdfs:subClassOf rdf:resource="http://www.w3.org/2006/time#TemporalEntity"/>
        <rdfs:comment xml:lang="en">A temporal entity with an extent or duration</rdfs:comment>
        <rdfs:isDefinedBy rdf:resource="http://www.w3.org/2006/time#"/>
        <rdfs:label xml:lang="en">Time interval</rdfs:label>
        <skos:definition xml:lang="en">A temporal entity with an extent or duration</skos:definition>
    </owl:Class>
    


    <!-- http://www.w3.org/2006/time#TemporalDuration -->


    <owl:Class rdf:about="http://www.w3.org/2006/time#TemporalDuration">
        <rdfs:comment xml:lang="en">Time extent; duration of a time interval separate from its particular start position</rdfs:comment>
        <rdfs:isDefinedBy rdf:resource="http://www.w3.org/2006/time#"/>
        <rdfs:label xml:lang="en">Temporal duration</rdfs:label>
        <skos:definition xml:lang="en">Time extent; duration of a time interval separate from its particular start position</skos:definition>
    </owl:Class>
    


    <!-- http://www.w3.org/2006/time#TemporalEntity -->


    <owl:Class rdf:about="http://www.w3.org/2006/time#TemporalEntity">
        <owl:equivalentClass>
            <owl:Class>
                <owl:unionOf rdf:parseType="Collection">
                    <rdf:Description rdf:about="http://www.w3.org/2006/time#Instant"/>
                    <rdf:Description rdf:about="http://www.w3.org/2006/time#Interval"/>
                </owl:unionOf>
            </owl:Class>
        </owl:equivalentClass>
        <rdfs:comment xml:lang="en">A temporal interval or instant.</rdfs:comment>
        <rdfs:isDefinedBy rdf:resource="http://www.w3.org/2006/time#"/>
        <rdfs:label xml:lang="en">Temporal entity</rdfs:label>
        <skos:definition xml:lang="en">A temporal interval or instant.</skos:definition>
    </owl:Class>
    


    <!-- http://www.w3.org/2006/time#TemporalUnit -->


    <owl:Class rdf:about="http://www.w3.org/2006/time#TemporalUnit">
        <rdfs:subClassOf rdf:resource="http://www.w3.org/2006/time#TemporalDuration"/>
        <rdfs:comment xml:lang="en">A standard duration, which provides a scale factor for a time extent, or the granularity or precision for a time position.</rdfs:comment>
        <rdfs:isDefinedBy rdf:resource="http://www.w3.org/2006/time#"/>
        <rdfs:label xml:lang="en">Temporal unit</rdfs:label>
        <skos:definition xml:lang="en">A standard duration, which provides a scale factor for a time extent, or the granularity or precision for a time position.</skos:definition>
        <skos:note xml:lang="en">Membership of the class TemporalUnit is open, to allow for other temporal units used in some technical applications (e.g. millions of years, Baha&apos;i month).</skos:note>
    </owl:Class>
    


    <!-- http://www.w3.org/ns/sosa/ActuatableProperty -->


    <owl:Class rdf:about="http://www.w3.org/ns/sosa/ActuatableProperty">
        <rdfs:comment xml:lang="en">Actuatable Property is an actuatable quality (property, characteristic) of any FeatureOfInterest.</rdfs:comment>
        <rdfs:isDefinedBy rdf:resource="http://www.w3.org/ns/sosa/"/>
        <rdfs:label xml:lang="en">Actuatable Property</rdfs:label>
        <skos:example xml:lang="en">A window actuator acts by changing the state between a frame and a window. The ability of the window to be opened and closed is its ActuatableProperty.</skos:example>
    </owl:Class>
    


    <!-- http://www.w3.org/ns/sosa/Actuation -->


    <owl:Class rdf:about="http://www.w3.org/ns/sosa/Actuation">
        <rdfs:comment xml:lang="en">An Actuation carries out an (Actuation) Procedure to change the state of the world using an Actuator.</rdfs:comment>
        <rdfs:isDefinedBy rdf:resource="http://www.w3.org/ns/sosa/"/>
        <rdfs:label xml:lang="en">Actuation</rdfs:label>
    </owl:Class>
    


    <!-- http://www.w3.org/ns/sosa/FeatureOfInterest -->


    <owl:Class rdf:about="http://www.w3.org/ns/sosa/FeatureOfInterest">
        <rdfs:subClassOf rdf:resource="http://def.isotc211.org/iso19156/2011/GeneralFeatureInstance#GFI_DomainFeature"/>
        <rdfs:comment>The thing whose property is being estimated or calculated in the course of an Observation to arrive at a Result, or whose property is being manipulated by an Actuator, or which is being sampled or transformed in an act of Sampling.</rdfs:comment>
        <rdfs:isDefinedBy rdf:resource="http://www.w3.org/ns/sosa/"/>
        <rdfs:label xml:lang="en">Feature Of Interest</rdfs:label>
    </owl:Class>
    


    <!-- http://www.w3.org/ns/sosa/ObservableProperty -->


    <owl:Class rdf:about="http://www.w3.org/ns/sosa/ObservableProperty">
        <rdfs:subClassOf rdf:resource="http://www.w3.org/ns/ssn/Property"/>
        <rdfs:comment>An observable quality (property, characteristic) of a FeatureOfInterest.</rdfs:comment>
        <rdfs:isDefinedBy rdf:resource="http://www.w3.org/ns/sosa/"/>
        <rdfs:label>Observable Property</rdfs:label>
    </owl:Class>
    


    <!-- http://www.w3.org/ns/sosa/Observation -->


    <owl:Class rdf:about="http://www.w3.org/ns/sosa/Observation">
        <rdfs:comment>If values are not provided for the following Observation properties, they may be provided by the ObservationCollection of which it is a member:
- hasFeatureOfInterest
- hasUltimateFeatureOfInterest
- madeBySensor
- observedProperty
- phenomenonTime
- resultTime
- usedProcedure</rdfs:comment>
        <rdfs:isDefinedBy rdf:resource="http://www.w3.org/ns/sosa/"/>
        <rdfs:label xml:lang="en">Observation</rdfs:label>
    </owl:Class>
    


    <!-- http://www.w3.org/ns/sosa/ObservationCollection -->


    <owl:Class rdf:about="http://www.w3.org/ns/sosa/ObservationCollection">
        <rdfs:subClassOf>
            <owl:Restriction>
                <owl:onProperty rdf:resource="http://www.w3.org/ns/sosa/hasMember"/>
                <owl:minCardinality rdf:datatype="http://www.w3.org/2001/XMLSchema#nonNegativeInteger">1</owl:minCardinality>
            </owl:Restriction>
        </rdfs:subClassOf>
        <rdfs:comment>Collection of observations, typically with one or more property shared by all of its members</rdfs:comment>
        <rdfs:isDefinedBy rdf:resource="http://www.w3.org/ns/ssn/ext/"/>
        <rdfs:label>Collection of observations</rdfs:label>
    </owl:Class>
    


    <!-- http://www.w3.org/ns/sosa/Platform -->


    <owl:Class rdf:about="http://www.w3.org/ns/sosa/Platform">
        <rdfs:comment xml:lang="en">A Platform is an entity that hosts other entities, particularly Sensors, Actuators, Samplers, and other Platforms (definition taken from http://www.w3.org/ns/sosa/Platform)</rdfs:comment>
        <rdfs:isDefinedBy rdf:resource="http://www.w3.org/ns/sosa/"/>
        <rdfs:label xml:lang="en">Platform</rdfs:label>
    </owl:Class>
    


    <!-- http://www.w3.org/ns/sosa/Procedure -->


    <owl:Class rdf:about="http://www.w3.org/ns/sosa/Procedure">
        <rdfs:comment xml:lang="en">A workflow, protocol, plan, algorithm, or computational method specifying how to make an Observation, create a Sample, or make a change to the state of the world (via an Actuator). A Procedure is re-usable, and might be involved in many Observations, Samplings, or Actuations. It explains the steps to be carried out to arrive at reproducible results.</rdfs:comment>
        <rdfs:isDefinedBy rdf:resource="http://www.w3.org/ns/sosa/"/>
        <rdfs:label xml:lang="en">Procedure</rdfs:label>
    </owl:Class>
    


    <!-- http://www.w3.org/ns/sosa/Result -->


    <owl:Class rdf:about="http://www.w3.org/ns/sosa/Result">
        <rdfs:comment xml:lang="en">The Result of an Observation, Actuation, or act of Sampling. To store an observation&apos;s simple result value one can use the hasSimpleResult property.</rdfs:comment>
        <rdfs:isDefinedBy rdf:resource="http://www.w3.org/ns/sosa/"/>
        <rdfs:label xml:lang="en">Result</rdfs:label>
        <skos:example xml:lang="en">The value 20 as the height of a certain tree together with the unit, e.g., Meter.</skos:example>
    </owl:Class>
    


    <!-- http://www.w3.org/ns/sosa/Sample -->


    <owl:Class rdf:about="http://www.w3.org/ns/sosa/Sample">
        <rdfs:comment xml:lang="en">Feature on which Observations may be made, which is intended to be representative of a FeatureOfInterest that is not fully accessible.</rdfs:comment>
        <rdfs:isDefinedBy rdf:resource="http://www.w3.org/ns/sosa/"/>
        <rdfs:label xml:lang="en">Sample</rdfs:label>
        <skos:example xml:lang="en">A &apos;station&apos; is essentially an identifiable locality where a sensor system or Process may be deployed and an observation made. In the context of the observation model, it connotes the &apos;world in the vicinity of the station&apos;, so the observed properties relate to the physical medium at the station, and not to any physical artifact such as a mooring, buoy, benchmark, monument, well, etc.</skos:example>
    </owl:Class>
    


    <!-- http://www.w3.org/ns/sosa/Sampling -->


    <owl:Class rdf:about="http://www.w3.org/ns/sosa/Sampling">
        <rdfs:comment xml:lang="en">An act of Sampling carries out a sampling Procedure to create or transform one or more samples.</rdfs:comment>
        <rdfs:isDefinedBy rdf:resource="http://www.w3.org/ns/sosa/"/>
        <rdfs:label xml:lang="en">Sampling</rdfs:label>
    </owl:Class>
    


    <!-- http://www.w3.org/ns/sosa/Sensor -->


    <owl:Class rdf:about="http://www.w3.org/ns/sosa/Sensor">
        <rdfs:comment xml:lang="en">Device, agent (including humans), or software (simulation) involved in, or implementing, a Procedure. Sensors respond to a stimulus, e.g., a change in the environment, or input data composed from the results of prior Observations, and generate a Result. Sensors can be hosted by Platforms.</rdfs:comment>
        <rdfs:isDefinedBy rdf:resource="http://www.w3.org/ns/sosa/"/>
        <rdfs:label xml:lang="en">Sensor</rdfs:label>
    </owl:Class>
    


    <!-- http://www.w3.org/ns/ssn/Deployment -->


    <owl:Class rdf:about="http://www.w3.org/ns/ssn/Deployment">
        <rdfs:comment>Deployment describes the Deployment of one or more Systems for a particular purpose. Deployment may be done on a Platform.</rdfs:comment>
        <rdfs:isDefinedBy rdf:resource="http://www.w3.org/ns/ssn/"/>
        <rdfs:label xml:lang="en">Deployment</rdfs:label>
    </owl:Class>
    


    <!-- http://www.w3.org/ns/ssn/Property -->


    <owl:Class rdf:about="http://www.w3.org/ns/ssn/Property">
        <rdfs:comment>Property is a quality of an entity. An aspect of an entity that is intrinsic to and cannot exist without the entity.</rdfs:comment>
        <rdfs:isDefinedBy rdf:resource="http://www.w3.org/ns/ssn/"/>
        <rdfs:label>Property</rdfs:label>
    </owl:Class>
    


    <!-- http://www.w3.org/ns/ssn/System -->


    <owl:Class rdf:about="http://www.w3.org/ns/ssn/System">
        <rdfs:comment xml:lang="en">System is a unit of abstraction for pieces of infrastructure that implement Procedures. A System may have components, its subsystems, which are other Systems. (Definition taken from http://www.w3.org/ns/ssn/System)</rdfs:comment>
        <rdfs:isDefinedBy rdf:resource="http://www.w3.org/ns/ssn/"/>
        <rdfs:label xml:lang="en">System</rdfs:label>
    </owl:Class>
    


    <!-- http://xmlns.com/foaf/0.1/Agent -->


    <owl:Class rdf:about="http://xmlns.com/foaf/0.1/Agent">
        <rdfs:subClassOf>
            <owl:Restriction>
                <owl:onProperty rdf:resource="http://xmlns.com/foaf/0.1/member"/>
                <owl:someValuesFrom rdf:resource="http://xmlns.com/foaf/0.1/Agent"/>
            </owl:Restriction>
        </rdfs:subClassOf>
        <rdfs:comment>The Agent class is the class of agents i.e. things that do stuff. A well known sub-class is foaf:Person, representing people. Other kinds of agents include foaf:Organization and foaf:Group.</rdfs:comment>
        <rdfs:isDefinedBy rdf:resource="http://xmlns.com/foaf/0.1/"/>
        <rdfs:label xml:lang="en">Agent</rdfs:label>
    </owl:Class>
    


    <!-- http://xmlns.com/foaf/0.1/Person -->


    <owl:Class rdf:about="http://xmlns.com/foaf/0.1/Person">
        <owl:equivalentClass rdf:resource="https://schema.org/Person"/>
        <rdfs:subClassOf rdf:resource="http://xmlns.com/foaf/0.1/Agent"/>
        <rdfs:comment>The foaf:Person class represents people. Something is a foaf:Person if it is a person. We don&apos;t nitpic about whether they&apos;re alive, dead, real, or imaginary. The foaf:Person class is a sub-class of the foaf:Agent class, since all people are considered &apos;agents&apos; in FOAF.</rdfs:comment>
        <rdfs:isDefinedBy rdf:resource="http://xmlns.com/foaf/0.1/"/>
        <rdfs:label xml:lang="en">Person</rdfs:label>
    </owl:Class>
    


    <!-- https://schema.org/Organization -->


    <owl:Class rdf:about="https://schema.org/Organization">
        <rdfs:subClassOf rdf:resource="http://xmlns.com/foaf/0.1/Agent"/>
        <rdfs:comment xml:lang="en">An organization such as a school, NGO, corporation, club, etc.</rdfs:comment>
        <rdfs:isDefinedBy rdf:resource="https://schema.org/Organization"/>
        <rdfs:label xml:lang="en">Organization</rdfs:label>
    </owl:Class>
    


    <!-- https://schema.org/Person -->


    <owl:Class rdf:about="https://schema.org/Person">
        <rdfs:comment xml:lang="en">A person (alive, dead, undead, or fictional).</rdfs:comment>
        <rdfs:isDefinedBy rdf:resource="https://schema.org/Person"/>
        <rdfs:label xml:lang="en">Person</rdfs:label>
    </owl:Class>
    


    <!-- https://schema.org/Role -->


    <owl:Class rdf:about="https://schema.org/Role">
        <rdfs:comment>Represents additional information about a relationship or property. For example a Role can be used to say that a &apos;member&apos; role linking some SportsTeam to a player occurred during a particular time period. Or that a Person&apos;s &apos;actor&apos; role in a Movie was for some particular characterName. Such properties can be attached to a Role entity, which is then associated with the main entities using ordinary properties like &apos;member&apos; or &apos;actor&apos;.&lt;br/&gt;&lt;br/&gt; </rdfs:comment>
        <rdfs:isDefinedBy rdf:resource="https://schema.org/Role"/>
        <rdfs:label xml:lang="en">Role</rdfs:label>
    </owl:Class>
    


    <!-- 
    ///////////////////////////////////////////////////////////////////////////////////////
    //
    // Individuals
    //
    ///////////////////////////////////////////////////////////////////////////////////////
     -->


    


    <!-- http://purl.oclc.org/NET/ssnx/qu/dim#AcousticsScheme -->


    <owl:NamedIndividual rdf:about="http://purl.oclc.org/NET/ssnx/qu/dim#AcousticsScheme">
        <rdf:type rdf:resource="http://www.w3.org/2004/02/skos/core#Scheme"/>
        <rdfs:comment>Named individual of AcousticsScheme</rdfs:comment>
        <rdfs:isDefinedBy rdf:resource="http://purl.oclc.org/NET/ssnx/qu/qu-rec20"/>
        <rdfs:label>Acoustics Scheme</rdfs:label>
    </owl:NamedIndividual>
    


    <!-- http://purl.oclc.org/NET/ssnx/qu/dim#ElectricityAndMagnetismScheme -->


    <owl:NamedIndividual rdf:about="http://purl.oclc.org/NET/ssnx/qu/dim#ElectricityAndMagnetismScheme">
        <rdf:type rdf:resource="http://www.w3.org/2004/02/skos/core#Scheme"/>
        <rdfs:comment>Named individual of ElectricityAndMagnetismScheme</rdfs:comment>
        <rdfs:isDefinedBy rdf:resource="http://purl.oclc.org/NET/ssnx/qu/qu-rec20"/>
        <rdfs:label>Electricity And Magnetism Scheme</rdfs:label>
    </owl:NamedIndividual>
    


    <!-- http://purl.oclc.org/NET/ssnx/qu/dim#HeatScheme -->


    <owl:NamedIndividual rdf:about="http://purl.oclc.org/NET/ssnx/qu/dim#HeatScheme">
        <rdf:type rdf:resource="http://www.w3.org/2004/02/skos/core#Scheme"/>
        <rdfs:comment>Named individual of HeatScheme</rdfs:comment>
        <rdfs:isDefinedBy rdf:resource="http://purl.oclc.org/NET/ssnx/qu/qu-rec20"/>
        <rdfs:label>Heat Scheme</rdfs:label>
    </owl:NamedIndividual>
    


    <!-- http://purl.oclc.org/NET/ssnx/qu/dim#LightAndRelatedElectromagneticRadiationsScheme -->


    <owl:NamedIndividual rdf:about="http://purl.oclc.org/NET/ssnx/qu/dim#LightAndRelatedElectromagneticRadiationsScheme">
        <rdf:type rdf:resource="http://www.w3.org/2004/02/skos/core#Scheme"/>
        <rdfs:comment>Named individual of LightAndRelatedElectromagneticRadiationsScheme</rdfs:comment>
        <rdfs:isDefinedBy rdf:resource="http://purl.oclc.org/NET/ssnx/qu/qu-rec20"/>
        <rdfs:label>Light And Related Electromagnetic Radiations Scheme</rdfs:label>
    </owl:NamedIndividual>
    


    <!-- http://purl.oclc.org/NET/ssnx/qu/dim#MechanicsScheme -->


    <owl:NamedIndividual rdf:about="http://purl.oclc.org/NET/ssnx/qu/dim#MechanicsScheme">
        <rdf:type rdf:resource="http://www.w3.org/2004/02/skos/core#Scheme"/>
        <rdfs:comment>Named individual of MechanicsScheme</rdfs:comment>
        <rdfs:isDefinedBy rdf:resource="http://purl.oclc.org/NET/ssnx/qu/qu-rec20"/>
        <rdfs:label>Mechanics Scheme</rdfs:label>
    </owl:NamedIndividual>
    


    <!-- http://purl.oclc.org/NET/ssnx/qu/dim#PeriodicAndRelatedPhenomenaScheme -->


    <owl:NamedIndividual rdf:about="http://purl.oclc.org/NET/ssnx/qu/dim#PeriodicAndRelatedPhenomenaScheme">
        <rdf:type rdf:resource="http://www.w3.org/2004/02/skos/core#Scheme"/>
        <rdfs:comment>Named individual of Periodic And Related Phenomena Scheme</rdfs:comment>
        <rdfs:isDefinedBy rdf:resource="http://purl.oclc.org/NET/ssnx/qu/qu-rec20"/>
        <rdfs:label>Periodic And Related Phenomena Scheme</rdfs:label>
    </owl:NamedIndividual>
    


    <!-- http://purl.oclc.org/NET/ssnx/qu/dim#PhysicalChemistryAndMolecularPhysicsScheme -->


    <owl:NamedIndividual rdf:about="http://purl.oclc.org/NET/ssnx/qu/dim#PhysicalChemistryAndMolecularPhysicsScheme">
        <rdf:type rdf:resource="http://www.w3.org/2004/02/skos/core#Scheme"/>
        <rdfs:comment>Named individual of PhysicalChemistryAndMolecularPhysicsScheme</rdfs:comment>
        <rdfs:isDefinedBy rdf:resource="http://purl.oclc.org/NET/ssnx/qu/qu-rec20"/>
        <rdfs:label>Physical Chemistry And Molecular Physics Scheme</rdfs:label>
    </owl:NamedIndividual>
    


    <!-- http://purl.oclc.org/NET/ssnx/qu/dim#SolidStatePhysicsScheme -->


    <owl:NamedIndividual rdf:about="http://purl.oclc.org/NET/ssnx/qu/dim#SolidStatePhysicsScheme">
        <rdf:type rdf:resource="http://www.w3.org/2004/02/skos/core#Scheme"/>
        <rdfs:comment>Named individual of SolidStatePhysicsScheme</rdfs:comment>
        <rdfs:isDefinedBy rdf:resource="http://purl.oclc.org/NET/ssnx/qu/qu-rec20"/>
        <rdfs:label>Solid State Physics Scheme</rdfs:label>
    </owl:NamedIndividual>
    


    <!-- http://purl.oclc.org/NET/ssnx/qu/dim#SpaceAndTimeScheme -->


    <owl:NamedIndividual rdf:about="http://purl.oclc.org/NET/ssnx/qu/dim#SpaceAndTimeScheme">
        <rdf:type rdf:resource="http://www.w3.org/2004/02/skos/core#Scheme"/>
        <rdfs:comment>Named individual of SpaceAndTimeScheme</rdfs:comment>
        <rdfs:isDefinedBy rdf:resource="http://purl.oclc.org/NET/ssnx/qu/qu-rec20"/>
        <rdfs:label>Space And Time Scheme</rdfs:label>
    </owl:NamedIndividual>
    


    <!-- http://purl.oclc.org/NET/ssnx/qu/quantity#acceleration -->


    <owl:NamedIndividual rdf:about="http://purl.oclc.org/NET/ssnx/qu/quantity#acceleration">
        <rdf:type rdf:resource="http://purl.oclc.org/NET/ssnx/qu/dim#Acceleration"/>
        <rdfs:comment>acceleration is a vector property that is an increase of speed of matter at a point per time in a direction. In other words: the derivative of the speed over time. Typically expressed as a = dv/dt.</rdfs:comment>
        <rdfs:isDefinedBy rdf:resource="http://purl.oclc.org/NET/ssnx/qu/qu-rec20"/>
        <rdfs:label>acceleration</rdfs:label>
        <skos:inScheme rdf:resource="http://purl.oclc.org/NET/ssnx/qu/dim#SpaceAndTimeScheme"/>
    </owl:NamedIndividual>
    


    <!-- http://purl.oclc.org/NET/ssnx/qu/quantity#carbonContent -->


    <owl:NamedIndividual rdf:about="http://purl.oclc.org/NET/ssnx/qu/quantity#carbonContent">
        <rdf:type rdf:resource="http://purl.oclc.org/NET/ssnx/qu/dim#Concentration"/>
        <rdfs:comment>carbon content is a concentration of carbon, both free and bounded</rdfs:comment>
        <rdfs:isDefinedBy rdf:resource="http://purl.oclc.org/NET/ssnx/qu/qu-rec20"/>
        <rdfs:label>carbon content</rdfs:label>
        <skos:inScheme rdf:resource="http://purl.oclc.org/NET/ssnx/qu/dim#PhysicalChemistryAndMolecularPhysicsScheme"/>
    </owl:NamedIndividual>
    


    <!-- http://purl.oclc.org/NET/ssnx/qu/quantity#compressibility -->


    <owl:NamedIndividual rdf:about="http://purl.oclc.org/NET/ssnx/qu/quantity#compressibility">
        <rdf:type rdf:resource="http://purl.oclc.org/NET/ssnx/qu/dim#Compressibility"/>
        <rdfs:comment>compressibility is a property that can be calculated from volume change due to pressure change as -(1/V).dV/dP</rdfs:comment>
        <rdfs:isDefinedBy rdf:resource="http://purl.oclc.org/NET/ssnx/qu/qu-rec20"/>
        <rdfs:label>compressibility</rdfs:label>
        <skos:inScheme rdf:resource="http://purl.oclc.org/NET/ssnx/qu/dim#HeatScheme"/>
        <skos:inScheme rdf:resource="http://purl.oclc.org/NET/ssnx/qu/dim#MechanicsScheme"/>
    </owl:NamedIndividual>
    


    <!-- http://purl.oclc.org/NET/ssnx/qu/quantity#concentration -->


    <owl:NamedIndividual rdf:about="http://purl.oclc.org/NET/ssnx/qu/quantity#concentration">
        <rdf:type rdf:resource="http://purl.oclc.org/NET/ssnx/qu/dim#Concentration"/>
        <rdfs:comment>concentration is a fraction that is the relative quantity of a substance in a mixture</rdfs:comment>
        <rdfs:isDefinedBy rdf:resource="http://purl.oclc.org/NET/ssnx/qu/qu-rec20"/>
        <rdfs:label>concentration</rdfs:label>
        <skos:inScheme rdf:resource="http://purl.oclc.org/NET/ssnx/qu/dim#PhysicalChemistryAndMolecularPhysicsScheme"/>
    </owl:NamedIndividual>
    


    <!-- http://purl.oclc.org/NET/ssnx/qu/quantity#criticalBuildUpSpeed -->


    <owl:NamedIndividual rdf:about="http://purl.oclc.org/NET/ssnx/qu/quantity#criticalBuildUpSpeed">
        <rdf:type rdf:resource="http://purl.oclc.org/NET/ssnx/qu/dim#RotationalSpeed"/>
        <rdfs:comment>critical build-up speed is a rotational speed that is the lowest speed at which the machine voltage builds up under specified conditions</rdfs:comment>
        <rdfs:isDefinedBy rdf:resource="http://purl.oclc.org/NET/ssnx/qu/qu-rec20"/>
        <rdfs:label>critical build-up speed</rdfs:label>
        <skos:inScheme rdf:resource="http://purl.oclc.org/NET/ssnx/qu/dim#AcousticsScheme"/>
        <skos:inScheme rdf:resource="http://purl.oclc.org/NET/ssnx/qu/dim#PeriodicAndRelatedPhenomenaScheme"/>
    </owl:NamedIndividual>
    


    <!-- http://purl.oclc.org/NET/ssnx/qu/quantity#criticalTorsionalSpeed -->


    <owl:NamedIndividual rdf:about="http://purl.oclc.org/NET/ssnx/qu/quantity#criticalTorsionalSpeed">
        <rdf:type rdf:resource="http://purl.oclc.org/NET/ssnx/qu/dim#RotationalSpeed"/>
        <rdfs:comment>critical torsional speed is a rotational speed at which the amplitudes of the vibrations of a machine rotor due to shaft torsional vibration reach their maximum values</rdfs:comment>
        <rdfs:isDefinedBy rdf:resource="http://purl.oclc.org/NET/ssnx/qu/qu-rec20"/>
        <rdfs:label>critical torsional speed</rdfs:label>
        <skos:inScheme rdf:resource="http://purl.oclc.org/NET/ssnx/qu/dim#AcousticsScheme"/>
        <skos:inScheme rdf:resource="http://purl.oclc.org/NET/ssnx/qu/dim#PeriodicAndRelatedPhenomenaScheme"/>
    </owl:NamedIndividual>
    


    <!-- http://purl.oclc.org/NET/ssnx/qu/quantity#criticalWhirlingSpeed -->


    <owl:NamedIndividual rdf:about="http://purl.oclc.org/NET/ssnx/qu/quantity#criticalWhirlingSpeed">
        <rdf:type rdf:resource="http://purl.oclc.org/NET/ssnx/qu/dim#RotationalSpeed"/>
        <rdfs:comment>critical whirling speed is a rotational speed at which the amplitudes of the vibrations of a machine rotor due to shaft whirling vibration reach their maximum values</rdfs:comment>
        <rdfs:isDefinedBy rdf:resource="http://purl.oclc.org/NET/ssnx/qu/qu-rec20"/>
        <rdfs:label>critical whirling speed</rdfs:label>
        <skos:inScheme rdf:resource="http://purl.oclc.org/NET/ssnx/qu/dim#AcousticsScheme"/>
        <skos:inScheme rdf:resource="http://purl.oclc.org/NET/ssnx/qu/dim#PeriodicAndRelatedPhenomenaScheme"/>
    </owl:NamedIndividual>
    


    <!-- http://purl.oclc.org/NET/ssnx/qu/quantity#density -->


    <owl:NamedIndividual rdf:about="http://purl.oclc.org/NET/ssnx/qu/quantity#density">
        <rdf:type rdf:resource="http://purl.oclc.org/NET/ssnx/qu/dim#Density"/>
        <rdfs:comment>density is a property that is a concentration of matter, measured as a mass per unit volume.</rdfs:comment>
        <rdfs:isDefinedBy rdf:resource="http://purl.oclc.org/NET/ssnx/qu/qu-rec20"/>
        <rdfs:label>density</rdfs:label>
        <skos:inScheme rdf:resource="http://purl.oclc.org/NET/ssnx/qu/dim#AcousticsScheme"/>
        <skos:inScheme rdf:resource="http://purl.oclc.org/NET/ssnx/qu/dim#MechanicsScheme"/>
        <skos:inScheme rdf:resource="http://purl.oclc.org/NET/ssnx/qu/dim#PhysicalChemistryAndMolecularPhysicsScheme"/>
    </owl:NamedIndividual>
    


    <!-- http://purl.oclc.org/NET/ssnx/qu/quantity#distance -->


    <owl:NamedIndividual rdf:about="http://purl.oclc.org/NET/ssnx/qu/quantity#distance">
        <rdf:type rdf:resource="http://purl.oclc.org/NET/ssnx/qu/dim#Distance"/>
        <rdfs:comment>distance is a vector property that is a measure of remoteness between two points, or minimum remoteness between lines or surfaces</rdfs:comment>
        <rdfs:isDefinedBy rdf:resource="http://purl.oclc.org/NET/ssnx/qu/qu-rec20"/>
        <rdfs:label>distance</rdfs:label>
        <skos:inScheme rdf:resource="http://purl.oclc.org/NET/ssnx/qu/dim#SpaceAndTimeScheme"/>
    </owl:NamedIndividual>
    


    <!-- http://purl.oclc.org/NET/ssnx/qu/quantity#energyFlowRate -->


    <owl:NamedIndividual rdf:about="http://purl.oclc.org/NET/ssnx/qu/quantity#energyFlowRate">
        <rdf:type rdf:resource="http://purl.oclc.org/NET/ssnx/qu/qu#PropertyKind"/>
        <rdfs:comment>Named individual of energyFlowRate</rdfs:comment>
        <rdfs:isDefinedBy rdf:resource="http://purl.oclc.org/NET/ssnx/qu/qu-rec20"/>
        <rdfs:label>energy flow rate</rdfs:label>
    </owl:NamedIndividual>
    


    <!-- http://purl.oclc.org/NET/ssnx/qu/quantity#fraction -->


    <owl:NamedIndividual rdf:about="http://purl.oclc.org/NET/ssnx/qu/quantity#fraction">
        <rdf:type rdf:resource="http://purl.oclc.org/NET/ssnx/qu/qu#PropertyKind"/>
        <rdfs:comment>Named individual of fraction</rdfs:comment>
        <rdfs:isDefinedBy rdf:resource="http://purl.oclc.org/NET/ssnx/qu/qu-rec20"/>
        <rdfs:label>fraction</rdfs:label>
    </owl:NamedIndividual>
    


    <!-- http://purl.oclc.org/NET/ssnx/qu/quantity#length -->


    <owl:NamedIndividual rdf:about="http://purl.oclc.org/NET/ssnx/qu/quantity#length">
        <rdf:type rdf:resource="http://purl.oclc.org/NET/ssnx/qu/dim#Distance"/>
        <rdfs:comment>length is a distance measured in the direction of the longest side of an item or in the direction of its main axis</rdfs:comment>
        <rdfs:isDefinedBy rdf:resource="http://purl.oclc.org/NET/ssnx/qu/qu-rec20"/>
        <rdfs:label>length</rdfs:label>
        <skos:inScheme rdf:resource="http://purl.oclc.org/NET/ssnx/qu/dim#SpaceAndTimeScheme"/>
    </owl:NamedIndividual>
    


    <!-- http://purl.oclc.org/NET/ssnx/qu/quantity#massPerTimePerArea -->


    <owl:NamedIndividual rdf:about="http://purl.oclc.org/NET/ssnx/qu/quantity#massPerTimePerArea">
        <rdf:type rdf:resource="http://purl.oclc.org/NET/ssnx/qu/dim#MassPerTimePerArea"/>
        <rdfs:comment>Named individual of massPerTimePerArea</rdfs:comment>
        <rdfs:isDefinedBy rdf:resource="http://purl.oclc.org/NET/ssnx/qu/qu-rec20"/>
        <rdfs:label>mass per time per area</rdfs:label>
        <skos:inScheme rdf:resource="http://purl.oclc.org/NET/ssnx/qu/dim#MechanicsScheme"/>
    </owl:NamedIndividual>
    


    <!-- http://purl.oclc.org/NET/ssnx/qu/quantity#power -->


    <owl:NamedIndividual rdf:about="http://purl.oclc.org/NET/ssnx/qu/quantity#power">
        <rdf:type rdf:resource="http://purl.oclc.org/NET/ssnx/qu/dim#Power"/>
        <rdfs:comment>power is an energy flow rate that is a rate of energy transfer</rdfs:comment>
        <rdfs:isDefinedBy rdf:resource="http://purl.oclc.org/NET/ssnx/qu/qu-rec20"/>
        <rdfs:label>power</rdfs:label>
        <skos:inScheme rdf:resource="http://purl.oclc.org/NET/ssnx/qu/dim#ElectricityAndMagnetismScheme"/>
        <skos:inScheme rdf:resource="http://purl.oclc.org/NET/ssnx/qu/dim#MechanicsScheme"/>
    </owl:NamedIndividual>
    


    <!-- http://purl.oclc.org/NET/ssnx/qu/quantity#pressure -->


    <owl:NamedIndividual rdf:about="http://purl.oclc.org/NET/ssnx/qu/quantity#pressure">
        <rdf:type rdf:resource="http://purl.oclc.org/NET/ssnx/qu/dim#StressOrPressure"/>
        <rdfs:comment>pressure is a property that is a force applied to, or distributed, over a surface. It is a force perpendicular to the area divided by area (p = dF/dA where dF is the perpendicular component of the force acting on the area element dA).</rdfs:comment>
        <rdfs:isDefinedBy rdf:resource="http://purl.oclc.org/NET/ssnx/qu/qu-rec20"/>
        <rdfs:label>pressure</rdfs:label>
        <skos:inScheme rdf:resource="http://purl.oclc.org/NET/ssnx/qu/dim#MechanicsScheme"/>
    </owl:NamedIndividual>
    


    <!-- http://purl.oclc.org/NET/ssnx/qu/quantity#property -->


    <owl:NamedIndividual rdf:about="http://purl.oclc.org/NET/ssnx/qu/quantity#property">
        <rdf:type rdf:resource="http://purl.oclc.org/NET/ssnx/qu/qu#PropertyKind"/>
        <rdfs:comment>Named individual of property</rdfs:comment>
        <rdfs:isDefinedBy rdf:resource="http://purl.oclc.org/NET/ssnx/qu/qu-rec20"/>
        <rdfs:label>property</rdfs:label>
    </owl:NamedIndividual>
    


    <!-- http://purl.oclc.org/NET/ssnx/qu/quantity#pseudovectorProperty -->


    <owl:NamedIndividual rdf:about="http://purl.oclc.org/NET/ssnx/qu/quantity#pseudovectorProperty">
        <rdf:type rdf:resource="http://purl.oclc.org/NET/ssnx/qu/qu#PropertyKind"/>
        <rdfs:comment>Named individual of pseudovectorProperty</rdfs:comment>
        <rdfs:isDefinedBy rdf:resource="http://purl.oclc.org/NET/ssnx/qu/qu-rec20"/>
        <rdfs:label>pseudo vector property</rdfs:label>
    </owl:NamedIndividual>
    


    <!-- http://purl.oclc.org/NET/ssnx/qu/quantity#radianceExposure -->


    <owl:NamedIndividual rdf:about="http://purl.oclc.org/NET/ssnx/qu/quantity#radianceExposure">
        <rdf:type rdf:resource="http://purl.oclc.org/NET/ssnx/qu/dim#RadianceExposure"/>
        <rdfs:comment>radiance exposure is a property</rdfs:comment>
        <rdfs:isDefinedBy rdf:resource="http://purl.oclc.org/NET/ssnx/qu/qu-rec20"/>
        <rdfs:label>radiance exposure</rdfs:label>
        <skos:inScheme rdf:resource="http://purl.oclc.org/NET/ssnx/qu/dim#LightAndRelatedElectromagneticRadiationsScheme"/>
    </owl:NamedIndividual>
    


    <!-- http://purl.oclc.org/NET/ssnx/qu/quantity#rotationalSpeed -->


    <owl:NamedIndividual rdf:about="http://purl.oclc.org/NET/ssnx/qu/quantity#rotationalSpeed">
        <rdf:type rdf:resource="http://purl.oclc.org/NET/ssnx/qu/dim#RotationalSpeed"/>
        <rdfs:comment>rotational speed is a property that is the rate of rotation of a material around an axis</rdfs:comment>
        <rdfs:isDefinedBy rdf:resource="http://purl.oclc.org/NET/ssnx/qu/qu-rec20"/>
        <rdfs:label>rotational speed</rdfs:label>
        <skos:inScheme rdf:resource="http://purl.oclc.org/NET/ssnx/qu/dim#AcousticsScheme"/>
        <skos:inScheme rdf:resource="http://purl.oclc.org/NET/ssnx/qu/dim#PeriodicAndRelatedPhenomenaScheme"/>
        <skos:inScheme rdf:resource="http://purl.oclc.org/NET/ssnx/qu/dim#SpaceAndTimeScheme"/>
    </owl:NamedIndividual>
    


    <!-- http://purl.oclc.org/NET/ssnx/qu/quantity#scalarProperty -->


    <owl:NamedIndividual rdf:about="http://purl.oclc.org/NET/ssnx/qu/quantity#scalarProperty">
        <rdf:type rdf:resource="http://purl.oclc.org/NET/ssnx/qu/qu#PropertyKind"/>
        <rdfs:comment>Named individual of scalarProperty</rdfs:comment>
        <rdfs:isDefinedBy rdf:resource="http://purl.oclc.org/NET/ssnx/qu/qu-rec20"/>
        <rdfs:label>scalar Property</rdfs:label>
    </owl:NamedIndividual>
    


    <!-- http://purl.oclc.org/NET/ssnx/qu/quantity#soundEnergyDensity -->


    <owl:NamedIndividual rdf:about="http://purl.oclc.org/NET/ssnx/qu/quantity#soundEnergyDensity">
        <rdf:type rdf:resource="http://purl.oclc.org/NET/ssnx/qu/dim#EnergyDensity"/>
        <rdfs:comment>sound energy density is a property that is an energy level due to sound per unit of volume</rdfs:comment>
        <rdfs:isDefinedBy rdf:resource="http://purl.oclc.org/NET/ssnx/qu/qu-rec20"/>
        <rdfs:label>sound energy density</rdfs:label>
        <skos:inScheme rdf:resource="http://purl.oclc.org/NET/ssnx/qu/dim#AcousticsScheme"/>
    </owl:NamedIndividual>
    


    <!-- http://purl.oclc.org/NET/ssnx/qu/quantity#soundIntensity -->


    <owl:NamedIndividual rdf:about="http://purl.oclc.org/NET/ssnx/qu/quantity#soundIntensity">
        <rdf:type rdf:resource="http://purl.oclc.org/NET/ssnx/qu/dim#EnergyFlux"/>
        <rdfs:comment>sound intensity is a property that is a sound power per unit of area</rdfs:comment>
        <rdfs:isDefinedBy rdf:resource="http://purl.oclc.org/NET/ssnx/qu/qu-rec20"/>
        <rdfs:label>sound intensity</rdfs:label>
        <skos:inScheme rdf:resource="http://purl.oclc.org/NET/ssnx/qu/dim#AcousticsScheme"/>
    </owl:NamedIndividual>
    


    <!-- http://purl.oclc.org/NET/ssnx/qu/quantity#soundPower -->


    <owl:NamedIndividual rdf:about="http://purl.oclc.org/NET/ssnx/qu/quantity#soundPower">
        <rdf:type rdf:resource="http://purl.oclc.org/NET/ssnx/qu/dim#Power"/>
        <rdfs:comment>sound power is a power of sound</rdfs:comment>
        <rdfs:isDefinedBy rdf:resource="http://purl.oclc.org/NET/ssnx/qu/qu-rec20"/>
        <rdfs:label>sound power</rdfs:label>
        <skos:inScheme rdf:resource="http://purl.oclc.org/NET/ssnx/qu/dim#AcousticsScheme"/>
    </owl:NamedIndividual>
    


    <!-- http://purl.oclc.org/NET/ssnx/qu/quantity#soundPressure -->


    <owl:NamedIndividual rdf:about="http://purl.oclc.org/NET/ssnx/qu/quantity#soundPressure">
        <rdf:type rdf:resource="http://purl.oclc.org/NET/ssnx/qu/dim#StressOrPressure"/>
        <rdfs:comment>sound pressure is a pressure that is the difference between the instantaneous total pressure and the static pressure</rdfs:comment>
        <rdfs:isDefinedBy rdf:resource="http://purl.oclc.org/NET/ssnx/qu/qu-rec20"/>
        <rdfs:label>sound pressure</rdfs:label>
        <skos:inScheme rdf:resource="http://purl.oclc.org/NET/ssnx/qu/dim#AcousticsScheme"/>
        <skos:inScheme rdf:resource="http://purl.oclc.org/NET/ssnx/qu/dim#MechanicsScheme"/>
    </owl:NamedIndividual>
    


    <!-- http://purl.oclc.org/NET/ssnx/qu/quantity#surfaceDensity -->


    <owl:NamedIndividual rdf:about="http://purl.oclc.org/NET/ssnx/qu/quantity#surfaceDensity">
        <rdf:type rdf:resource="http://purl.oclc.org/NET/ssnx/qu/dim#SurfaceDensity"/>
        <rdfs:comment>surface density is a property that is a mass per unit of area</rdfs:comment>
        <rdfs:isDefinedBy rdf:resource="http://purl.oclc.org/NET/ssnx/qu/qu-rec20"/>
        <rdfs:label>surface density</rdfs:label>
        <skos:inScheme rdf:resource="http://purl.oclc.org/NET/ssnx/qu/dim#MechanicsScheme"/>
    </owl:NamedIndividual>
    


    <!-- http://purl.oclc.org/NET/ssnx/qu/quantity#synchronousPullOutTorque -->


    <owl:NamedIndividual rdf:about="http://purl.oclc.org/NET/ssnx/qu/quantity#synchronousPullOutTorque">
        <rdf:type rdf:resource="http://purl.oclc.org/NET/ssnx/qu/dim#Energy"/>
        <rdfs:comment>synchronous pull-out torque is a torque that is the maximum torque that a synchronous machine can develop without loss of synchronism while operating at rated voltage, frequency and excitation</rdfs:comment>
        <rdfs:isDefinedBy rdf:resource="http://purl.oclc.org/NET/ssnx/qu/qu-rec20"/>
        <rdfs:label>synchronous pull-out torque</rdfs:label>
        <skos:inScheme rdf:resource="http://purl.oclc.org/NET/ssnx/qu/dim#MechanicsScheme"/>
    </owl:NamedIndividual>
    


    <!-- http://purl.oclc.org/NET/ssnx/qu/quantity#synchronousSpeed -->


    <owl:NamedIndividual rdf:about="http://purl.oclc.org/NET/ssnx/qu/quantity#synchronousSpeed">
        <rdf:type rdf:resource="http://purl.oclc.org/NET/ssnx/qu/dim#RotationalSpeed"/>
        <rdfs:comment>synchronous speed is a rotational speed that results from the frequency of the system to which the machine is connected and either the number of poles or the number of projections in the machine</rdfs:comment>
        <rdfs:isDefinedBy rdf:resource="http://purl.oclc.org/NET/ssnx/qu/qu-rec20"/>
        <rdfs:label>synchronous speed</rdfs:label>
        <skos:inScheme rdf:resource="http://purl.oclc.org/NET/ssnx/qu/dim#AcousticsScheme"/>
        <skos:inScheme rdf:resource="http://purl.oclc.org/NET/ssnx/qu/dim#PeriodicAndRelatedPhenomenaScheme"/>
    </owl:NamedIndividual>
    


    <!-- http://purl.oclc.org/NET/ssnx/qu/quantity#temperature -->


    <owl:NamedIndividual rdf:about="http://purl.oclc.org/NET/ssnx/qu/quantity#temperature">
        <rdf:type rdf:resource="http://purl.oclc.org/NET/ssnx/qu/dim#Temperature"/>
        <rdfs:comment>Named individual of temperature</rdfs:comment>
        <rdfs:isDefinedBy rdf:resource="http://purl.oclc.org/NET/ssnx/qu/qu-rec20"/>
        <rdfs:label>temperature</rdfs:label>
        <skos:inScheme rdf:resource="http://purl.oclc.org/NET/ssnx/qu/dim#HeatScheme"/>
        <skos:inScheme rdf:resource="http://purl.oclc.org/NET/ssnx/qu/dim#SolidStatePhysicsScheme"/>
    </owl:NamedIndividual>
    


    <!-- http://purl.oclc.org/NET/ssnx/qu/quantity#torque -->


    <owl:NamedIndividual rdf:about="http://purl.oclc.org/NET/ssnx/qu/quantity#torque">
        <rdf:type rdf:resource="http://purl.oclc.org/NET/ssnx/qu/dim#Energy"/>
        <rdfs:comment>torque is a property that is a twisting force being a product of a force and a distance. The force is applied to something that has a role as a lever and the distance is the distance between the point on the lever where the force applies and the fulcrum of the lever</rdfs:comment>
        <rdfs:isDefinedBy rdf:resource="http://purl.oclc.org/NET/ssnx/qu/qu-rec20"/>
        <rdfs:label>torque</rdfs:label>
        <skos:inScheme rdf:resource="http://purl.oclc.org/NET/ssnx/qu/dim#MechanicsScheme"/>
    </owl:NamedIndividual>
    


    <!-- http://purl.oclc.org/NET/ssnx/qu/quantity#vapourCompressibility -->


    <owl:NamedIndividual rdf:about="http://purl.oclc.org/NET/ssnx/qu/quantity#vapourCompressibility">
        <rdf:type rdf:resource="http://purl.oclc.org/NET/ssnx/qu/dim#Compressibility"/>
        <rdfs:comment>vapour compressibility is a compressibility of a vapour</rdfs:comment>
        <rdfs:isDefinedBy rdf:resource="http://purl.oclc.org/NET/ssnx/qu/qu-rec20"/>
        <rdfs:label>vapour compressibility</rdfs:label>
        <skos:inScheme rdf:resource="http://purl.oclc.org/NET/ssnx/qu/dim#HeatScheme"/>
        <skos:inScheme rdf:resource="http://purl.oclc.org/NET/ssnx/qu/dim#PhysicalChemistryAndMolecularPhysicsScheme"/>
    </owl:NamedIndividual>
    


    <!-- http://purl.oclc.org/NET/ssnx/qu/quantity#vapourPressure -->


    <owl:NamedIndividual rdf:about="http://purl.oclc.org/NET/ssnx/qu/quantity#vapourPressure">
        <rdf:type rdf:resource="http://purl.oclc.org/NET/ssnx/qu/dim#StressOrPressure"/>
        <rdfs:comment>vapour pressure is a pressure of the vapour phase of a substance over the liquid phase when the phases are in equilibrium</rdfs:comment>
        <rdfs:isDefinedBy rdf:resource="http://purl.oclc.org/NET/ssnx/qu/qu-rec20"/>
        <rdfs:label>vapour pressure</rdfs:label>
        <skos:inScheme rdf:resource="http://purl.oclc.org/NET/ssnx/qu/dim#MechanicsScheme"/>
    </owl:NamedIndividual>
    


    <!-- http://purl.oclc.org/NET/ssnx/qu/quantity#vectorProperty -->


    <owl:NamedIndividual rdf:about="http://purl.oclc.org/NET/ssnx/qu/quantity#vectorProperty">
        <rdf:type rdf:resource="http://purl.oclc.org/NET/ssnx/qu/qu#PropertyKind"/>
        <rdfs:comment>Named individual of vectorProperty</rdfs:comment>
        <rdfs:isDefinedBy rdf:resource="http://purl.oclc.org/NET/ssnx/qu/qu-rec20"/>
        <rdfs:label>vector property</rdfs:label>
    </owl:NamedIndividual>
    


    <!-- http://purl.oclc.org/NET/ssnx/qu/quantity#velocity -->


    <owl:NamedIndividual rdf:about="http://purl.oclc.org/NET/ssnx/qu/quantity#velocity">
        <rdf:type rdf:resource="http://purl.oclc.org/NET/ssnx/qu/dim#VelocityOrSpeed"/>
        <rdfs:comment>velocity is a vector property that is time rate of motion of matter at a point in a fixed direction. Typically also used for the relative velocity with reference to a point on the earth (v = ds/dt  where s is the displacement and t is the time)</rdfs:comment>
        <rdfs:isDefinedBy rdf:resource="http://purl.oclc.org/NET/ssnx/qu/qu-rec20"/>
        <rdfs:label>velocity</rdfs:label>
        <skos:inScheme rdf:resource="http://purl.oclc.org/NET/ssnx/qu/dim#LightAndRelatedElectromagneticRadiationsScheme"/>
        <skos:inScheme rdf:resource="http://purl.oclc.org/NET/ssnx/qu/dim#SpaceAndTimeScheme"/>
    </owl:NamedIndividual>
    


    <!-- http://www.w3.org/2006/time#unitDay -->


    <owl:NamedIndividual rdf:about="http://www.w3.org/2006/time#unitDay">
        <rdf:type rdf:resource="http://www.w3.org/2006/time#TemporalUnit"/>
        <rdfs:comment>Day (unit of temporal duration)</rdfs:comment>
        <rdfs:isDefinedBy rdf:resource="http://www.w3.org/2006/time#"/>
        <rdfs:label xml:lang="en">Day (unit of temporal duration)</rdfs:label>
    </owl:NamedIndividual>
    


    <!-- http://www.w3.org/2006/time#unitHour -->


    <owl:NamedIndividual rdf:about="http://www.w3.org/2006/time#unitHour">
        <rdf:type rdf:resource="http://www.w3.org/2006/time#TemporalUnit"/>
        <rdfs:comment>Hour (unit of temporal duration)</rdfs:comment>
        <rdfs:isDefinedBy rdf:resource="http://www.w3.org/2006/time#"/>
        <rdfs:label xml:lang="en">Hour (unit of temporal duration)</rdfs:label>
    </owl:NamedIndividual>
    


    <!-- http://www.w3.org/2006/time#unitMinute -->


    <owl:NamedIndividual rdf:about="http://www.w3.org/2006/time#unitMinute">
        <rdf:type rdf:resource="http://www.w3.org/2006/time#TemporalUnit"/>
        <rdfs:comment>Minute (unit of temporal duration)</rdfs:comment>
        <rdfs:isDefinedBy rdf:resource="http://www.w3.org/2006/time#"/>
        <rdfs:label xml:lang="en">Minute (unit of temporal duration)</rdfs:label>
    </owl:NamedIndividual>
    


    <!-- http://www.w3.org/2006/time#unitMonth -->


    <owl:NamedIndividual rdf:about="http://www.w3.org/2006/time#unitMonth">
        <rdf:type rdf:resource="http://www.w3.org/2006/time#TemporalUnit"/>
        <rdfs:comment>Month (unit of temporal duration)</rdfs:comment>
        <rdfs:isDefinedBy rdf:resource="http://www.w3.org/2006/time#"/>
        <rdfs:label xml:lang="en">Month (unit of temporal duration)</rdfs:label>
    </owl:NamedIndividual>
    


    <!-- http://www.w3.org/2006/time#unitSecond -->


    <owl:NamedIndividual rdf:about="http://www.w3.org/2006/time#unitSecond">
        <rdf:type rdf:resource="http://www.w3.org/2006/time#TemporalUnit"/>
        <rdfs:comment>Second (unit of temporal duration)</rdfs:comment>
        <rdfs:isDefinedBy rdf:resource="http://www.w3.org/2006/time#"/>
        <rdfs:label xml:lang="en">Second (unit of temporal duration)</rdfs:label>
    </owl:NamedIndividual>
    


    <!-- http://www.w3.org/2006/time#unitWeek -->


    <owl:NamedIndividual rdf:about="http://www.w3.org/2006/time#unitWeek">
        <rdf:type rdf:resource="http://www.w3.org/2006/time#TemporalUnit"/>
        <rdfs:comment>Week (unit of temporal duration)</rdfs:comment>
        <rdfs:isDefinedBy rdf:resource="http://www.w3.org/2006/time#"/>
        <rdfs:label xml:lang="en">Week (unit of temporal duration)</rdfs:label>
    </owl:NamedIndividual>
    


    <!-- http://www.w3.org/2006/time#unitYear -->


    <owl:NamedIndividual rdf:about="http://www.w3.org/2006/time#unitYear">
        <rdf:type rdf:resource="http://www.w3.org/2006/time#TemporalUnit"/>
        <rdfs:comment>Year (unit of temporal duration)</rdfs:comment>
        <rdfs:isDefinedBy rdf:resource="http://www.w3.org/2006/time#"/>
        <rdfs:label xml:lang="en">Year (unit of temporal duration)</rdfs:label>
    </owl:NamedIndividual>
    


    <!-- 
    ///////////////////////////////////////////////////////////////////////////////////////
    //
    // Annotations
    //
    ///////////////////////////////////////////////////////////////////////////////////////
     -->


    <rdf:Description rdf:about="http://purl.org/dc/terms/contributor">
        <rdfs:comment>An entity responsible for making contributions to the content of the resource</rdfs:comment>
        <rdfs:isDefinedBy rdf:resource="http://purl.org/dc/terms/"/>
        <rdfs:label>Contributor</rdfs:label>
    </rdf:Description>
    <rdf:Description rdf:about="http://purl.org/dc/terms/creator">
        <rdfs:comment>An entity primarily responsible for making the content of the resource</rdfs:comment>
        <rdfs:isDefinedBy rdf:resource="http://purl.org/dc/terms/"/>
        <rdfs:label>Creator</rdfs:label>
    </rdf:Description>
    <rdf:Description rdf:about="http://purl.org/dc/terms/description">
        <rdfs:comment>An account of the content of the resource</rdfs:comment>
        <rdfs:isDefinedBy rdf:resource="http://purl.org/dc/terms/"/>
        <rdfs:label>Description</rdfs:label>
    </rdf:Description>
    <rdf:Description rdf:about="http://purl.org/dc/terms/rights">
        <rdfs:comment>Information about rights held in and over the resource</rdfs:comment>
        <rdfs:isDefinedBy rdf:resource="http://purl.org/dc/terms/"/>
        <rdfs:label>Rights Management</rdfs:label>
    </rdf:Description>
    <rdf:Description rdf:about="http://purl.org/dc/terms/title">
        <rdfs:comment>A name given to the resource</rdfs:comment>
        <rdfs:isDefinedBy rdf:resource="http://purl.org/dc/terms/"/>
        <rdfs:label>Title</rdfs:label>
    </rdf:Description>
    <rdf:Description rdf:about="http://xmlns.com/foaf/0.1/maker">
        <rdfs:comment>An agent that made this thing</rdfs:comment>
        <rdfs:isDefinedBy rdf:resource="http://xmlns.com/foaf/0.1/"/>
        <rdfs:label>maker</rdfs:label>
    </rdf:Description>
    <rdf:Description rdf:about="https://schema.org/name">
        <rdfs:comment>The name of the item.</rdfs:comment>
        <rdfs:isDefinedBy rdf:resource="http://schema.org/Thing"/>
        <rdfs:label xml:lang="en">name</rdfs:label>
    </rdf:Description>
    <rdf:Description rdf:about="https://schema.org/telephone">
        <rdfs:comment>The telephone number.</rdfs:comment>
        <rdfs:isDefinedBy rdf:resource="http://schema.org/ContactPoint"/>
        <rdfs:isDefinedBy rdf:resource="http://schema.org/Organization"/>
        <rdfs:isDefinedBy rdf:resource="http://schema.org/Person"/>
        <rdfs:isDefinedBy rdf:resource="http://schema.org/Place"/>
        <rdfs:label xml:lang="en">telephone</rdfs:label>
    </rdf:Description>
</rdf:RDF>



<!-- Generated by the OWL API (version 5.1.18) https://github.com/owlcs/owlapi/ -->


