@prefix : <https://w3id.org/cybele/> .
@prefix qb: <http://purl.org/linked-data/cube#> .
@prefix dct: <http://purl.org/dc/terms/> .
@prefix owl: <http://www.w3.org/2002/07/owl#> .
@prefix rdf: <http://www.w3.org/1999/02/22-rdf-syntax-ns#> .
@prefix xml: <http://www.w3.org/XML/1998/namespace> .
@prefix xsd: <http://www.w3.org/2001/XMLSchema#> .
@prefix dcat: <http://www.w3.org/ns/dcat#> .
@prefix foaf: <http://xmlns.com/foaf/0.1/> .
@prefix prov: <http://www.w3.org/ns/prov#> .
@prefix rdfs: <http://www.w3.org/2000/01/rdf-schema#> .
@prefix skos: <http://www.w3.org/2004/02/skos/core#> .
@prefix stat: <http://data.europa.eu/m8g/> .
@prefix schema: <https://schema.org/> .
@prefix af-inspire:	<http://inspire.ec.europa.eu/schemas/af/3.0#> .
@prefix act-inspire:	<http://inspire.ec.europa.eu/schemas/act-core/3.0#> .
@prefix foodie: <http://foodie-cloud.com/model/foodie#> .
@prefix saref4agri: <https://saref.etsi.org/saref4agri/> .
@prefix common: <http://portele.de/ont/inspire/baseInspire#> .
@prefix fiware: <https://smartdatamodels.org/> .
@prefix fiware-agrifood: <https://smartdatamodels.org/dataModel.Agrifood/> .
@prefix ngsi-ld: <https://uri.etsi.org/ngsi-ld/> .
@prefix iso19109: <http://def.seegrid.csiro.au/isotc211/iso19109/2005/feature#> .
@prefix iso19150-2: <http://def.seegrid.csiro.au/isotc211/iso19150/-2/2012/basic#> .
@prefix geo:   <http://www.opengis.net/ont/geosparql#> .
@prefix wgs84_pos: <http://www.w3.org/2003/01/geo/wgs84_pos#> .
@prefix sf: <http://www.opengis.net/ont/sf#> .
@base <https://w3id.org/demeter/> .

<https://w3id.org/demeter/agri/agriFeature> a owl:Ontology ;
                            owl:versionIRI <https://w3id.org/demeter/agri/agriFeature/3.0> ;
                            dct:contributor [ schema:affiliation [ foaf:name "OGC"
                                                                 ] ;
                                              foaf:name "Rob Atkinson"
                                            ] ,
                                            [ schema:affiliation [ foaf:name "ICCS"
                                                                 ] ;
                                              foaf:name "Ioanna Roussaki"
                                            ] ;
                            dct:creator [ schema:affiliation [ foaf:name "PSNC"
                                                             ] ;
                                          rdfs:seeAlso <http://orcid.org/0000-0003-4289-4922> ;
                                          foaf:name "Raul Palma"
                                        ] ;
                            owl:imports <https://w3id.org/demeter/agri/agriCommon/3.0> ;
                            dct:description "The DEMETER AgriFeature is one of the agri profiles of DEMETER AIM. This profile was created by reusing and aligning well-known ontologies and vocabularies"@en ;
                            dct:rights "This vocabulary is distributed under Creative Commons Attribution 4.0 License - http://creativecommons.org/licenses/by/4.0"@en ;
                            dct:title "DEMETER AgriFeature"@en ;
                            rdfs:label "DEMETER AgriFeature"@en ;
                            rdfs:comment "The DEMETER Agriculture Information Model (AIM) is the common vocabulary in DEMETER project providing the basis for semantic interoperability across smart farming solutions"@en ;
                            owl:versionInfo "3.0" ;
                            foaf:maker [ foaf:homepage <https://h2020-demeter.eu/> ;
                                         foaf:name "DEMETER project"
                                       ] .

#################################################################
#    Annotation properties
#################################################################


#################################################################
#    Datatypes
#################################################################


#################################################################
#    Object Properties
#################################################################

###  https://saref.etsi.org/saref4agri/contains
saref4agri:contains a owl:ObjectProperty ;
          owl:inverseOf saref4agri:isContainedIn ;
          rdfs:label "contains" ;
          rdfs:comment "A realtion to represent the contained land parcel" ;
          rdfs:isDefinedBy <https://saref.etsi.org/saref4agri/> .

###  https://saref.etsi.org/saref4agri/isContainedIn
saref4agri:isContainedIn a owl:ObjectProperty ;
               rdfs:label "is contained in"@en ;
               rdfs:comment "A relation inverse of s4agri:contains" ;
               rdfs:isDefinedBy <https://saref.etsi.org/saref4agri/> .

###  http://inspire.ec.europa.eu/schemas/af/3.0#activity
af-inspire:activity
        a               owl:ObjectProperty ;
        rdfs:range      act-inspire:EconomicActivityNACEValue ;
        skos:prefLabel  "activity"@en ;
        rdfs:label "activity"@en ;
        rdfs:comment "A relation to the classification of the economic activity of the site" ;
        rdfs:isDefinedBy <http://inspire.ec.europa.eu/schemas/af/3.0#> .

###  http://inspire.ec.europa.eu/schemas/af/3.0#contains
af-inspire:contains
        a               owl:ObjectProperty ;
        rdfs:range      af-inspire:Site ;
        skos:prefLabel  "contains"@en ;
        rdfs:label "contains"@en ;
        rdfs:comment "A relation from Holding to Site " ;
        rdfs:isDefinedBy <http://inspire.ec.europa.eu/schemas/af/3.0#> .

###  http://foodie-cloud.com/model/foodie#containsPlot
foodie:containsPlot
        a               owl:ObjectProperty ;
        rdfs:range      foodie:Plot ;
        skos:prefLabel  "containsPlot"@en ;
        rdfs:label "containsPlot"@en ;
        rdfs:comment "A relation from Site to Plot " ;
        rdfs:isDefinedBy <http://foodie-cloud.com/model/foodie> .

###  http://foodie-cloud.com/model/foodie#containsZone
foodie:containsZone  a  owl:ObjectProperty ;
        rdfs:range      foodie:ManagementZone ;
        skos:prefLabel  "containsZone"@en ;
        rdfs:label "containsZone"@en ;
        rdfs:comment "A relation from Plot to Management zone" ;
        rdfs:isDefinedBy <http://foodie-cloud.com/model/foodie> .

###  http://foodie-cloud.com/model/foodie#originType
foodie:originType  a    owl:ObjectProperty ;
        rdfs:range      foodie:OriginTypeValue ;
        skos:prefLabel  "originType"@en ;
        rdfs:label "containsZone"@en ;
        rdfs:comment "A relation to the origin of a Plot when taking into consideration only two options: manual (created by human/user) and system (produced by the platform" ;
        rdfs:isDefinedBy <http://foodie-cloud.com/model/foodie> .

###  http://foodie-cloud.com/model/foodie#crop
foodie:crop  	a   owl:ObjectProperty ;
        skos:prefLabel  "crop"@en ;
        rdfs:label "crop"@en ;
        rdfs:comment "A relation from Plot to CropSpecies" ;
        rdfs:isDefinedBy <http://foodie-cloud.com/model/foodie> .

###  http://foodie-cloud.com/model/foodie#machine
foodie:machine	a       owl:ObjectProperty ;
        rdfs:range      foodie:MachineType ;
        skos:prefLabel  "machine"@en ;
        rdfs:label "machine"@en ;
        rdfs:comment "A relation from Intervention to MachineType" ;
        rdfs:isDefinedBy <http://foodie-cloud.com/model/foodie> .

###  http://foodie-cloud.com/model/foodie#tractor
foodie:tractor	a	owl:ObjectProperty ;
        rdfs:range      foodie:TractorType ;
        skos:prefLabel  "tractor"@en ;
        rdfs:label "tractor"@en ;
        rdfs:comment "A relation from Intervention to TractorType" ;
        rdfs:isDefinedBy <http://foodie-cloud.com/model/foodie> .

###  http://foodie-cloud.com/model/foodie#holdingSite
foodie:holdingSite  a  owl:ObjectProperty ;
        rdfs:range      af-inspire:Holding ;
        skos:prefLabel  "holdingSite"@en ;
        rdfs:label "holdingSite"@en ;
        rdfs:comment "A relation from Site to Holding" ;
        rdfs:isDefinedBy <http://foodie-cloud.com/model/foodie> .

###  http://foodie-cloud.com/model/foodie#holdingPlot
foodie:holdingPlot  a  owl:ObjectProperty ;
        rdfs:range      af-inspire:Site ;
        skos:prefLabel  "holdingPlot"@en ;
        rdfs:label "holdingPlot"@en ;
        rdfs:comment "A relation from Plot to Site" ;
        rdfs:isDefinedBy <http://foodie-cloud.com/model/foodie> .

###  http://foodie-cloud.com/model/foodie#holdingZone
foodie:holdingZone  a  owl:ObjectProperty ;
        rdfs:range      foodie:Plot ;
        skos:prefLabel  "holdingZone"@en ;
        rdfs:label "holdingPlot"@en ;
        rdfs:comment "A relation from Management Zone to Plot" ;
        rdfs:isDefinedBy <http://foodie-cloud.com/model/foodie> .

### https://smartdatamodels.org/dataModel.Agrifood/hasAgriCrop
fiware-agrifood:hasAgriCrop	a   owl:ObjectProperty ;
        rdfs:label   		"hasAgriCrop"@en ;
        rdfs:comment		"Reference to the crop associated with this parcel" ;
        rdfs:isDefinedBy <https://github.com/smart-data-models/dataModel.Agrifood/blob/master/AgriParcel/schema.json> .

### https://smartdatamodels.org/dataModel.Agrifood/hasAgriParcelParent
fiware-agrifood:hasAgriParcelParent	a      owl:ObjectProperty ;
        rdfs:label   		"hasAgriParcelParent"@en ;
        rdfs:comment		"Reference to the parent AgriParcel" ;
        rdfs:isDefinedBy <https://github.com/smart-data-models/dataModel.Agrifood/blob/master/AgriParcel/schema.json> .

### https://smartdatamodels.org/dataModel.Agrifood/hasAgriParcelChildren
fiware-agrifood:hasAgriParcelChildren	a      owl:ObjectProperty ;
        rdfs:label   		"hasAgriParcelChildren"@en ;
        rdfs:comment		"Related sub AgriParcel records to which this entity relates" ;
        rdfs:isDefinedBy <https://github.com/smart-data-models/dataModel.Agrifood/blob/master/AgriParcel/schema.json> .

### https://smartdatamodels.org/dataModel.Agrifood/hasAgriSoil
fiware-agrifood:hasAgriSoil	a      owl:ObjectProperty ;
        rdfs:label   		"hasAgriSoil"@en ;
        rdfs:comment		"Reference to the soil associated with this parcel of land" ;
        rdfs:isDefinedBy <https://github.com/smart-data-models/dataModel.Agrifood/blob/master/AgriParcel/schema.json> .

### https://smartdatamodels.org/dataModel.Agrifood/landLocation
fiware-agrifood:landLocation	a      owl:ObjectProperty ;
        rdfs:label   		"landLocation"@en ;
        rdfs:comment		"Geometry defining the boundaries of the farm land" ;
        rdfs:isDefinedBy <https://github.com/smart-data-models/dataModel.Agrifood/blob/master/AgriFarm/schema.json> .

### https://smartdatamodels.org/dataModel.Agrifood/hasAgriParcel
fiware-agrifood:hasAgriParcel	a      owl:ObjectProperty ;
        rdfs:label   		"hasAgriParcel"@en ;
        rdfs:comment		"List of agri parcels belonging to the farm" ;
        rdfs:isDefinedBy <https://github.com/smart-data-models/dataModel.Agrifood/blob/master/AgriFarm/schema.json> .

### https://uri.etsi.org/ngsi-ld/location
ngsi-ld:location	a      owl:ObjectProperty ;
        rdfs:label   		"location"@en ;
        rdfs:comment		"The geo:json encoded polygon / multi-polygon describing this item.  It can be Point, LineString, Polygon, MultiPoint, MultiLineString or MultiPolygon" ;
        rdfs:isDefinedBy <https://uri.etsi.org/ngsi-ld/v1/ngsi-ld-core-context-v1.6.jsonld> .


#################################################################
#    Data properties
#################################################################

### https://smartdatamodels.org/dataModel.Agrifood/area
fiware-agrifood:area	a      owl:DatatypeProperty ;
        rdfs:label   		"area"@en ;
        rdfs:comment		"The area of the parcel nominally in square meters." ;
        rdfs:isDefinedBy <https://github.com/smart-data-models/dataModel.Agrifood/blob/master/AgriParcel/schema.json> .

### https://smartdatamodels.org/dataModel.Agrifood/cropStatus
fiware-agrifood:cropStatus	a      owl:DatatypeProperty ;
        rdfs:label   		"cropStatus"@en ;
        rdfs:comment		"A choice from an enumerated list describing the crop planting status One of: seeded, justBorn, growing, maturing, readyForHarvesting." ;
        rdfs:isDefinedBy <https://github.com/smart-data-models/dataModel.Agrifood/blob/master/AgriParcel/schema.json> .

### https://smartdatamodels.org/dataModel.Agrifood/lastPlantedAt
fiware-agrifood:lastPlantedAt	a owl:DatatypeProperty ;
        rdfs:range      xsd:dateTime ;
        rdfs:label   		"lastPlantedAt"@en ;
        rdfs:comment		"Indicates the date when the crop was last planted." ;
        rdfs:isDefinedBy <https://github.com/smart-data-models/dataModel.Agrifood/blob/master/AgriParcel/schema.json> .


#################################################################
#    Classes
#################################################################

###  https://saref.etsi.org/saref4agri/Farm
saref4agri:Farm a owl:Class ;
      rdfs:subClassOf <http://www.opengis.net/ont/geosparql#Feature> ,
                      [ a owl:Restriction ;
                        owl:onProperty saref4agri:contains ;
                        owl:someValuesFrom saref4agri:Building
                      ] ,
                      [ a owl:Restriction ;
                        owl:onProperty saref4agri:contains ;
                        owl:someValuesFrom saref4agri:Parcel
                      ] ,
                      [ a owl:Restriction ;
                        owl:onProperty saref4agri:hasName ;
                        owl:maxCardinality "1"^^xsd:nonNegativeInteger
                      ] ;
      rdfs:comment "A plot of land used for the scope of farming which can contain buildings and parcels."@en ;
      rdfs:label "Farm" ;
      rdfs:isDefinedBy <https://saref.etsi.org/saref4agri/> .

###  https://saref.etsi.org/saref4agri/Building
saref4agri:Building a owl:Class ;
          rdfs:subClassOf <http://www.opengis.net/ont/geosparql#Feature> ,
                          [ a owl:Restriction ;
                            owl:onProperty saref4agri:contains ;
                            owl:someValuesFrom saref4agri:BuildingSpace
                          ] ,
                          [ a owl:Restriction ;
                            owl:onProperty saref4agri:hasName ;
                            owl:maxCardinality "1"^^xsd:nonNegativeInteger
                          ] ;
          rdfs:comment "A building represents a structure that provides shelter for its occupants or contents and stands in one place. The building is also used to provide a basic element within the spatial structure hierarchy for the components of a building project (together with site, storey, and space)."@en ;
          rdfs:label "Building" ;
          rdfs:isDefinedBy <https://saref.etsi.org/saref4agri/> .


###  https://saref.etsi.org/saref4agri/BuildingSpace
saref4agri:BuildingSpace a owl:Class ;
               rdfs:subClassOf <http://www.opengis.net/ont/geosparql#Feature> ;
               rdfs:comment "An entity used to define the physical spaces of the building. A building space contains devices or building objects."@en ;
               rdfs:label "Building space"@en ;
               rdfs:isDefinedBy <https://saref.etsi.org/saref4agri/> .


###  https://saref.etsi.org/saref4agri/Parcel
saref4agri:Parcel a owl:Class ;
        rdfs:subClassOf <http://www.opengis.net/ont/geosparql#Feature> ,
                        [ a owl:Restriction ;
                          owl:onProperty saref4agri:contains ;
                          owl:someValuesFrom saref4agri:Crop
                        ] ,
                        [ a owl:Restriction ;
                          owl:onProperty saref4agri:hasName ;
                          owl:maxQualifiedCardinality "1"^^xsd:nonNegativeInteger ;
                          owl:onDataRange xsd:string
                        ] ;
        rdfs:comment "An area of land, which might be used for grazing animals or planting crops. The parcel is defined as an undividable logical area of land which contains homogeneous items."@en ;
        rdfs:label "Parcel" ;
        rdfs:isDefinedBy <https://saref.etsi.org/saref4agri/> .

###  http://inspire.ec.europa.eu/schemas/af/3.0#Holding
af-inspire:Holding  a           owl:Class ;
        rdfs:subClassOf  act-inspire:ActivityComplex, geo:Feature ;
        rdfs:subClassOf  [ a                   owl:Restriction ;
                           owl:minCardinality  "1"^^xsd:int ;
                           owl:onProperty      af-inspire:contains
                         ] ;
        rdfs:subClassOf  [ a                   owl:Restriction ;
                           owl:cardinality  	"1"^^xsd:int ;
                           owl:onProperty      geo:hasGeometry
                         ] ;
				skos:prefLabel   "Holding"@en ;
        rdfs:label "Holding"@en ;
        rdfs:comment "The whole area and all infrastructures included on it, covering the same or different sites, under the control of an operator to perform agricultural or aquaculture activities" ;
        rdfs:isDefinedBy <http://inspire.ec.europa.eu/schemas/af/3.0#> .

###  http://inspire.ec.europa.eu/schemas/af/3.0#Site
af-inspire:Site  a           owl:Class ;
        rdfs:subClassOf  geo:Feature ;
        rdfs:subClassOf  [ a                   owl:Restriction ;
                           owl:minCardinality  "1"^^xsd:int ;
                           owl:onProperty      af-inspire:activity
                         ] ;
        rdfs:subClassOf  [ a                   owl:Restriction ;
                           owl:maxCardinality  "1"^^xsd:int ;
                           owl:onProperty      prov:invalidatedAtTime
                         ] ;
        rdfs:subClassOf  [ a                owl:Restriction ;
                           owl:maxCardinality  "1"^^xsd:int ;
                           owl:onProperty   prov:generatedAtTime
                         ] ;
        rdfs:subClassOf  [ a                owl:Restriction ;
                           owl:cardinality  "1"^^xsd:int ;
                           owl:onProperty   foodie:code
                         ] ;
        rdfs:subClassOf  [ a                   owl:Restriction ;
                           owl:cardinality  	"1"^^xsd:int ;
                           owl:onProperty      geo:hasGeometry
                         ] ;
        rdfs:subClassOf  [ a                owl:Restriction ;
                           owl:cardinality  "1"^^xsd:int ;
                           owl:onProperty   common:validFrom
                         ] ;
        rdfs:subClassOf  [ a                   owl:Restriction ;
                           owl:maxCardinality  "1"^^xsd:int ;
                           owl:onProperty      common:validTo
                         ] ;
        rdfs:subClassOf  [ a                   owl:Restriction ;
                           owl:minCardinality  	"1"^^xsd:int ;
                           owl:onProperty      foodie:containsPlot
                         ] ;
        skos:prefLabel   "Site"@en ;
        rdfs:label "Site"@en ;
        rdfs:comment "A agricultural or aquacultural facility. All land at a same or distinct geographic location under the management control of a holding covering activities, products and services. This includes all infrastructure, equipment and materials." ; 
        rdfs:isDefinedBy <http://inspire.ec.europa.eu/schemas/af/3.0#> .

###  http://foodie-cloud.com/model/foodie#Plot
foodie:Plot  a           owl:Class ;
        rdfs:subClassOf  geo:Feature ;
        rdfs:subClassOf  [ a                   owl:Restriction ;
                           owl:maxCardinality  "1"^^xsd:int ;
                           owl:onProperty      prov:invalidatedAtTime
                         ] ;
        rdfs:subClassOf  [ a                owl:Restriction ;
                           owl:maxCardinality  "1"^^xsd:int ;
                           owl:onProperty   prov:generatedAtTime
                         ] ;
        rdfs:subClassOf  [ a                owl:Restriction ;
                           owl:cardinality  "1"^^xsd:int ;
                           owl:onProperty   foodie:code
                         ] ;
        rdfs:subClassOf  [ a                owl:Restriction ;
                           owl:cardinality  "1"^^xsd:int ;
                           owl:onProperty   common:validFrom
                         ] ;
        rdfs:subClassOf  [ a                   owl:Restriction ;
                           owl:maxCardinality  "1"^^xsd:int ;
                           owl:onProperty      common:validTo
                         ] ;
        rdfs:subClassOf  [ a                   owl:Restriction ;
                           owl:maxCardinality  "1"^^xsd:int ;
                           owl:onProperty      foodie:description
                         ] ;
        rdfs:subClassOf  [ a                   owl:Restriction ;
                           owl:minCardinality  "1"^^xsd:int ;
                           owl:onProperty      geo:hasGeometry
                         ] ;
        skos:prefLabel   "Plot"@en ;
        rdfs:label "Plot"@en ;
        rdfs:comment "A continuous area of agricultural land with one type of crop species, cultivated by one user in one farming mode, e.g., conventional, transitional, organic farming" ; 
        rdfs:isDefinedBy <http://foodie-cloud.com/model/foodie> .

###  http://foodie-cloud.com/model/foodie#ManagementZone
foodie:ManagementZone
        a                owl:Class ;
        rdfs:subClassOf  geo:Feature ;
        rdfs:subClassOf  [ a                   owl:Restriction ;
                           owl:maxCardinality  "1"^^xsd:int ;
                           owl:onProperty      prov:invalidatedAtTime
                         ] ;
        rdfs:subClassOf  [ a                   owl:Restriction ;
                           owl:maxCardinality  "1"^^xsd:int ;
                           owl:onProperty      common:validTo
                         ] ;
        rdfs:subClassOf  [ a                   owl:Restriction ;
                           owl:maxCardinality  "1"^^xsd:int ;
                           owl:onProperty      common:validFrom
                         ] ;
        rdfs:subClassOf  [ a                owl:Restriction ;
                           owl:maxCardinality  "1"^^xsd:int ;
                           owl:onProperty   foodie:notes
                         ] ;
        rdfs:subClassOf  [ a                   owl:Restriction ;
                           owl:minCardinality  "1"^^xsd:int ;
                           owl:onProperty      geo:hasGeometry
                         ] ;
        rdfs:subClassOf  [ a                owl:Restriction ;
                           owl:cardinality  "1"^^xsd:int ;
                           owl:onProperty   prov:generatedAtTime
                         ] ;
        rdfs:subClassOf  [ a                owl:Restriction ;
                           owl:cardinality  "1"^^xsd:int ;
                           owl:onProperty   foodie:code
                         ] ;
        skos:prefLabel   "ManagementZone"@en ;
        rdfs:label "ManagementZone"@en ;
        rdfs:comment "A spatial subset of a Plot that has specific properties like electric conductivity, organic matter, pH, soil texture, soil type or soil nutrients" ; 
        rdfs:isDefinedBy <http://foodie-cloud.com/model/foodie> .

###  http://foodie-cloud.com/model/foodie#OriginTypeValue
foodie:OriginTypeValue	a	owl:Class ;
				rdfs:subClassOf  skos:Concept ;
        skos:prefLabel   "OriginTypeValue"@en ;
        rdfs:label "OriginTypeValue"@en ;
        rdfs:comment "Origin of a Plot when taking into consideration only two options: manual (created by human user) and system generated" ; 
        rdfs:isDefinedBy <http://foodie-cloud.com/model/foodie> .

###  http://inspire.ec.europa.eu/schemas/act-core/3.0#EconomicActivityNACEValue
act-inspire:EconomicActivityNACEValue a owl:Class ;
                                        rdfs:subClassOf  skos:Concept ;
      rdfs:label "EconomicActivityNACEValue" ;
      rdfs:label "EconomicActivityNACEValue"@en ;
      rdfs:comment "The classification of the economic activity according to the NACE" ; 
      rdfs:isDefinedBy <http://inspire.ec.europa.eu/schemas/act-core/3.0#> .

### https://smartdatamodels.org/dataModel.Agrifood/AgriParcel
fiware-agrifood:AgriParcel	a owl:Class ;
			rdfs:label "Agri Parcel" ;
			rdfs:comment "This entity contains a harmonised description of a generic parcel of land. This entity is primarily associated with the agricultural vertical and related IoT applications." ;
			rdfs:isDefinedBy <https://github.com/smart-data-models/dataModel.Agrifood/blob/master/AgriParcel/schema.json> .

### https://smartdatamodels.org/dataModel.Agrifood/AgriFarm
fiware-agrifood:AgriFarm	a owl:Class ;
			rdfs:label "Agri Farm" ;
			rdfs:comment "This entity contains a harmonised description of a generic farm made up of buildings and parcels. This entity is primarily associated with the agricultural vertical and related IoT applications." ;
			rdfs:isDefinedBy <https://github.com/smart-data-models/dataModel.Agrifood/blob/master/AgriFarm/schema.json> .

### https://smartdatamodels.org/dataModel.Agrifood/AgriGreenhouse
fiware-agrifood:AgriGreenhouse	a owl:Class ;
			rdfs:subClassOf  fiware-agrifood:AgriParcel ;
			rdfs:label "Agri Greenhouse" ;
			rdfs:comment "This entity contains a harmonised description of the conditions recorded within a generic greenhouse, a type of AgriParcel. This entity is primarily associated with the agricultural vertical and related IoT applications." ;
			rdfs:isDefinedBy <https://github.com/smart-data-models/dataModel.Agrifood/blob/master/AgriGreenhouse/schema.json> .

#################################################################
#    Alignments
#################################################################

saref4agri:Farm owl:equivalentClass af-inspire:Holding .
saref4agri:Farm owl:equivalentClass fiware-agrifood:AgriFarm .
saref4agri:Parcel owl:equivalentClass foodie:Plot .
saref4agri:Parcel owl:equivalentClass fiware-agrifood:AgriParcel .
foodie:crop owl:equivalentProperty fiware-agrifood:hasAgriCrop .
geo:hasGeometry owl:equivalentProperty wgs84_pos:location .
ngsi-ld:location rdfs:subPropertyOf geo:hasGeometry .
fiware-agrifood:landLocation rdfs:subPropertyOf ngsi-ld:location .
af-inspire:contains rdfs:subPropertyOf saref4agri:contains .
foodie:containsPlot rdfs:subPropertyOf saref4agri:contains .
foodie:containsZone rdfs:subPropertyOf saref4agri:contains .
fiware-agrifood:hasAgriParcelChildren rdfs:subPropertyOf saref4agri:contains .
fiware-agrifood:hasAgriParcel rdfs:subPropertyOf saref4agri:contains .
foodie:holdingSite rdfs:subPropertyOf saref4agri:isContainedIn .
foodie:holdingPlot rdfs:subPropertyOf saref4agri:isContainedIn .
foodie:holdingZone rdfs:subPropertyOf saref4agri:isContainedIn .
fiware-agrifood:hasAgriParcelParent rdfs:subPropertyOf saref4agri:isContainedIn .
saref4agri:contains rdfs:subPropertyOf geo:sfContains .
saref4agri:isContainedIn rdfs:subPropertyOf geo:sfWithin .

#################################################################
#    Individuals
#################################################################
