<rdf:RDF
    xmlns:wgs84_pos="http://www.w3.org/2003/01/geo/wgs84_pos#"
    xmlns:af-inspire="http://inspire.ec.europa.eu/schemas/af/3.0#"
    xmlns:sf="http://www.opengis.net/ont/sf#"
    xmlns:common="http://portele.de/ont/inspire/baseInspire#"
    xmlns:dct="http://purl.org/dc/terms/"
    xmlns:saref4agri="https://saref.etsi.org/saref4agri/"
    xmlns:prov="http://www.w3.org/ns/prov#"
    xmlns:skos="http://www.w3.org/2004/02/skos/core#"
    xmlns:foodie="http://foodie-cloud.com/model/foodie#"
    xmlns:xsd="http://www.w3.org/2001/XMLSchema#"
    xmlns:rdf="http://www.w3.org/1999/02/22-rdf-syntax-ns#"
    xmlns:schema="https://schema.org/"
    xmlns:fiware="https://smartdatamodels.org/"
    xmlns:iso19109="http://def.seegrid.csiro.au/isotc211/iso19109/2005/feature#"
    xmlns:iso19150-2="http://def.seegrid.csiro.au/isotc211/iso19150/-2/2012/basic#"
    xmlns:stat="http://data.europa.eu/m8g/"
    xmlns:rdfs="http://www.w3.org/2000/01/rdf-schema#"
    xmlns:ngsi-ld="https://uri.etsi.org/ngsi-ld/"
    xmlns:owl="http://www.w3.org/2002/07/owl#"
    xmlns:qb="http://purl.org/linked-data/cube#"
    xmlns:geo="http://www.opengis.net/ont/geosparql#"
    xmlns:dcat="http://www.w3.org/ns/dcat#"
    xmlns="https://w3id.org/cybele/"
    xmlns:act-inspire="http://inspire.ec.europa.eu/schemas/act-core/3.0#"
    xmlns:foaf="http://xmlns.com/foaf/0.1/"
    xmlns:fiware-agrifood="https://smartdatamodels.org/dataModel.Agrifood/" > 
  <rdf:Description rdf:nodeID="A0">
    <owl:onProperty rdf:resource="http://portele.de/ont/inspire/baseInspire#validFrom"/>
    <owl:maxCardinality rdf:datatype="http://www.w3.org/2001/XMLSchema#int">1</owl:maxCardinality>
    <rdf:type rdf:resource="http://www.w3.org/2002/07/owl#Restriction"/>
  </rdf:Description>
  <rdf:Description rdf:about="https://smartdatamodels.org/dataModel.Agrifood/landLocation">
    <rdfs:subPropertyOf rdf:resource="https://uri.etsi.org/ngsi-ld/location"/>
    <rdfs:isDefinedBy rdf:resource="https://github.com/smart-data-models/dataModel.Agrifood/blob/master/AgriFarm/schema.json"/>
    <rdfs:comment>Geometry defining the boundaries of the farm land</rdfs:comment>
    <rdfs:label xml:lang="en">landLocation</rdfs:label>
    <rdf:type rdf:resource="http://www.w3.org/2002/07/owl#ObjectProperty"/>
  </rdf:Description>
  <rdf:Description rdf:about="http://www.opengis.net/ont/geosparql#hasGeometry">
    <owl:equivalentProperty rdf:resource="http://www.w3.org/2003/01/geo/wgs84_pos#location"/>
  </rdf:Description>
  <rdf:Description rdf:about="http://foodie-cloud.com/model/foodie#crop">
    <owl:equivalentProperty rdf:resource="https://smartdatamodels.org/dataModel.Agrifood/hasAgriCrop"/>
    <rdfs:isDefinedBy rdf:resource="http://foodie-cloud.com/model/foodie"/>
    <rdfs:comment>A relation from Plot to CropSpecies</rdfs:comment>
    <rdfs:label xml:lang="en">crop</rdfs:label>
    <skos:prefLabel xml:lang="en">crop</skos:prefLabel>
    <rdf:type rdf:resource="http://www.w3.org/2002/07/owl#ObjectProperty"/>
  </rdf:Description>
  <rdf:Description rdf:about="http://foodie-cloud.com/model/foodie#OriginTypeValue">
    <rdfs:isDefinedBy rdf:resource="http://foodie-cloud.com/model/foodie"/>
    <rdfs:comment>Origin of a Plot when taking into consideration only two options: manual (created by human user) and system generated</rdfs:comment>
    <rdfs:label xml:lang="en">OriginTypeValue</rdfs:label>
    <skos:prefLabel xml:lang="en">OriginTypeValue</skos:prefLabel>
    <rdfs:subClassOf rdf:resource="http://www.w3.org/2004/02/skos/core#Concept"/>
    <rdf:type rdf:resource="http://www.w3.org/2002/07/owl#Class"/>
  </rdf:Description>
  <rdf:Description rdf:nodeID="A1">
    <owl:onProperty rdf:resource="http://portele.de/ont/inspire/baseInspire#validTo"/>
    <owl:maxCardinality rdf:datatype="http://www.w3.org/2001/XMLSchema#int">1</owl:maxCardinality>
    <rdf:type rdf:resource="http://www.w3.org/2002/07/owl#Restriction"/>
  </rdf:Description>
  <rdf:Description rdf:nodeID="A2">
    <owl:onProperty rdf:resource="http://portele.de/ont/inspire/baseInspire#validFrom"/>
    <owl:cardinality rdf:datatype="http://www.w3.org/2001/XMLSchema#int">1</owl:cardinality>
    <rdf:type rdf:resource="http://www.w3.org/2002/07/owl#Restriction"/>
  </rdf:Description>
  <rdf:Description rdf:nodeID="A3">
    <owl:onProperty rdf:resource="http://foodie-cloud.com/model/foodie#containsPlot"/>
    <owl:minCardinality rdf:datatype="http://www.w3.org/2001/XMLSchema#int">1</owl:minCardinality>
    <rdf:type rdf:resource="http://www.w3.org/2002/07/owl#Restriction"/>
  </rdf:Description>
  <rdf:Description rdf:about="http://foodie-cloud.com/model/foodie#containsZone">
    <rdfs:subPropertyOf rdf:resource="https://saref.etsi.org/saref4agri/contains"/>
    <rdfs:isDefinedBy rdf:resource="http://foodie-cloud.com/model/foodie"/>
    <rdfs:comment>A relation from Plot to Management zone</rdfs:comment>
    <rdfs:label xml:lang="en">containsZone</rdfs:label>
    <skos:prefLabel xml:lang="en">containsZone</skos:prefLabel>
    <rdfs:range rdf:resource="http://foodie-cloud.com/model/foodie#ManagementZone"/>
    <rdf:type rdf:resource="http://www.w3.org/2002/07/owl#ObjectProperty"/>
  </rdf:Description>
  <rdf:Description rdf:nodeID="A4">
    <owl:maxCardinality rdf:datatype="http://www.w3.org/2001/XMLSchema#nonNegativeInteger">1</owl:maxCardinality>
    <owl:onProperty rdf:resource="https://saref.etsi.org/saref4agri/hasName"/>
    <rdf:type rdf:resource="http://www.w3.org/2002/07/owl#Restriction"/>
  </rdf:Description>
  <rdf:Description rdf:nodeID="A5">
    <owl:onProperty rdf:resource="http://portele.de/ont/inspire/baseInspire#validFrom"/>
    <owl:cardinality rdf:datatype="http://www.w3.org/2001/XMLSchema#int">1</owl:cardinality>
    <rdf:type rdf:resource="http://www.w3.org/2002/07/owl#Restriction"/>
  </rdf:Description>
  <rdf:Description rdf:nodeID="A6">
    <owl:onProperty rdf:resource="http://inspire.ec.europa.eu/schemas/af/3.0#contains"/>
    <owl:minCardinality rdf:datatype="http://www.w3.org/2001/XMLSchema#int">1</owl:minCardinality>
    <rdf:type rdf:resource="http://www.w3.org/2002/07/owl#Restriction"/>
  </rdf:Description>
  <rdf:Description rdf:nodeID="A7">
    <owl:onProperty rdf:resource="http://foodie-cloud.com/model/foodie#notes"/>
    <owl:maxCardinality rdf:datatype="http://www.w3.org/2001/XMLSchema#int">1</owl:maxCardinality>
    <rdf:type rdf:resource="http://www.w3.org/2002/07/owl#Restriction"/>
  </rdf:Description>
  <rdf:Description rdf:about="https://saref.etsi.org/saref4agri/isContainedIn">
    <rdfs:subPropertyOf rdf:resource="http://www.opengis.net/ont/geosparql#sfWithin"/>
    <rdfs:isDefinedBy rdf:resource="https://saref.etsi.org/saref4agri/"/>
    <rdfs:comment>A relation inverse of s4agri:contains</rdfs:comment>
    <rdfs:label xml:lang="en">is contained in</rdfs:label>
    <rdf:type rdf:resource="http://www.w3.org/2002/07/owl#ObjectProperty"/>
  </rdf:Description>
  <rdf:Description rdf:nodeID="A8">
    <owl:onProperty rdf:resource="http://portele.de/ont/inspire/baseInspire#validTo"/>
    <owl:maxCardinality rdf:datatype="http://www.w3.org/2001/XMLSchema#int">1</owl:maxCardinality>
    <rdf:type rdf:resource="http://www.w3.org/2002/07/owl#Restriction"/>
  </rdf:Description>
  <rdf:Description rdf:nodeID="A9">
    <owl:onProperty rdf:resource="http://www.w3.org/ns/prov#invalidatedAtTime"/>
    <owl:maxCardinality rdf:datatype="http://www.w3.org/2001/XMLSchema#int">1</owl:maxCardinality>
    <rdf:type rdf:resource="http://www.w3.org/2002/07/owl#Restriction"/>
  </rdf:Description>
  <rdf:Description rdf:about="https://saref.etsi.org/saref4agri/BuildingSpace">
    <rdfs:isDefinedBy rdf:resource="https://saref.etsi.org/saref4agri/"/>
    <rdfs:label xml:lang="en">Building space</rdfs:label>
    <rdfs:comment xml:lang="en">An entity used to define the physical spaces of the building. A building space contains devices or building objects.</rdfs:comment>
    <rdfs:subClassOf rdf:resource="http://www.opengis.net/ont/geosparql#Feature"/>
    <rdf:type rdf:resource="http://www.w3.org/2002/07/owl#Class"/>
  </rdf:Description>
  <rdf:Description rdf:about="https://saref.etsi.org/saref4agri/Building">
    <rdfs:isDefinedBy rdf:resource="https://saref.etsi.org/saref4agri/"/>
    <rdfs:label>Building</rdfs:label>
    <rdfs:comment xml:lang="en">A building represents a structure that provides shelter for its occupants or contents and stands in one place. The building is also used to provide a basic element within the spatial structure hierarchy for the components of a building project (together with site, storey, and space).</rdfs:comment>
    <rdfs:subClassOf rdf:nodeID="A4"/>
    <rdfs:subClassOf rdf:nodeID="A10"/>
    <rdfs:subClassOf rdf:resource="http://www.opengis.net/ont/geosparql#Feature"/>
    <rdf:type rdf:resource="http://www.w3.org/2002/07/owl#Class"/>
  </rdf:Description>
  <rdf:Description rdf:about="https://smartdatamodels.org/dataModel.Agrifood/hasAgriParcel">
    <rdfs:subPropertyOf rdf:resource="https://saref.etsi.org/saref4agri/contains"/>
    <rdfs:isDefinedBy rdf:resource="https://github.com/smart-data-models/dataModel.Agrifood/blob/master/AgriFarm/schema.json"/>
    <rdfs:comment>List of agri parcels belonging to the farm</rdfs:comment>
    <rdfs:label xml:lang="en">hasAgriParcel</rdfs:label>
    <rdf:type rdf:resource="http://www.w3.org/2002/07/owl#ObjectProperty"/>
  </rdf:Description>
  <rdf:Description rdf:nodeID="A11">
    <foaf:name>Rob Atkinson</foaf:name>
    <schema:affiliation rdf:nodeID="A12"/>
  </rdf:Description>
  <rdf:Description rdf:nodeID="A10">
    <owl:someValuesFrom rdf:resource="https://saref.etsi.org/saref4agri/BuildingSpace"/>
    <owl:onProperty rdf:resource="https://saref.etsi.org/saref4agri/contains"/>
    <rdf:type rdf:resource="http://www.w3.org/2002/07/owl#Restriction"/>
  </rdf:Description>
  <rdf:Description rdf:about="https://saref.etsi.org/saref4agri/Farm">
    <rdfs:comment xml:lang="en">A plot of land used for the scope of farming which can contain buildings and parcels.</rdfs:comment>
    <rdfs:subClassOf rdf:nodeID="A13"/>
    <owl:equivalentClass rdf:resource="http://inspire.ec.europa.eu/schemas/af/3.0#Holding"/>
    <rdfs:subClassOf rdf:resource="http://www.opengis.net/ont/geosparql#Feature"/>
    <rdf:type rdf:resource="http://www.w3.org/2002/07/owl#Class"/>
    <rdfs:label>Farm</rdfs:label>
    <rdfs:subClassOf rdf:nodeID="A14"/>
    <owl:equivalentClass rdf:resource="https://smartdatamodels.org/dataModel.Agrifood/AgriFarm"/>
    <rdfs:subClassOf rdf:nodeID="A15"/>
    <rdfs:isDefinedBy rdf:resource="https://saref.etsi.org/saref4agri/"/>
  </rdf:Description>
  <rdf:Description rdf:nodeID="A16">
    <foaf:name>DEMETER project</foaf:name>
    <foaf:homepage rdf:resource="https://h2020-demeter.eu/"/>
  </rdf:Description>
  <rdf:Description rdf:about="https://smartdatamodels.org/dataModel.Agrifood/area">
    <rdfs:isDefinedBy rdf:resource="https://github.com/smart-data-models/dataModel.Agrifood/blob/master/AgriParcel/schema.json"/>
    <rdfs:comment>The area of the parcel nominally in square meters.</rdfs:comment>
    <rdfs:label xml:lang="en">area</rdfs:label>
    <rdf:type rdf:resource="http://www.w3.org/2002/07/owl#DatatypeProperty"/>
  </rdf:Description>
  <rdf:Description rdf:nodeID="A17">
    <owl:onProperty rdf:resource="http://www.w3.org/ns/prov#invalidatedAtTime"/>
    <owl:maxCardinality rdf:datatype="http://www.w3.org/2001/XMLSchema#int">1</owl:maxCardinality>
    <rdf:type rdf:resource="http://www.w3.org/2002/07/owl#Restriction"/>
  </rdf:Description>
  <rdf:Description rdf:nodeID="A18">
    <owl:someValuesFrom rdf:resource="https://saref.etsi.org/saref4agri/Crop"/>
    <owl:onProperty rdf:resource="https://saref.etsi.org/saref4agri/contains"/>
    <rdf:type rdf:resource="http://www.w3.org/2002/07/owl#Restriction"/>
  </rdf:Description>
  <rdf:Description rdf:about="https://smartdatamodels.org/dataModel.Agrifood/hasAgriParcelChildren">
    <rdfs:subPropertyOf rdf:resource="https://saref.etsi.org/saref4agri/contains"/>
    <rdfs:isDefinedBy rdf:resource="https://github.com/smart-data-models/dataModel.Agrifood/blob/master/AgriParcel/schema.json"/>
    <rdfs:comment>Related sub AgriParcel records to which this entity relates</rdfs:comment>
    <rdfs:label xml:lang="en">hasAgriParcelChildren</rdfs:label>
    <rdf:type rdf:resource="http://www.w3.org/2002/07/owl#ObjectProperty"/>
  </rdf:Description>
  <rdf:Description rdf:about="https://saref.etsi.org/saref4agri/contains">
    <rdfs:subPropertyOf rdf:resource="http://www.opengis.net/ont/geosparql#sfContains"/>
    <rdfs:isDefinedBy rdf:resource="https://saref.etsi.org/saref4agri/"/>
    <rdfs:comment>A realtion to represent the contained land parcel</rdfs:comment>
    <rdfs:label>contains</rdfs:label>
    <owl:inverseOf rdf:resource="https://saref.etsi.org/saref4agri/isContainedIn"/>
    <rdf:type rdf:resource="http://www.w3.org/2002/07/owl#ObjectProperty"/>
  </rdf:Description>
  <rdf:Description rdf:about="http://foodie-cloud.com/model/foodie#holdingPlot">
    <rdfs:subPropertyOf rdf:resource="https://saref.etsi.org/saref4agri/isContainedIn"/>
    <rdfs:isDefinedBy rdf:resource="http://foodie-cloud.com/model/foodie"/>
    <rdfs:comment>A relation from Plot to Site</rdfs:comment>
    <rdfs:label xml:lang="en">holdingPlot</rdfs:label>
    <skos:prefLabel xml:lang="en">holdingPlot</skos:prefLabel>
    <rdfs:range rdf:resource="http://inspire.ec.europa.eu/schemas/af/3.0#Site"/>
    <rdf:type rdf:resource="http://www.w3.org/2002/07/owl#ObjectProperty"/>
  </rdf:Description>
  <rdf:Description rdf:about="https://smartdatamodels.org/dataModel.Agrifood/AgriParcel">
    <rdfs:isDefinedBy rdf:resource="https://github.com/smart-data-models/dataModel.Agrifood/blob/master/AgriParcel/schema.json"/>
    <rdfs:comment>This entity contains a harmonised description of a generic parcel of land. This entity is primarily associated with the agricultural vertical and related IoT applications.</rdfs:comment>
    <rdfs:label>Agri Parcel</rdfs:label>
    <rdf:type rdf:resource="http://www.w3.org/2002/07/owl#Class"/>
  </rdf:Description>
  <rdf:Description rdf:about="https://smartdatamodels.org/dataModel.Agrifood/hasAgriParcelParent">
    <rdfs:subPropertyOf rdf:resource="https://saref.etsi.org/saref4agri/isContainedIn"/>
    <rdfs:isDefinedBy rdf:resource="https://github.com/smart-data-models/dataModel.Agrifood/blob/master/AgriParcel/schema.json"/>
    <rdfs:comment>Reference to the parent AgriParcel</rdfs:comment>
    <rdfs:label xml:lang="en">hasAgriParcelParent</rdfs:label>
    <rdf:type rdf:resource="http://www.w3.org/2002/07/owl#ObjectProperty"/>
  </rdf:Description>
  <rdf:Description rdf:about="https://w3id.org/demeter/agri/agriFeature">
    <rdf:type rdf:resource="http://www.w3.org/2002/07/owl#Ontology"/>
    <owl:versionIRI rdf:resource="https://w3id.org/demeter/agri/agriFeature/2.0"/>
    <dct:rights xml:lang="en">This vocabulary is distributed under Creative Commons Attribution 4.0 License - http://creativecommons.org/licenses/by/4.0</dct:rights>
    <dct:title xml:lang="en">DEMETER AgriFeature</dct:title>
    <dct:description xml:lang="en">The DEMETER AgriFeature is one of the agri profiles of DEMETER AIM. This profile was created by reusing and aligning well-known ontologies and vocabularies</dct:description>
    <owl:imports rdf:resource="https://w3id.org/demeter/agri/agriCommon"/>
    <dct:creator rdf:nodeID="A19"/>
    <dct:contributor rdf:nodeID="A11"/>
    <rdfs:comment xml:lang="en">The DEMETER Agriculture Information Model (AIM) is the common vocabulary in DEMETER project providing the basis for semantic interoperability across smart farming solutions</rdfs:comment>
    <dct:contributor rdf:nodeID="A20"/>
    <foaf:maker rdf:nodeID="A16"/>
    <owl:versionInfo>2.0</owl:versionInfo>
    <rdfs:label xml:lang="en">DEMETER AgriFeature</rdfs:label>
  </rdf:Description>
  <rdf:Description rdf:nodeID="A21">
    <owl:onProperty rdf:resource="http://www.opengis.net/ont/geosparql#hasGeometry"/>
    <owl:minCardinality rdf:datatype="http://www.w3.org/2001/XMLSchema#int">1</owl:minCardinality>
    <rdf:type rdf:resource="http://www.w3.org/2002/07/owl#Restriction"/>
  </rdf:Description>
  <rdf:Description rdf:about="http://inspire.ec.europa.eu/schemas/act-core/3.0#EconomicActivityNACEValue">
    <rdfs:isDefinedBy rdf:resource="http://inspire.ec.europa.eu/schemas/act-core/3.0#"/>
    <rdfs:comment>The classification of the economic activity according to the NACE</rdfs:comment>
    <rdfs:label xml:lang="en">EconomicActivityNACEValue</rdfs:label>
    <rdfs:label>EconomicActivityNACEValue</rdfs:label>
    <rdfs:subClassOf rdf:resource="http://www.w3.org/2004/02/skos/core#Concept"/>
    <rdf:type rdf:resource="http://www.w3.org/2002/07/owl#Class"/>
  </rdf:Description>
  <rdf:Description rdf:about="http://inspire.ec.europa.eu/schemas/af/3.0#contains">
    <rdfs:subPropertyOf rdf:resource="https://saref.etsi.org/saref4agri/contains"/>
    <rdfs:isDefinedBy rdf:resource="http://inspire.ec.europa.eu/schemas/af/3.0#"/>
    <rdfs:comment>A relation from Holding to Site </rdfs:comment>
    <rdfs:label xml:lang="en">contains</rdfs:label>
    <skos:prefLabel xml:lang="en">contains</skos:prefLabel>
    <rdfs:range rdf:resource="http://inspire.ec.europa.eu/schemas/af/3.0#Site"/>
    <rdf:type rdf:resource="http://www.w3.org/2002/07/owl#ObjectProperty"/>
  </rdf:Description>
  <rdf:Description rdf:about="http://foodie-cloud.com/model/foodie#holdingSite">
    <rdfs:subPropertyOf rdf:resource="https://saref.etsi.org/saref4agri/isContainedIn"/>
    <rdfs:isDefinedBy rdf:resource="http://foodie-cloud.com/model/foodie"/>
    <rdfs:comment>A relation from Site to Holding</rdfs:comment>
    <rdfs:label xml:lang="en">holdingSite</rdfs:label>
    <skos:prefLabel xml:lang="en">holdingSite</skos:prefLabel>
    <rdfs:range rdf:resource="http://inspire.ec.europa.eu/schemas/af/3.0#Holding"/>
    <rdf:type rdf:resource="http://www.w3.org/2002/07/owl#ObjectProperty"/>
  </rdf:Description>
  <rdf:Description rdf:nodeID="A13">
    <owl:someValuesFrom rdf:resource="https://saref.etsi.org/saref4agri/Parcel"/>
    <owl:onProperty rdf:resource="https://saref.etsi.org/saref4agri/contains"/>
    <rdf:type rdf:resource="http://www.w3.org/2002/07/owl#Restriction"/>
  </rdf:Description>
  <rdf:Description rdf:nodeID="A15">
    <owl:maxCardinality rdf:datatype="http://www.w3.org/2001/XMLSchema#nonNegativeInteger">1</owl:maxCardinality>
    <owl:onProperty rdf:resource="https://saref.etsi.org/saref4agri/hasName"/>
    <rdf:type rdf:resource="http://www.w3.org/2002/07/owl#Restriction"/>
  </rdf:Description>
  <rdf:Description rdf:about="http://foodie-cloud.com/model/foodie#ManagementZone">
    <rdfs:subClassOf rdf:nodeID="A9"/>
    <rdfs:subClassOf rdf:nodeID="A22"/>
    <rdfs:subClassOf rdf:resource="http://www.opengis.net/ont/geosparql#Feature"/>
    <rdfs:subClassOf rdf:nodeID="A0"/>
    <rdf:type rdf:resource="http://www.w3.org/2002/07/owl#Class"/>
    <rdfs:subClassOf rdf:nodeID="A7"/>
    <rdfs:isDefinedBy rdf:resource="http://foodie-cloud.com/model/foodie"/>
    <rdfs:subClassOf rdf:nodeID="A23"/>
    <skos:prefLabel xml:lang="en">ManagementZone</skos:prefLabel>
    <rdfs:subClassOf rdf:nodeID="A24"/>
    <rdfs:comment>A spatial subset of a Plot that has specific properties like electric conductivity, organic matter, pH, soil texture, soil type or soil nutrients</rdfs:comment>
    <rdfs:label xml:lang="en">ManagementZone</rdfs:label>
    <rdfs:subClassOf rdf:nodeID="A25"/>
  </rdf:Description>
  <rdf:Description rdf:nodeID="A22">
    <owl:onProperty rdf:resource="http://www.opengis.net/ont/geosparql#hasGeometry"/>
    <owl:minCardinality rdf:datatype="http://www.w3.org/2001/XMLSchema#int">1</owl:minCardinality>
    <rdf:type rdf:resource="http://www.w3.org/2002/07/owl#Restriction"/>
  </rdf:Description>
  <rdf:Description rdf:about="https://smartdatamodels.org/dataModel.Agrifood/hasAgriSoil">
    <rdfs:isDefinedBy rdf:resource="https://github.com/smart-data-models/dataModel.Agrifood/blob/master/AgriParcel/schema.json"/>
    <rdfs:comment>Reference to the soil associated with this parcel of land</rdfs:comment>
    <rdfs:label xml:lang="en">hasAgriSoil</rdfs:label>
    <rdf:type rdf:resource="http://www.w3.org/2002/07/owl#ObjectProperty"/>
  </rdf:Description>
  <rdf:Description rdf:about="https://smartdatamodels.org/dataModel.Agrifood/cropStatus">
    <rdfs:isDefinedBy rdf:resource="https://github.com/smart-data-models/dataModel.Agrifood/blob/master/AgriParcel/schema.json"/>
    <rdfs:comment>A choice from an enumerated list describing the crop planting status One of: seeded, justBorn, growing, maturing, readyForHarvesting.</rdfs:comment>
    <rdfs:label xml:lang="en">cropStatus</rdfs:label>
    <rdf:type rdf:resource="http://www.w3.org/2002/07/owl#DatatypeProperty"/>
  </rdf:Description>
  <rdf:Description rdf:nodeID="A12">
    <foaf:name>OGC</foaf:name>
  </rdf:Description>
  <rdf:Description rdf:nodeID="A23">
    <owl:onProperty rdf:resource="http://foodie-cloud.com/model/foodie#code"/>
    <owl:cardinality rdf:datatype="http://www.w3.org/2001/XMLSchema#int">1</owl:cardinality>
    <rdf:type rdf:resource="http://www.w3.org/2002/07/owl#Restriction"/>
  </rdf:Description>
  <rdf:Description rdf:about="https://smartdatamodels.org/dataModel.Agrifood/AgriFarm">
    <rdfs:isDefinedBy rdf:resource="https://github.com/smart-data-models/dataModel.Agrifood/blob/master/AgriFarm/schema.json"/>
    <rdfs:comment>This entity contains a harmonised description of a generic farm made up of buildings and parcels. This entity is primarily associated with the agricultural vertical and related IoT applications.</rdfs:comment>
    <rdfs:label>Agri Farm</rdfs:label>
    <rdf:type rdf:resource="http://www.w3.org/2002/07/owl#Class"/>
  </rdf:Description>
  <rdf:Description rdf:nodeID="A14">
    <owl:someValuesFrom rdf:resource="https://saref.etsi.org/saref4agri/Building"/>
    <owl:onProperty rdf:resource="https://saref.etsi.org/saref4agri/contains"/>
    <rdf:type rdf:resource="http://www.w3.org/2002/07/owl#Restriction"/>
  </rdf:Description>
  <rdf:Description rdf:about="http://inspire.ec.europa.eu/schemas/af/3.0#Holding">
    <rdfs:isDefinedBy rdf:resource="http://inspire.ec.europa.eu/schemas/af/3.0#"/>
    <rdfs:comment>The whole area and all infrastructures included on it, covering the same or different sites, under the control of an operator to perform agricultural or aquaculture activities</rdfs:comment>
    <rdfs:label xml:lang="en">Holding</rdfs:label>
    <skos:prefLabel xml:lang="en">Holding</skos:prefLabel>
    <rdfs:subClassOf rdf:nodeID="A26"/>
    <rdfs:subClassOf rdf:nodeID="A6"/>
    <rdfs:subClassOf rdf:resource="http://www.opengis.net/ont/geosparql#Feature"/>
    <rdfs:subClassOf rdf:resource="http://inspire.ec.europa.eu/schemas/act-core/3.0#ActivityComplex"/>
    <rdf:type rdf:resource="http://www.w3.org/2002/07/owl#Class"/>
  </rdf:Description>
  <rdf:Description rdf:about="http://foodie-cloud.com/model/foodie#Plot">
    <rdfs:label xml:lang="en">Plot</rdfs:label>
    <rdfs:subClassOf rdf:nodeID="A27"/>
    <rdfs:subClassOf rdf:nodeID="A21"/>
    <rdfs:comment>A continuous area of agricultural land with one type of crop species, cultivated by one user in one farming mode, e.g., conventional, transitional, organic farming</rdfs:comment>
    <rdf:type rdf:resource="http://www.w3.org/2002/07/owl#Class"/>
    <rdfs:subClassOf rdf:nodeID="A2"/>
    <rdfs:subClassOf rdf:nodeID="A28"/>
    <rdfs:subClassOf rdf:nodeID="A29"/>
    <skos:prefLabel xml:lang="en">Plot</skos:prefLabel>
    <rdfs:subClassOf rdf:nodeID="A30"/>
    <rdfs:subClassOf rdf:nodeID="A8"/>
    <rdfs:subClassOf rdf:resource="http://www.opengis.net/ont/geosparql#Feature"/>
    <rdfs:isDefinedBy rdf:resource="http://foodie-cloud.com/model/foodie"/>
  </rdf:Description>
  <rdf:Description rdf:nodeID="A31">
    <owl:onDataRange rdf:resource="http://www.w3.org/2001/XMLSchema#string"/>
    <owl:maxQualifiedCardinality rdf:datatype="http://www.w3.org/2001/XMLSchema#nonNegativeInteger">1</owl:maxQualifiedCardinality>
    <owl:onProperty rdf:resource="https://saref.etsi.org/saref4agri/hasName"/>
    <rdf:type rdf:resource="http://www.w3.org/2002/07/owl#Restriction"/>
  </rdf:Description>
  <rdf:Description rdf:about="http://inspire.ec.europa.eu/schemas/af/3.0#Site">
    <skos:prefLabel xml:lang="en">Site</skos:prefLabel>
    <rdfs:isDefinedBy rdf:resource="http://inspire.ec.europa.eu/schemas/af/3.0#"/>
    <rdfs:subClassOf rdf:nodeID="A32"/>
    <rdfs:subClassOf rdf:nodeID="A33"/>
    <rdfs:subClassOf rdf:nodeID="A1"/>
    <rdfs:subClassOf rdf:resource="http://www.opengis.net/ont/geosparql#Feature"/>
    <rdfs:subClassOf rdf:nodeID="A17"/>
    <rdfs:subClassOf rdf:nodeID="A34"/>
    <rdfs:subClassOf rdf:nodeID="A3"/>
    <rdfs:label xml:lang="en">Site</rdfs:label>
    <rdfs:subClassOf rdf:nodeID="A5"/>
    <rdf:type rdf:resource="http://www.w3.org/2002/07/owl#Class"/>
    <rdfs:subClassOf rdf:nodeID="A35"/>
    <rdfs:comment>A agricultural or aquacultural facility. All land at a same or distinct geographic location under the management control of a holding covering activities, products and services. This includes all infrastructure, equipment and materials.</rdfs:comment>
  </rdf:Description>
  <rdf:Description rdf:nodeID="A35">
    <owl:onProperty rdf:resource="http://inspire.ec.europa.eu/schemas/af/3.0#activity"/>
    <owl:minCardinality rdf:datatype="http://www.w3.org/2001/XMLSchema#int">1</owl:minCardinality>
    <rdf:type rdf:resource="http://www.w3.org/2002/07/owl#Restriction"/>
  </rdf:Description>
  <rdf:Description rdf:about="http://foodie-cloud.com/model/foodie#holdingZone">
    <rdfs:subPropertyOf rdf:resource="https://saref.etsi.org/saref4agri/isContainedIn"/>
    <rdfs:isDefinedBy rdf:resource="http://foodie-cloud.com/model/foodie"/>
    <rdfs:comment>A relation from Management Zone to Plot</rdfs:comment>
    <rdfs:label xml:lang="en">holdingPlot</rdfs:label>
    <skos:prefLabel xml:lang="en">holdingZone</skos:prefLabel>
    <rdfs:range rdf:resource="http://foodie-cloud.com/model/foodie#Plot"/>
    <rdf:type rdf:resource="http://www.w3.org/2002/07/owl#ObjectProperty"/>
  </rdf:Description>
  <rdf:Description rdf:nodeID="A26">
    <owl:onProperty rdf:resource="http://www.opengis.net/ont/geosparql#hasGeometry"/>
    <owl:cardinality rdf:datatype="http://www.w3.org/2001/XMLSchema#int">1</owl:cardinality>
    <rdf:type rdf:resource="http://www.w3.org/2002/07/owl#Restriction"/>
  </rdf:Description>
  <rdf:Description rdf:nodeID="A34">
    <owl:onProperty rdf:resource="http://foodie-cloud.com/model/foodie#code"/>
    <owl:cardinality rdf:datatype="http://www.w3.org/2001/XMLSchema#int">1</owl:cardinality>
    <rdf:type rdf:resource="http://www.w3.org/2002/07/owl#Restriction"/>
  </rdf:Description>
  <rdf:Description rdf:about="http://foodie-cloud.com/model/foodie#originType">
    <rdfs:isDefinedBy rdf:resource="http://foodie-cloud.com/model/foodie"/>
    <rdfs:comment>A relation to the origin of a Plot when taking into consideration only two options: manual (created by human/user) and system (produced by the platform</rdfs:comment>
    <rdfs:label xml:lang="en">containsZone</rdfs:label>
    <skos:prefLabel xml:lang="en">originType</skos:prefLabel>
    <rdfs:range rdf:resource="http://foodie-cloud.com/model/foodie#OriginTypeValue"/>
    <rdf:type rdf:resource="http://www.w3.org/2002/07/owl#ObjectProperty"/>
  </rdf:Description>
  <rdf:Description rdf:about="https://smartdatamodels.org/dataModel.Agrifood/AgriGreenhouse">
    <rdfs:isDefinedBy rdf:resource="https://github.com/smart-data-models/dataModel.Agrifood/blob/master/AgriGreenhouse/schema.json"/>
    <rdfs:comment>This entity contains a harmonised description of the conditions recorded within a generic greenhouse, a type of AgriParcel. This entity is primarily associated with the agricultural vertical and related IoT applications.</rdfs:comment>
    <rdfs:label>Agri Greenhouse</rdfs:label>
    <rdfs:subClassOf rdf:resource="https://smartdatamodels.org/AgriParcel"/>
    <rdf:type rdf:resource="http://www.w3.org/2002/07/owl#Class"/>
  </rdf:Description>
  <rdf:Description rdf:about="https://smartdatamodels.org/dataModel.Agrifood/lastPlantedAt">
    <rdfs:isDefinedBy rdf:resource="https://github.com/smart-data-models/dataModel.Agrifood/blob/master/AgriParcel/schema.json"/>
    <rdfs:comment>Indicates the date when the crop was last planted.</rdfs:comment>
    <rdfs:label xml:lang="en">lastPlantedAt</rdfs:label>
    <rdfs:range rdf:resource="http://www.w3.org/2001/XMLSchema#dateTime"/>
    <rdf:type rdf:resource="http://www.w3.org/2002/07/owl#DatatypeProperty"/>
  </rdf:Description>
  <rdf:Description rdf:nodeID="A30">
    <owl:onProperty rdf:resource="http://foodie-cloud.com/model/foodie#code"/>
    <owl:cardinality rdf:datatype="http://www.w3.org/2001/XMLSchema#int">1</owl:cardinality>
    <rdf:type rdf:resource="http://www.w3.org/2002/07/owl#Restriction"/>
  </rdf:Description>
  <rdf:Description rdf:about="http://foodie-cloud.com/model/foodie#tractor">
    <rdfs:isDefinedBy rdf:resource="http://foodie-cloud.com/model/foodie"/>
    <rdfs:comment>A relation from Intervention to TractorType</rdfs:comment>
    <rdfs:label xml:lang="en">tractor</rdfs:label>
    <skos:prefLabel xml:lang="en">tractor</skos:prefLabel>
    <rdfs:range rdf:resource="http://foodie-cloud.com/model/foodie#TractorType"/>
    <rdf:type rdf:resource="http://www.w3.org/2002/07/owl#ObjectProperty"/>
  </rdf:Description>
  <rdf:Description rdf:about="http://foodie-cloud.com/model/foodie#machine">
    <rdfs:isDefinedBy rdf:resource="http://foodie-cloud.com/model/foodie"/>
    <rdfs:comment>A relation from Intervention to MachineType</rdfs:comment>
    <rdfs:label xml:lang="en">machine</rdfs:label>
    <skos:prefLabel xml:lang="en">machine</skos:prefLabel>
    <rdfs:range rdf:resource="http://foodie-cloud.com/model/foodie#MachineType"/>
    <rdf:type rdf:resource="http://www.w3.org/2002/07/owl#ObjectProperty"/>
  </rdf:Description>
  <rdf:Description rdf:nodeID="A28">
    <owl:onProperty rdf:resource="http://www.w3.org/ns/prov#invalidatedAtTime"/>
    <owl:maxCardinality rdf:datatype="http://www.w3.org/2001/XMLSchema#int">1</owl:maxCardinality>
    <rdf:type rdf:resource="http://www.w3.org/2002/07/owl#Restriction"/>
  </rdf:Description>
  <rdf:Description rdf:nodeID="A24">
    <owl:onProperty rdf:resource="http://www.w3.org/ns/prov#generatedAtTime"/>
    <owl:cardinality rdf:datatype="http://www.w3.org/2001/XMLSchema#int">1</owl:cardinality>
    <rdf:type rdf:resource="http://www.w3.org/2002/07/owl#Restriction"/>
  </rdf:Description>
  <rdf:Description rdf:about="https://smartdatamodels.org/dataModel.Agrifood/hasAgriCrop">
    <rdfs:isDefinedBy rdf:resource="https://github.com/smart-data-models/dataModel.Agrifood/blob/master/AgriParcel/schema.json"/>
    <rdfs:comment>Reference to the crop associated with this parcel</rdfs:comment>
    <rdfs:label xml:lang="en">hasAgriCrop</rdfs:label>
    <rdf:type rdf:resource="http://www.w3.org/2002/07/owl#ObjectProperty"/>
  </rdf:Description>
  <rdf:Description rdf:nodeID="A27">
    <owl:onProperty rdf:resource="http://foodie-cloud.com/model/foodie#description"/>
    <owl:maxCardinality rdf:datatype="http://www.w3.org/2001/XMLSchema#int">1</owl:maxCardinality>
    <rdf:type rdf:resource="http://www.w3.org/2002/07/owl#Restriction"/>
  </rdf:Description>
  <rdf:Description rdf:nodeID="A36">
    <foaf:name>PSNC</foaf:name>
  </rdf:Description>
  <rdf:Description rdf:nodeID="A20">
    <foaf:name>Ioanna Roussaki</foaf:name>
    <schema:affiliation rdf:nodeID="A37"/>
  </rdf:Description>
  <rdf:Description rdf:nodeID="A29">
    <owl:onProperty rdf:resource="http://www.w3.org/ns/prov#generatedAtTime"/>
    <owl:maxCardinality rdf:datatype="http://www.w3.org/2001/XMLSchema#int">1</owl:maxCardinality>
    <rdf:type rdf:resource="http://www.w3.org/2002/07/owl#Restriction"/>
  </rdf:Description>
  <rdf:Description rdf:about="https://saref.etsi.org/saref4agri/Parcel">
    <owl:equivalentClass rdf:resource="https://smartdatamodels.org/dataModel.Agrifood/AgriParcel"/>
    <owl:equivalentClass rdf:resource="http://foodie-cloud.com/model/foodie#Plot"/>
    <rdfs:isDefinedBy rdf:resource="https://saref.etsi.org/saref4agri/"/>
    <rdfs:label>Parcel</rdfs:label>
    <rdfs:comment xml:lang="en">An area of land, which might be used for grazing animals or planting crops. The parcel is defined as an undividable logical area of land which contains homogeneous items.</rdfs:comment>
    <rdfs:subClassOf rdf:nodeID="A31"/>
    <rdfs:subClassOf rdf:nodeID="A18"/>
    <rdfs:subClassOf rdf:resource="http://www.opengis.net/ont/geosparql#Feature"/>
    <rdf:type rdf:resource="http://www.w3.org/2002/07/owl#Class"/>
  </rdf:Description>
  <rdf:Description rdf:nodeID="A33">
    <owl:onProperty rdf:resource="http://www.opengis.net/ont/geosparql#hasGeometry"/>
    <owl:cardinality rdf:datatype="http://www.w3.org/2001/XMLSchema#int">1</owl:cardinality>
    <rdf:type rdf:resource="http://www.w3.org/2002/07/owl#Restriction"/>
  </rdf:Description>
  <rdf:Description rdf:about="http://foodie-cloud.com/model/foodie#containsPlot">
    <rdfs:subPropertyOf rdf:resource="https://saref.etsi.org/saref4agri/contains"/>
    <rdfs:isDefinedBy rdf:resource="http://foodie-cloud.com/model/foodie"/>
    <rdfs:comment>A relation from Site to Plot </rdfs:comment>
    <rdfs:label xml:lang="en">containsPlot</rdfs:label>
    <skos:prefLabel xml:lang="en">containsPlot</skos:prefLabel>
    <rdfs:range rdf:resource="http://foodie-cloud.com/model/foodie#Plot"/>
    <rdf:type rdf:resource="http://www.w3.org/2002/07/owl#ObjectProperty"/>
  </rdf:Description>
  <rdf:Description rdf:nodeID="A25">
    <owl:onProperty rdf:resource="http://portele.de/ont/inspire/baseInspire#validTo"/>
    <owl:maxCardinality rdf:datatype="http://www.w3.org/2001/XMLSchema#int">1</owl:maxCardinality>
    <rdf:type rdf:resource="http://www.w3.org/2002/07/owl#Restriction"/>
  </rdf:Description>
  <rdf:Description rdf:about="http://inspire.ec.europa.eu/schemas/af/3.0#activity">
    <rdfs:isDefinedBy rdf:resource="http://inspire.ec.europa.eu/schemas/af/3.0#"/>
    <rdfs:comment>A relation to the classification of the economic activity of the site</rdfs:comment>
    <rdfs:label xml:lang="en">activity</rdfs:label>
    <skos:prefLabel xml:lang="en">activity</skos:prefLabel>
    <rdfs:range rdf:resource="http://inspire.ec.europa.eu/schemas/act-core/3.0#EconomicActivityNACEValue"/>
    <rdf:type rdf:resource="http://www.w3.org/2002/07/owl#ObjectProperty"/>
  </rdf:Description>
  <rdf:Description rdf:nodeID="A37">
    <foaf:name>ICCS</foaf:name>
  </rdf:Description>
  <rdf:Description rdf:nodeID="A32">
    <owl:onProperty rdf:resource="http://www.w3.org/ns/prov#generatedAtTime"/>
    <owl:maxCardinality rdf:datatype="http://www.w3.org/2001/XMLSchema#int">1</owl:maxCardinality>
    <rdf:type rdf:resource="http://www.w3.org/2002/07/owl#Restriction"/>
  </rdf:Description>
  <rdf:Description rdf:about="https://uri.etsi.org/ngsi-ld/location">
    <rdfs:subPropertyOf rdf:resource="http://www.opengis.net/ont/geosparql#hasGeometry"/>
    <rdfs:isDefinedBy rdf:resource="https://uri.etsi.org/ngsi-ld/v1/ngsi-ld-core-context-v1.6.jsonld"/>
    <rdfs:comment>The geo:json encoded polygon / multi-polygon describing this item.  It can be Point, LineString, Polygon, MultiPoint, MultiLineString or MultiPolygon</rdfs:comment>
    <rdfs:label xml:lang="en">location</rdfs:label>
    <rdf:type rdf:resource="http://www.w3.org/2002/07/owl#ObjectProperty"/>
  </rdf:Description>
  <rdf:Description rdf:nodeID="A19">
    <foaf:name>Raul Palma</foaf:name>
    <rdfs:seeAlso rdf:resource="http://orcid.org/0000-0003-4289-4922"/>
    <schema:affiliation rdf:nodeID="A36"/>
  </rdf:Description>
</rdf:RDF>
