<rdf:RDF
    xmlns:af-inspire="http://inspire.ec.europa.eu/schemas/af/3.0#"
    xmlns:saref="https://saref.etsi.org/core/"
    xmlns:common="http://portele.de/ont/inspire/baseInspire#"
    xmlns:dct="http://purl.org/dc/terms/"
    xmlns:obo="http://purl.obolibrary.org/obo/"
    xmlns:saref4agri="https://saref.etsi.org/saref4agri/"
    xmlns:prov="http://www.w3.org/ns/prov#"
    xmlns:sosa="http://www.w3.org/ns/sosa/"
    xmlns:iso19103="http://def.seegrid.csiro.au/isotc211/iso19103/2005/basic#"
    xmlns:skos="http://www.w3.org/2004/02/skos/core#"
    xmlns:foodie="http://foodie-cloud.com/model/foodie#"
    xmlns:xsd="http://www.w3.org/2001/XMLSchema#"
    xmlns:rdf="http://www.w3.org/1999/02/22-rdf-syntax-ns#"
    xmlns:iso19115-citation="http://def.seegrid.csiro.au/isotc211/iso19115/2003/citation#"
    xmlns:schema="https://schema.org/"
    xmlns:fiware="https://smartdatamodels.org/"
    xmlns:iso19109="http://def.seegrid.csiro.au/isotc211/iso19109/2005/feature#"
    xmlns:iso19150-2="http://def.seegrid.csiro.au/isotc211/iso19150/-2/2012/basic#"
    xmlns:stat="http://data.europa.eu/m8g/"
    xmlns:rdfs="http://www.w3.org/2000/01/rdf-schema#"
    xmlns:owl="http://www.w3.org/2002/07/owl#"
    xmlns:qb="http://purl.org/linked-data/cube#"
    xmlns:iso19108="http://def.seegrid.csiro.au/isotc211/iso19108/2002/temporal#"
    xmlns:geo="http://www.opengis.net/ont/geosparql#"
    xmlns:dcat="http://www.w3.org/ns/dcat#"
    xmlns="https://w3id.org/cybele/"
    xmlns:act-inspire="http://inspire.ec.europa.eu/schemas/act-core/3.0#"
    xmlns:ssn="http://www.w3.org/ns/ssn/"
    xmlns:foaf="http://xmlns.com/foaf/0.1/"
    xmlns:fiware-agrifood="https://smartdatamodels.org/dataModel.Agrifood/" > 
  <rdf:Description rdf:nodeID="A0">
    <owl:onProperty rdf:resource="http://foodie-cloud.com/model/foodie#price"/>
    <owl:maxCardinality rdf:datatype="http://www.w3.org/2001/XMLSchema#int">1</owl:maxCardinality>
    <rdf:type rdf:resource="http://www.w3.org/2002/07/owl#Restriction"/>
  </rdf:Description>
  <rdf:Description rdf:nodeID="A1">
    <owl:onProperty rdf:resource="http://foodie-cloud.com/model/foodie#productType"/>
    <owl:cardinality rdf:datatype="http://www.w3.org/2001/XMLSchema#int">1</owl:cardinality>
    <rdf:type rdf:resource="http://www.w3.org/2002/07/owl#Restriction"/>
  </rdf:Description>
  <rdf:Description rdf:about="https://smartdatamodels.org/dataModel.Agrifood/hasAgriProductType">
    <rdfs:isDefinedBy rdf:resource="https://github.com/smart-data-models/dataModel.Agrifood/blob/master/AgriParcelOperation/schema.json"/>
    <rdfs:comment>Reference to the AgriProductType used/ applied.</rdfs:comment>
    <rdfs:label xml:lang="en">hasAgriProductType</rdfs:label>
    <rdf:type rdf:resource="http://www.w3.org/2002/07/owl#ObjectProperty"/>
  </rdf:Description>
  <rdf:Description rdf:about="http://foodie-cloud.com/model/foodie#productQuantity">
    <rdfs:isDefinedBy rdf:resource="http://foodie-cloud.com/model/foodie"/>
    <rdfs:comment>Reference to denote the measured quantity of an ingredient in the product prepartion entity</rdfs:comment>
    <rdfs:label>productQuantity</rdfs:label>
    <skos:prefLabel xml:lang="en">productQuantity</skos:prefLabel>
    <rdfs:range rdf:resource="http://def.seegrid.csiro.au/isotc211/iso19103/2005/basic#Measure"/>
    <rdf:type rdf:resource="http://www.w3.org/2002/07/owl#ObjectProperty"/>
  </rdf:Description>
  <rdf:Description rdf:about="http://foodie-cloud.com/model/foodie#Product">
    <skos:prefLabel xml:lang="en">Product</skos:prefLabel>
    <rdfs:subClassOf rdf:nodeID="A2"/>
    <rdfs:subClassOf rdf:nodeID="A3"/>
    <owl:equivalentClass rdf:resource="https://smartdatamodels.org/dataModel.Agrifood/AgriProductType"/>
    <rdfs:isDefinedBy rdf:resource="http://foodie-cloud.com/model/foodie"/>
    <rdfs:subClassOf rdf:nodeID="A4"/>
    <rdfs:subClassOf rdf:nodeID="A5"/>
    <rdf:type rdf:resource="http://www.w3.org/2002/07/owl#Class"/>
    <rdfs:label>Product</rdfs:label>
    <rdfs:subClassOf rdf:nodeID="A6"/>
    <rdfs:subClassOf rdf:nodeID="A0"/>
    <rdfs:subClassOf rdf:nodeID="A7"/>
    <rdfs:comment>This entity defines a product</rdfs:comment>
    <rdfs:subClassOf rdf:resource="http://www.opengis.net/ont/geosparql#Feature"/>
    <rdfs:subClassOf rdf:nodeID="A1"/>
  </rdf:Description>
  <rdf:Description rdf:nodeID="A7">
    <owl:onProperty rdf:resource="http://foodie-cloud.com/model/foodie#storageHandling"/>
    <owl:maxCardinality rdf:datatype="http://www.w3.org/2001/XMLSchema#int">1</owl:maxCardinality>
    <rdf:type rdf:resource="http://www.w3.org/2002/07/owl#Restriction"/>
  </rdf:Description>
  <rdf:Description rdf:nodeID="A8">
    <owl:onProperty rdf:resource="http://foodie-cloud.com/model/foodie#code"/>
    <owl:maxCardinality rdf:datatype="http://www.w3.org/2001/XMLSchema#int">1</owl:maxCardinality>
    <rdf:type rdf:resource="http://www.w3.org/2002/07/owl#Restriction"/>
  </rdf:Description>
  <rdf:Description rdf:about="http://foodie-cloud.com/model/foodie#safetyInstructions">
    <rdfs:isDefinedBy rdf:resource="http://foodie-cloud.com/model/foodie"/>
    <rdfs:comment>The property defines the information on safe manipulation of the Product</rdfs:comment>
    <rdfs:label>safetyInstructions</rdfs:label>
    <skos:prefLabel xml:lang="en">safetyInstructions</skos:prefLabel>
    <rdfs:range rdf:resource="http://www.w3.org/2001/XMLSchema#string"/>
    <rdf:type rdf:resource="http://www.w3.org/2002/07/owl#DatatypeProperty"/>
  </rdf:Description>
  <rdf:Description rdf:nodeID="A6">
    <owl:onProperty rdf:resource="http://foodie-cloud.com/model/foodie#safetyInstructions"/>
    <owl:maxCardinality rdf:datatype="http://www.w3.org/2001/XMLSchema#int">1</owl:maxCardinality>
    <rdf:type rdf:resource="http://www.w3.org/2002/07/owl#Restriction"/>
  </rdf:Description>
  <rdf:Description rdf:about="http://foodie-cloud.com/model/foodie#ingredientName">
    <rdfs:subPropertyOf rdf:resource="https://smartdatamodels.org/name"/>
    <rdfs:isDefinedBy rdf:resource="http://foodie-cloud.com/model/foodie"/>
    <rdfs:comment>Designation under which the Ingredient is commonly known</rdfs:comment>
    <rdfs:label>ingredientName</rdfs:label>
    <skos:prefLabel xml:lang="en">ingredientName</skos:prefLabel>
    <rdfs:range rdf:resource="http://www.w3.org/2001/XMLSchema#string"/>
    <rdf:type rdf:resource="http://www.w3.org/2002/07/owl#DatatypeProperty"/>
  </rdf:Description>
  <rdf:Description rdf:about="http://foodie-cloud.com/model/foodie#nutrient">
    <rdfs:isDefinedBy rdf:resource="http://foodie-cloud.com/model/foodie"/>
    <rdfs:comment>Reference to the Product Nutrients entity related to a product entity</rdfs:comment>
    <rdfs:label>nutrient</rdfs:label>
    <skos:prefLabel xml:lang="en">nutrient</skos:prefLabel>
    <rdfs:range rdf:resource="http://foodie-cloud.com/model/foodie#ProductNutrients"/>
    <rdf:type rdf:resource="http://www.w3.org/2002/07/owl#ObjectProperty"/>
  </rdf:Description>
  <rdf:Description rdf:about="http://foodie-cloud.com/model/foodie#productKind">
    <rdfs:isDefinedBy rdf:resource="http://foodie-cloud.com/model/foodie"/>
    <rdfs:comment>Reference to the product kind value entity related to a product entity</rdfs:comment>
    <rdfs:label>productKind</rdfs:label>
    <skos:prefLabel xml:lang="en">productKind</skos:prefLabel>
    <rdfs:range rdf:resource="http://foodie-cloud.com/model/foodie#ProductKindValue"/>
    <rdf:type rdf:resource="http://www.w3.org/2002/07/owl#ObjectProperty"/>
  </rdf:Description>
  <rdf:Description rdf:nodeID="A9">
    <owl:onProperty rdf:resource="http://foodie-cloud.com/model/foodie#ingredientName"/>
    <owl:cardinality rdf:datatype="http://www.w3.org/2001/XMLSchema#int">1</owl:cardinality>
    <rdf:type rdf:resource="http://www.w3.org/2002/07/owl#Restriction"/>
  </rdf:Description>
  <rdf:Description rdf:nodeID="A4">
    <owl:onProperty rdf:resource="http://foodie-cloud.com/model/foodie#productName"/>
    <owl:minCardinality rdf:datatype="http://www.w3.org/2001/XMLSchema#int">1</owl:minCardinality>
    <rdf:type rdf:resource="http://www.w3.org/2002/07/owl#Restriction"/>
  </rdf:Description>
  <rdf:Description rdf:about="http://foodie-cloud.com/model/foodie#solventQuantity">
    <rdfs:isDefinedBy rdf:resource="http://foodie-cloud.com/model/foodie"/>
    <rdfs:comment>Reference to denote the quantity of measure (e.g. solvent) in the product prepartion entity</rdfs:comment>
    <rdfs:label>solventQuantity</rdfs:label>
    <skos:prefLabel xml:lang="en">solventQuantity</skos:prefLabel>
    <rdfs:range rdf:resource="http://def.seegrid.csiro.au/isotc211/iso19103/2005/basic#Measure"/>
    <rdf:type rdf:resource="http://www.w3.org/2002/07/owl#ObjectProperty"/>
  </rdf:Description>
  <rdf:Description rdf:about="http://foodie-cloud.com/model/foodie#nutrientName">
    <rdfs:subPropertyOf rdf:resource="https://smartdatamodels.org/name"/>
    <rdfs:isDefinedBy rdf:resource="http://foodie-cloud.com/model/foodie"/>
    <rdfs:comment>Designation under which the nutrient is commonly known</rdfs:comment>
    <rdfs:label>ingredientName</rdfs:label>
    <skos:prefLabel xml:lang="en">nutrientName</skos:prefLabel>
    <rdfs:range rdf:resource="http://www.w3.org/2001/XMLSchema#string"/>
    <rdf:type rdf:resource="http://www.w3.org/2002/07/owl#DatatypeProperty"/>
  </rdf:Description>
  <rdf:Description rdf:about="http://foodie-cloud.com/model/foodie#ingredientAmount">
    <rdfs:isDefinedBy rdf:resource="http://foodie-cloud.com/model/foodie"/>
    <rdfs:comment>Reference to product nutrients entity to denote the measured amount of an specific ingredient</rdfs:comment>
    <rdfs:label>ingredientAmount</rdfs:label>
    <skos:prefLabel xml:lang="en">ingredientAmount</skos:prefLabel>
    <rdfs:range rdf:resource="http://def.seegrid.csiro.au/isotc211/iso19103/2005/basic#Measure"/>
    <rdf:type rdf:resource="http://www.w3.org/2002/07/owl#ObjectProperty"/>
  </rdf:Description>
  <rdf:Description rdf:about="http://foodie-cloud.com/model/foodie#manufacturer">
    <rdfs:isDefinedBy rdf:resource="http://foodie-cloud.com/model/foodie"/>
    <rdfs:comment>Reference to the responsible party entity related to a product entity defining the manufacturer relationship</rdfs:comment>
    <rdfs:label>manufacturer</rdfs:label>
    <skos:prefLabel xml:lang="en">manufacturer</skos:prefLabel>
    <rdfs:range rdf:resource="http://def.seegrid.csiro.au/isotc211/iso19115/2003/citation#ResponsibleParty"/>
    <rdf:type rdf:resource="http://www.w3.org/2002/07/owl#ObjectProperty"/>
  </rdf:Description>
  <rdf:Description rdf:nodeID="A2">
    <owl:onProperty rdf:resource="http://foodie-cloud.com/model/foodie#productKind"/>
    <owl:cardinality rdf:datatype="http://www.w3.org/2001/XMLSchema#int">1</owl:cardinality>
    <rdf:type rdf:resource="http://www.w3.org/2002/07/owl#Restriction"/>
  </rdf:Description>
  <rdf:Description rdf:nodeID="A10">
    <foaf:name>PSNC</foaf:name>
  </rdf:Description>
  <rdf:Description rdf:about="http://foodie-cloud.com/model/foodie#registerUrl">
    <rdfs:isDefinedBy rdf:resource="http://foodie-cloud.com/model/foodie"/>
    <rdfs:comment>Link to the national or any other relevant register where the Product was registered</rdfs:comment>
    <rdfs:label>registerUrl</rdfs:label>
    <skos:prefLabel xml:lang="en">registerUrl</skos:prefLabel>
    <rdfs:range rdf:resource="http://www.w3.org/2001/XMLSchema#anyURI"/>
    <rdf:type rdf:resource="http://www.w3.org/2002/07/owl#DatatypeProperty"/>
  </rdf:Description>
  <rdf:Description rdf:nodeID="A11">
    <owl:onProperty rdf:resource="http://foodie-cloud.com/model/foodie#solventQuantity"/>
    <owl:maxCardinality rdf:datatype="http://www.w3.org/2001/XMLSchema#int">1</owl:maxCardinality>
    <rdf:type rdf:resource="http://www.w3.org/2002/07/owl#Restriction"/>
  </rdf:Description>
  <rdf:Description rdf:about="http://foodie-cloud.com/model/foodie#ActiveIngredients">
    <rdfs:isDefinedBy rdf:resource="http://foodie-cloud.com/model/foodie"/>
    <rdfs:comment>This entity holds the information of the active ingredients (e.g. incredient name, ingredient code, ingredient amount) for a product</rdfs:comment>
    <rdfs:label>ActiveIngredients</rdfs:label>
    <skos:prefLabel xml:lang="en">ActiveIngredients</skos:prefLabel>
    <rdfs:subClassOf rdf:nodeID="A8"/>
    <rdfs:subClassOf rdf:nodeID="A12"/>
    <rdfs:subClassOf rdf:nodeID="A9"/>
    <rdf:type rdf:resource="http://www.w3.org/2002/07/owl#Class"/>
  </rdf:Description>
  <rdf:Description rdf:about="http://purl.obolibrary.org/obo/RO_0002180">
    <rdfs:isDefinedBy rdf:resource="http://purl.obolibrary.org/obo/"/>
    <rdfs:comment>w 'has component' p if w 'has part' p and w is such that it can be directly disassembled into into n parts p, p2, p3, ..., pn, where these parts are of similar type.</rdfs:comment>
    <rdfs:label>hasComponent</rdfs:label>
    <rdf:type rdf:resource="http://www.w3.org/2002/07/owl#ObjectProperty"/>
  </rdf:Description>
  <rdf:Description rdf:about="http://purl.obolibrary.org/obo/HANCESTRO_0308">
    <rdfs:isDefinedBy rdf:resource="http://purl.obolibrary.org/obo/"/>
    <rdfs:comment>has country of origin</rdfs:comment>
    <rdfs:label>hasCountryOfOrigin</rdfs:label>
    <rdf:type rdf:resource="http://www.w3.org/2002/07/owl#ObjectProperty"/>
  </rdf:Description>
  <rdf:Description rdf:about="http://foodie-cloud.com/model/foodie#nutrientProduct">
    <rdfs:isDefinedBy rdf:resource="http://foodie-cloud.com/model/foodie"/>
    <rdfs:comment>Reference to the Product entity from  product nutrients entity</rdfs:comment>
    <rdfs:label>nutrientProduct</rdfs:label>
    <skos:prefLabel xml:lang="en">nutrientProduct</skos:prefLabel>
    <rdfs:range rdf:resource="http://foodie-cloud.com/model/foodie#Product"/>
    <rdf:type rdf:resource="http://www.w3.org/2002/07/owl#ObjectProperty"/>
  </rdf:Description>
  <rdf:Description rdf:about="http://foodie-cloud.com/model/foodie#storageHandling">
    <rdfs:isDefinedBy rdf:resource="http://foodie-cloud.com/model/foodie"/>
    <rdfs:comment>The property defines the information on the safe storage of the Product</rdfs:comment>
    <rdfs:label>storageHandling</rdfs:label>
    <skos:prefLabel xml:lang="en">storageHandling</skos:prefLabel>
    <rdfs:range rdf:resource="http://www.w3.org/2001/XMLSchema#string"/>
    <rdf:type rdf:resource="http://www.w3.org/2002/07/owl#DatatypeProperty"/>
  </rdf:Description>
  <rdf:Description rdf:about="http://foodie-cloud.com/model/foodie#nutrientMeasure">
    <rdfs:isDefinedBy rdf:resource="http://foodie-cloud.com/model/foodie"/>
    <rdfs:comment>Textual description of a method for an estimation of the nutrient amount in the Product</rdfs:comment>
    <rdfs:label>nutrientMeasure</rdfs:label>
    <skos:prefLabel xml:lang="en">nutrientMeasure</skos:prefLabel>
    <rdfs:range rdf:resource="http://www.w3.org/2001/XMLSchema#string"/>
    <rdf:type rdf:resource="http://www.w3.org/2002/07/owl#DatatypeProperty"/>
  </rdf:Description>
  <rdf:Description rdf:nodeID="A13">
    <owl:onProperty rdf:resource="http://foodie-cloud.com/model/foodie#nutrientMeasure"/>
    <owl:maxCardinality rdf:datatype="http://www.w3.org/2001/XMLSchema#int">1</owl:maxCardinality>
    <rdf:type rdf:resource="http://www.w3.org/2002/07/owl#Restriction"/>
  </rdf:Description>
  <rdf:Description rdf:about="http://foodie-cloud.com/model/foodie#ProductNutrients">
    <rdfs:subClassOf rdf:nodeID="A13"/>
    <rdfs:label>ProductNutrients</rdfs:label>
    <rdf:type rdf:resource="http://www.w3.org/2002/07/owl#Class"/>
    <rdfs:isDefinedBy rdf:resource="http://foodie-cloud.com/model/foodie"/>
    <rdfs:comment>This entity holds the information of the nutrients (e.g. nutrient name, nutrient measure, nutrient amount) used for a product</rdfs:comment>
    <rdfs:subClassOf rdf:nodeID="A14"/>
    <skos:prefLabel xml:lang="en">ProductNutrients</skos:prefLabel>
    <rdfs:subClassOf rdf:resource="http://www.opengis.net/ont/geosparql#Feature"/>
    <rdfs:subClassOf rdf:nodeID="A15"/>
    <rdfs:subClassOf rdf:nodeID="A16"/>
  </rdf:Description>
  <rdf:Description rdf:nodeID="A15">
    <owl:onProperty rdf:resource="http://foodie-cloud.com/model/foodie#nutrientName"/>
    <owl:cardinality rdf:datatype="http://www.w3.org/2001/XMLSchema#int">1</owl:cardinality>
    <rdf:type rdf:resource="http://www.w3.org/2002/07/owl#Restriction"/>
  </rdf:Description>
  <rdf:Description rdf:nodeID="A17">
    <foaf:name>DEMETER project</foaf:name>
    <foaf:homepage rdf:resource="https://h2020-demeter.eu/"/>
  </rdf:Description>
  <rdf:Description rdf:about="http://foodie-cloud.com/model/foodie#productCode">
    <rdfs:isDefinedBy rdf:resource="http://foodie-cloud.com/model/foodie"/>
    <rdfs:comment>Indentifing code of a product. Unique identification of the Product.</rdfs:comment>
    <rdfs:label>productCode</rdfs:label>
    <skos:prefLabel xml:lang="en">productCode</skos:prefLabel>
    <rdfs:range rdf:resource="http://www.w3.org/2001/XMLSchema#string"/>
    <rdf:type rdf:resource="http://www.w3.org/2002/07/owl#DatatypeProperty"/>
  </rdf:Description>
  <rdf:Description rdf:nodeID="A18">
    <foaf:name>ICCS</foaf:name>
  </rdf:Description>
  <rdf:Description rdf:nodeID="A19">
    <foaf:name>OGC</foaf:name>
  </rdf:Description>
  <rdf:Description rdf:nodeID="A20">
    <foaf:name>Raul Palma</foaf:name>
    <rdfs:seeAlso rdf:resource="http://orcid.org/0000-0003-4289-4922"/>
    <schema:affiliation rdf:nodeID="A10"/>
  </rdf:Description>
  <rdf:Description rdf:nodeID="A21">
    <owl:onProperty rdf:resource="http://foodie-cloud.com/model/foodie#safetyPeriod"/>
    <owl:cardinality rdf:datatype="http://www.w3.org/2001/XMLSchema#int">1</owl:cardinality>
    <rdf:type rdf:resource="http://www.w3.org/2002/07/owl#Restriction"/>
  </rdf:Description>
  <rdf:Description rdf:about="https://smartdatamodels.org/dataModel.Agrifood/root">
    <rdfs:isDefinedBy rdf:resource="https://github.com/smart-data-models/dataModel.Agrifood/blob/master/AgriProductType/schema.json"/>
    <rdfs:comment>A logical indicator that this product is the root of an AgriProductType hierarchy. Logical true indicates it is the root.</rdfs:comment>
    <rdfs:label xml:lang="en">root</rdfs:label>
    <rdf:type rdf:resource="http://www.w3.org/2002/07/owl#DatatypeProperty"/>
  </rdf:Description>
  <rdf:Description rdf:nodeID="A5">
    <owl:onProperty rdf:resource="http://foodie-cloud.com/model/foodie#description"/>
    <owl:maxCardinality rdf:datatype="http://www.w3.org/2001/XMLSchema#int">1</owl:maxCardinality>
    <rdf:type rdf:resource="http://www.w3.org/2002/07/owl#Restriction"/>
  </rdf:Description>
  <rdf:Description rdf:about="https://smartdatamodels.org/dataModel.Agrifood/hasAgriProductTypeParent">
    <rdfs:subPropertyOf rdf:resource="https://smartdatamodels.org/dataModel.Agrifood/hasAgriProductType"/>
    <rdfs:isDefinedBy rdf:resource="https://github.com/smart-data-models/dataModel.Agrifood/blob/master/AgriProductType/schema.json"/>
    <rdfs:comment>Reference to the parent product type i.e. immediately above the entity in the hierarchy.</rdfs:comment>
    <rdfs:label xml:lang="en">hasAgriProductTypeParent</rdfs:label>
    <rdf:type rdf:resource="http://www.w3.org/2002/07/owl#ObjectProperty"/>
  </rdf:Description>
  <rdf:Description rdf:about="http://foodie-cloud.com/model/foodie#ProductPreparation">
    <rdfs:isDefinedBy rdf:resource="http://foodie-cloud.com/model/foodie"/>
    <rdfs:comment>This entity defines the preparation of a product (e.g. quantities of the ingredients)</rdfs:comment>
    <rdfs:label>ProductPreparation</rdfs:label>
    <skos:prefLabel xml:lang="en">ProductPreparation</skos:prefLabel>
    <rdfs:subClassOf rdf:nodeID="A22"/>
    <rdfs:subClassOf rdf:nodeID="A21"/>
    <rdfs:subClassOf rdf:nodeID="A11"/>
    <rdfs:subClassOf rdf:resource="http://www.opengis.net/ont/geosparql#Feature"/>
    <rdf:type rdf:resource="http://www.w3.org/2002/07/owl#Class"/>
  </rdf:Description>
  <rdf:Description rdf:about="http://foodie-cloud.com/model/foodie#productType">
    <rdfs:isDefinedBy rdf:resource="http://foodie-cloud.com/model/foodie"/>
    <rdfs:comment>Type of the Product, e.g. pesticide, as a free text. The types of Product vary from country to country as well as from farmer to farmer</rdfs:comment>
    <rdfs:label>productType</rdfs:label>
    <skos:prefLabel xml:lang="en">productType</skos:prefLabel>
    <rdfs:range rdf:resource="http://www.w3.org/2001/XMLSchema#string"/>
    <rdf:type rdf:resource="http://www.w3.org/2002/07/owl#DatatypeProperty"/>
  </rdf:Description>
  <rdf:Description rdf:about="https://w3id.org/demeter/agri/agriProduct">
    <dct:rights xml:lang="en">This vocabulary is distributed under Creative Commons Attribution 4.0 License - http://creativecommons.org/licenses/by/4.0</dct:rights>
    <rdfs:label xml:lang="en">DEMETER AgriProduct</rdfs:label>
    <rdfs:comment xml:lang="en">The DEMETER Agriculture Information Model (AIM) is the common vocabulary in DEMETER project providing the basis for semantic interoperability across smart farming solutions</rdfs:comment>
    <owl:versionInfo>2.0</owl:versionInfo>
    <rdf:type rdf:resource="http://www.w3.org/2002/07/owl#Ontology"/>
    <dct:title xml:lang="en">DEMETER AgriProduct</dct:title>
    <foaf:maker rdf:nodeID="A17"/>
    <dct:description xml:lang="en">The DEMETER AgriProduct is one of the agri profiles of DEMETER AIM. This profile was created by reusing and aligning well-known ontologies and vocabularies</dct:description>
    <dct:contributor rdf:nodeID="A23"/>
    <owl:versionIRI rdf:resource="https://w3id.org/demeter/agri/agriProduct/2.0"/>
    <dct:contributor rdf:nodeID="A24"/>
    <dct:creator rdf:nodeID="A20"/>
    <owl:imports rdf:resource="https://w3id.org/demeter/agri/agriCommon"/>
  </rdf:Description>
  <rdf:Description rdf:nodeID="A24">
    <foaf:name>Rob Atkinson</foaf:name>
    <schema:affiliation rdf:nodeID="A19"/>
  </rdf:Description>
  <rdf:Description rdf:about="http://purl.obolibrary.org/obo/RO_0002473">
    <rdfs:isDefinedBy rdf:resource="http://purl.obolibrary.org/obo/"/>
    <rdfs:comment>composed_primarily_of y if and only if more than half of the mass of x is made from y or units of the same type as y</rdfs:comment>
    <rdfs:label>composedPrimarilyOf</rdfs:label>
    <rdf:type rdf:resource="http://www.w3.org/2002/07/owl#ObjectProperty"/>
  </rdf:Description>
  <rdf:Description rdf:nodeID="A23">
    <foaf:name>Ioanna Roussaki</foaf:name>
    <schema:affiliation rdf:nodeID="A18"/>
  </rdf:Description>
  <rdf:Description rdf:nodeID="A12">
    <owl:onProperty rdf:resource="http://foodie-cloud.com/model/foodie#ingredientAmount"/>
    <owl:maxCardinality rdf:datatype="http://www.w3.org/2001/XMLSchema#int">1</owl:maxCardinality>
    <rdf:type rdf:resource="http://www.w3.org/2002/07/owl#Restriction"/>
  </rdf:Description>
  <rdf:Description rdf:about="http://purl.obolibrary.org/obo/FOODON_00001301">
    <rdfs:isDefinedBy rdf:resource="http://purl.obolibrary.org/obo/"/>
    <rdfs:comment>has food substance analog</rdfs:comment>
    <rdfs:label>hasFoodSubstanceAnalog</rdfs:label>
    <rdf:type rdf:resource="http://www.w3.org/2002/07/owl#ObjectProperty"/>
  </rdf:Description>
  <rdf:Description rdf:nodeID="A14">
    <owl:onProperty rdf:resource="http://foodie-cloud.com/model/foodie#nutrientAmount"/>
    <owl:maxCardinality rdf:datatype="http://www.w3.org/2001/XMLSchema#int">1</owl:maxCardinality>
    <rdf:type rdf:resource="http://www.w3.org/2002/07/owl#Restriction"/>
  </rdf:Description>
  <rdf:Description rdf:about="http://foodie-cloud.com/model/foodie#productName">
    <rdfs:subPropertyOf rdf:resource="https://smartdatamodels.org/name"/>
    <rdfs:isDefinedBy rdf:resource="http://foodie-cloud.com/model/foodie"/>
    <rdfs:comment>The property defines the designation under which the Product is commonly known</rdfs:comment>
    <rdfs:label>productName</rdfs:label>
    <skos:prefLabel xml:lang="en">productName</skos:prefLabel>
    <rdfs:range rdf:resource="http://www.w3.org/2001/XMLSchema#string"/>
    <rdf:type rdf:resource="http://www.w3.org/2002/07/owl#DatatypeProperty"/>
  </rdf:Description>
  <rdf:Description rdf:about="http://foodie-cloud.com/model/foodie#registrationCode">
    <rdfs:isDefinedBy rdf:resource="http://foodie-cloud.com/model/foodie"/>
    <rdfs:comment>Indentifing the registration code of a product. Unique identification of a Product according to the national or any other relevant registration scheme.</rdfs:comment>
    <rdfs:label>registrationCode</rdfs:label>
    <skos:prefLabel xml:lang="en">registrationCode</skos:prefLabel>
    <rdfs:range rdf:resource="http://www.w3.org/2001/XMLSchema#string"/>
    <rdf:type rdf:resource="http://www.w3.org/2002/07/owl#DatatypeProperty"/>
  </rdf:Description>
  <rdf:Description rdf:nodeID="A3">
    <owl:onProperty rdf:resource="http://foodie-cloud.com/model/foodie#manufacturer"/>
    <owl:minCardinality rdf:datatype="http://www.w3.org/2001/XMLSchema#int">1</owl:minCardinality>
    <rdf:type rdf:resource="http://www.w3.org/2002/07/owl#Restriction"/>
  </rdf:Description>
  <rdf:Description rdf:about="https://smartdatamodels.org/dataModel.Agrifood/AgriProductType">
    <rdfs:isDefinedBy rdf:resource="https://github.com/smart-data-models/dataModel.Agrifood/blob/master/AgriProductType/schema.json"/>
    <rdfs:comment>This entity contains a harmonised description of a generic agricultural product type. This entity is primarily associated with the agricultural vertical and related IoT applications. The AgriProductType includes a hierarchical structure that allows product types to be grouped in a flexible way.</rdfs:comment>
    <rdfs:label>AgriProductType</rdfs:label>
    <rdf:type rdf:resource="http://www.w3.org/2002/07/owl#Class"/>
  </rdf:Description>
  <rdf:Description rdf:about="http://foodie-cloud.com/model/foodie#ProductKindValue">
    <rdfs:isDefinedBy rdf:resource="http://foodie-cloud.com/model/foodie"/>
    <rdfs:comment>This entity holds the information of the kind/type of product (e.g. oragnic, mineral) as codelist</rdfs:comment>
    <rdfs:label>ProductNutrients</rdfs:label>
    <skos:prefLabel xml:lang="en">ProductKindValue</skos:prefLabel>
    <rdfs:subClassOf rdf:resource="http://www.w3.org/2004/02/skos/core#Concept"/>
    <rdf:type rdf:resource="http://www.w3.org/2002/07/owl#Class"/>
  </rdf:Description>
  <rdf:Description rdf:about="http://foodie-cloud.com/model/foodie#nutrientAmount">
    <rdfs:isDefinedBy rdf:resource="http://foodie-cloud.com/model/foodie"/>
    <rdfs:comment>Reference to product nutrients entity to denote the measured amount of an specific nutrient</rdfs:comment>
    <rdfs:label>nutrientAmount</rdfs:label>
    <skos:prefLabel xml:lang="en">nutrientAmount</skos:prefLabel>
    <rdfs:range rdf:resource="http://def.seegrid.csiro.au/isotc211/iso19103/2005/basic#Measure"/>
    <rdf:type rdf:resource="http://www.w3.org/2002/07/owl#ObjectProperty"/>
  </rdf:Description>
  <rdf:Description rdf:nodeID="A16">
    <owl:onProperty rdf:resource="http://foodie-cloud.com/model/foodie#nutrientProduct"/>
    <owl:cardinality rdf:datatype="http://www.w3.org/2001/XMLSchema#int">1</owl:cardinality>
    <rdf:type rdf:resource="http://www.w3.org/2002/07/owl#Restriction"/>
  </rdf:Description>
  <rdf:Description rdf:nodeID="A22">
    <owl:onProperty rdf:resource="http://foodie-cloud.com/model/foodie#productQuantity"/>
    <owl:cardinality rdf:datatype="http://www.w3.org/2001/XMLSchema#int">1</owl:cardinality>
    <rdf:type rdf:resource="http://www.w3.org/2002/07/owl#Restriction"/>
  </rdf:Description>
  <rdf:Description rdf:about="http://foodie-cloud.com/model/foodie#safetyPeriod">
    <rdfs:isDefinedBy rdf:resource="http://foodie-cloud.com/model/foodie"/>
    <rdfs:comment>Reference to denote the time period for an element in the product prepartion entity</rdfs:comment>
    <rdfs:label>safetyPeriod</rdfs:label>
    <skos:prefLabel xml:lang="en">safetyPeriod</skos:prefLabel>
    <rdfs:range rdf:resource="http://def.seegrid.csiro.au/isotc211/iso19108/2002/temporal#Period"/>
    <rdf:type rdf:resource="http://www.w3.org/2002/07/owl#ObjectProperty"/>
  </rdf:Description>
  <rdf:Description rdf:about="https://smartdatamodels.org/dataModel.Agrifood/hasAgriProductTypeChildren">
    <rdfs:subPropertyOf rdf:resource="https://smartdatamodels.org/dataModel.Agrifood/hasAgriProductType"/>
    <rdfs:isDefinedBy rdf:resource="https://github.com/smart-data-models/dataModel.Agrifood/blob/master/AgriProductType/schema.json"/>
    <rdfs:comment>Reference to child product types i.e. immediately below this entity in the hierarchy.</rdfs:comment>
    <rdfs:label xml:lang="en">hasAgriProductTypeChildren</rdfs:label>
    <rdf:type rdf:resource="http://www.w3.org/2002/07/owl#ObjectProperty"/>
  </rdf:Description>
  <rdf:Description rdf:about="http://foodie-cloud.com/model/foodie#productSubType">
    <rdfs:isDefinedBy rdf:resource="http://foodie-cloud.com/model/foodie"/>
    <rdfs:comment>More detailed classification of a type of the Product, e.g. biochemical insecticide, as a free text. The sub-types of Product vary from country to country as well as from farmer to farmer</rdfs:comment>
    <rdfs:label>productSubType</rdfs:label>
    <skos:prefLabel xml:lang="en">productSubType</skos:prefLabel>
    <rdfs:range rdf:resource="http://www.w3.org/2001/XMLSchema#string"/>
    <rdf:type rdf:resource="http://www.w3.org/2002/07/owl#DatatypeProperty"/>
  </rdf:Description>
</rdf:RDF>
