<rdf:RDF
    xmlns:af-inspire="http://inspire.ec.europa.eu/schemas/af/3.0#"
    xmlns:demeterAgriCrop="https://w3id.org/demeter/agri/agriCrop#"
    xmlns:saref="https://saref.etsi.org/core/"
    xmlns:common="http://portele.de/ont/inspire/baseInspire#"
    xmlns:dct="http://purl.org/dc/terms/"
    xmlns:obo="http://purl.obolibrary.org/obo/"
    xmlns:saref4agri="https://saref.etsi.org/saref4agri/"
    xmlns:prov="http://www.w3.org/ns/prov#"
    xmlns:iso19103="http://def.seegrid.csiro.au/isotc211/iso19103/2005/basic#"
    xmlns:skos="http://www.w3.org/2004/02/skos/core#"
    xmlns:foodie="http://foodie-cloud.com/model/foodie#"
    xmlns:xsd="http://www.w3.org/2001/XMLSchema#"
    xmlns:rdf="http://www.w3.org/1999/02/22-rdf-syntax-ns#"
    xmlns:schema="https://schema.org/"
    xmlns:fiware="https://smartdatamodels.org/"
    xmlns:iso19109="http://def.seegrid.csiro.au/isotc211/iso19109/2005/feature#"
    xmlns:iso19150-2="http://def.seegrid.csiro.au/isotc211/iso19150/-2/2012/basic#"
    xmlns:fiware-weather="https://smartdatamodels.org/dataModel.Weather/"
    xmlns:stat="http://data.europa.eu/m8g/"
    xmlns:rdfs="http://www.w3.org/2000/01/rdf-schema#"
    xmlns:ngsi-ld="https://uri.etsi.org/ngsi-ld/"
    xmlns:owl="http://www.w3.org/2002/07/owl#"
    xmlns:qb="http://purl.org/linked-data/cube#"
    xmlns:geo="http://www.opengis.net/ont/geosparql#"
    xmlns:dcat="http://www.w3.org/ns/dcat#"
    xmlns="https://w3id.org/cybele/"
    xmlns:act-inspire="http://inspire.ec.europa.eu/schemas/act-core/3.0#"
    xmlns:ssn="http://www.w3.org/ns/ssn/"
    xmlns:foaf="http://xmlns.com/foaf/0.1/"
    xmlns:fiware-agrifood="https://smartdatamodels.org/dataModel.Agrifood/" > 
  <rdf:Description rdf:about="https://smartdatamodels.org/dataModel.Agrifood/plantingFrom">
    <rdfs:isDefinedBy rdf:resource="https://github.com/smart-data-models/dataModel.Agrifood/blob/master/AgriCrop/schema.json"/>
    <rdfs:comment>A list of the recommended planting interval date(s) for this crop. Specified using ISO8601 repeating date intervals:
interval, description
Where interval is in the form of start date/end date
--MM-DD/--MM-DD
Meaning repeat each year from this start date to this end date.</rdfs:comment>
    <rdfs:label xml:lang="en">plantingFrom</rdfs:label>
    <rdf:type rdf:resource="http://www.w3.org/2002/07/owl#DatatypeProperty"/>
  </rdf:Description>
  <rdf:Description rdf:nodeID="A0">
    <owl:onProperty rdf:resource="http://foodie-cloud.com/model/foodie#code"/>
    <owl:maxCardinality rdf:datatype="http://www.w3.org/2001/XMLSchema#int">1</owl:maxCardinality>
    <rdf:type rdf:resource="http://www.w3.org/2002/07/owl#Restriction"/>
  </rdf:Description>
  <rdf:Description rdf:nodeID="A1">
    <owl:someValuesFrom rdf:resource="http://www.w3.org/2001/XMLSchema#dateTime"/>
    <owl:onProperty rdf:resource="https://saref.etsi.org/saref4agri/hasPlantDate"/>
    <rdf:type rdf:resource="http://www.w3.org/2002/07/owl#Restriction"/>
  </rdf:Description>
  <rdf:Description rdf:nodeID="A2">
    <owl:onProperty rdf:resource="http://foodie-cloud.com/model/foodie#genus"/>
    <owl:maxCardinality rdf:datatype="http://www.w3.org/2001/XMLSchema#int">1</owl:maxCardinality>
    <rdf:type rdf:resource="http://www.w3.org/2002/07/owl#Restriction"/>
  </rdf:Description>
  <rdf:Description rdf:nodeID="A3">
    <foaf:name>Rob Atkinson</foaf:name>
    <schema:affiliation rdf:nodeID="A4"/>
  </rdf:Description>
  <rdf:Description rdf:about="http://foodie-cloud.com/model/foodie#productionAmount">
    <rdfs:isDefinedBy rdf:resource="http://foodie-cloud.com/model/foodie"/>
    <rdfs:label>productionAmount</rdfs:label>
    <rdfs:comment>The value of a physical quantity of produced variety, together with its unit</rdfs:comment>
    <skos:prefLabel xml:lang="en">productionAmount</skos:prefLabel>
    <rdfs:range rdf:resource="http://def.seegrid.csiro.au/isotc211/iso19103/2005/basic#Measure"/>
    <rdf:type rdf:resource="http://www.w3.org/2002/07/owl#ObjectProperty"/>
  </rdf:Description>
  <rdf:Description rdf:nodeID="A5">
    <owl:onProperty rdf:resource="http://foodie-cloud.com/model/foodie#variety"/>
    <owl:cardinality rdf:datatype="http://www.w3.org/2001/XMLSchema#int">1</owl:cardinality>
    <rdf:type rdf:resource="http://www.w3.org/2002/07/owl#Restriction"/>
  </rdf:Description>
  <rdf:Description rdf:nodeID="A6">
    <owl:onProperty rdf:resource="http://foodie-cloud.com/model/foodie#cropArea"/>
    <owl:minCardinality rdf:datatype="http://www.w3.org/2001/XMLSchema#int">1</owl:minCardinality>
    <rdf:type rdf:resource="http://www.w3.org/2002/07/owl#Restriction"/>
  </rdf:Description>
  <rdf:Description rdf:nodeID="A7">
    <owl:onProperty rdf:resource="http://foodie-cloud.com/model/foodie#variety"/>
    <owl:maxCardinality rdf:datatype="http://www.w3.org/2001/XMLSchema#int">1</owl:maxCardinality>
    <rdf:type rdf:resource="http://www.w3.org/2002/07/owl#Restriction"/>
  </rdf:Description>
  <rdf:Description rdf:nodeID="A8">
    <owl:someValuesFrom rdf:resource="http://www.w3.org/2001/XMLSchema#dateTime"/>
    <owl:onProperty rdf:resource="https://saref.etsi.org/saref4agri/hasHarvestDate"/>
    <rdf:type rdf:resource="http://www.w3.org/2002/07/owl#Restriction"/>
  </rdf:Description>
  <rdf:Description rdf:about="http://foodie-cloud.com/model/foodie#CropSpecies">
    <rdfs:isDefinedBy rdf:resource="http://foodie-cloud.com/model/foodie"/>
    <rdfs:comment xml:lang="en">An entity for the species of the Crops grown in a plot. The planted crop species</rdfs:comment>
    <rdfs:subClassOf rdf:nodeID="A9"/>
    <skos:prefLabel xml:lang="en">CropSpecies</skos:prefLabel>
    <rdfs:subClassOf rdf:nodeID="A10"/>
    <rdfs:subClassOf rdf:nodeID="A6"/>
    <rdfs:subClassOf rdf:resource="http://www.opengis.net/ont/geosparql#Feature"/>
    <rdfs:subClassOf rdf:nodeID="A11"/>
    <rdf:type rdf:resource="http://www.w3.org/2002/07/owl#Class"/>
    <rdfs:subClassOf rdf:nodeID="A12"/>
    <rdfs:label>CropSpecies</rdfs:label>
    <rdfs:subClassOf rdf:nodeID="A13"/>
  </rdf:Description>
  <rdf:Description rdf:nodeID="A14">
    <foaf:name>DEMETER project</foaf:name>
    <foaf:homepage rdf:resource="https://h2020-demeter.eu/"/>
  </rdf:Description>
  <rdf:Description rdf:about="https://saref.etsi.org/saref4agri/generates">
    <rdfs:isDefinedBy rdf:resource="https://saref.etsi.org/saref4agri/"/>
    <rdfs:label xml:lang="en">generates</rdfs:label>
    <rdfs:comment>A relation to represent the yield generated by a Crop.</rdfs:comment>
    <rdfs:subPropertyOf rdf:resource="https://saref.etsi.org/core/hasProperty"/>
    <rdf:type rdf:resource="http://www.w3.org/2002/07/owl#ObjectProperty"/>
  </rdf:Description>
  <rdf:Description rdf:about="http://foodie-cloud.com/model/foodie#cropSpecies">
    <rdfs:isDefinedBy rdf:resource="http://foodie-cloud.com/model/foodie"/>
    <rdfs:label>cropSpecies</rdfs:label>
    <rdfs:comment>Relation to the designation under which the CropSpecies is commonly known; such designation is expressed as a CropType</rdfs:comment>
    <skos:prefLabel xml:lang="en">cropSpecies</skos:prefLabel>
    <rdfs:range rdf:resource="http://foodie-cloud.com/model/foodie#CropType"/>
    <rdf:type rdf:resource="http://www.w3.org/2002/07/owl#ObjectProperty"/>
  </rdf:Description>
  <rdf:Description rdf:about="https://saref.etsi.org/saref4agri/receives">
    <rdfs:isDefinedBy rdf:resource="https://saref.etsi.org/saref4agri/"/>
    <rdfs:label>receives</rdfs:label>
    <rdfs:comment>A relation to represent the intake/consumption of certain substances in a Crop.</rdfs:comment>
    <rdfs:subPropertyOf rdf:resource="https://saref.etsi.org/core/hasProperty"/>
    <rdf:type rdf:resource="http://www.w3.org/2002/07/owl#ObjectProperty"/>
  </rdf:Description>
  <rdf:Description rdf:nodeID="A15">
    <owl:onProperty rdf:resource="http://foodie-cloud.com/model/foodie#species"/>
    <owl:maxCardinality rdf:datatype="http://www.w3.org/2001/XMLSchema#int">1</owl:maxCardinality>
    <rdf:type rdf:resource="http://www.w3.org/2002/07/owl#Restriction"/>
  </rdf:Description>
  <rdf:Description rdf:about="http://foodie-cloud.com/model/foodie#CropType">
    <rdfs:subClassOf rdf:nodeID="A7"/>
    <rdfs:label>CropType</rdfs:label>
    <skos:prefLabel xml:lang="en">CropType</skos:prefLabel>
    <rdfs:subClassOf rdf:nodeID="A16"/>
    <rdfs:subClassOf rdf:nodeID="A0"/>
    <rdfs:subClassOf rdf:nodeID="A2"/>
    <rdfs:subClassOf rdf:nodeID="A15"/>
    <rdf:type rdf:resource="http://www.w3.org/2002/07/owl#Class"/>
    <rdfs:subClassOf rdf:nodeID="A17"/>
    <rdfs:comment xml:lang="en">Designation under which the CropSpecies is commonly known</rdfs:comment>
    <rdfs:subClassOf rdf:nodeID="A18"/>
    <rdfs:isDefinedBy rdf:resource="http://foodie-cloud.com/model/foodie"/>
  </rdf:Description>
  <rdf:Description rdf:about="http://foodie-cloud.com/model/foodie#family">
    <rdfs:isDefinedBy rdf:resource="http://foodie-cloud.com/model/foodie"/>
    <rdfs:label>family</rdfs:label>
    <rdfs:comment>a principal taxonomic category that ranks above genus and below order</rdfs:comment>
    <skos:prefLabel xml:lang="en">family</skos:prefLabel>
    <rdfs:range rdf:resource="http://www.w3.org/2001/XMLSchema#string"/>
    <rdf:type rdf:resource="http://www.w3.org/2002/07/owl#DatatypeProperty"/>
  </rdf:Description>
  <rdf:Description rdf:about="http://foodie-cloud.com/model/foodie#variety">
    <rdfs:isDefinedBy rdf:resource="http://foodie-cloud.com/model/foodie"/>
    <rdfs:label>variety</rdfs:label>
    <rdfs:comment>a taxonomic category that ranks below subspecies (where present) or species, its mem-bers differing from others of the same subspecies or species in minor but permanent or heritable characteristics</rdfs:comment>
    <skos:prefLabel xml:lang="en">variety</skos:prefLabel>
    <rdfs:range rdf:resource="http://www.w3.org/2001/XMLSchema#string"/>
    <rdf:type rdf:resource="http://www.w3.org/2002/07/owl#DatatypeProperty"/>
  </rdf:Description>
  <rdf:Description rdf:nodeID="A19">
    <foaf:name>Raul Palma</foaf:name>
    <rdfs:seeAlso rdf:resource="http://orcid.org/0000-0003-4289-4922"/>
    <schema:affiliation rdf:nodeID="A20"/>
  </rdf:Description>
  <rdf:Description rdf:nodeID="A21">
    <foaf:name>ICCS</foaf:name>
  </rdf:Description>
  <rdf:Description rdf:about="https://smartdatamodels.org/dataModel.Agrifood/AgriCrop">
    <rdfs:isDefinedBy rdf:resource="https://github.com/smart-data-models/dataModel.Agrifood/blob/master/AgriCrop/schema.json"/>
    <rdfs:comment>This entity contains a harmonised description of a generic crop. This entity is primarily associated with the agricultural vertical and related IoT applications.</rdfs:comment>
    <rdfs:label>Agri Crop</rdfs:label>
    <rdf:type rdf:resource="http://www.w3.org/2002/07/owl#Class"/>
  </rdf:Description>
  <rdf:Description rdf:nodeID="A16">
    <owl:onProperty rdf:resource="http://foodie-cloud.com/model/foodie#family"/>
    <owl:maxCardinality rdf:datatype="http://www.w3.org/2001/XMLSchema#int">1</owl:maxCardinality>
    <rdf:type rdf:resource="http://www.w3.org/2002/07/owl#Restriction"/>
  </rdf:Description>
  <rdf:Description rdf:about="https://smartdatamodels.org/dataModel.Agrifood/hasAgriSoil">
    <rdfs:isDefinedBy rdf:resource="https://github.com/smart-data-models/dataModel.Agrifood/blob/master/AgriCrop/schema.json"/>
    <rdfs:comment>Reference to the recommended types of soil suitable for growing this crop</rdfs:comment>
    <rdfs:label xml:lang="en">cropHasAgriSoil</rdfs:label>
    <rdf:type rdf:resource="http://www.w3.org/2002/07/owl#ObjectProperty"/>
  </rdf:Description>
  <rdf:Description rdf:nodeID="A22">
    <foaf:name>Ioanna Roussaki</foaf:name>
    <schema:affiliation rdf:nodeID="A21"/>
  </rdf:Description>
  <rdf:Description rdf:nodeID="A9">
    <owl:onProperty rdf:resource="http://www.w3.org/ns/prov#generatedAtTime"/>
    <owl:maxCardinality rdf:datatype="http://www.w3.org/2001/XMLSchema#int">1</owl:maxCardinality>
    <rdf:type rdf:resource="http://www.w3.org/2002/07/owl#Restriction"/>
  </rdf:Description>
  <rdf:Description rdf:about="http://foodie-cloud.com/model/foodie#production">
    <rdfs:isDefinedBy rdf:resource="http://foodie-cloud.com/model/foodie"/>
    <rdfs:label>production</rdfs:label>
    <rdfs:comment>Relation to entity containing relevant production-related data, that is defined as a ProductionType</rdfs:comment>
    <skos:prefLabel xml:lang="en">production</skos:prefLabel>
    <rdfs:range rdf:resource="http://foodie-cloud.com/model/foodie#ProductionType"/>
    <rdf:type rdf:resource="http://www.w3.org/2002/07/owl#ObjectProperty"/>
  </rdf:Description>
  <rdf:Description rdf:about="https://smartdatamodels.org/dataModel.Agrifood/harvestingInterval">
    <rdfs:isDefinedBy rdf:resource="https://github.com/smart-data-models/dataModel.Agrifood/blob/master/AgriCrop/schema.json"/>
    <rdfs:comment>A list of the recommended harvesting interval date(s) for this crop. Specified using ISO8601 repeating date intervals:
interval, description
Where interval is in the form of start date/end date
--MM-DD/--MM-DD
Meaning repeat each year from this start date to this end date.</rdfs:comment>
    <rdfs:label xml:lang="en">harvestingInterval</rdfs:label>
    <rdf:type rdf:resource="http://www.w3.org/2002/07/owl#DatatypeProperty"/>
  </rdf:Description>
  <rdf:Description rdf:nodeID="A4">
    <foaf:name>OGC</foaf:name>
  </rdf:Description>
  <rdf:Description rdf:about="http://foodie-cloud.com/model/foodie#productionDate">
    <rdfs:isDefinedBy rdf:resource="http://foodie-cloud.com/model/foodie"/>
    <rdfs:label>productionDate</rdfs:label>
    <rdfs:comment>date and time of production, e.g., when it was inserted or changed in the database</rdfs:comment>
    <skos:prefLabel xml:lang="en">productionDate</skos:prefLabel>
    <rdfs:range rdf:resource="http://www.w3.org/2001/XMLSchema#dateTime"/>
    <rdf:type rdf:resource="http://www.w3.org/2002/07/owl#DatatypeProperty"/>
  </rdf:Description>
  <rdf:Description rdf:about="https://w3id.org/demeter/agri/agriCrop#expectedBloomingStart">
    <rdfs:isDefinedBy rdf:resource="https://w3id.org/demeter/agri/agriCrop#"/>
    <rdfs:comment>Expected Blooming Start</rdfs:comment>
    <rdfs:label>Expected Blooming Start</rdfs:label>
    <rdfs:range rdf:resource="http://www.w3.org/2001/XMLSchema#dateTime"/>
    <rdf:type rdf:resource="http://www.w3.org/2002/07/owl#DatatypeProperty"/>
  </rdf:Description>
  <rdf:Description rdf:about="http://foodie-cloud.com/model/foodie#species">
    <rdfs:isDefinedBy rdf:resource="http://foodie-cloud.com/model/foodie"/>
    <rdfs:label>species</rdfs:label>
    <rdfs:comment>a group of living organisms consisting of similar individuals capable of exchanging genes or interbreeding</rdfs:comment>
    <skos:prefLabel xml:lang="en">species</skos:prefLabel>
    <rdfs:range rdf:resource="http://www.w3.org/2001/XMLSchema#string"/>
    <rdf:type rdf:resource="http://www.w3.org/2002/07/owl#DatatypeProperty"/>
  </rdf:Description>
  <rdf:Description rdf:about="https://smartdatamodels.org/dataModel.Agrifood/hasAgriPest">
    <rdfs:isDefinedBy rdf:resource="https://github.com/smart-data-models/dataModel.Agrifood/blob/master/AgriCrop/schema.json"/>
    <rdfs:comment>Reference to the pests known to attack this crop.</rdfs:comment>
    <rdfs:label xml:lang="en">hasAgriPest</rdfs:label>
    <rdf:type rdf:resource="http://www.w3.org/2002/07/owl#ObjectProperty"/>
  </rdf:Description>
  <rdf:Description rdf:nodeID="A13">
    <owl:onProperty rdf:resource="http://foodie-cloud.com/model/foodie#cropSpecies"/>
    <owl:cardinality rdf:datatype="http://www.w3.org/2001/XMLSchema#int">1</owl:cardinality>
    <rdf:type rdf:resource="http://www.w3.org/2002/07/owl#Restriction"/>
  </rdf:Description>
  <rdf:Description rdf:nodeID="A17">
    <owl:onProperty rdf:resource="http://foodie-cloud.com/model/foodie#description"/>
    <owl:maxCardinality rdf:datatype="http://www.w3.org/2001/XMLSchema#int">1</owl:maxCardinality>
    <rdf:type rdf:resource="http://www.w3.org/2002/07/owl#Restriction"/>
  </rdf:Description>
  <rdf:Description rdf:nodeID="A10">
    <owl:onProperty rdf:resource="http://portele.de/ont/inspire/baseInspire#validFrom"/>
    <owl:cardinality rdf:datatype="http://www.w3.org/2001/XMLSchema#int">1</owl:cardinality>
    <rdf:type rdf:resource="http://www.w3.org/2002/07/owl#Restriction"/>
  </rdf:Description>
  <rdf:Description rdf:about="https://w3id.org/demeter/agri/agriCrop#expectedBloomingEnd">
    <rdfs:isDefinedBy rdf:resource="https://w3id.org/demeter/agri/agriCrop#"/>
    <rdfs:comment>Expected Blooming End</rdfs:comment>
    <rdfs:label>Expected Blooming End</rdfs:label>
    <rdfs:range rdf:resource="http://www.w3.org/2001/XMLSchema#dateTime"/>
    <rdf:type rdf:resource="http://www.w3.org/2002/07/owl#DatatypeProperty"/>
  </rdf:Description>
  <rdf:Description rdf:about="https://w3id.org/demeter/agri/agriCrop">
    <rdf:type rdf:resource="http://www.w3.org/2002/07/owl#Ontology"/>
    <dct:description xml:lang="en">The DEMETER AgriCrop is one of the agri profiles of DEMETER AIM. This profile was created by reusing and aligning well-known ontologies and vocabularies</dct:description>
    <dct:contributor rdf:nodeID="A3"/>
    <owl:imports rdf:resource="https://w3id.org/demeter/agri/agriCommon"/>
    <rdfs:label>DEMETER AgriCrop</rdfs:label>
    <dct:title xml:lang="en">DEMETER AgriCrop</dct:title>
    <dct:contributor rdf:nodeID="A22"/>
    <dct:rights xml:lang="en">This vocabulary is distributed under Creative Commons Attribution 4.0 License - http://creativecommons.org/licenses/by/4.0</dct:rights>
    <foaf:maker rdf:nodeID="A14"/>
    <owl:versionInfo>3.0</owl:versionInfo>
    <owl:versionIRI rdf:resource="https://w3id.org/demeter/agri/agriCrop/3.0"/>
    <dct:creator rdf:nodeID="A19"/>
    <rdfs:comment xml:lang="en">The DEMETER Agriculture Information Model (AIM) is the common vocabulary in DEMETER project providing the basis for semantic interoperability across smart farming solutions</rdfs:comment>
  </rdf:Description>
  <rdf:Description rdf:about="https://w3id.org/demeter/agri/agriCrop#numberOfHivesNeeded">
    <rdfs:isDefinedBy rdf:resource="https://w3id.org/demeter/agri/agriCrop#"/>
    <rdfs:comment>Number Of Hives Needed</rdfs:comment>
    <rdfs:label>Number Of Hives Needed</rdfs:label>
    <rdfs:range rdf:resource="http://www.w3.org/2001/XMLSchema#dateTime"/>
    <rdf:type rdf:resource="http://www.w3.org/2002/07/owl#DatatypeProperty"/>
  </rdf:Description>
  <rdf:Description rdf:about="http://foodie-cloud.com/model/foodie#cropArea">
    <rdfs:isDefinedBy rdf:resource="http://foodie-cloud.com/model/foodie"/>
    <rdfs:label>cropArea</rdfs:label>
    <rdfs:comment>The geometry defining the spatial extent of the CropSpecies on the Plot</rdfs:comment>
    <skos:prefLabel xml:lang="en">cropArea</skos:prefLabel>
    <rdfs:range rdf:resource="http://www.opengis.net/ont/geosparql#Geometry"/>
    <rdf:type rdf:resource="http://www.w3.org/2002/07/owl#ObjectProperty"/>
  </rdf:Description>
  <rdf:Description rdf:nodeID="A20">
    <foaf:name>PSNC</foaf:name>
  </rdf:Description>
  <rdf:Description rdf:about="https://smartdatamodels.org/dataModel.Agrifood/hasAgriFertiliser">
    <rdfs:isDefinedBy rdf:resource="https://github.com/smart-data-models/dataModel.Agrifood/blob/master/AgriCrop/schema.json"/>
    <rdfs:comment>Reference to the recommended types of fertiliser suitable for growing this crop</rdfs:comment>
    <rdfs:label xml:lang="en">hasAgriFertiliser</rdfs:label>
    <rdf:type rdf:resource="http://www.w3.org/2002/07/owl#ObjectProperty"/>
  </rdf:Description>
  <rdf:Description rdf:about="https://saref.etsi.org/saref4agri/Crop">
    <rdf:type rdf:resource="http://www.w3.org/2002/07/owl#Class"/>
    <rdfs:comment xml:lang="en">A collection of cultivated plants that is grown on a large scale commercially, especially a cereal, fruit, or vegetable.</rdfs:comment>
    <rdfs:subClassOf rdf:nodeID="A8"/>
    <rdfs:label>Crop</rdfs:label>
    <rdfs:isDefinedBy rdf:resource="https://saref.etsi.org/saref4agri/"/>
    <rdfs:subClassOf rdf:nodeID="A23"/>
    <rdfs:subClassOf rdf:resource="https://saref.etsi.org/core/FeatureOfInterest"/>
    <owl:equivalentClass rdf:resource="http://foodie-cloud.com/model/foodie#CropSpecies"/>
    <rdfs:subClassOf rdf:nodeID="A1"/>
    <owl:equivalentClass rdf:resource="https://smartdatamodels.org/dataModel.Agrifood/AgriCrop"/>
  </rdf:Description>
  <rdf:Description rdf:nodeID="A23">
    <owl:someValuesFrom rdf:resource="http://purl.obolibrary.org/obo/TAXRANK_0000000"/>
    <owl:onProperty rdf:resource="http://purl.obolibrary.org/obo/TAXRANK_1000000"/>
    <rdf:type rdf:resource="http://www.w3.org/2002/07/owl#Restriction"/>
  </rdf:Description>
  <rdf:Description rdf:nodeID="A18">
    <owl:onProperty rdf:resource="http://foodie-cloud.com/model/foodie#notes"/>
    <owl:maxCardinality rdf:datatype="http://www.w3.org/2001/XMLSchema#int">1</owl:maxCardinality>
    <rdf:type rdf:resource="http://www.w3.org/2002/07/owl#Restriction"/>
  </rdf:Description>
  <rdf:Description rdf:about="http://foodie-cloud.com/model/foodie#ProductionType">
    <rdfs:isDefinedBy rdf:resource="http://foodie-cloud.com/model/foodie"/>
    <rdfs:label>ProductionType</rdfs:label>
    <rdfs:comment xml:lang="en">An entity containing relevant production-related data</rdfs:comment>
    <skos:prefLabel xml:lang="en">ProductionType</skos:prefLabel>
    <rdfs:subClassOf rdf:nodeID="A24"/>
    <rdfs:subClassOf rdf:nodeID="A25"/>
    <rdfs:subClassOf rdf:nodeID="A5"/>
    <rdf:type rdf:resource="http://www.w3.org/2002/07/owl#Class"/>
  </rdf:Description>
  <rdf:Description rdf:about="https://saref.etsi.org/saref4agri/hasHarvestDate">
    <owl:equivalentProperty rdf:resource="http://foodie-cloud.com/model/foodie#productionDate"/>
    <rdfs:isDefinedBy rdf:resource="https://saref.etsi.org/saref4agri/"/>
    <rdfs:label>has harvest date</rdfs:label>
    <rdfs:comment>A relation to express the day the crop is harvested.</rdfs:comment>
    <rdfs:range rdf:resource="http://www.w3.org/2001/XMLSchema#dateTime"/>
    <rdfs:subPropertyOf rdf:resource="http://www.w3.org/2002/07/owl#topDataProperty"/>
    <rdf:type rdf:resource="http://www.w3.org/2002/07/owl#DatatypeProperty"/>
  </rdf:Description>
  <rdf:Description rdf:nodeID="A25">
    <owl:onProperty rdf:resource="http://foodie-cloud.com/model/foodie#productionDate"/>
    <owl:cardinality rdf:datatype="http://www.w3.org/2001/XMLSchema#int">1</owl:cardinality>
    <rdf:type rdf:resource="http://www.w3.org/2002/07/owl#Restriction"/>
  </rdf:Description>
  <rdf:Description rdf:nodeID="A11">
    <owl:onProperty rdf:resource="http://www.w3.org/ns/prov#invalidatedAtTime"/>
    <owl:maxCardinality rdf:datatype="http://www.w3.org/2001/XMLSchema#int">1</owl:maxCardinality>
    <rdf:type rdf:resource="http://www.w3.org/2002/07/owl#Restriction"/>
  </rdf:Description>
  <rdf:Description rdf:about="http://foodie-cloud.com/model/foodie#genus">
    <rdfs:isDefinedBy rdf:resource="http://foodie-cloud.com/model/foodie"/>
    <rdfs:label>genus</rdfs:label>
    <rdfs:comment>a principal taxonomic category that ranks above species and below family</rdfs:comment>
    <skos:prefLabel xml:lang="en">genus</skos:prefLabel>
    <rdfs:range rdf:resource="http://www.w3.org/2001/XMLSchema#string"/>
    <rdf:type rdf:resource="http://www.w3.org/2002/07/owl#DatatypeProperty"/>
  </rdf:Description>
  <rdf:Description rdf:nodeID="A24">
    <owl:onProperty rdf:resource="http://foodie-cloud.com/model/foodie#productionAmount"/>
    <owl:maxCardinality rdf:datatype="http://www.w3.org/2001/XMLSchema#int">1</owl:maxCardinality>
    <rdf:type rdf:resource="http://www.w3.org/2002/07/owl#Restriction"/>
  </rdf:Description>
  <rdf:Description rdf:about="https://saref.etsi.org/saref4agri/hasPlantDate">
    <rdfs:isDefinedBy rdf:resource="https://saref.etsi.org/saref4agri/"/>
    <rdfs:label>has plant date</rdfs:label>
    <rdfs:comment>A relation to express the day the crop is planted.</rdfs:comment>
    <rdfs:range rdf:resource="http://www.w3.org/2001/XMLSchema#dateTime"/>
    <rdfs:subPropertyOf rdf:resource="http://www.w3.org/2002/07/owl#topDataProperty"/>
    <rdf:type rdf:resource="http://www.w3.org/2002/07/owl#DatatypeProperty"/>
  </rdf:Description>
  <rdf:Description rdf:nodeID="A12">
    <owl:onProperty rdf:resource="http://portele.de/ont/inspire/baseInspire#validTo"/>
    <owl:maxCardinality rdf:datatype="http://www.w3.org/2001/XMLSchema#int">1</owl:maxCardinality>
    <rdf:type rdf:resource="http://www.w3.org/2002/07/owl#Restriction"/>
  </rdf:Description>
</rdf:RDF>
