<rdf:RDF
    xmlns:qudt="http://qudt.org/schema/qudt/"
    xmlns:demeterAgriCommon="https://w3id.org/demeter/agri/agriCommon#"
    xmlns="https://w3id.org/demeter/"
    xmlns:af-inspire="http://inspire.ec.europa.eu/schemas/af/3.0#"
    xmlns:saref="https://saref.etsi.org/core/"
    xmlns:common="http://portele.de/ont/inspire/baseInspire#"
    xmlns:dct="http://purl.org/dc/terms/"
    xmlns:obo="http://purl.obolibrary.org/obo/"
    xmlns:saref4agri="https://saref.etsi.org/saref4agri/"
    xmlns:prov="http://www.w3.org/ns/prov#"
    xmlns:sosa="http://www.w3.org/ns/sosa/"
    xmlns:iso19103="http://def.seegrid.csiro.au/isotc211/iso19103/2005/basic#"
    xmlns:skos="http://www.w3.org/2004/02/skos/core#"
    xmlns:foodie="http://foodie-cloud.com/model/foodie#"
    xmlns:ecrop="https://w3id.org/demeter/agri/ecrop/"
    xmlns:xsd="http://www.w3.org/2001/XMLSchema#"
    xmlns:rdf="http://www.w3.org/1999/02/22-rdf-syntax-ns#"
    xmlns:iso19115-citation="http://def.seegrid.csiro.au/isotc211/iso19115/2003/citation#"
    xmlns:schema="https://schema.org/"
    xmlns:fiware="https://smartdatamodels.org/"
    xmlns:iso19109="http://def.seegrid.csiro.au/isotc211/iso19109/2005/feature#"
    xmlns:iso19150-2="http://def.seegrid.csiro.au/isotc211/iso19150/-2/2012/basic#"
    xmlns:stat="http://data.europa.eu/m8g/"
    xmlns:rdfs="http://www.w3.org/2000/01/rdf-schema#"
    xmlns:owl="http://www.w3.org/2002/07/owl#"
    xmlns:qb="http://purl.org/linked-data/cube#"
    xmlns:geo="http://www.opengis.net/ont/geosparql#"
    xmlns:dcat="http://www.w3.org/ns/dcat#"
    xmlns:act-inspire="http://inspire.ec.europa.eu/schemas/act-core/3.0#"
    xmlns:ssn="http://www.w3.org/ns/ssn/"
    xmlns:foaf="http://xmlns.com/foaf/0.1/"
    xmlns:fiware-agrifood="https://smartdatamodels.org/dataModel.Agrifood/" > 
  <rdf:Description rdf:about="http://www.w3.org/ns/prov#generatedAtTime">
    <rdfs:subPropertyOf rdf:resource="https://saref.etsi.org/core/hasTimestamp"/>
  </rdf:Description>
  <rdf:Description rdf:about="https://smartdatamodels.org/dataModel.Agrifood/version">
    <rdfs:isDefinedBy rdf:resource="https://github.com/smart-data-models/dataModel.Agrifood/blob/master/AgriApp/schema.json"/>
    <rdfs:comment>The version of the App</rdfs:comment>
    <rdfs:label xml:lang="en">version</rdfs:label>
    <rdf:type rdf:resource="http://www.w3.org/2002/07/owl#DatatypeProperty"/>
  </rdf:Description>
  <rdf:Description rdf:about="https://schema.org/streetAddress">
    <rdfs:isDefinedBy rdf:resource="https://schema.org/streetAddress"/>
    <rdfs:comment>he street address. For example, 1600 Amphitheatre Pkwy.</rdfs:comment>
    <rdfs:label>streetAddress</rdfs:label>
    <rdf:type rdf:resource="http://www.w3.org/2002/07/owl#DatatypeProperty"/>
  </rdf:Description>
  <rdf:Description rdf:about="http://purl.obolibrary.org/obo/TAXRANK_1000000">
    <rdfs:isDefinedBy rdf:resource="http://purl.obolibrary.org/obo/"/>
    <rdfs:comment xml:lang="en">has rank annotation property from obo namespace taxonomic rank</rdfs:comment>
    <rdfs:label xml:lang="en">has_rank</rdfs:label>
    <rdf:type rdf:resource="http://www.w3.org/2002/07/owl#AnnotationProperty"/>
  </rdf:Description>
  <rdf:Description rdf:about="https://w3id.org/demeter/agri/agriCommon#imageFormat">
    <rdfs:isDefinedBy rdf:resource="https://w3id.org/demeter/agri/agriCommon#"/>
    <rdfs:comment>The format of the image, e.g., tiff, jpg</rdfs:comment>
    <rdfs:label>imageFormat</rdfs:label>
    <rdfs:domain rdf:resource="https://w3id.org/demeter/agri/agriCommon#Image"/>
    <rdfs:subPropertyOf rdf:resource="https://schema.org/encodingFormat"/>
    <rdf:type rdf:resource="http://www.w3.org/2002/07/owl#DatatypeProperty"/>
  </rdf:Description>
  <rdf:Description rdf:about="https://smartdatamodels.org/dataModel.Agrifood/agroVocConcept">
    <rdfs:isDefinedBy rdf:resource="https://github.com/smart-data-models/dataModel.Agrifood/blob/master/AgriCrop/schema.json"/>
    <rdfs:comment>The link with the defined concept into the AgroVoc vocabulary</rdfs:comment>
    <rdfs:label xml:lang="en">agroVocConcept</rdfs:label>
    <rdf:type rdf:resource="http://www.w3.org/2002/07/owl#ObjectProperty"/>
  </rdf:Description>
  <rdf:Description rdf:about="http://purl.obolibrary.org/obo/TAXRANK_0000000">
    <rdfs:isDefinedBy rdf:resource="http://purl.obolibrary.org/obo/"/>
    <rdfs:label xml:lang="en">taxonomic_rank</rdfs:label>
    <rdf:type rdf:resource="http://www.w3.org/2002/07/owl#Class"/>
  </rdf:Description>
  <rdf:Description rdf:nodeID="A0">
    <foaf:name>ICCS</foaf:name>
  </rdf:Description>
  <rdf:Description rdf:nodeID="A1">
    <owl:someValuesFrom rdf:resource="https://saref.etsi.org/saref4agri/Farm"/>
    <owl:onProperty rdf:resource="https://saref.etsi.org/saref4agri/managesFarm"/>
    <rdf:type rdf:resource="http://www.w3.org/2002/07/owl#Restriction"/>
  </rdf:Description>
  <rdf:Description rdf:about="http://foodie-cloud.com/model/foodie#price">
    <rdfs:isDefinedBy rdf:resource="http://foodie-cloud.com/model/foodie"/>
    <rdfs:comment>Relation depicting price of a any resource e.g. Product, Treatment etc</rdfs:comment>
    <rdfs:label>price</rdfs:label>
    <skos:prefLabel xml:lang="en">price</skos:prefLabel>
    <rdfs:range rdf:resource="http://www.w3.org/2001/XMLSchema#string"/>
    <rdf:type rdf:resource="http://www.w3.org/2002/07/owl#DatatypeProperty"/>
  </rdf:Description>
  <rdf:Description rdf:about="https://saref.etsi.org/core/hasTimestamp">
    <rdfs:label xml:lang="en">has timestamp</rdfs:label>
    <rdfs:isDefinedBy rdf:resource="https://saref.etsi.org/core/"/>
    <rdfs:comment>A relationship stating the timestamp of an entity (e.g. a measurement)</rdfs:comment>
    <rdfs:range rdf:resource="http://www.w3.org/2001/XMLSchema#dateTime"/>
    <rdf:type rdf:resource="http://www.w3.org/2002/07/owl#DatatypeProperty"/>
  </rdf:Description>
  <rdf:Description rdf:about="https://w3id.org/demeter/agri/agriCommon#password">
    <rdfs:isDefinedBy rdf:resource="https://w3id.org/demeter/agri/agriCommon#"/>
    <rdfs:comment>Password</rdfs:comment>
    <rdfs:label>Password</rdfs:label>
    <rdfs:range rdf:resource="http://www.w3.org/2001/XMLSchema#string"/>
    <rdf:type rdf:resource="http://www.w3.org/2002/07/owl#DatatypeProperty"/>
  </rdf:Description>
  <rdf:Description rdf:about="https://saref.etsi.org/saref4agri/Farmer">
    <rdfs:isDefinedBy rdf:resource="https://saref.etsi.org/saref4agri/"/>
    <rdfs:label xml:lang="en">Farmer</rdfs:label>
    <rdfs:comment>A class to decsribe a saref4agri farmer as subcass of a foaf:Person</rdfs:comment>
    <rdfs:subClassOf rdf:nodeID="A2"/>
    <rdfs:subClassOf rdf:nodeID="A3"/>
    <rdfs:subClassOf rdf:resource="http://xmlns.com/foaf/0.1/Person"/>
    <rdf:type rdf:resource="http://www.w3.org/2002/07/owl#Class"/>
  </rdf:Description>
  <rdf:Description rdf:about="https://saref.etsi.org/saref4agri/hasName">
    <owl:equivalentProperty rdf:resource="https://smartdatamodels.org/name"/>
    <rdfs:isDefinedBy rdf:resource="https://saref.etsi.org/saref4agri/"/>
    <rdfs:label>has name</rdfs:label>
    <rdfs:comment>A relation to express the name of an entity (e.g.,animal).</rdfs:comment>
    <rdfs:range rdf:resource="http://www.w3.org/2001/XMLSchema#string"/>
    <rdf:type rdf:resource="http://www.w3.org/2002/07/owl#DatatypeProperty"/>
  </rdf:Description>
  <rdf:Description rdf:about="https://saref.etsi.org/saref4agri/managesFarm">
    <rdfs:isDefinedBy rdf:resource="https://saref.etsi.org/saref4agri/"/>
    <rdfs:comment xml:lang="en">manages farm</rdfs:comment>
    <rdfs:label xml:lang="en">manages farm</rdfs:label>
    <rdf:type rdf:resource="http://www.w3.org/2002/07/owl#ObjectProperty"/>
  </rdf:Description>
  <rdf:Description rdf:about="https://smartdatamodels.org/dataProvider">
    <rdfs:isDefinedBy rdf:resource="https://github.com/smart-data-models/dataModel.Agrifood/blob/master/AgriApp/schemaDTDL.json"/>
    <rdfs:comment>A sequence of characters identifying the provider of the harmonised data entity</rdfs:comment>
    <rdfs:label xml:lang="en">dataProvider</rdfs:label>
    <rdf:type rdf:resource="http://www.w3.org/2002/07/owl#DatatypeProperty"/>
  </rdf:Description>
  <rdf:Description rdf:about="https://schema.org/addressCountry">
    <rdfs:isDefinedBy rdf:resource="https://schema.org/addressCountry"/>
    <rdfs:comment>The country. For example, USA. You can also provide the two-letter ISO 3166-1 alpha-2 country code</rdfs:comment>
    <rdfs:label>addressCountry</rdfs:label>
    <rdf:type rdf:resource="http://www.w3.org/2002/07/owl#DatatypeProperty"/>
  </rdf:Description>
  <rdf:Description rdf:about="https://w3id.org/demeter/agri/ecrop/contractSeller">
    <rdfs:isDefinedBy rdf:resource="https://unece.org/fileadmin/DAM/cefact/brs/BRS_eCROP_v1.pdf"/>
    <rdfs:comment>The seller party for an agricultural contract</rdfs:comment>
    <rdfs:label>contractSeller</rdfs:label>
    <rdf:type rdf:resource="http://www.w3.org/2002/07/owl#ObjectProperty"/>
  </rdf:Description>
  <rdf:Description rdf:about="http://portele.de/ont/inspire/baseInspire#validFrom">
    <rdfs:isDefinedBy rdf:resource="http://portele.de/ont/inspire/baseInspire#"/>
    <rdfs:comment>begin of real-world phenomenon</rdfs:comment>
    <rdfs:label>valid from</rdfs:label>
    <skos:prefLabel xml:lang="en">valid from</skos:prefLabel>
    <rdfs:range rdf:resource="http://www.w3.org/2001/XMLSchema#dateTime"/>
    <rdf:type rdf:resource="http://www.w3.org/2002/07/owl#DatatypeProperty"/>
  </rdf:Description>
  <rdf:Description rdf:about="http://foodie-cloud.com/model/foodie#type">
    <rdfs:isDefinedBy rdf:resource="http://foodie-cloud.com/model/foodie"/>
    <rdfs:comment>Relation specifying the type of an enity, e.g., Intervention</rdfs:comment>
    <rdfs:label>type</rdfs:label>
    <skos:prefLabel xml:lang="en">type</skos:prefLabel>
    <rdfs:range rdf:resource="http://www.w3.org/2001/XMLSchema#string"/>
    <rdf:type rdf:resource="http://www.w3.org/2002/07/owl#DatatypeProperty"/>
  </rdf:Description>
  <rdf:Description rdf:about="https://smartdatamodels.org/name">
    <rdfs:subPropertyOf rdf:resource="https://schema.org/name"/>
    <rdfs:isDefinedBy rdf:resource="https://github.com/smart-data-models/dataModel.Agrifood/blob/master/AgriApp/schemaDTDL.json"/>
    <rdfs:comment>The name of this item</rdfs:comment>
    <rdfs:label xml:lang="en">name</rdfs:label>
    <rdf:type rdf:resource="http://www.w3.org/2002/07/owl#DatatypeProperty"/>
  </rdf:Description>
  <rdf:Description rdf:nodeID="A2">
    <owl:allValuesFrom rdf:resource="http://www.w3.org/2001/XMLSchema#string"/>
    <owl:onProperty rdf:resource="https://saref.etsi.org/saref4agri/hasName"/>
    <rdf:type rdf:resource="http://www.w3.org/2002/07/owl#Restriction"/>
  </rdf:Description>
  <rdf:Description rdf:about="https://w3id.org/demeter/agri/ecrop/AgriculturalCertificate">
    <rdfs:comment>The written or spoken contract between two or more parties for the expressed purpose of specifying the required agricultural produce, products or services</rdfs:comment>
    <rdfs:label>AgriculturalContract</rdfs:label>
    <rdfs:isDefinedBy rdf:resource="https://unece.org/fileadmin/DAM/cefact/brs/BRS_eCROP_v1.pdf"/>
    <rdfs:comment>A legal proof of ownership, worthiness or qualification to operate an agricultural item</rdfs:comment>
    <rdfs:label>AgriculturalCertificate</rdfs:label>
    <rdf:type rdf:resource="http://www.w3.org/2002/07/owl#Class"/>
  </rdf:Description>
  <rdf:Description rdf:about="https://smartdatamodels.org/alternateName">
    <rdfs:subPropertyOf rdf:resource="https://smartdatamodels.org/name"/>
    <rdfs:isDefinedBy rdf:resource="https://github.com/smart-data-models/dataModel.Agrifood/blob/master/AgriApp/schemaDTDL.json"/>
    <rdfs:comment>An alternative name for this item</rdfs:comment>
    <rdfs:label xml:lang="en">alternateName</rdfs:label>
    <rdf:type rdf:resource="http://www.w3.org/2002/07/owl#DatatypeProperty"/>
  </rdf:Description>
  <rdf:Description rdf:about="http://foodie-cloud.com/model/foodie#description">
    <rdfs:isDefinedBy rdf:resource="http://foodie-cloud.com/model/foodie"/>
    <rdfs:comment>Any further information related to an entity that may help for a better understanding</rdfs:comment>
    <rdfs:label>description</rdfs:label>
    <skos:prefLabel xml:lang="en">description</skos:prefLabel>
    <rdfs:range rdf:resource="http://www.w3.org/2001/XMLSchema#string"/>
    <rdf:type rdf:resource="http://www.w3.org/2002/07/owl#DatatypeProperty"/>
  </rdf:Description>
  <rdf:Description rdf:about="https://smartdatamodels.org/address">
    <rdfs:isDefinedBy rdf:resource="https://github.com/smart-data-models/dataModel.Agrifood/blob/master/AgriApp/schemaDTDL.json"/>
    <rdfs:comment>The mailing address</rdfs:comment>
    <rdfs:label xml:lang="en">address</rdfs:label>
    <rdf:type rdf:resource="http://www.w3.org/2002/07/owl#ObjectProperty"/>
  </rdf:Description>
  <rdf:Description rdf:about="https://w3id.org/demeter/agri/agriCommon#imageHeight">
    <rdfs:isDefinedBy rdf:resource="https://w3id.org/demeter/agri/agriCommon#"/>
    <rdfs:comment>The height of the image, e.g., 3 or 3 cm^^cdt:ucum</rdfs:comment>
    <rdfs:label>imageHeight</rdfs:label>
    <rdfs:domain rdf:resource="https://w3id.org/demeter/agri/agriCommon#Image"/>
    <rdfs:subPropertyOf rdf:resource="https://saref.etsi.org/core/hasValue"/>
    <rdfs:subPropertyOf rdf:resource="https://schema.org/height"/>
    <rdf:type rdf:resource="http://www.w3.org/2002/07/owl#DatatypeProperty"/>
  </rdf:Description>
  <rdf:Description rdf:about="https://smartdatamodels.org/dataModel.Agrifood/category">
    <owl:equivalentProperty rdf:resource="http://foodie-cloud.com/model/foodie#type"/>
    <rdfs:isDefinedBy rdf:resource="https://github.com/smart-data-models/dataModel.Agrifood/blob/master/AgriParcel/schema.json"/>
    <rdfs:comment>The category of the entity, e.g., parcel of land e.g.: **arable, grassland, vineyard, orchard, mixed crop, lowland, upland, set-aside, forestry, wetland.**, alert (traffic, naturalDisaster, weather, environment, health, security, agriculture).</rdfs:comment>
    <rdfs:label xml:lang="en">category</rdfs:label>
    <rdf:type rdf:resource="http://www.w3.org/2002/07/owl#DatatypeProperty"/>
  </rdf:Description>
  <rdf:Description rdf:nodeID="A4">
    <foaf:name>Raul Palma</foaf:name>
    <rdfs:seeAlso rdf:resource="http://orcid.org/0000-0003-4289-4922"/>
    <schema:affiliation rdf:nodeID="A5"/>
  </rdf:Description>
  <rdf:Description rdf:about="http://portele.de/ont/inspire/baseInspire#validTo">
    <rdfs:isDefinedBy rdf:resource="http://portele.de/ont/inspire/baseInspire#"/>
    <rdfs:comment>end of real-world phenomenon</rdfs:comment>
    <rdfs:label>valid to</rdfs:label>
    <skos:prefLabel xml:lang="en">valid to</skos:prefLabel>
    <rdfs:range rdf:resource="http://www.w3.org/2001/XMLSchema#dateTime"/>
    <rdf:type rdf:resource="http://www.w3.org/2002/07/owl#DatatypeProperty"/>
  </rdf:Description>
  <rdf:Description rdf:nodeID="A6">
    <foaf:name>DEMETER project</foaf:name>
    <foaf:homepage rdf:resource="https://h2020-demeter.eu/"/>
  </rdf:Description>
  <rdf:Description rdf:about="https://w3id.org/demeter/agri/ecrop/contractBuyer">
    <rdfs:isDefinedBy rdf:resource="https://unece.org/fileadmin/DAM/cefact/brs/BRS_eCROP_v1.pdf"/>
    <rdfs:comment>The buyer party for an agricultural contract</rdfs:comment>
    <rdfs:label>contractBuyer</rdfs:label>
    <rdf:type rdf:resource="http://www.w3.org/2002/07/owl#ObjectProperty"/>
  </rdf:Description>
  <rdf:Description rdf:about="https://smartdatamodels.org/dateCreated">
    <rdfs:subPropertyOf rdf:resource="https://saref.etsi.org/core/hasTimestamp"/>
    <rdfs:isDefinedBy rdf:resource="https://github.com/smart-data-models/dataModel.Agrifood/blob/master/AgriApp/schemaDTDL.json"/>
    <rdfs:comment>Entity creation timestamp. This will usually be allocated by the storage platform</rdfs:comment>
    <rdfs:label xml:lang="en">dateCreated</rdfs:label>
    <rdfs:range rdf:resource="http://www.w3.org/2001/XMLSchema#dateTime"/>
    <rdf:type rdf:resource="http://www.w3.org/2002/07/owl#DatatypeProperty"/>
  </rdf:Description>
  <rdf:Description rdf:about="https://smartdatamodels.org/dateModified">
    <rdfs:isDefinedBy rdf:resource="https://github.com/smart-data-models/dataModel.Agrifood/blob/master/AgriApp/schemaDTDL.json"/>
    <rdfs:comment>Timestamp of the last modification of the entity. This will usually be allocated by the storage platform</rdfs:comment>
    <rdfs:label xml:lang="en">dateModified</rdfs:label>
    <rdfs:range rdf:resource="http://www.w3.org/2001/XMLSchema#dateTime"/>
    <rdf:type rdf:resource="http://www.w3.org/2002/07/owl#DatatypeProperty"/>
  </rdf:Description>
  <rdf:Description rdf:about="http://foodie-cloud.com/model/foodie#code">
    <rdfs:isDefinedBy rdf:resource="http://foodie-cloud.com/model/foodie"/>
    <rdfs:comment>Unique identification of an entity, e.g., ActiveIngredient</rdfs:comment>
    <rdfs:label>code</rdfs:label>
    <skos:prefLabel xml:lang="en">code</skos:prefLabel>
    <rdfs:range rdf:resource="http://www.w3.org/2001/XMLSchema#string"/>
    <rdf:type rdf:resource="http://www.w3.org/2002/07/owl#DatatypeProperty"/>
  </rdf:Description>
  <rdf:Description rdf:about="https://saref.etsi.org/core/hasDescription">
    <owl:equivalentProperty rdf:resource="http://foodie-cloud.com/model/foodie#description"/>
    <rdfs:label xml:lang="en">has description</rdfs:label>
    <rdfs:isDefinedBy rdf:resource="https://saref.etsi.org/core/"/>
    <rdfs:comment>A relationship providing a description of an entity (e.g., device)</rdfs:comment>
    <rdfs:range rdf:resource="http://www.w3.org/2001/XMLSchema#string"/>
    <rdf:type rdf:resource="http://www.w3.org/2002/07/owl#DatatypeProperty"/>
  </rdf:Description>
  <rdf:Description rdf:about="https://w3id.org/demeter/agri/agriCommon#Image">
    <rdfs:isDefinedBy rdf:resource="https://w3id.org/demeter/agri/agriCommon#"/>
    <rdfs:comment>An image object</rdfs:comment>
    <rdfs:label>Image</rdfs:label>
    <rdfs:subClassOf rdf:resource="https://schema.org/ImageObject"/>
    <rdf:type rdf:resource="http://www.w3.org/2002/07/owl#Class"/>
  </rdf:Description>
  <rdf:Description rdf:nodeID="A7">
    <foaf:name>Ioanna Roussaki</foaf:name>
    <schema:affiliation rdf:nodeID="A0"/>
  </rdf:Description>
  <rdf:Description rdf:about="https://w3id.org/demeter/agri/agriCommon#imageWidth">
    <rdfs:isDefinedBy rdf:resource="https://w3id.org/demeter/agri/agriCommon#"/>
    <rdfs:comment>The width of the image, e.g., 3 or 3 cm^^cdt:ucum</rdfs:comment>
    <rdfs:label>imageWidth</rdfs:label>
    <rdfs:domain rdf:resource="https://w3id.org/demeter/agri/agriCommon#Image"/>
    <rdfs:subPropertyOf rdf:resource="https://saref.etsi.org/core/hasValue"/>
    <rdfs:subPropertyOf rdf:resource="https://schema.org/width"/>
    <rdf:type rdf:resource="http://www.w3.org/2002/07/owl#DatatypeProperty"/>
  </rdf:Description>
  <rdf:Description rdf:about="https://w3id.org/demeter/agri/agriCommon">
    <dct:rights xml:lang="en">This vocabulary is distributed under Creative Commons Attribution 4.0 License - http://creativecommons.org/licenses/by/4.0</dct:rights>
    <rdfs:comment xml:lang="en">The Agriculture Information Model (AIM) is the common vocabulary in DEMETER project providing the basis for semantic interoperability across smart farming solutions</rdfs:comment>
    <rdf:type rdf:resource="http://www.w3.org/2002/07/owl#Ontology"/>
    <owl:imports rdf:resource="https://w3id.org/demeter/crossDomain"/>
    <owl:versionIRI rdf:resource="https://w3id.org/demeter/agri/agriCommon/2.0"/>
    <dct:creator rdf:nodeID="A4"/>
    <foaf:maker rdf:nodeID="A6"/>
    <owl:versionInfo>2.0</owl:versionInfo>
    <dct:description xml:lang="en">AgriCommon is one of the agri profiles of the Agriculture Information Model (AIM). This profile was created by reusing and aligning well-known ontologies and vocabularies</dct:description>
    <dct:title xml:lang="en">AIM AgriCommon</dct:title>
    <rdfs:label xml:lang="en">AIM AgriCommon</rdfs:label>
    <dct:contributor rdf:nodeID="A8"/>
    <dct:contributor rdf:nodeID="A7"/>
  </rdf:Description>
  <rdf:Description rdf:nodeID="A3">
    <owl:someValuesFrom rdf:resource="https://saref.etsi.org/saref4agri/Farm"/>
    <owl:onProperty rdf:resource="https://saref.etsi.org/saref4agri/managesFarm"/>
    <rdf:type rdf:resource="http://www.w3.org/2002/07/owl#Restriction"/>
  </rdf:Description>
  <rdf:Description rdf:nodeID="A9">
    <foaf:name>OGC</foaf:name>
  </rdf:Description>
  <rdf:Description rdf:about="https://w3id.org/demeter/agri/agriCommon#imageDataType">
    <rdfs:isDefinedBy rdf:resource="https://w3id.org/demeter/agri/agriCommon#"/>
    <rdfs:comment>The data type of the image, e.g., NDVI</rdfs:comment>
    <rdfs:label>imageDataType</rdfs:label>
    <rdfs:domain rdf:resource="https://w3id.org/demeter/agri/agriCommon#Image"/>
    <rdf:type rdf:resource="http://www.w3.org/2002/07/owl#DatatypeProperty"/>
  </rdf:Description>
  <rdf:Description rdf:about="http://foodie-cloud.com/model/foodie#notes">
    <rdfs:isDefinedBy rdf:resource="http://foodie-cloud.com/model/foodie"/>
    <rdfs:comment>Relation depicting additional information for a recource or entity</rdfs:comment>
    <rdfs:label>notes</rdfs:label>
    <skos:prefLabel xml:lang="en">notes</skos:prefLabel>
    <rdfs:range rdf:resource="http://www.w3.org/2001/XMLSchema#string"/>
    <rdf:type rdf:resource="http://www.w3.org/2002/07/owl#DatatypeProperty"/>
  </rdf:Description>
  <rdf:Description rdf:about="http://def.seegrid.csiro.au/isotc211/iso19115/2003/citation#ResponsibleParty">
    <owl:equivalentClass rdf:resource="http://xmlns.com/foaf/0.1/Agent"/>
  </rdf:Description>
  <rdf:Description rdf:about="https://smartdatamodels.org/source">
    <rdfs:isDefinedBy rdf:resource="https://github.com/smart-data-models/dataModel.Agrifood/blob/master/AgriApp/schemaDTDL.json"/>
    <rdfs:comment>A sequence of characters giving the original source of the entity data as a URL. Recommended to be the fully qualified domain name of the source provider, or the URL to the source object.</rdfs:comment>
    <rdfs:label xml:lang="en">source</rdfs:label>
    <rdf:type rdf:resource="http://www.w3.org/2002/07/owl#DatatypeProperty"/>
  </rdf:Description>
  <rdf:Description rdf:about="https://w3id.org/demeter/agri/agriCommon#userName">
    <rdfs:isDefinedBy rdf:resource="https://w3id.org/demeter/agri/agriCommon#"/>
    <rdfs:comment>User Name</rdfs:comment>
    <rdfs:label>User Name</rdfs:label>
    <rdfs:range rdf:resource="http://www.w3.org/2001/XMLSchema#string"/>
    <rdf:type rdf:resource="http://www.w3.org/2002/07/owl#DatatypeProperty"/>
  </rdf:Description>
  <rdf:Description rdf:about="https://schema.org/addressLocality">
    <rdfs:isDefinedBy rdf:resource="https://schema.org/addressLocality"/>
    <rdfs:comment>The locality in which the street address is, and which is in the region. For example, Mountain View</rdfs:comment>
    <rdfs:label>addressLocality</rdfs:label>
    <rdf:type rdf:resource="http://www.w3.org/2002/07/owl#DatatypeProperty"/>
  </rdf:Description>
  <rdf:Description rdf:nodeID="A8">
    <foaf:name>Rob Atkinson</foaf:name>
    <schema:affiliation rdf:nodeID="A9"/>
  </rdf:Description>
  <rdf:Description rdf:nodeID="A10">
    <owl:allValuesFrom rdf:resource="http://www.w3.org/2001/XMLSchema#string"/>
    <owl:onProperty rdf:resource="https://saref.etsi.org/saref4agri/hasName"/>
    <rdf:type rdf:resource="http://www.w3.org/2002/07/owl#Restriction"/>
  </rdf:Description>
  <rdf:Description rdf:nodeID="A5">
    <foaf:name>PSNC</foaf:name>
  </rdf:Description>
  <rdf:Description rdf:about="https://w3id.org/demeter/agri/agriCommon#eppoConcept">
    <rdfs:isDefinedBy rdf:resource="https://w3id.org/demeter/agri/agriCommon#"/>
    <rdfs:comment>The link with the defined concept into the EPPO vocabulary</rdfs:comment>
    <rdfs:label xml:lang="en">eppoConcept</rdfs:label>
    <rdf:type rdf:resource="http://www.w3.org/2002/07/owl#ObjectProperty"/>
  </rdf:Description>
  <rdf:Description rdf:about="https://w3id.org/demeter/agri/agriCommon#imageURL">
    <rdfs:isDefinedBy rdf:resource="https://w3id.org/demeter/agri/agriCommon#"/>
    <rdfs:comment>Actual bytes of the image object, i.e., image file</rdfs:comment>
    <rdfs:label>imageURL</rdfs:label>
    <rdfs:domain rdf:resource="https://w3id.org/demeter/agri/agriCommon#Image"/>
    <rdfs:range rdf:resource="http://www.w3.org/2001/XMLSchema#anyURI"/>
    <rdfs:subPropertyOf rdf:resource="https://schema.org/contentUrl"/>
    <rdf:type rdf:resource="http://www.w3.org/2002/07/owl#DatatypeProperty"/>
  </rdf:Description>
  <rdf:Description rdf:about="https://schema.org/addressRegion">
    <rdfs:isDefinedBy rdf:resource="https://schema.org/addressRegion"/>
    <rdfs:comment>The region in which the locality is, and which is in the country. For example, California or another appropriate first-level Administrative division</rdfs:comment>
    <rdfs:label>addressRegion</rdfs:label>
    <rdf:type rdf:resource="http://www.w3.org/2002/07/owl#DatatypeProperty"/>
  </rdf:Description>
  <rdf:Description rdf:about="https://saref.etsi.org/saref4agri/FarmHolding">
    <rdfs:isDefinedBy rdf:resource="https://saref.etsi.org/saref4agri/"/>
    <rdfs:label xml:lang="en">Farm holding</rdfs:label>
    <rdfs:comment>A class to decsribe a saref4agri farm holding as subcass of an org:Organization</rdfs:comment>
    <rdfs:subClassOf rdf:nodeID="A10"/>
    <rdfs:subClassOf rdf:nodeID="A1"/>
    <rdfs:subClassOf rdf:resource="https://schema.org/Organization"/>
    <rdf:type rdf:resource="http://www.w3.org/2002/07/owl#Class"/>
  </rdf:Description>
</rdf:RDF>
