<rdf:RDF
    xmlns:af-inspire="http://inspire.ec.europa.eu/schemas/af/3.0#"
    xmlns:saref="https://saref.etsi.org/core/"
    xmlns:common="http://portele.de/ont/inspire/baseInspire#"
    xmlns:dct="http://purl.org/dc/terms/"
    xmlns:saref4agri="https://saref.etsi.org/saref4agri/"
    xmlns:prov="http://www.w3.org/ns/prov#"
    xmlns:sosa="http://www.w3.org/ns/sosa/"
    xmlns:iso19103="http://def.seegrid.csiro.au/isotc211/iso19103/2005/basic#"
    xmlns:skos="http://www.w3.org/2004/02/skos/core#"
    xmlns:foodie="http://foodie-cloud.com/model/foodie#"
    xmlns:xsd="http://www.w3.org/2001/XMLSchema#"
    xmlns:rdf="http://www.w3.org/1999/02/22-rdf-syntax-ns#"
    xmlns:iso19115-citation="http://def.seegrid.csiro.au/isotc211/iso19115/2003/citation#"
    xmlns:schema="https://schema.org/"
    xmlns:fiware="https://smartdatamodels.org/"
    xmlns:iso19109="http://def.seegrid.csiro.au/isotc211/iso19109/2005/feature#"
    xmlns:iso19150-2="http://def.seegrid.csiro.au/isotc211/iso19150/-2/2012/basic#"
    xmlns:stat="http://data.europa.eu/m8g/"
    xmlns:rdfs="http://www.w3.org/2000/01/rdf-schema#"
    xmlns:ngsi-ld="https://uri.etsi.org/ngsi-ld/"
    xmlns:owl="http://www.w3.org/2002/07/owl#"
    xmlns:qb="http://purl.org/linked-data/cube#"
    xmlns:iso19108="http://def.seegrid.csiro.au/isotc211/iso19108/2002/temporal#"
    xmlns:geo="http://www.opengis.net/ont/geosparql#"
    xmlns:dcat="http://www.w3.org/ns/dcat#"
    xmlns="https://w3id.org/cybele/"
    xmlns:act-inspire="http://inspire.ec.europa.eu/schemas/act-core/3.0#"
    xmlns:ssn="http://www.w3.org/ns/ssn/"
    xmlns:foaf="http://xmlns.com/foaf/0.1/"
    xmlns:fiware-agrifood="https://smartdatamodels.org/dataModel.Agrifood/" > 
  <rdf:Description rdf:nodeID="A0">
    <owl:onProperty rdf:resource="http://foodie-cloud.com/model/foodie#treatmentPlanCreation"/>
    <owl:cardinality rdf:datatype="http://www.w3.org/2001/XMLSchema#int">1</owl:cardinality>
    <rdf:type rdf:resource="http://www.w3.org/2002/07/owl#Restriction"/>
  </rdf:Description>
  <rdf:Description rdf:about="http://foodie-cloud.com/model/foodie#interventionGeometry">
    <rdfs:isDefinedBy rdf:resource="http://foodie-cloud.com/model/foodie"/>
    <rdfs:comment>A Relation to the geometry defining the spatial extent of the Intervention</rdfs:comment>
    <rdfs:label>interventionGeometry</rdfs:label>
    <skos:prefLabel xml:lang="en">interventionGeometry</skos:prefLabel>
    <rdfs:range rdf:resource="http://www.opengis.net/ont/geosparql#Geometry"/>
    <rdf:type rdf:resource="http://www.w3.org/2002/07/owl#ObjectProperty"/>
  </rdf:Description>
  <rdf:Description rdf:about="https://smartdatamodels.org/dataModel.Agrifood/hasOperator">
    <rdfs:isDefinedBy rdf:resource="https://github.com/smart-data-models/dataModel.Agrifood/blob/master/AgriParcelOperation/schema.json"/>
    <rdfs:comment>Reference to the operator conducting the operation</rdfs:comment>
    <rdfs:label xml:lang="en">hasOperator</rdfs:label>
    <rdf:type rdf:resource="http://www.w3.org/2002/07/owl#ObjectProperty"/>
  </rdf:Description>
  <rdf:Description rdf:nodeID="A1">
    <owl:onProperty rdf:resource="http://foodie-cloud.com/model/foodie#status"/>
    <owl:cardinality rdf:datatype="http://www.w3.org/2001/XMLSchema#int">1</owl:cardinality>
    <rdf:type rdf:resource="http://www.w3.org/2002/07/owl#Restriction"/>
  </rdf:Description>
  <rdf:Description rdf:nodeID="A2">
    <owl:onProperty rdf:resource="http://foodie-cloud.com/model/foodie#price"/>
    <owl:maxCardinality rdf:datatype="http://www.w3.org/2001/XMLSchema#int">1</owl:maxCardinality>
    <rdf:type rdf:resource="http://www.w3.org/2002/07/owl#Restriction"/>
  </rdf:Description>
  <rdf:Description rdf:about="http://foodie-cloud.com/model/foodie#operator">
    <owl:equivalentProperty rdf:resource="https://smartdatamodels.org/dataModel.Agrifood/hasOperator"/>
    <rdfs:isDefinedBy rdf:resource="http://foodie-cloud.com/model/foodie"/>
    <rdfs:comment>A Relation to the person(s) who has conducted an Intervention</rdfs:comment>
    <rdfs:label>operator</rdfs:label>
    <skos:prefLabel xml:lang="en">operator</skos:prefLabel>
    <rdfs:range rdf:resource="http://def.seegrid.csiro.au/isotc211/iso19115/2003/citation#ResponsibleParty"/>
    <rdf:type rdf:resource="http://www.w3.org/2002/07/owl#ObjectProperty"/>
  </rdf:Description>
  <rdf:Description rdf:nodeID="A3">
    <owl:onProperty rdf:resource="http://foodie-cloud.com/model/foodie#price"/>
    <owl:maxCardinality rdf:datatype="http://www.w3.org/2001/XMLSchema#int">1</owl:maxCardinality>
    <rdf:type rdf:resource="http://www.w3.org/2002/07/owl#Restriction"/>
  </rdf:Description>
  <rdf:Description rdf:nodeID="A4">
    <owl:onProperty rdf:resource="http://foodie-cloud.com/model/foodie#type"/>
    <owl:cardinality rdf:datatype="http://www.w3.org/2001/XMLSchema#int">1</owl:cardinality>
    <rdf:type rdf:resource="http://www.w3.org/2002/07/owl#Restriction"/>
  </rdf:Description>
  <rdf:Description rdf:nodeID="A5">
    <owl:onProperty rdf:resource="http://foodie-cloud.com/model/foodie#campaign"/>
    <owl:minCardinality rdf:datatype="http://www.w3.org/2001/XMLSchema#int">1</owl:minCardinality>
    <rdf:type rdf:resource="http://www.w3.org/2002/07/owl#Restriction"/>
  </rdf:Description>
  <rdf:Description rdf:about="http://foodie-cloud.com/model/foodie#status">
    <owl:equivalentProperty rdf:resource="https://uri.etsi.org/ngsi-ld/status"/>
    <rdfs:isDefinedBy rdf:resource="http://foodie-cloud.com/model/foodie"/>
    <rdfs:comment>Status of the intervention, e.g. approved, pending, completed as a free text</rdfs:comment>
    <rdfs:label>status</rdfs:label>
    <skos:prefLabel xml:lang="en">status</skos:prefLabel>
    <rdfs:range rdf:resource="http://www.w3.org/2001/XMLSchema#string"/>
    <rdf:type rdf:resource="http://www.w3.org/2002/07/owl#DatatypeProperty"/>
  </rdf:Description>
  <rdf:Description rdf:nodeID="A6">
    <owl:onProperty rdf:resource="http://foodie-cloud.com/model/foodie#interventionGeometry"/>
    <owl:minCardinality rdf:datatype="http://www.w3.org/2001/XMLSchema#int">1</owl:minCardinality>
    <rdf:type rdf:resource="http://www.w3.org/2002/07/owl#Restriction"/>
  </rdf:Description>
  <rdf:Description rdf:nodeID="A7">
    <owl:onProperty rdf:resource="http://foodie-cloud.com/model/foodie#minimumDose"/>
    <owl:maxCardinality rdf:datatype="http://www.w3.org/2001/XMLSchema#int">1</owl:maxCardinality>
    <rdf:type rdf:resource="http://www.w3.org/2002/07/owl#Restriction"/>
  </rdf:Description>
  <rdf:Description rdf:nodeID="A8">
    <owl:onProperty rdf:resource="http://foodie-cloud.com/model/foodie#quantity"/>
    <owl:cardinality rdf:datatype="http://www.w3.org/2001/XMLSchema#int">1</owl:cardinality>
    <rdf:type rdf:resource="http://www.w3.org/2002/07/owl#Restriction"/>
  </rdf:Description>
  <rdf:Description rdf:about="http://foodie-cloud.com/model/foodie#supervisor">
    <rdfs:isDefinedBy rdf:resource="http://foodie-cloud.com/model/foodie"/>
    <rdfs:comment>A Relation from Intervention to ResponsibleParty. ResponsibleParty contains the entity who carries out the intervention (a person or a body who has the power and authority to give instructions and guarantee the conducted Intervention)</rdfs:comment>
    <rdfs:label>supervisor</rdfs:label>
    <skos:prefLabel xml:lang="en">supervisor</skos:prefLabel>
    <rdfs:range rdf:resource="http://def.seegrid.csiro.au/isotc211/iso19115/2003/citation#ResponsibleParty"/>
    <rdf:type rdf:resource="http://www.w3.org/2002/07/owl#ObjectProperty"/>
  </rdf:Description>
  <rdf:Description rdf:nodeID="A9">
    <owl:onProperty rdf:resource="http://foodie-cloud.com/model/foodie#treatmentDescription"/>
    <owl:maxCardinality rdf:datatype="http://www.w3.org/2001/XMLSchema#int">1</owl:maxCardinality>
    <rdf:type rdf:resource="http://www.w3.org/2002/07/owl#Restriction"/>
  </rdf:Description>
  <rdf:Description rdf:about="http://foodie-cloud.com/model/foodie#creationDateTime">
    <rdfs:isDefinedBy rdf:resource="http://foodie-cloud.com/model/foodie"/>
    <rdfs:comment>date and time of the observed operation/intervention.</rdfs:comment>
    <rdfs:label>creationDateTime</rdfs:label>
    <skos:prefLabel xml:lang="en">creationDateTime</skos:prefLabel>
    <rdfs:range rdf:resource="http://www.w3.org/2001/XMLSchema#dateTime"/>
    <rdf:type rdf:resource="http://www.w3.org/2002/07/owl#DatatypeProperty"/>
  </rdf:Description>
  <rdf:Description rdf:nodeID="A10">
    <owl:onProperty rdf:resource="http://portele.de/ont/inspire/baseInspire#validFrom"/>
    <owl:cardinality rdf:datatype="http://www.w3.org/2001/XMLSchema#int">1</owl:cardinality>
    <rdf:type rdf:resource="http://www.w3.org/2002/07/owl#Restriction"/>
  </rdf:Description>
  <rdf:Description rdf:about="https://smartdatamodels.org/dataModel.Agrifood/endedAt">
    <rdfs:subPropertyOf rdf:resource="http://portele.de/ont/inspire/baseInspire#validTo"/>
    <rdfs:isDefinedBy rdf:resource="https://github.com/smart-data-models/dataModel.Agrifood/blob/master/AgriParcelOperation/schema.json"/>
    <rdfs:comment>Timestamp when the operation actually finished.</rdfs:comment>
    <rdfs:label xml:lang="en">endedAt</rdfs:label>
    <rdfs:range rdf:resource="http://www.w3.org/2001/XMLSchema#dateTime"/>
    <rdf:type rdf:resource="http://www.w3.org/2002/07/owl#DatatypeProperty"/>
  </rdf:Description>
  <rdf:Description rdf:nodeID="A11">
    <owl:onProperty rdf:resource="http://foodie-cloud.com/model/foodie#supervisor"/>
    <owl:maxCardinality rdf:datatype="http://www.w3.org/2001/XMLSchema#int">1</owl:maxCardinality>
    <rdf:type rdf:resource="http://www.w3.org/2002/07/owl#Restriction"/>
  </rdf:Description>
  <rdf:Description rdf:about="https://smartdatamodels.org/dataModel.Agrifood/quantity">
    <rdfs:isDefinedBy rdf:resource="https://github.com/smart-data-models/dataModel.Agrifood/blob/master/AgriParcelOperation/schema.json"/>
    <rdfs:comment>The total quantity of water or product used/ applied. It is recommended this is measured in litres for liquids or kilogrammes for solids.</rdfs:comment>
    <rdfs:label xml:lang="en">quantity</rdfs:label>
    <rdf:type rdf:resource="http://www.w3.org/2002/07/owl#DatatypeProperty"/>
  </rdf:Description>
  <rdf:Description rdf:nodeID="A12">
    <owl:onProperty rdf:resource="http://foodie-cloud.com/model/foodie#notes"/>
    <owl:maxCardinality rdf:datatype="http://www.w3.org/2001/XMLSchema#int">1</owl:maxCardinality>
    <rdf:type rdf:resource="http://www.w3.org/2002/07/owl#Restriction"/>
  </rdf:Description>
  <rdf:Description rdf:about="http://foodie-cloud.com/model/foodie#period">
    <rdfs:isDefinedBy rdf:resource="http://foodie-cloud.com/model/foodie"/>
    <rdfs:comment>A Relation from CampaignType to Period entity indicating the period to which the TreatmentPlan was designed. Typically a campaign may be an agronomical year or a season e.g. between 2015-03-01 and 2015-09-30</rdfs:comment>
    <rdfs:label>period</rdfs:label>
    <skos:prefLabel xml:lang="en">period</skos:prefLabel>
    <rdfs:range rdf:resource="http://def.seegrid.csiro.au/isotc211/iso19108/2002/temporal#Period"/>
    <rdf:type rdf:resource="http://www.w3.org/2002/07/owl#ObjectProperty"/>
  </rdf:Description>
  <rdf:Description rdf:nodeID="A13">
    <owl:onProperty rdf:resource="http://foodie-cloud.com/model/foodie#evidenceParty"/>
    <owl:minCardinality rdf:datatype="http://www.w3.org/2001/XMLSchema#int">1</owl:minCardinality>
    <rdf:type rdf:resource="http://www.w3.org/2002/07/owl#Restriction"/>
  </rdf:Description>
  <rdf:Description rdf:about="http://foodie-cloud.com/model/foodie#treatmentPlanCreation">
    <rdfs:isDefinedBy rdf:resource="http://foodie-cloud.com/model/foodie"/>
    <rdfs:comment>Date and time of the creation of the operation/intervention plan</rdfs:comment>
    <rdfs:label>treatmentPlanCreation</rdfs:label>
    <skos:prefLabel xml:lang="en">treatmentPlanCreation</skos:prefLabel>
    <rdfs:range rdf:resource="http://www.w3.org/2001/XMLSchema#dateTime"/>
    <rdf:type rdf:resource="http://www.w3.org/2002/07/owl#DatatypeProperty"/>
  </rdf:Description>
  <rdf:Description rdf:about="http://foodie-cloud.com/model/foodie#maximumDose">
    <rdfs:isDefinedBy rdf:resource="http://foodie-cloud.com/model/foodie"/>
    <rdfs:comment>A Relation from DoseUnit to Measure entity, indicating the maximumDose</rdfs:comment>
    <rdfs:label>maximumDose</rdfs:label>
    <skos:prefLabel xml:lang="en">maximumDose</skos:prefLabel>
    <rdfs:range rdf:resource="http://def.seegrid.csiro.au/isotc211/iso19103/2005/basic#Measure"/>
    <rdf:type rdf:resource="http://www.w3.org/2002/07/owl#ObjectProperty"/>
  </rdf:Description>
  <rdf:Description rdf:nodeID="A14">
    <foaf:name>OGC</foaf:name>
  </rdf:Description>
  <rdf:Description rdf:nodeID="A15">
    <foaf:name>Ioanna Roussaki</foaf:name>
    <schema:affiliation rdf:nodeID="A16"/>
  </rdf:Description>
  <rdf:Description rdf:about="http://foodie-cloud.com/model/foodie#CampaignType">
    <rdfs:isDefinedBy rdf:resource="http://foodie-cloud.com/model/foodie"/>
    <rdfs:comment>An entity defining the types of campaigns</rdfs:comment>
    <rdfs:label>CampaignType</rdfs:label>
    <skos:prefLabel xml:lang="en">CampaignType</skos:prefLabel>
    <rdfs:subClassOf rdf:nodeID="A17"/>
    <rdf:type rdf:resource="http://www.w3.org/2002/07/owl#Class"/>
  </rdf:Description>
  <rdf:Description rdf:about="http://foodie-cloud.com/model/foodie#treatmentPurpose">
    <rdfs:isDefinedBy rdf:resource="http://foodie-cloud.com/model/foodie"/>
    <rdfs:comment>A Relation from Treatment to TreatmentPurposeValue codelist, e.g., disease, fertilization, pest, weed</rdfs:comment>
    <rdfs:label>treatmentPurpose</rdfs:label>
    <skos:prefLabel xml:lang="en">treatmentPurpose</skos:prefLabel>
    <rdfs:range rdf:resource="http://foodie-cloud.com/model/foodie#TreatmentPurposeValue"/>
    <rdf:type rdf:resource="http://www.w3.org/2002/07/owl#ObjectProperty"/>
  </rdf:Description>
  <rdf:Description rdf:nodeID="A16">
    <foaf:name>ICCS</foaf:name>
  </rdf:Description>
  <rdf:Description rdf:about="https://smartdatamodels.org/dataModel.Agrifood/hasAgriParcel">
    <rdfs:isDefinedBy rdf:resource="https://github.com/smart-data-models/dataModel.Agrifood/blob/master/AgriParcelOperation/schema.json"/>
    <rdfs:comment>Reference to the AgriParcel to which this entity relates.</rdfs:comment>
    <rdfs:label xml:lang="en">operationHasAgriParcel</rdfs:label>
    <rdf:type rdf:resource="http://www.w3.org/2002/07/owl#ObjectProperty"/>
  </rdf:Description>
  <rdf:Description rdf:nodeID="A18">
    <owl:onProperty rdf:resource="http://foodie-cloud.com/model/foodie#treatmentPlanCode"/>
    <owl:maxCardinality rdf:datatype="http://www.w3.org/2001/XMLSchema#int">1</owl:maxCardinality>
    <rdf:type rdf:resource="http://www.w3.org/2002/07/owl#Restriction"/>
  </rdf:Description>
  <rdf:Description rdf:about="http://foodie-cloud.com/model/foodie#treatmentProduct">
    <owl:equivalentProperty rdf:resource="https://smartdatamodels.org/dataModel.Agrifood/hasAgriProductType"/>
    <rdfs:isDefinedBy rdf:resource="http://foodie-cloud.com/model/foodie"/>
    <rdfs:comment>A Relation from Treatment to Product entity.</rdfs:comment>
    <rdfs:label>treatmentProduct</rdfs:label>
    <skos:prefLabel xml:lang="en">treatmentProduct</skos:prefLabel>
    <rdfs:range rdf:resource="http://foodie-cloud.com/model/foodie#Product"/>
    <rdf:type rdf:resource="http://www.w3.org/2002/07/owl#ObjectProperty"/>
  </rdf:Description>
  <rdf:Description rdf:about="http://foodie-cloud.com/model/foodie#flowAdjustment">
    <rdfs:isDefinedBy rdf:resource="http://foodie-cloud.com/model/foodie"/>
    <rdfs:comment>A Relation from Treatment to Measure entity, indicating whether a flow adjustment was needed for the application of the Treatment, be expressed together with its unit </rdfs:comment>
    <rdfs:label>flowAdjustment</rdfs:label>
    <skos:prefLabel xml:lang="en">flowAdjustment</skos:prefLabel>
    <rdfs:range rdf:resource="http://def.seegrid.csiro.au/isotc211/iso19103/2005/basic#Measure"/>
    <rdf:type rdf:resource="http://www.w3.org/2002/07/owl#ObjectProperty"/>
  </rdf:Description>
  <rdf:Description rdf:about="http://foodie-cloud.com/model/foodie#treatmentPlanCode">
    <rdfs:isDefinedBy rdf:resource="http://foodie-cloud.com/model/foodie"/>
    <rdfs:comment>Identification code of the observed operation/intervention.</rdfs:comment>
    <rdfs:label>treatmentPlanCode</rdfs:label>
    <skos:prefLabel xml:lang="en">treatmentPlanCode</skos:prefLabel>
    <rdfs:range rdf:resource="http://www.w3.org/2001/XMLSchema#string"/>
    <rdf:type rdf:resource="http://www.w3.org/2002/07/owl#DatatypeProperty"/>
  </rdf:Description>
  <rdf:Description rdf:nodeID="A19">
    <owl:onProperty rdf:resource="http://portele.de/ont/inspire/baseInspire#validTo"/>
    <owl:maxCardinality rdf:datatype="http://www.w3.org/2001/XMLSchema#int">1</owl:maxCardinality>
    <rdf:type rdf:resource="http://www.w3.org/2002/07/owl#Restriction"/>
  </rdf:Description>
  <rdf:Description rdf:nodeID="A20">
    <owl:onProperty rdf:resource="http://foodie-cloud.com/model/foodie#creationDateTime"/>
    <owl:cardinality rdf:datatype="http://www.w3.org/2001/XMLSchema#int">1</owl:cardinality>
    <rdf:type rdf:resource="http://www.w3.org/2002/07/owl#Restriction"/>
  </rdf:Description>
  <rdf:Description rdf:about="http://foodie-cloud.com/model/foodie#TreatmentPurposeValue">
    <rdfs:isDefinedBy rdf:resource="http://foodie-cloud.com/model/foodie"/>
    <rdfs:comment>An entity defining the purpose of an Intervention/Treatment as codelist, e.g., disease (i.e. a pathological condition that affects part or all of production in the Plot), fertilization (i.e. a need to apply a fertilizer to soil), pest (i.e. a plant or animal detrimental to a human), weed (i.e. to reduce plants considered undesirable in a particular situation)</rdfs:comment>
    <rdfs:label>TreatmentPurposeValue</rdfs:label>
    <skos:prefLabel xml:lang="en">TreatmentPurposeValue</skos:prefLabel>
    <rdfs:subClassOf rdf:resource="http://www.w3.org/2004/02/skos/core#Concept"/>
    <rdf:type rdf:resource="http://www.w3.org/2002/07/owl#Class"/>
  </rdf:Description>
  <rdf:Description rdf:nodeID="A21">
    <foaf:name>Raul Palma</foaf:name>
    <rdfs:seeAlso rdf:resource="http://orcid.org/0000-0003-4289-4922"/>
    <schema:affiliation rdf:nodeID="A22"/>
  </rdf:Description>
  <rdf:Description rdf:nodeID="A23">
    <foaf:name>DEMETER project</foaf:name>
    <foaf:homepage rdf:resource="https://h2020-demeter.eu/"/>
  </rdf:Description>
  <rdf:Description rdf:nodeID="A24">
    <owl:onProperty rdf:resource="http://foodie-cloud.com/model/foodie#areaDose"/>
    <owl:maxCardinality rdf:datatype="http://www.w3.org/2001/XMLSchema#int">1</owl:maxCardinality>
    <rdf:type rdf:resource="http://www.w3.org/2002/07/owl#Restriction"/>
  </rdf:Description>
  <rdf:Description rdf:nodeID="A25">
    <owl:onProperty rdf:resource="http://foodie-cloud.com/model/foodie#flowAdjustment"/>
    <owl:maxCardinality rdf:datatype="http://www.w3.org/2001/XMLSchema#int">1</owl:maxCardinality>
    <rdf:type rdf:resource="http://www.w3.org/2002/07/owl#Restriction"/>
  </rdf:Description>
  <rdf:Description rdf:about="https://smartdatamodels.org/dataModel.Agrifood/operationType">
    <rdfs:subPropertyOf rdf:resource="http://foodie-cloud.com/model/foodie#type"/>
    <rdfs:isDefinedBy rdf:resource="https://github.com/smart-data-models/dataModel.Agrifood/blob/master/AgriParcelOperation/schema.json"/>
    <rdfs:comment>A choice from an enumerated list describing the operation performed on the parcel. One of: fertiliser, inspection, pesticide, water, other.</rdfs:comment>
    <rdfs:label xml:lang="en">operationType</rdfs:label>
    <rdf:type rdf:resource="http://www.w3.org/2002/07/owl#DatatypeProperty"/>
  </rdf:Description>
  <rdf:Description rdf:about="http://foodie-cloud.com/model/foodie#interventionPlot">
    <owl:equivalentProperty rdf:resource="https://smartdatamodels.org/dataModel.Agrifood/hasAgriParcel"/>
    <rdfs:isDefinedBy rdf:resource="http://foodie-cloud.com/model/foodie"/>
    <rdfs:comment>A Relation from Intervention to Plot. A plot can have few intervetions.</rdfs:comment>
    <rdfs:label>interventionPlot</rdfs:label>
    <skos:prefLabel xml:lang="en">interventionPlot</skos:prefLabel>
    <rdfs:range rdf:resource="http://foodie-cloud.com/model/foodie#Plot"/>
    <rdf:type rdf:resource="http://www.w3.org/2002/07/owl#ObjectProperty"/>
  </rdf:Description>
  <rdf:Description rdf:nodeID="A26">
    <owl:onProperty rdf:resource="http://foodie-cloud.com/model/foodie#type"/>
    <owl:cardinality rdf:datatype="http://www.w3.org/2001/XMLSchema#int">1</owl:cardinality>
    <rdf:type rdf:resource="http://www.w3.org/2002/07/owl#Restriction"/>
  </rdf:Description>
  <rdf:Description rdf:about="http://foodie-cloud.com/model/foodie#DoseUnit">
    <rdfs:isDefinedBy rdf:resource="http://foodie-cloud.com/model/foodie"/>
    <rdfs:comment>An entity defining the Doses for operation/intervention</rdfs:comment>
    <rdfs:label>DoseUnit</rdfs:label>
    <skos:prefLabel xml:lang="en">DoseUnit</skos:prefLabel>
    <rdfs:subClassOf rdf:nodeID="A27"/>
    <rdfs:subClassOf rdf:nodeID="A7"/>
    <rdf:type rdf:resource="http://www.w3.org/2002/07/owl#Class"/>
  </rdf:Description>
  <rdf:Description rdf:about="http://foodie-cloud.com/model/foodie#pressure">
    <rdfs:isDefinedBy rdf:resource="http://foodie-cloud.com/model/foodie"/>
    <rdfs:comment>A Relation from Treatment to Measure entity, indicating the recommended pressure for the application of the Treatment that should be expressed together with its unit</rdfs:comment>
    <rdfs:label>pressure</rdfs:label>
    <skos:prefLabel xml:lang="en">pressure</skos:prefLabel>
    <rdfs:range rdf:resource="http://def.seegrid.csiro.au/isotc211/iso19103/2005/basic#Measure"/>
    <rdf:type rdf:resource="http://www.w3.org/2002/07/owl#ObjectProperty"/>
  </rdf:Description>
  <rdf:Description rdf:nodeID="A28">
    <owl:onProperty rdf:resource="http://foodie-cloud.com/model/foodie#interventionPlot"/>
    <owl:maxCardinality rdf:datatype="http://www.w3.org/2001/XMLSchema#int">1</owl:maxCardinality>
    <rdf:type rdf:resource="http://www.w3.org/2002/07/owl#Restriction"/>
  </rdf:Description>
  <rdf:Description rdf:nodeID="A29">
    <owl:onProperty rdf:resource="http://foodie-cloud.com/model/foodie#description"/>
    <owl:cardinality rdf:datatype="http://www.w3.org/2001/XMLSchema#int">1</owl:cardinality>
    <rdf:type rdf:resource="http://www.w3.org/2002/07/owl#Restriction"/>
  </rdf:Description>
  <rdf:Description rdf:nodeID="A30">
    <owl:onProperty rdf:resource="http://foodie-cloud.com/model/foodie#treatmentProduct"/>
    <owl:minCardinality rdf:datatype="http://www.w3.org/2001/XMLSchema#int">1</owl:minCardinality>
    <rdf:type rdf:resource="http://www.w3.org/2002/07/owl#Restriction"/>
  </rdf:Description>
  <rdf:Description rdf:nodeID="A31">
    <owl:onProperty rdf:resource="http://foodie-cloud.com/model/foodie#formOfTreatment"/>
    <owl:cardinality rdf:datatype="http://www.w3.org/2001/XMLSchema#int">1</owl:cardinality>
    <rdf:type rdf:resource="http://www.w3.org/2002/07/owl#Restriction"/>
  </rdf:Description>
  <rdf:Description rdf:nodeID="A27">
    <owl:onProperty rdf:resource="http://foodie-cloud.com/model/foodie#maximumDose"/>
    <owl:maxCardinality rdf:datatype="http://www.w3.org/2001/XMLSchema#int">1</owl:maxCardinality>
    <rdf:type rdf:resource="http://www.w3.org/2002/07/owl#Restriction"/>
  </rdf:Description>
  <rdf:Description rdf:nodeID="A32">
    <owl:onProperty rdf:resource="http://foodie-cloud.com/model/foodie#pressure"/>
    <owl:maxCardinality rdf:datatype="http://www.w3.org/2001/XMLSchema#int">1</owl:maxCardinality>
    <rdf:type rdf:resource="http://www.w3.org/2002/07/owl#Restriction"/>
  </rdf:Description>
  <rdf:Description rdf:about="http://foodie-cloud.com/model/foodie#campaign">
    <rdfs:isDefinedBy rdf:resource="http://foodie-cloud.com/model/foodie"/>
    <rdfs:comment>A Relation from TreatmentPlan to CampaignType entity including the period to which the TreatmentPlan was designed</rdfs:comment>
    <rdfs:label>planProduct</rdfs:label>
    <skos:prefLabel xml:lang="en">campaign</skos:prefLabel>
    <rdfs:range rdf:resource="http://foodie-cloud.com/model/foodie#CampaignType"/>
    <rdf:type rdf:resource="http://www.w3.org/2002/07/owl#ObjectProperty"/>
  </rdf:Description>
  <rdf:Description rdf:about="http://foodie-cloud.com/model/foodie#Treatment">
    <rdfs:subClassOf rdf:resource="http://www.opengis.net/ont/geosparql#Feature"/>
    <owl:equivalentClass rdf:resource="https://smartdatamodels.org/dataModel.Agrifood/AgriParcelOperation"/>
    <rdfs:subClassOf rdf:nodeID="A32"/>
    <rdfs:subClassOf rdf:nodeID="A33"/>
    <rdfs:label>Treatment</rdfs:label>
    <rdfs:subClassOf rdf:nodeID="A31"/>
    <rdfs:subClassOf rdf:nodeID="A24"/>
    <rdfs:subClassOf rdf:nodeID="A3"/>
    <rdfs:subClassOf rdf:nodeID="A8"/>
    <rdfs:comment>An entity defining the attributes of Treatments</rdfs:comment>
    <skos:prefLabel xml:lang="en">Treatment</skos:prefLabel>
    <rdfs:subClassOf rdf:resource="http://foodie-cloud.com/model/foodie#Intervention"/>
    <rdfs:isDefinedBy rdf:resource="http://foodie-cloud.com/model/foodie"/>
    <rdfs:subClassOf rdf:nodeID="A34"/>
    <rdfs:subClassOf rdf:nodeID="A25"/>
    <rdfs:subClassOf rdf:nodeID="A35"/>
    <rdfs:subClassOf rdf:nodeID="A9"/>
    <rdf:type rdf:resource="http://www.w3.org/2002/07/owl#Class"/>
    <rdfs:subClassOf rdf:nodeID="A30"/>
  </rdf:Description>
  <rdf:Description rdf:about="https://smartdatamodels.org/dataModel.Agrifood/result">
    <rdfs:subPropertyOf rdf:resource="http://foodie-cloud.com/model/foodie#notes"/>
    <rdfs:isDefinedBy rdf:resource="https://github.com/smart-data-models/dataModel.Agrifood/blob/master/AgriParcelOperation/schema.json"/>
    <rdfs:comment>A description of the results of the operation. One of: ok, aborted, failed.</rdfs:comment>
    <rdfs:label xml:lang="en">result</rdfs:label>
    <rdf:type rdf:resource="http://www.w3.org/2002/07/owl#DatatypeProperty"/>
  </rdf:Description>
  <rdf:Description rdf:about="http://foodie-cloud.com/model/foodie#plan">
    <rdfs:isDefinedBy rdf:resource="http://foodie-cloud.com/model/foodie"/>
    <rdfs:comment>A Relation from Treatment to TreatmentPlan entity.</rdfs:comment>
    <rdfs:label>plan</rdfs:label>
    <skos:prefLabel xml:lang="en">plan</skos:prefLabel>
    <rdfs:range rdf:resource="http://foodie-cloud.com/model/foodie#TreatmentPlan"/>
    <rdf:type rdf:resource="http://www.w3.org/2002/07/owl#ObjectProperty"/>
  </rdf:Description>
  <rdf:Description rdf:about="http://foodie-cloud.com/model/foodie#formOfTreatment">
    <rdfs:isDefinedBy rdf:resource="http://foodie-cloud.com/model/foodie"/>
    <rdfs:comment>A Relation from Treatment to FormOfTreatmentValue codelist, e.g., manual (i.e. conducted manually by a person), applicationMachine (i.e. automatic or semi-automatic application by a machine), aerial (i.e. aerial application from an airplane);</rdfs:comment>
    <rdfs:label>formOfTreatment</rdfs:label>
    <skos:prefLabel xml:lang="en">formOfTreatment</skos:prefLabel>
    <rdfs:range rdf:resource="http://foodie-cloud.com/model/foodie#FormOfTreatmentValue"/>
    <rdf:type rdf:resource="http://www.w3.org/2002/07/owl#ObjectProperty"/>
  </rdf:Description>
  <rdf:Description rdf:about="https://smartdatamodels.org/dataModel.Agrifood/waterSource">
    <rdfs:isDefinedBy rdf:resource="https://github.com/smart-data-models/dataModel.Agrifood/blob/master/AgriParcelOperation/schema.json"/>
    <rdfs:comment>Type of water sources. One of: borehole, rainfall, river, rainwater capture, water dam, commercial supply.</rdfs:comment>
    <rdfs:label xml:lang="en">waterSource</rdfs:label>
    <rdf:type rdf:resource="http://www.w3.org/2002/07/owl#DatatypeProperty"/>
  </rdf:Description>
  <rdf:Description rdf:about="http://foodie-cloud.com/model/foodie#FormOfTreatmentValue">
    <rdfs:isDefinedBy rdf:resource="http://foodie-cloud.com/model/foodie"/>
    <rdfs:comment>An entity defining the form of Intervention/Treatment as codelist, e.g., manual (i.e. conducted manually by a person), applicationMachine (i.e. automatic or semi-automatic application by a machine), aerial (i.e. aerial application from an airplane)</rdfs:comment>
    <rdfs:label>FormOfTreatmentValue</rdfs:label>
    <skos:prefLabel xml:lang="en">FormOfTreatmentValue</skos:prefLabel>
    <rdfs:subClassOf rdf:resource="http://www.w3.org/2004/02/skos/core#Concept"/>
    <rdf:type rdf:resource="http://www.w3.org/2002/07/owl#Class"/>
  </rdf:Description>
  <rdf:Description rdf:about="https://smartdatamodels.org/dataModel.Agrifood/irrigationRecord">
    <rdfs:isDefinedBy rdf:resource="https://github.com/smart-data-models/dataModel.Agrifood/blob/master/AgriParcelOperation/schema.json"/>
    <rdfs:comment>Relationship with the irrigation record of the execution</rdfs:comment>
    <rdfs:label xml:lang="en">irrigationRecord</rdfs:label>
    <rdf:type rdf:resource="http://www.w3.org/2002/07/owl#DatatypeProperty"/>
  </rdf:Description>
  <rdf:Description rdf:nodeID="A35">
    <owl:onProperty rdf:resource="http://foodie-cloud.com/model/foodie#motionSpeed"/>
    <owl:maxCardinality rdf:datatype="http://www.w3.org/2001/XMLSchema#int">1</owl:maxCardinality>
    <rdf:type rdf:resource="http://www.w3.org/2002/07/owl#Restriction"/>
  </rdf:Description>
  <rdf:Description rdf:about="http://foodie-cloud.com/model/foodie#applicationWidth">
    <rdfs:isDefinedBy rdf:resource="http://foodie-cloud.com/model/foodie"/>
    <rdfs:comment>A Relation from Treatment to Measure entity, indicating a width in which a machine is capable to apply the Treatment, expressed together with its unit</rdfs:comment>
    <rdfs:label>flowAdjustment</rdfs:label>
    <skos:prefLabel xml:lang="en">applicationWidth</skos:prefLabel>
    <rdfs:range rdf:resource="http://def.seegrid.csiro.au/isotc211/iso19103/2005/basic#Measure"/>
    <rdf:type rdf:resource="http://www.w3.org/2002/07/owl#ObjectProperty"/>
  </rdf:Description>
  <rdf:Description rdf:about="https://smartdatamodels.org/dataModel.Agrifood/startedAt">
    <rdfs:subPropertyOf rdf:resource="http://portele.de/ont/inspire/baseInspire#validFrom"/>
    <rdfs:isDefinedBy rdf:resource="https://github.com/smart-data-models/dataModel.Agrifood/blob/master/AgriParcelOperation/schema.json"/>
    <rdfs:comment>Timestamp when the operation actually started to be performed.</rdfs:comment>
    <rdfs:label xml:lang="en">startedAt</rdfs:label>
    <rdfs:range rdf:resource="http://www.w3.org/2001/XMLSchema#dateTime"/>
    <rdf:type rdf:resource="http://www.w3.org/2002/07/owl#DatatypeProperty"/>
  </rdf:Description>
  <rdf:Description rdf:about="https://smartdatamodels.org/dataModel.Agrifood/plannedStartAt">
    <rdfs:isDefinedBy rdf:resource="https://github.com/smart-data-models/dataModel.Agrifood/blob/master/AgriParcelOperation/schema.json"/>
    <rdfs:comment>The planned start date/timestamp for the operation. Note that this is advisory and the actual time the operation starts may be before or after the planned start.</rdfs:comment>
    <rdfs:label xml:lang="en">plannedStartAt</rdfs:label>
    <rdfs:range rdf:resource="http://www.w3.org/2001/XMLSchema#dateTime"/>
    <rdf:type rdf:resource="http://www.w3.org/2002/07/owl#DatatypeProperty"/>
  </rdf:Description>
  <rdf:Description rdf:about="https://w3id.org/demeter/agri/agriIntervention">
    <dct:contributor rdf:nodeID="A36"/>
    <dct:contributor rdf:nodeID="A15"/>
    <dct:description xml:lang="en">The DEMETER AgriIntervention is one of the agri profiles of DEMETER AIM. This profile was created by reusing and aligning well-known ontologies and vocabularies</dct:description>
    <dct:creator rdf:nodeID="A21"/>
    <rdfs:label xml:lang="en">DEMETER AgriIntervention</rdfs:label>
    <owl:versionInfo>3.0</owl:versionInfo>
    <rdfs:comment xml:lang="en">The DEMETER Agriculture Information Model (AIM) is the common vocabulary in DEMETER project providing the basis for semantic interoperability across smart farming solutions</rdfs:comment>
    <owl:imports rdf:resource="https://w3id.org/demeter/agri/agriCommon"/>
    <rdf:type rdf:resource="http://www.w3.org/2002/07/owl#Ontology"/>
    <owl:versionIRI rdf:resource="https://w3id.org/demeter/agri/agriIntervention/3.0"/>
    <foaf:maker rdf:nodeID="A23"/>
    <dct:title xml:lang="en">DEMETER AgriIntervention</dct:title>
    <dct:rights xml:lang="en">This vocabulary is distributed under Creative Commons Attribution 4.0 License - http://creativecommons.org/licenses/by/4.0</dct:rights>
  </rdf:Description>
  <rdf:Description rdf:about="http://foodie-cloud.com/model/foodie#interventionZone">
    <rdfs:isDefinedBy rdf:resource="http://foodie-cloud.com/model/foodie"/>
    <rdfs:comment>A Relation from Intervention to ManagementZone.</rdfs:comment>
    <rdfs:label>interventionZone</rdfs:label>
    <skos:prefLabel xml:lang="en">interventionZone</skos:prefLabel>
    <rdfs:range rdf:resource="http://foodie-cloud.com/model/foodie#ManagementZone"/>
    <rdf:type rdf:resource="http://www.w3.org/2002/07/owl#ObjectProperty"/>
  </rdf:Description>
  <rdf:Description rdf:about="http://foodie-cloud.com/model/foodie#motionSpeed">
    <rdfs:isDefinedBy rdf:resource="http://foodie-cloud.com/model/foodie"/>
    <rdfs:comment>A Relation from Treatment to Measure entity, indicating recommended speed for the application of the treatment that should be expressed together with its unit</rdfs:comment>
    <rdfs:label>motionSpeed</rdfs:label>
    <skos:prefLabel xml:lang="en">motionSpeed</skos:prefLabel>
    <rdfs:range rdf:resource="http://def.seegrid.csiro.au/isotc211/iso19103/2005/basic#Measure"/>
    <rdf:type rdf:resource="http://www.w3.org/2002/07/owl#ObjectProperty"/>
  </rdf:Description>
  <rdf:Description rdf:about="http://foodie-cloud.com/model/foodie#evidenceParty">
    <rdfs:isDefinedBy rdf:resource="http://foodie-cloud.com/model/foodie"/>
    <rdfs:comment>A Relation to a person or a body who inserted the Intervention into the database</rdfs:comment>
    <rdfs:label>evidenceParty</rdfs:label>
    <skos:prefLabel xml:lang="en">evidenceParty</skos:prefLabel>
    <rdfs:range rdf:resource="http://def.seegrid.csiro.au/isotc211/iso19115/2003/citation#ResponsibleParty"/>
    <rdf:type rdf:resource="http://www.w3.org/2002/07/owl#ObjectProperty"/>
  </rdf:Description>
  <rdf:Description rdf:about="http://foodie-cloud.com/model/foodie#treatmentDescription">
    <rdfs:isDefinedBy rdf:resource="http://foodie-cloud.com/model/foodie"/>
    <rdfs:comment>Description of the observed operation/intervention.</rdfs:comment>
    <rdfs:label>treatmentDescription</rdfs:label>
    <skos:prefLabel xml:lang="en">treatmentDescription</skos:prefLabel>
    <rdfs:range rdf:resource="http://www.w3.org/2001/XMLSchema#string"/>
    <rdf:type rdf:resource="http://www.w3.org/2002/07/owl#DatatypeProperty"/>
  </rdf:Description>
  <rdf:Description rdf:about="http://foodie-cloud.com/model/foodie#Intervention">
    <rdfs:subClassOf rdf:nodeID="A26"/>
    <rdf:type rdf:resource="http://www.w3.org/2002/07/owl#Class"/>
    <rdfs:subClassOf rdf:nodeID="A37"/>
    <rdfs:isDefinedBy rdf:resource="http://foodie-cloud.com/model/foodie"/>
    <rdfs:subClassOf rdf:nodeID="A2"/>
    <rdfs:subClassOf rdf:nodeID="A13"/>
    <rdfs:subClassOf rdf:nodeID="A11"/>
    <rdfs:subClassOf rdf:nodeID="A10"/>
    <skos:prefLabel xml:lang="en">Intervention</skos:prefLabel>
    <rdfs:subClassOf rdf:nodeID="A6"/>
    <rdfs:subClassOf rdf:resource="http://www.opengis.net/ont/geosparql#Feature"/>
    <rdfs:subClassOf rdf:nodeID="A28"/>
    <rdfs:subClassOf rdf:nodeID="A19"/>
    <rdfs:comment>An entity of operation or intervention.</rdfs:comment>
    <rdfs:subClassOf rdf:nodeID="A1"/>
    <rdfs:subClassOf rdf:nodeID="A20"/>
    <rdfs:label>Intervention</rdfs:label>
    <rdfs:subClassOf rdf:nodeID="A12"/>
  </rdf:Description>
  <rdf:Description rdf:about="https://smartdatamodels.org/dataModel.Agrifood/AgriParcelOperation">
    <rdfs:isDefinedBy rdf:resource="https://github.com/smart-data-models/dataModel.Agrifood/blob/master/AgriParcelOperation/schema.json"/>
    <rdfs:comment>This entity contains a harmonised description of a generic operations performed on a parcel of land. This entity is primarily associated with the agricultural vertical and related IoT applications.</rdfs:comment>
    <rdfs:label>AgriParcelOperation</rdfs:label>
    <rdf:type rdf:resource="http://www.w3.org/2002/07/owl#Class"/>
  </rdf:Description>
  <rdf:Description rdf:nodeID="A34">
    <owl:onProperty rdf:resource="http://foodie-cloud.com/model/foodie#applicationWidth"/>
    <owl:maxCardinality rdf:datatype="http://www.w3.org/2001/XMLSchema#int">1</owl:maxCardinality>
    <rdf:type rdf:resource="http://www.w3.org/2002/07/owl#Restriction"/>
  </rdf:Description>
  <rdf:Description rdf:about="https://smartdatamodels.org/dataModel.Agrifood/reportedAt">
    <rdfs:isDefinedBy rdf:resource="https://github.com/smart-data-models/dataModel.Agrifood/blob/master/AgriParcelOperation/schema.json"/>
    <rdfs:comment>Timestamp when the event/ fault was reported.</rdfs:comment>
    <rdfs:label xml:lang="en">reportedAt</rdfs:label>
    <rdfs:range rdf:resource="http://www.w3.org/2001/XMLSchema#dateTime"/>
    <rdf:type rdf:resource="http://www.w3.org/2002/07/owl#DatatypeProperty"/>
  </rdf:Description>
  <rdf:Description rdf:nodeID="A38">
    <owl:onProperty rdf:resource="http://foodie-cloud.com/model/foodie#planProduct"/>
    <owl:minCardinality rdf:datatype="http://www.w3.org/2001/XMLSchema#int">1</owl:minCardinality>
    <rdf:type rdf:resource="http://www.w3.org/2002/07/owl#Restriction"/>
  </rdf:Description>
  <rdf:Description rdf:about="http://foodie-cloud.com/model/foodie#areaDose">
    <rdfs:isDefinedBy rdf:resource="http://foodie-cloud.com/model/foodie"/>
    <rdfs:comment>A Relation from Treatment to DoseUnit entity, indicating the minimum and maximum application rate of the Treatment together with their unit</rdfs:comment>
    <rdfs:label>areaDose</rdfs:label>
    <skos:prefLabel xml:lang="en">areaDose</skos:prefLabel>
    <rdfs:range rdf:resource="http://foodie-cloud.com/model/foodie#DoseUnit"/>
    <rdf:type rdf:resource="http://www.w3.org/2002/07/owl#ObjectProperty"/>
  </rdf:Description>
  <rdf:Description rdf:about="https://smartdatamodels.org/dataModel.Agrifood/plannedEndAt">
    <rdfs:isDefinedBy rdf:resource="https://github.com/smart-data-models/dataModel.Agrifood/blob/master/AgriParcelOperation/schema.json"/>
    <rdfs:comment>The planned end date/timestamp for the operation. Note that this is advisory and the actual time the operation finishes may be before or after the planned end.</rdfs:comment>
    <rdfs:label xml:lang="en">plannedEndAt</rdfs:label>
    <rdfs:range rdf:resource="http://www.w3.org/2001/XMLSchema#dateTime"/>
    <rdf:type rdf:resource="http://www.w3.org/2002/07/owl#DatatypeProperty"/>
  </rdf:Description>
  <rdf:Description rdf:about="http://foodie-cloud.com/model/foodie#planProduct">
    <rdfs:isDefinedBy rdf:resource="http://foodie-cloud.com/model/foodie"/>
    <rdfs:comment>A Relation from TreatmentPlan to Product entity.</rdfs:comment>
    <rdfs:label>planProduct</rdfs:label>
    <skos:prefLabel xml:lang="en">planProduct</skos:prefLabel>
    <rdfs:range rdf:resource="http://foodie-cloud.com/model/foodie#Product"/>
    <rdf:type rdf:resource="http://www.w3.org/2002/07/owl#ObjectProperty"/>
  </rdf:Description>
  <rdf:Description rdf:nodeID="A22">
    <foaf:name>PSNC</foaf:name>
  </rdf:Description>
  <rdf:Description rdf:nodeID="A36">
    <foaf:name>Rob Atkinson</foaf:name>
    <schema:affiliation rdf:nodeID="A14"/>
  </rdf:Description>
  <rdf:Description rdf:nodeID="A37">
    <owl:onProperty rdf:resource="http://foodie-cloud.com/model/foodie#description"/>
    <owl:cardinality rdf:datatype="http://www.w3.org/2001/XMLSchema#int">1</owl:cardinality>
    <rdf:type rdf:resource="http://www.w3.org/2002/07/owl#Restriction"/>
  </rdf:Description>
  <rdf:Description rdf:about="https://uri.etsi.org/ngsi-ld/status">
    <rdfs:isDefinedBy rdf:resource="https://uri.etsi.org/ngsi-ld/v1/ngsi-ld-core-context-v1.6.jsonld"/>
    <rdfs:comment>A choice from an enumerated list describing the status. One of: planned, ongoing, finished, scheduled, cancelled.</rdfs:comment>
    <rdfs:label xml:lang="en">status</rdfs:label>
    <rdf:type rdf:resource="http://www.w3.org/2002/07/owl#DatatypeProperty"/>
  </rdf:Description>
  <rdf:Description rdf:about="http://foodie-cloud.com/model/foodie#quantity">
    <owl:equivalentProperty rdf:resource="https://smartdatamodels.org/dataModel.Agrifood/quantity"/>
    <rdfs:isDefinedBy rdf:resource="http://foodie-cloud.com/model/foodie"/>
    <rdfs:comment>A Relation from Treatment to Measure entity, indicating the value of a physical quantity of applied Treatment, together with its unit.</rdfs:comment>
    <rdfs:label>quantity</rdfs:label>
    <skos:prefLabel xml:lang="en">quantity</skos:prefLabel>
    <rdfs:range rdf:resource="http://def.seegrid.csiro.au/isotc211/iso19103/2005/basic#Measure"/>
    <rdf:type rdf:resource="http://www.w3.org/2002/07/owl#ObjectProperty"/>
  </rdf:Description>
  <rdf:Description rdf:nodeID="A33">
    <owl:onProperty rdf:resource="http://foodie-cloud.com/model/foodie#plan"/>
    <owl:maxCardinality rdf:datatype="http://www.w3.org/2001/XMLSchema#int">1</owl:maxCardinality>
    <rdf:type rdf:resource="http://www.w3.org/2002/07/owl#Restriction"/>
  </rdf:Description>
  <rdf:Description rdf:nodeID="A39">
    <owl:onProperty rdf:resource="http://foodie-cloud.com/model/foodie#notes"/>
    <owl:maxCardinality rdf:datatype="http://www.w3.org/2001/XMLSchema#int">1</owl:maxCardinality>
    <rdf:type rdf:resource="http://www.w3.org/2002/07/owl#Restriction"/>
  </rdf:Description>
  <rdf:Description rdf:about="http://foodie-cloud.com/model/foodie#TreatmentPlan">
    <rdfs:subClassOf rdf:nodeID="A39"/>
    <rdfs:subClassOf rdf:nodeID="A0"/>
    <rdf:type rdf:resource="http://www.w3.org/2002/07/owl#Class"/>
    <rdfs:subClassOf rdf:nodeID="A5"/>
    <rdfs:subClassOf rdf:resource="http://www.opengis.net/ont/geosparql#Feature"/>
    <rdfs:subClassOf rdf:nodeID="A38"/>
    <rdfs:label>TreatmentPlan</rdfs:label>
    <rdfs:comment>An entity defining the Treatment plans</rdfs:comment>
    <rdfs:isDefinedBy rdf:resource="http://foodie-cloud.com/model/foodie"/>
    <rdfs:subClassOf rdf:nodeID="A29"/>
    <rdfs:subClassOf rdf:nodeID="A4"/>
    <skos:prefLabel xml:lang="en">TreatmentPlan</skos:prefLabel>
    <rdfs:subClassOf rdf:nodeID="A18"/>
  </rdf:Description>
  <rdf:Description rdf:about="http://foodie-cloud.com/model/foodie#minimumDose">
    <rdfs:isDefinedBy rdf:resource="http://foodie-cloud.com/model/foodie"/>
    <rdfs:comment>A Relation from DoseUnit to Measure entity, indicating the minimuDose</rdfs:comment>
    <rdfs:label>minimumDose</rdfs:label>
    <skos:prefLabel xml:lang="en">minimumDose</skos:prefLabel>
    <rdfs:range rdf:resource="http://def.seegrid.csiro.au/isotc211/iso19103/2005/basic#Measure"/>
    <rdf:type rdf:resource="http://www.w3.org/2002/07/owl#ObjectProperty"/>
  </rdf:Description>
  <rdf:Description rdf:nodeID="A17">
    <owl:onProperty rdf:resource="http://foodie-cloud.com/model/foodie#period"/>
    <owl:minCardinality rdf:datatype="http://www.w3.org/2001/XMLSchema#int">1</owl:minCardinality>
    <rdf:type rdf:resource="http://www.w3.org/2002/07/owl#Restriction"/>
  </rdf:Description>
</rdf:RDF>
