@prefix : <https://w3id.org/cybele/> .
@prefix qb: <http://purl.org/linked-data/cube#> .
@prefix dct: <http://purl.org/dc/terms/> .
@prefix owl: <http://www.w3.org/2002/07/owl#> .
@prefix rdf: <http://www.w3.org/1999/02/22-rdf-syntax-ns#> .
@prefix xml: <http://www.w3.org/XML/1998/namespace> .
@prefix xsd: <http://www.w3.org/2001/XMLSchema#> .
@prefix dcat: <http://www.w3.org/ns/dcat#> .
@prefix foaf: <http://xmlns.com/foaf/0.1/> .
@prefix prov: <http://www.w3.org/ns/prov#> .
@prefix rdfs: <http://www.w3.org/2000/01/rdf-schema#> .
@prefix skos: <http://www.w3.org/2004/02/skos/core#> .
@prefix stat: <http://data.europa.eu/m8g/> .
@prefix schema: <https://schema.org/> .
@prefix af-inspire:	<http://inspire.ec.europa.eu/schemas/af/3.0#> .
@prefix act-inspire:	<http://inspire.ec.europa.eu/schemas/act-core/3.0#> .
@prefix foodie: <http://foodie-cloud.com/model/foodie#> .
@prefix saref4agri: <https://saref.etsi.org/saref4agri/> .
@prefix common: <http://portele.de/ont/inspire/baseInspire#> .
@prefix fiware: <https://smartdatamodels.org/> .
@prefix fiware-agrifood: <https://smartdatamodels.org/dataModel.Agrifood/> .
@prefix iso19109: <http://def.seegrid.csiro.au/isotc211/iso19109/2005/feature#> .
@prefix iso19150-2: <http://def.seegrid.csiro.au/isotc211/iso19150/-2/2012/basic#> .
@prefix iso19103: <http://def.seegrid.csiro.au/isotc211/iso19103/2005/basic#> .
@prefix iso19115-citation: <http://def.seegrid.csiro.au/isotc211/iso19115/2003/citation#> .
@prefix iso19108: <http://def.seegrid.csiro.au/isotc211/iso19108/2002/temporal#> .
@prefix geo:   <http://www.opengis.net/ont/geosparql#> .
@prefix ssn: <http://www.w3.org/ns/ssn/> .
@prefix sosa: <http://www.w3.org/ns/sosa/> .
@prefix saref: <https://saref.etsi.org/core/> .
@prefix ngsi-ld: <https://uri.etsi.org/ngsi-ld/> .
@base <https://w3id.org/demeter/> .

<https://w3id.org/demeter/agri/agriIntervention> a owl:Ontology ;
                            owl:versionIRI <https://w3id.org/demeter/agri/agriIntervention/2.0> ;
                            dct:contributor [ schema:affiliation [ foaf:name "OGC"
                                                                 ] ;
                                              foaf:name "Rob Atkinson"
                                            ] ,
                                            [ schema:affiliation [ foaf:name "ICCS"
                                                                 ] ;
                                              foaf:name "Ioanna Roussaki"
                                            ] ;
                            dct:creator [ schema:affiliation [ foaf:name "PSNC"
                                                             ] ;
                                          rdfs:seeAlso <http://orcid.org/0000-0003-4289-4922> ;
                                          foaf:name "Raul Palma"
                                        ] ;
                            owl:imports <https://w3id.org/demeter/agri/agriCommon> ;
                            dct:description "The DEMETER AgriIntervention is one of the agri profiles of DEMETER AIM. This profile was created by reusing and aligning well-known ontologies and vocabularies"@en ;
                            dct:rights "This vocabulary is distributed under Creative Commons Attribution 4.0 License - http://creativecommons.org/licenses/by/4.0"@en ;
                            dct:title "DEMETER AgriIntervention"@en ;
                            rdfs:label "DEMETER AgriIntervention"@en ;
                            rdfs:comment "The DEMETER Agriculture Information Model (AIM) is the common vocabulary in DEMETER project providing the basis for semantic interoperability across smart farming solutions"@en ;
                            owl:versionInfo "2.0" ;
                            foaf:maker [ foaf:homepage <https://h2020-demeter.eu/> ;
                                         foaf:name "DEMETER project"
                                       ] .

#################################################################
#    Annotation properties
#################################################################


#################################################################
#    Datatypes
#################################################################


#################################################################
#    Object Properties
#################################################################

###  http://foodie-cloud.com/model/foodie#interventionPlot
foodie:interventionPlot
        a               owl:ObjectProperty ;
        rdfs:range      foodie:Plot ;
        skos:prefLabel  "interventionPlot"@en ;
        rdfs:label "interventionPlot" ;
        rdfs:comment "A Relation from Intervention to Plot. A plot can have few intervetions." ;
        rdfs:isDefinedBy <http://foodie-cloud.com/model/foodie> .

###  http://foodie-cloud.com/model/foodie#interventionZone
foodie:interventionZone
        a               owl:ObjectProperty ;
        rdfs:range      foodie:ManagementZone ;
        skos:prefLabel  "interventionZone"@en ;
        rdfs:label "interventionZone" ;
        rdfs:comment "A Relation from Intervention to ManagementZone." ;
        rdfs:isDefinedBy <http://foodie-cloud.com/model/foodie> .

###  http://foodie-cloud.com/model/foodie#supervisor
foodie:supervisor  a    owl:ObjectProperty ;
        rdfs:range      iso19115-citation:ResponsibleParty ;
        skos:prefLabel  "supervisor"@en ;
        rdfs:label "supervisor" ;
        rdfs:comment "A Relation from Intervention to ResponsibleParty. ResponsibleParty contains the entity who carries out the intervention (a person or a body who has the power and authority to give instructions and guarantee the conducted Intervention)" ;
        rdfs:isDefinedBy <http://foodie-cloud.com/model/foodie> .

###  http://foodie-cloud.com/model/foodie#interventionGeometry
foodie:interventionGeometry
        a               owl:ObjectProperty ;
        rdfs:range      geo:Geometry ;
        skos:prefLabel  "interventionGeometry"@en ;
        rdfs:label "interventionGeometry" ;
        rdfs:comment "A Relation to the geometry defining the spatial extent of the Intervention" ;
        rdfs:isDefinedBy <http://foodie-cloud.com/model/foodie> .

###  http://foodie-cloud.com/model/foodie#evidenceParty
foodie:evidenceParty  a  owl:ObjectProperty ;
        rdfs:range      iso19115-citation:ResponsibleParty ;
        skos:prefLabel  "evidenceParty"@en ;
        rdfs:label "evidenceParty" ;
        rdfs:comment "A Relation to a person or a body who inserted the Intervention into the database" ;
        rdfs:isDefinedBy <http://foodie-cloud.com/model/foodie> .

###  http://foodie-cloud.com/model/foodie#operator
foodie:operator  a      owl:ObjectProperty ;
        rdfs:range      iso19115-citation:ResponsibleParty ;
        skos:prefLabel  "operator"@en ;
        rdfs:label "operator" ;
        rdfs:comment "A Relation to the person(s) who has conducted an Intervention" ;
        rdfs:isDefinedBy <http://foodie-cloud.com/model/foodie> .

###  http://foodie-cloud.com/model/foodie#formOfTreatment
foodie:formOfTreatment
        a               owl:ObjectProperty ;
        rdfs:range      foodie:FormOfTreatmentValue ;
        skos:prefLabel  "formOfTreatment"@en ;
        rdfs:label "formOfTreatment" ;
        rdfs:comment "A Relation from Treatment to FormOfTreatmentValue codelist, e.g., manual (i.e. conducted manually by a person), applicationMachine (i.e. automatic or semi-automatic application by a machine), aerial (i.e. aerial application from an airplane);" ;
        rdfs:isDefinedBy <http://foodie-cloud.com/model/foodie> .

###  http://foodie-cloud.com/model/foodie#treatmentPurpose
foodie:treatmentPurpose
        a               owl:ObjectProperty ;
        rdfs:range      foodie:TreatmentPurposeValue ;
        skos:prefLabel  "treatmentPurpose"@en ;
        rdfs:label "treatmentPurpose" ;
        rdfs:comment "A Relation from Treatment to TreatmentPurposeValue codelist, e.g., disease, fertilization, pest, weed" ;
        rdfs:isDefinedBy <http://foodie-cloud.com/model/foodie> .

###  http://foodie-cloud.com/model/foodie#areaDose
foodie:areaDose  a      owl:ObjectProperty ;
        rdfs:range      foodie:DoseUnit ;
        skos:prefLabel  "areaDose"@en ;
        rdfs:label "areaDose" ;
        rdfs:comment "A Relation from Treatment to DoseUnit entity, indicating the minimum and maximum application rate of the Treatment together with their unit" ;
        rdfs:isDefinedBy <http://foodie-cloud.com/model/foodie> .

###  http://foodie-cloud.com/model/foodie#plan
foodie:plan  a          owl:ObjectProperty ;
        rdfs:range      foodie:TreatmentPlan ;
        skos:prefLabel  "plan"@en ;
        rdfs:label "plan" ;
        rdfs:comment "A Relation from Treatment to TreatmentPlan entity." ;
        rdfs:isDefinedBy <http://foodie-cloud.com/model/foodie> .

###  http://foodie-cloud.com/model/foodie#motionSpeed
foodie:motionSpeed  a   owl:ObjectProperty ;
        rdfs:range      iso19103:Measure ;
        skos:prefLabel  "motionSpeed"@en ;
        rdfs:label "motionSpeed" ;
        rdfs:comment "A Relation from Treatment to Measure entity, indicating recommended speed for the application of the treatment that should be expressed together with its unit" ;
        rdfs:isDefinedBy <http://foodie-cloud.com/model/foodie> .

###  http://foodie-cloud.com/model/foodie#treatmentProduct
foodie:treatmentProduct
        a               owl:ObjectProperty ;
        rdfs:range      foodie:Product ;
        skos:prefLabel  "treatmentProduct"@en ;
        rdfs:label "treatmentProduct" ;
        rdfs:comment "A Relation from Treatment to Product entity." ;
        rdfs:isDefinedBy <http://foodie-cloud.com/model/foodie> .

###  http://foodie-cloud.com/model/foodie#quantity
foodie:quantity  a      owl:ObjectProperty ;
        rdfs:range      iso19103:Measure ;
        skos:prefLabel  "quantity"@en ;
        rdfs:label "quantity" ;
        rdfs:comment "A Relation from Treatment to Measure entity, indicating the value of a physical quantity of applied Treatment, together with its unit." ;
        rdfs:isDefinedBy <http://foodie-cloud.com/model/foodie> .

###  http://foodie-cloud.com/model/foodie#flowAdjustment
foodie:flowAdjustment
        a               owl:ObjectProperty ;
        rdfs:range      iso19103:Measure ;
        skos:prefLabel  "flowAdjustment"@en ;
        rdfs:label "flowAdjustment" ;
        rdfs:comment "A Relation from Treatment to Measure entity, indicating whether a flow adjustment was needed for the application of the Treatment, be expressed together with its unit " ;
        rdfs:isDefinedBy <http://foodie-cloud.com/model/foodie> .

###  http://foodie-cloud.com/model/foodie#applicationWidth
foodie:applicationWidth
        a               owl:ObjectProperty ;
        rdfs:range      iso19103:Measure ;
        skos:prefLabel  "applicationWidth"@en ;
        rdfs:label "flowAdjustment" ;
        rdfs:comment "A Relation from Treatment to Measure entity, indicating a width in which a machine is capable to apply the Treatment, expressed together with its unit" ;
        rdfs:isDefinedBy <http://foodie-cloud.com/model/foodie> .

###  http://foodie-cloud.com/model/foodie#pressure
foodie:pressure  a      owl:ObjectProperty ;
        rdfs:range      iso19103:Measure ;
        skos:prefLabel  "pressure"@en ;
        rdfs:label "pressure" ;
        rdfs:comment "A Relation from Treatment to Measure entity, indicating the recommended pressure for the application of the Treatment that should be expressed together with its unit" ;
        rdfs:isDefinedBy <http://foodie-cloud.com/model/foodie> .

###  http://foodie-cloud.com/model/foodie#planProduct
foodie:planProduct  a   owl:ObjectProperty ;
        rdfs:range      foodie:Product ;
        skos:prefLabel  "planProduct"@en ;
        rdfs:label "planProduct" ;
        rdfs:comment "A Relation from TreatmentPlan to Product entity." ;
        rdfs:isDefinedBy <http://foodie-cloud.com/model/foodie> .

###  http://foodie-cloud.com/model/foodie#campaign
foodie:campaign  a      owl:ObjectProperty ;
        rdfs:range      foodie:CampaignType ;
        skos:prefLabel  "campaign"@en ;
        rdfs:label "planProduct" ;
        rdfs:comment "A Relation from TreatmentPlan to CampaignType entity including the period to which the TreatmentPlan was designed" ;
        rdfs:isDefinedBy <http://foodie-cloud.com/model/foodie> .

###  http://foodie-cloud.com/model/foodie#period
foodie:period  a      owl:ObjectProperty ;
        rdfs:range      iso19108:Period ;
        skos:prefLabel  "period"@en ;
        rdfs:label "period" ;
        rdfs:comment "A Relation from CampaignType to Period entity indicating the period to which the TreatmentPlan was designed. Typically a campaign may be an agronomical year or a season e.g. between 2015-03-01 and 2015-09-30" ;
        rdfs:isDefinedBy <http://foodie-cloud.com/model/foodie> .

###  http://foodie-cloud.com/model/foodie#minimumDose
foodie:minimumDose
			a   owl:ObjectProperty ;
        rdfs:range      iso19103:Measure ;
        skos:prefLabel  "minimumDose"@en ;
        rdfs:label "minimumDose" ;
        rdfs:comment "A Relation from DoseUnit to Measure entity, indicating the minimuDose" ;
        rdfs:isDefinedBy <http://foodie-cloud.com/model/foodie> .

###  http://foodie-cloud.com/model/foodie#maximumDose
foodie:maximumDose
			a   owl:ObjectProperty ;
        rdfs:range      iso19103:Measure ;
        skos:prefLabel  "maximumDose"@en ;
        rdfs:label "maximumDose" ;
        rdfs:comment "A Relation from DoseUnit to Measure entity, indicating the maximumDose" ;
        rdfs:isDefinedBy <http://foodie-cloud.com/model/foodie> .

### https://smartdatamodels.org/dataModel.Agrifood/hasAgriParcel
fiware-agrifood:hasAgriParcel	a	owl:ObjectProperty ;
        rdfs:label   		"operationHasAgriParcel"@en ;
        rdfs:comment		"Reference to the AgriParcel to which this entity relates." ;
        rdfs:isDefinedBy <https://github.com/smart-data-models/dataModel.Agrifood/blob/master/AgriParcelOperation/schema.json> .

### https://smartdatamodels.org/dataModel.Agrifood/hasOperator
fiware-agrifood:hasOperator	a   owl:ObjectProperty ;
        rdfs:label   		"hasOperator"@en ;
        rdfs:comment		"Reference to the operator conducting the operation" ;
        rdfs:isDefinedBy <https://github.com/smart-data-models/dataModel.Agrifood/blob/master/AgriParcelOperation/schema.json> .


#################################################################
#    Data properties
#################################################################

###  http://foodie-cloud.com/model/foodie#status
foodie:status  a        owl:DatatypeProperty ;
        rdfs:range      xsd:string ;
        skos:prefLabel  "status"@en ;
        rdfs:label "status" ;
        rdfs:comment "Status of the intervention, e.g. approved, pending, completed as a free text" ;
        rdfs:isDefinedBy <http://foodie-cloud.com/model/foodie> .

###  http://foodie-cloud.com/model/foodie#creationDateTime
foodie:creationDateTime
        a               owl:DatatypeProperty ;
        rdfs:range      xsd:dateTime ;
        skos:prefLabel  "creationDateTime"@en ;
        rdfs:label "creationDateTime" ;
        rdfs:comment "date and time of the observed operation/intervention." ;
        rdfs:isDefinedBy <http://foodie-cloud.com/model/foodie> .

###  http://foodie-cloud.com/model/foodie#treatmentDescription
foodie:treatmentDescription
        a               owl:DatatypeProperty ;
        rdfs:range      xsd:string ;
        skos:prefLabel  "treatmentDescription"@en ;
        rdfs:label "treatmentDescription" ;
        rdfs:comment "Description of the observed operation/intervention." ;
        rdfs:isDefinedBy <http://foodie-cloud.com/model/foodie> .

###  http://foodie-cloud.com/model/foodie#treatmentPlanCode
foodie:treatmentPlanCode
        a               owl:DatatypeProperty ;
        rdfs:range      xsd:string ;
        skos:prefLabel  "treatmentPlanCode"@en ;
        rdfs:label "treatmentPlanCode" ;
        rdfs:comment "Identification code of the observed operation/intervention." ;
        rdfs:isDefinedBy <http://foodie-cloud.com/model/foodie> .

###  http://foodie-cloud.com/model/foodie#treatmentPlanCreation
foodie:treatmentPlanCreation
        a               owl:DatatypeProperty ;
        rdfs:range      xsd:dateTime ;
        skos:prefLabel  "treatmentPlanCreation"@en ;
        rdfs:label "treatmentPlanCreation" ;
        rdfs:comment "Date and time of the creation of the operation/intervention plan" ;
        rdfs:isDefinedBy <http://foodie-cloud.com/model/foodie> .

### https://smartdatamodels.org/dataModel.Agrifood/plannedStartAt
fiware-agrifood:plannedStartAt	a	owl:DatatypeProperty ;
        rdfs:range      xsd:dateTime ;
        rdfs:label   		"plannedStartAt"@en ;
        rdfs:comment		"The planned start date/timestamp for the operation. Note that this is advisory and the actual time the operation starts may be before or after the planned start." ;
        rdfs:isDefinedBy <https://github.com/smart-data-models/dataModel.Agrifood/blob/master/AgriParcelOperation/schema.json> .

### https://smartdatamodels.org/dataModel.Agrifood/plannedEndAt
fiware-agrifood:plannedEndAt	a   owl:DatatypeProperty ;
        rdfs:range      xsd:dateTime ;
        rdfs:label   		"plannedEndAt"@en ;
        rdfs:comment		"The planned end date/timestamp for the operation. Note that this is advisory and the actual time the operation finishes may be before or after the planned end." ;
        rdfs:isDefinedBy <https://github.com/smart-data-models/dataModel.Agrifood/blob/master/AgriParcelOperation/schema.json> .

### https://smartdatamodels.org/dataModel.Agrifood/operationType
fiware-agrifood:operationType	a   owl:DatatypeProperty ;
        rdfs:label   		"operationType"@en ;
        rdfs:comment		"A choice from an enumerated list describing the operation performed on the parcel. One of: fertiliser, inspection, pesticide, water, other." ;
        rdfs:isDefinedBy <https://github.com/smart-data-models/dataModel.Agrifood/blob/master/AgriParcelOperation/schema.json> .

### https://smartdatamodels.org/dataModel.Agrifood/result
fiware-agrifood:result	a      owl:DatatypeProperty ;
        rdfs:label   		"result"@en ;
        rdfs:comment		"A description of the results of the operation. One of: ok, aborted, failed." ;
        rdfs:isDefinedBy <https://github.com/smart-data-models/dataModel.Agrifood/blob/master/AgriParcelOperation/schema.json> .

### https://uri.etsi.org/ngsi-ld/status
ngsi-ld:status	a      owl:DatatypeProperty ;
        rdfs:label   		"status"@en ;
        rdfs:comment		"A choice from an enumerated list describing the status. One of: planned, ongoing, finished, scheduled, cancelled." ;
        rdfs:isDefinedBy <https://uri.etsi.org/ngsi-ld/v1/ngsi-ld-core-context-v1.6.jsonld> .

### https://smartdatamodels.org/dataModel.Agrifood/startedAt
fiware-agrifood:startedAt	a     owl:DatatypeProperty ;
        rdfs:range      xsd:dateTime ;
        rdfs:label   		"startedAt"@en ;
        rdfs:comment		"Timestamp when the operation actually started to be performed." ;
        rdfs:isDefinedBy <https://github.com/smart-data-models/dataModel.Agrifood/blob/master/AgriParcelOperation/schema.json> .

### https://smartdatamodels.org/dataModel.Agrifood/endedAt
fiware-agrifood:endedAt	a       owl:DatatypeProperty ;
        rdfs:range      xsd:dateTime ;
        rdfs:label   		"endedAt"@en ;
        rdfs:comment		"Timestamp when the operation actually finished." ;
        rdfs:isDefinedBy <https://github.com/smart-data-models/dataModel.Agrifood/blob/master/AgriParcelOperation/schema.json> .

### https://smartdatamodels.org/dataModel.Agrifood/reportedAt
fiware-agrifood:reportedAt	a     owl:DatatypeProperty ;
        rdfs:range      xsd:dateTime ;
        rdfs:label   		"reportedAt"@en ;
        rdfs:comment		"Timestamp when the event/ fault was reported." ;
        rdfs:isDefinedBy <https://github.com/smart-data-models/dataModel.Agrifood/blob/master/AgriParcelOperation/schema.json> .

### https://smartdatamodels.org/dataModel.Agrifood/quantity
fiware-agrifood:quantity	a      owl:DatatypeProperty ;
        rdfs:label   		"quantity"@en ;
        rdfs:comment		"The total quantity of water or product used/ applied. It is recommended this is measured in litres for liquids or kilogrammes for solids." ;
        rdfs:isDefinedBy <https://github.com/smart-data-models/dataModel.Agrifood/blob/master/AgriParcelOperation/schema.json> .

### https://smartdatamodels.org/dataModel.Agrifood/waterSource
fiware-agrifood:waterSource	a   owl:DatatypeProperty ;
        rdfs:label   		"waterSource"@en ;
        rdfs:comment		"Type of water sources. One of: borehole, rainfall, river, rainwater capture, water dam, commercial supply." ;
        rdfs:isDefinedBy <https://github.com/smart-data-models/dataModel.Agrifood/blob/master/AgriParcelOperation/schema.json> .

### https://smartdatamodels.org/dataModel.Agrifood/irrigationRecord
fiware-agrifood:irrigationRecord	a	owl:DatatypeProperty ;
        rdfs:label   		"irrigationRecord"@en ;
        rdfs:comment		"Relationship with the irrigation record of the execution" ;
        rdfs:isDefinedBy <https://github.com/smart-data-models/dataModel.Agrifood/blob/master/AgriParcelOperation/schema.json> .

#################################################################
#    Classes
#################################################################

### http://foodie-cloud.com/model/foodie#Intervention
foodie:Intervention  a   owl:Class ;
        rdfs:subClassOf  geo:Feature;
        rdfs:subClassOf  [ a                   owl:Restriction ;
                           owl:maxCardinality  "1"^^xsd:int ;
                           owl:onProperty      foodie:notes
                         ] ;
        rdfs:subClassOf  [ a                owl:Restriction ;
                           owl:cardinality  "1"^^xsd:int ;
                           owl:onProperty   foodie:description
                         ] ;
        rdfs:subClassOf  [ a                owl:Restriction ;
                           owl:cardinality  "1"^^xsd:int ;
                           owl:onProperty   foodie:type
                         ] ;
        rdfs:subClassOf  [ a                   owl:Restriction ;
                           owl:maxCardinality  "1"^^xsd:int ;
                           owl:onProperty      foodie:interventionPlot
                         ] ;
        rdfs:subClassOf  [ a                owl:Restriction ;
                           owl:cardinality  "1"^^xsd:int ;
                           owl:onProperty   foodie:status
                         ] ;
        rdfs:subClassOf  [ a                   owl:Restriction ;
                           owl:maxCardinality  "1"^^xsd:int ;
                           owl:onProperty      foodie:supervisor
                         ] ;
        rdfs:subClassOf  [ a                   owl:Restriction ;
                           owl:minCardinality  "1"^^xsd:int ;
                           owl:onProperty      foodie:interventionGeometry
                         ] ;
        rdfs:subClassOf  [ a                   owl:Restriction ;
                           owl:maxCardinality  "1"^^xsd:int ;
                           owl:onProperty      foodie:price
                         ] ;
        rdfs:subClassOf  [ a                   owl:Restriction ;
                           owl:minCardinality  "1"^^xsd:int ;
                           owl:onProperty      foodie:evidenceParty
                         ] ;
        rdfs:subClassOf  [ a                owl:Restriction ;
                           owl:cardinality  "1"^^xsd:int ;
                           owl:onProperty   foodie:creationDateTime
                         ] ;
        rdfs:subClassOf  [ a                owl:Restriction ;
                           owl:cardinality  "1"^^xsd:int ;
                           owl:onProperty   common:validFrom
                         ] ;
        rdfs:subClassOf  [ a                   owl:Restriction ;
                           owl:maxCardinality  "1"^^xsd:int ;
                           owl:onProperty      common:validTo
                         ] ;
        skos:prefLabel   "Intervention"@en ;
        rdfs:label "Intervention" ;
        rdfs:comment "An entity of operation or intervention." ;
        rdfs:isDefinedBy <http://foodie-cloud.com/model/foodie> .

### http://foodie-cloud.com/model/foodie#Treatment
foodie:Treatment  a      owl:Class ;
        rdfs:subClassOf  geo:Feature , foodie:Intervention ;
        rdfs:subClassOf  [ a                owl:Restriction ;
                           owl:cardinality  "1"^^xsd:int ;
                           owl:onProperty   foodie:formOfTreatment
                         ] ;
        rdfs:subClassOf  [ a                   owl:Restriction ;
                           owl:maxCardinality  "1"^^xsd:int ;
                           owl:onProperty      foodie:areaDose
                         ] ;
        rdfs:subClassOf  [ a                   owl:Restriction ;
                           owl:maxCardinality  "1"^^xsd:int ;
                           owl:onProperty      foodie:plan
                         ] ;
        rdfs:subClassOf  [ a                   owl:Restriction ;
                           owl:maxCardinality  "1"^^xsd:int ;
                           owl:onProperty      foodie:price
                         ] ;
        rdfs:subClassOf  [ a                   owl:Restriction ;
                           owl:maxCardinality  "1"^^xsd:int ;
                           owl:onProperty      foodie:motionSpeed
                         ] ;
        rdfs:subClassOf  [ a                   owl:Restriction ;
                           owl:minCardinality  "1"^^xsd:int ;
                           owl:onProperty      foodie:treatmentProduct
                         ] ;
        rdfs:subClassOf  [ a                owl:Restriction ;
                           owl:cardinality  "1"^^xsd:int ;
                           owl:onProperty   foodie:quantity
                         ] ;
        rdfs:subClassOf  [ a                   owl:Restriction ;
                           owl:maxCardinality  "1"^^xsd:int ;
                           owl:onProperty      foodie:flowAdjustment
                         ] ;
        rdfs:subClassOf  [ a                   owl:Restriction ;
                           owl:maxCardinality  "1"^^xsd:int ;
                           owl:onProperty      foodie:applicationWidth
                         ] ;
        rdfs:subClassOf  [ a                   owl:Restriction ;
                           owl:maxCardinality  "1"^^xsd:int ;
                           owl:onProperty      foodie:treatmentDescription
                         ] ;
        rdfs:subClassOf  [ a                   owl:Restriction ;
                           owl:maxCardinality  "1"^^xsd:int ;
                           owl:onProperty      foodie:pressure
                         ] ;
        skos:prefLabel   "Treatment"@en ;
        rdfs:label "Treatment" ;
        rdfs:comment "An entity defining the attributes of Treatments" ;
        rdfs:isDefinedBy <http://foodie-cloud.com/model/foodie> .

### http://foodie-cloud.com/model/foodie#TreatmentPlan
foodie:TreatmentPlan  a  owl:Class ;
        rdfs:subClassOf  geo:Feature ;
        rdfs:subClassOf  [ a                owl:Restriction ;
                           owl:cardinality  "1"^^xsd:int ;
                           owl:onProperty   foodie:type
                         ] ;
        rdfs:subClassOf  [ a                   owl:Restriction ;
                           owl:maxCardinality  "1"^^xsd:int ;
                           owl:onProperty      foodie:notes
                         ] ;
        rdfs:subClassOf  [ a                   owl:Restriction ;
                           owl:minCardinality  "1"^^xsd:int ;
                           owl:onProperty      foodie:planProduct
                         ] ;
        rdfs:subClassOf  [ a                   owl:Restriction ;
                           owl:maxCardinality  "1"^^xsd:int ;
                           owl:onProperty      foodie:treatmentPlanCode
                         ] ;
        rdfs:subClassOf  [ a                   owl:Restriction ;
                           owl:minCardinality  "1"^^xsd:int ;
                           owl:onProperty      foodie:campaign
                         ] ;
        rdfs:subClassOf  [ a                owl:Restriction ;
                           owl:cardinality  "1"^^xsd:int ;
                           owl:onProperty   foodie:treatmentPlanCreation
                         ] ;
        rdfs:subClassOf  [ a                owl:Restriction ;
                           owl:cardinality  "1"^^xsd:int ;
                           owl:onProperty   foodie:description
                         ] ;
        skos:prefLabel   "TreatmentPlan"@en ;
        rdfs:label "TreatmentPlan" ;
        rdfs:comment "An entity defining the Treatment plans" ;
        rdfs:isDefinedBy <http://foodie-cloud.com/model/foodie> .

### http://foodie-cloud.com/model/foodie#DoseUnit
foodie:DoseUnit  a       owl:Class ;
        rdfs:subClassOf  [ a                   owl:Restriction ;
                           owl:maxCardinality  "1"^^xsd:int ;
                           owl:onProperty      foodie:minimumDose
                         ] ;
        rdfs:subClassOf  [ a                   owl:Restriction ;
                           owl:maxCardinality  "1"^^xsd:int ;
                           owl:onProperty      foodie:maximumDose
                         ] ;
        skos:prefLabel   "DoseUnit"@en ;
        rdfs:label "DoseUnit" ;
        rdfs:comment "An entity defining the Doses for operation/intervention" ;
        rdfs:isDefinedBy <http://foodie-cloud.com/model/foodie> .


### http://foodie-cloud.com/model/foodie#CampaignType
foodie:CampaignType  a           owl:Class ;
        rdfs:subClassOf  [ a                   owl:Restriction ;
                           owl:minCardinality  "1"^^xsd:int ;
                           owl:onProperty      foodie:period
                         ] ;
        skos:prefLabel   "CampaignType"@en ;
        rdfs:label "CampaignType" ;
        rdfs:comment "An entity defining the types of campaigns" ;
        rdfs:isDefinedBy <http://foodie-cloud.com/model/foodie> .

### http://foodie-cloud.com/model/foodie#TreatmentPurposeValue
foodie:TreatmentPurposeValue
        a                owl:Class ;
        rdfs:subClassOf  skos:Concept ;
        skos:prefLabel   "TreatmentPurposeValue"@en ;
        rdfs:label "TreatmentPurposeValue" ;
        rdfs:comment "An entity defining the purpose of an Intervention/Treatment as codelist, e.g., disease (i.e. a pathological condition that affects part or all of production in the Plot), fertilization (i.e. a need to apply a fertilizer to soil), pest (i.e. a plant or animal detrimental to a human), weed (i.e. to reduce plants considered undesirable in a particular situation)" ;
        rdfs:isDefinedBy <http://foodie-cloud.com/model/foodie> .

### http://foodie-cloud.com/model/foodie#FormOfTreatmentValue
foodie:FormOfTreatmentValue
        a                owl:Class ;
        rdfs:subClassOf  skos:Concept ;
        skos:prefLabel   "FormOfTreatmentValue"@en ;
        rdfs:label "FormOfTreatmentValue" ;
        rdfs:comment "An entity defining the form of Intervention/Treatment as codelist, e.g., manual (i.e. conducted manually by a person), applicationMachine (i.e. automatic or semi-automatic application by a machine), aerial (i.e. aerial application from an airplane)" ;
        rdfs:isDefinedBy <http://foodie-cloud.com/model/foodie> .

### https://smartdatamodels.org/dataModel.Agrifood/AgriParcelOperation
fiware-agrifood:AgriParcelOperation	a owl:Class ;
			rdfs:label "AgriParcelOperation" ;
			rdfs:comment "This entity contains a harmonised description of a generic operations performed on a parcel of land. This entity is primarily associated with the agricultural vertical and related IoT applications." ;
			rdfs:isDefinedBy <https://github.com/smart-data-models/dataModel.Agrifood/blob/master/AgriParcelOperation/schema.json> .


#################################################################
#    Alignments
#################################################################
foodie:Treatment owl:equivalentClass fiware-agrifood:AgriParcelOperation .
foodie:interventionPlot owl:equivalentProperty fiware-agrifood:hasAgriParcel .
fiware-agrifood:operationType rdfs:subPropertyOf foodie:type .
fiware-agrifood:result rdfs:subPropertyOf foodie:notes .
foodie:status owl:equivalentProperty ngsi-ld:status .
foodie:operator owl:equivalentProperty fiware-agrifood:hasOperator .
fiware-agrifood:startedAt rdfs:subPropertyOf common:validFrom .
fiware-agrifood:endedAt rdfs:subPropertyOf common:validTo .
foodie:treatmentProduct owl:equivalentProperty fiware-agrifood:hasAgriProductType .
foodie:quantity owl:equivalentProperty fiware-agrifood:quantity .

#################################################################
#    Individuals
#################################################################
