@prefix : <https://w3id.org/cybele/> .
@prefix qb: <http://purl.org/linked-data/cube#> .
@prefix dct: <http://purl.org/dc/terms/> .
@prefix owl: <http://www.w3.org/2002/07/owl#> .
@prefix rdf: <http://www.w3.org/1999/02/22-rdf-syntax-ns#> .
@prefix xml: <http://www.w3.org/XML/1998/namespace> .
@prefix xsd: <http://www.w3.org/2001/XMLSchema#> .
@prefix dcat: <http://www.w3.org/ns/dcat#> .
@prefix foaf: <http://xmlns.com/foaf/0.1/> .
@prefix prov: <http://www.w3.org/ns/prov#> .
@prefix rdfs: <http://www.w3.org/2000/01/rdf-schema#> .
@prefix skos: <http://www.w3.org/2004/02/skos/core#> .
@prefix stat: <http://data.europa.eu/m8g/> .
@prefix schema: <https://schema.org/> .
@prefix af-inspire:	<http://inspire.ec.europa.eu/schemas/af/3.0#> .
@prefix act-inspire:	<http://inspire.ec.europa.eu/schemas/act-core/3.0#> .
@prefix foodie: <http://foodie-cloud.com/model/foodie#> .
@prefix saref4agri: <https://w3id.org/def/saref4agri#> .
@prefix common: <http://portele.de/ont/inspire/baseInspire#> .
@prefix fiware: <https://uri.fiware.org/ns/data-models#> .
@prefix iso19109: <http://def.seegrid.csiro.au/isotc211/iso19109/2005/feature#> .
@prefix iso19150-2: <http://def.seegrid.csiro.au/isotc211/iso19150/-2/2012/basic#> .
@prefix iso19103: <http://def.seegrid.csiro.au/isotc211/iso19103/2005/basic#> .
@prefix iso19115-citation: <http://def.seegrid.csiro.au/isotc211/iso19115/2003/citation#> .
@prefix geo:   <http://www.opengis.net/ont/geosparql#> .
@prefix ssn: <http://www.w3.org/ns/ssn/> .
@prefix sosa: <http://www.w3.org/ns/sosa/> .
@prefix saref: <https://w3id.org/saref#> .
@prefix obo: <http://purl.obolibrary.org/obo/> .
@prefix demeterAgriCommon: <https://w3id.org/demeter/agri/agriCommon#> .
@prefix qudt: <http://qudt.org/schema/qudt/> .
@base <https://w3id.org/demeter/> .

<https://w3id.org/demeter/agri/agriCommon> rdf:type owl:Ontology ;
                            owl:versionIRI <https://w3id.org/demeter/agri/agriCommon/2.0> ;
                            dct:contributor [ schema:affiliation [ foaf:name "OGC"
                                                                 ] ;
                                              foaf:name "Rob Atkinson"
                                            ] ,
                                            [ schema:affiliation [ foaf:name "ICCS"
                                                                 ] ;
                                              foaf:name "Ioanna Roussaki"
                                            ] ;
                            dct:creator [ schema:affiliation [ foaf:name "PSNC"
                                                             ] ;
                                          rdfs:seeAlso <http://orcid.org/0000-0003-4289-4922> ;
                                          foaf:name "Raul Palma"
                                        ] ;
                            owl:imports <https://w3id.org/demeter/crossDomain> ;
                            dct:description "The DEMETER AgriCommon is one of the agri profiles of DEMETER AIM. This profile was created by reusing and aligning well-known ontologies and vocabularies"@en ;
                            dct:rights "This vocabulary is distributed under Creative Commons Attribution 4.0 License - http://creativecommons.org/licenses/by/4.0"@en ;
                            dct:title "DEMETER AgriCommon"@en ;
                            rdfs:comment "The DEMETER Agriculture Information Model (AIM) is the common vocabulary in DEMETER project providing the basis for semantic interoperability across smart farming solutions"@en ;
                            owl:versionInfo "2.0" ;
                            foaf:maker [ foaf:homepage <https://h2020-demeter.eu/> ;
                                         foaf:name "DEMETER project"
                                       ] .

#################################################################
#    Annotation properties
#################################################################


###  http://purl.obolibrary.org/obo/TAXRANK_1000000
<http://purl.obolibrary.org/obo/TAXRANK_1000000> rdf:type owl:AnnotationProperty ;
                                                 rdfs:label "has_rank"@en ;
                                                 rdfs:isDefinedBy <http://purl.obolibrary.org/obo/> . 


#################################################################
#    Datatypes
#################################################################

#################################################################
#    Object Properties
#################################################################

###  https://w3id.org/def/saref4agri#managesFarm
saref4agri:managesFarm rdf:type owl:ObjectProperty ;
             rdfs:label "manages farm"@en .

### https://uri.fiware.org/ns/data-models#agroVocConcept
fiware:agroVocConcept	a      owl:ObjectProperty ;
        rdfs:label   		"agroVocConcept"@en ;
        rdfs:comment		"URL of the FAO entity" ;
        rdfs:isDefinedBy <https://github.com/smart-data-models/dataModel.Agrifood/blob/master/AgriCrop/schema.json> .  

###  https://w3id.org/demeter/agri/agriCommon#eppoConcept
demeterAgriCommon:eppoConcept	a      owl:ObjectProperty ;
        rdfs:label   		"eppoConcept"@en ;
        rdfs:comment		"URL of the EPPO entity" ;
        rdfs:isDefinedBy <https://w3id.org/demeter/agri/agriCommon#> .
                                                                             			  			                                              
#################################################################
#    Data properties
#################################################################

###  https://w3id.org/demeter/agri/agriCommon#userName
demeterAgriCommon:userName rdf:type owl:DatatypeProperty ;
         rdfs:range xsd:string ;
         rdfs:label "User Name" ;
         rdfs:isDefinedBy <https://w3id.org/demeter/agri/agriCommon#> .

###  https://w3id.org/demeter/agri/agriCommon#password
demeterAgriCommon:password rdf:type owl:DatatypeProperty ;
         rdfs:range xsd:string ;
         rdfs:label "Password" ;
         rdfs:isDefinedBy <https://w3id.org/demeter/agri/agriCommon#> .

###  https://w3id.org/def/saref4agri#hasName
saref4agri:hasName rdf:type owl:DatatypeProperty ;
         rdfs:range xsd:string ;
         rdfs:label "A relation to express the name of an entity (e.g.,animal)." ,
                    "has name" ;
         rdfs:isDefinedBy <https://w3id.org/def/saref4agri#> .

###  https://w3id.org/saref#hasDescription
<https://w3id.org/saref#hasDescription> rdf:type owl:DatatypeProperty ;
                                        rdfs:range xsd:string ;
                                        rdfs:comment "A relationship providing a description of an entity (e.g., device)" ;
                                        rdfs:isDefinedBy <https://w3id.org/saref#> ;
                                        rdfs:label "has description"@en .

###  https://w3id.org/saref#hasTimestamp
<https://w3id.org/saref#hasTimestamp> rdf:type owl:DatatypeProperty ;
                                      rdfs:range      xsd:dateTime ;  
                                      rdfs:isDefinedBy <https://w3id.org/saref#> ;
                                      rdfs:label "has timestamp"@en .                                                           

###  http://www.w3.org/ns/prov#generatedAtTime
prov:generatedAtTime
				a								owl:DatatypeProperty ;
				rdfs:label 			"generatedAtTime" ;
				rdfs:comment		"The time at which an entity was completely created and is available for use."@en ;
				rdfs:range 			xsd:dateTime ;
				rdfs:isDefinedBy	<http://www.w3.org/ns/prov-o#> .

###  http://www.w3.org/ns/prov#invalidatedAtTime				
prov:invalidatedAtTime
				a								owl:DatatypeProperty ;
				rdfs:label			"invalidatedAtTime" ;
				rdfs:comment		"The time at which an entity was invalidated (i.e., no longer usable)."@en ;
				rdfs:range			xsd:dateTime ;
				rdfs:isDefinedBy	<http://www.w3.org/ns/prov-o#> .
				
###  http://foodie-cloud.com/model/foodie#code
foodie:code  a          owl:DatatypeProperty ;
        rdfs:range      xsd:string ;
        skos:prefLabel  "code"@en ;
        rdfs:isDefinedBy <http://foodie-cloud.com/model/foodie> .

###  http://foodie-cloud.com/model/foodie#description        
foodie:description  a   owl:DatatypeProperty ;
        rdfs:range      xsd:string ;
        skos:prefLabel  "description"@en ;
        rdfs:isDefinedBy <http://foodie-cloud.com/model/foodie> .

###  http://foodie-cloud.com/model/foodie#notes        
foodie:notes  a         owl:DatatypeProperty ;
        rdfs:range      xsd:string ;
        skos:prefLabel  "notes"@en ;
        rdfs:isDefinedBy <http://foodie-cloud.com/model/foodie> .        

###  http://foodie-cloud.com/model/foodie#price                
foodie:price  a         owl:DatatypeProperty ;
        rdfs:range      xsd:string ;
        skos:prefLabel  "price"@en ;
        rdfs:isDefinedBy <http://foodie-cloud.com/model/foodie> .
        
###  http://foodie-cloud.com/model/foodie#type        
foodie:type  a          owl:DatatypeProperty ;
        rdfs:range      xsd:string ;
        skos:prefLabel  "type"@en ;
        rdfs:isDefinedBy <http://foodie-cloud.com/model/foodie> .
        				
###  <http://portele.de/ont/inspire/baseInspire#validFrom> 
common:validFrom	a      owl:DatatypeProperty ;
        rdfs:range       xsd:dateTime ;
        skos:prefLabel   "begin of real-world phenomenon"@en ;
        rdfs:isDefinedBy <http://portele.de/ont/inspire/baseInspire#> .

###  <http://portele.de/ont/inspire/baseInspire#validTo> 
common:validTo	a        owl:DatatypeProperty ;
        rdfs:range       xsd:dateTime ;        
        skos:prefLabel   "end of real-world phenomenon"@en ;
        rdfs:isDefinedBy <http://portele.de/ont/inspire/baseInspire#> .
        
### https://uri.fiware.org/ns/data-models#createdAt
fiware:createdAt	a      owl:DatatypeProperty ;
        rdfs:range      xsd:dateTime ;  
        rdfs:label   		"createdAt"@en ;
        rdfs:comment		"Indicates the date/ time that the instance of the entity was created in ISO 8601 format. The value of this will be set by the server when the entity was created" ;
        rdfs:isDefinedBy <https://github.com/GSMADeveloper/NGSI-LD-Entities/blob/master/definitions/Agri-Parcel.md> , <https://github.com/GSMADeveloper/NGSI-LD-Entities/blob/master/definitions/Agri-Crop.md>.

### https://uri.fiware.org/ns/data-models#modifiedAt
fiware:modifiedAt	a      owl:DatatypeProperty ;
        rdfs:range      xsd:dateTime ;  
        rdfs:label   		"modifiedAt"@en ;
        rdfs:comment		"Indicates the date/ time when the entity was last modified in ISO 8601 format. The value of this will be set by the server when the entity was modified, if the entity has not been modified it may have a null value." ;
        rdfs:isDefinedBy <https://github.com/GSMADeveloper/NGSI-LD-Entities/blob/master/definitions/Agri-Parcel.md> .

### https://uri.fiware.org/ns/data-models#source
fiware:source	a      owl:DatatypeProperty ;
        rdfs:label   		"source"@en ;
        rdfs:comment		"Specifies the URL to the source of this data (either organisation or where relevant more specific source)" ;
        rdfs:isDefinedBy <https://github.com/GSMADeveloper/NGSI-LD-Entities/blob/master/definitions/Agri-Parcel.md> .
                       
### https://uri.fiware.org/ns/data-models#dataProvider
fiware:dataProvider	a      owl:DatatypeProperty ;
        rdfs:label   		"dataProvider"@en ;
        rdfs:comment		"Specifies the URL to information about the provider of this information" ;
        rdfs:isDefinedBy <https://github.com/GSMADeveloper/NGSI-LD-Entities/blob/master/definitions/Agri-Parcel.md> .

### https://uri.fiware.org/ns/data-models#entityVersion
fiware:entityVersion	a      owl:DatatypeProperty ;
        rdfs:label   		"entityVersion"@en ;
        rdfs:comment		"The entity specification version as a number. A version number of 2.0 or later denotes the entity is represented using NGSI-LD" ;
        rdfs:isDefinedBy <https://github.com/GSMADeveloper/NGSI-LD-Entities/blob/master/definitions/Agri-Parcel.md> .

### https://uri.fiware.org/ns/data-models#name
fiware:name	a      owl:DatatypeProperty ;
        rdfs:label   		"name"@en ;
        rdfs:comment		"The name of this [entity]" ;
        rdfs:isDefinedBy <https://github.com/GSMADeveloper/NGSI-LD-Entities/blob/master/definitions/Agri-Parcel.md> , <https://github.com/GSMADeveloper/NGSI-LD-Entities/blob/master/definitions/Agri-Pest.md> , <https://github.com/GSMADeveloper/NGSI-LD-Entities/blob/master/definitions/Agri-Crop.md> , <https://github.com/GSMADeveloper/NGSI-LD-Entities/blob/master/definitions/Agri-Product-Type.md> .
        
### https://uri.fiware.org/ns/data-models#alternateName
fiware:alternateName	a      owl:DatatypeProperty ;
        rdfs:label   		"alternateName"@en ;
        rdfs:comment		"An alternative name for this [entity]" ;
        rdfs:isDefinedBy <https://github.com/GSMADeveloper/NGSI-LD-Entities/blob/master/definitions/Agri-Crop.md> .        
        
### https://uri.fiware.org/ns/data-models#description
fiware:description	a      owl:DatatypeProperty ;
        rdfs:label   		"description"@en ;
        rdfs:comment		"A description of the [entity]." ;
        rdfs:isDefinedBy <https://github.com/GSMADeveloper/NGSI-LD-Entities/blob/master/definitions/Agri-Parcel.md> , <https://github.com/GSMADeveloper/NGSI-LD-Entities/blob/master/definitions/Agri-Pest.md> , <https://github.com/GSMADeveloper/NGSI-LD-Entities/blob/master/definitions/Agri-Product-Type.md> , <https://github.com/GSMADeveloper/NGSI-LD-Entities/blob/master/definitions/Agri-Crop.md> .
                
### https://uri.fiware.org/ns/data-models#category
fiware:category	a      owl:DatatypeProperty ;     
        rdfs:label   		"category"@en ;
        rdfs:comment		"The category of the entity, e.g., parcel of land (arable, grassland, vineyard, orchard, mixed crop, lowland, upland, set-aside, forestry, wetland), alert (Traffic jam, accidents, weather conditions, high level of pollutants)." ;
        rdfs:isDefinedBy <https://github.com/GSMADeveloper/NGSI-LD-Entities/blob/master/definitions/Agri-Parcel.md> , <https://fiware.github.io/data-models/specs/Alert/doc/spec.html> .                        

###  https://w3id.org/demeter/agri/agriCommon#imageURL
demeterAgriCommon:imageURL rdf:type owl:DatatypeProperty ;
        rdfs:subPropertyOf <https://schema.org/contentUrl> ;
        rdfs:range  xsd:anyURI ;
        rdfs:domain  demeterAgriCommon:Image ;
        rdfs:label "imageURL" ;
        rdfs:comment "Actual bytes of the image object, i.e., image file" ;
        rdfs:isDefinedBy <https://w3id.org/demeter/agri/agriCommon#> .

###  https://w3id.org/demeter/agri/agriCommon#imageHeight
demeterAgriCommon:imageHeight rdf:type owl:DatatypeProperty ;
        rdfs:subPropertyOf <https://schema.org/height> , saref:hasValue ;
        rdfs:domain  demeterAgriCommon:Image ;
        rdfs:label "imageHeight" ;
        rdfs:comment "The height of the image, e.g., 3 or 3 cm^^cdt:ucum" ;
        rdfs:isDefinedBy <https://w3id.org/demeter/agri/agriCommon#> .

###  https://w3id.org/demeter/agri/agriCommon#imageWidth
demeterAgriCommon:imageWidth rdf:type owl:DatatypeProperty ;
        rdfs:subPropertyOf <https://schema.org/width> , saref:hasValue ;   
        rdfs:domain  demeterAgriCommon:Image ;     
        rdfs:label "imageWidth" ;
        rdfs:comment "The width of the image, e.g., 3 or 3 cm^^cdt:ucum" ;
        rdfs:isDefinedBy <https://w3id.org/demeter/agri/agriCommon#> .

###  https://w3id.org/demeter/agri/agriCommon#imageDataType
demeterAgriCommon:imageDataType rdf:type owl:DatatypeProperty ;
        rdfs:domain  demeterAgriCommon:Image ;
        rdfs:label "imageDataType" ;
        rdfs:comment "The data type of the image, e.g., NDVI" ;
        rdfs:isDefinedBy <https://w3id.org/demeter/agri/agriCommon#> .        

###  https://w3id.org/demeter/agri/agriCommon#imageFormat
demeterAgriCommon:imageFormat rdf:type owl:DatatypeProperty ;
        rdfs:subPropertyOf <https://schema.org/encodingFormat> ;   
        rdfs:domain  demeterAgriCommon:Image ;     
        rdfs:label "imageFormat" ;
        rdfs:comment "The format of the image, e.g., tiff, jpg" ;
        rdfs:isDefinedBy <https://w3id.org/demeter/agri/agriCommon#> .

#################################################################
#    Classes
#################################################################
                                  
                                  
###  https://w3id.org/def/saref4agri#FarmHolding
saref4agri:FarmHolding rdf:type owl:Class ;
             rdfs:subClassOf <https://schema.org/Organization> ,
                             [ rdf:type owl:Restriction ;
                               owl:onProperty saref4agri:managesFarm ;
                               owl:someValuesFrom saref4agri:Farm
                             ] ,
                             [ rdf:type owl:Restriction ;
                               owl:onProperty saref4agri:hasName ;
                               owl:allValuesFrom xsd:string
                             ] ;
             rdfs:comment "A class to decsribe a saref4agri farm holding as subcass of an org:Organization" ;
             rdfs:label "Farm holding"@en .


###  https://w3id.org/def/saref4agri#Farmer
saref4agri:Farmer rdf:type owl:Class ;
        rdfs:subClassOf <http://xmlns.com/foaf/0.1/Person> ,
                        [ rdf:type owl:Restriction ;
                          owl:onProperty saref4agri:managesFarm ;
                          owl:someValuesFrom saref4agri:Farm
                        ] ,
                        [ rdf:type owl:Restriction ;
                          owl:onProperty saref4agri:hasName ;
                          owl:allValuesFrom xsd:string
                        ] ;
        rdfs:comment "A class to decsribe a saref4agri farmer as subcass of a foaf:Person" ;
        rdfs:label "Farmer"@en .

###  http://purl.obolibrary.org/obo/TAXRANK_0000000
<http://purl.obolibrary.org/obo/TAXRANK_0000000> rdf:type owl:Class ;
                                                 rdfs:label "taxonomic_rank"@en ;
                                                 rdfs:isDefinedBy <http://purl.obolibrary.org/obo/> .

###  https://w3id.org/demeter/agri/agriCommon#Image
demeterAgriCommon:Image rdf:type owl:Class ;
        rdfs:subClassOf <https://schema.org/ImageObject> ;
        rdfs:label "Image" ;
        rdfs:comment "An image object" ;
        rdfs:isDefinedBy <https://w3id.org/demeter/agri/agriCommon#> .



#################################################################
#    Alignments
#################################################################

fiware:name rdfs:subPropertyOf schema:name .
saref4agri:hasName owl:equivalentProperty fiware:name .
fiware:alternateName rdfs:subPropertyOf fiware:name .
saref:hasDescription owl:equivalentProperty foodie:description .
saref:hasDescription owl:equivalentProperty fiware:description .
foodie:description owl:equivalentProperty fiware:description .
prov:generatedAtTime rdfs:subPropertyOf saref:hasTimestamp .
fiware:createdAt rdfs:subPropertyOf saref:hasTimestamp .
iso19115-citation:ResponsibleParty owl:equivalentClass foaf:Agent .
fiware:category owl:equivalentProperty foodie:type .

#################################################################
#    Individuals
#################################################################

