@prefix : <https://w3id.org/cybele/> .
@prefix qb: <http://purl.org/linked-data/cube#> .
@prefix dct: <http://purl.org/dc/terms/> .
@prefix owl: <http://www.w3.org/2002/07/owl#> .
@prefix rdf: <http://www.w3.org/1999/02/22-rdf-syntax-ns#> .
@prefix xml: <http://www.w3.org/XML/1998/namespace> .
@prefix xsd: <http://www.w3.org/2001/XMLSchema#> .
@prefix dcat: <http://www.w3.org/ns/dcat#> .
@prefix foaf: <http://xmlns.com/foaf/0.1/> .
@prefix prov: <http://www.w3.org/ns/prov#> .
@prefix rdfs: <http://www.w3.org/2000/01/rdf-schema#> .
@prefix skos: <http://www.w3.org/2004/02/skos/core#> .
@prefix stat: <http://data.europa.eu/m8g/> .
@prefix schema: <https://schema.org/> .
@prefix af-inspire:	<http://inspire.ec.europa.eu/schemas/af/3.0#> .
@prefix act-inspire:	<http://inspire.ec.europa.eu/schemas/act-core/3.0#> .
@prefix foodie: <http://foodie-cloud.com/model/foodie#> .
@prefix saref4agri: <https://saref.etsi.org/saref4agri/> .
@prefix common: <http://portele.de/ont/inspire/baseInspire#> .
@prefix fiware: <https://smartdatamodels.org/> .
@prefix fiware-agrifood: <https://smartdatamodels.org/dataModel.Agrifood/> .
@prefix fiware-weather: <https://smartdatamodels.org/dataModel.Weather/> .
@prefix ngsi-ld: <https://uri.etsi.org/ngsi-ld/> .
@prefix iso19109: <http://def.seegrid.csiro.au/isotc211/iso19109/2005/feature#> .
@prefix iso19150-2: <http://def.seegrid.csiro.au/isotc211/iso19150/-2/2012/basic#> .
@prefix iso19103: <http://def.seegrid.csiro.au/isotc211/iso19103/2005/basic#> .
@prefix geo: <http://www.opengis.net/ont/geosparql#> .
@prefix saref: <https://saref.etsi.org/core/> .
@prefix ssn: <http://www.w3.org/ns/ssn/> .
@prefix obo: <http://purl.obolibrary.org/obo/> .
@prefix demeterAgriCrop: <https://w3id.org/demeter/agri/agriCrop#> .
@base <https://w3id.org/demeter/> .

<https://w3id.org/demeter/agri/agriCrop> a owl:Ontology ;
                            owl:versionIRI <https://w3id.org/demeter/agri/agriCrop/2.0> ;
                            dct:contributor [ schema:affiliation [ foaf:name "OGC"
                                                                 ] ;
                                              foaf:name "Rob Atkinson"
                                            ] ,
                                            [ schema:affiliation [ foaf:name "ICCS"
                                                                 ] ;
                                              foaf:name "Ioanna Roussaki"
                                            ] ;
                            dct:creator [ schema:affiliation [ foaf:name "PSNC"
                                                             ] ;
                                          rdfs:seeAlso <http://orcid.org/0000-0003-4289-4922> ;
                                          foaf:name "Raul Palma"
                                        ] ;
                            owl:imports <https://w3id.org/demeter/agri/agriCommon/2.0> ;
                            dct:description "The DEMETER AgriCrop is one of the agri profiles of DEMETER AIM. This profile was created by reusing and aligning well-known ontologies and vocabularies"@en ;
                            dct:rights "This vocabulary is distributed under Creative Commons Attribution 4.0 License - http://creativecommons.org/licenses/by/4.0"@en ;
                            dct:title "DEMETER AgriCrop"@en ;
                            rdfs:label "DEMETER AgriCrop" ;
                            rdfs:comment "The DEMETER Agriculture Information Model (AIM) is the common vocabulary in DEMETER project providing the basis for semantic interoperability across smart farming solutions"@en ;
                            owl:versionInfo "2.0" ;
                            foaf:maker [ foaf:homepage <https://h2020-demeter.eu/> ;
                                         foaf:name "DEMETER project"
                                       ] .

#################################################################
#    Annotation properties
#################################################################


#################################################################
#    Datatypes
#################################################################


#################################################################
#    Object Properties
#################################################################


###  https://saref.etsi.org/saref4agri/generates
saref4agri:generates a owl:ObjectProperty ;
           rdfs:subPropertyOf saref:hasProperty ;
           rdfs:comment "A relation to represent the yield generated by a Crop." ;
           rdfs:label "generates"@en ;
           rdfs:isDefinedBy <https://saref.etsi.org/saref4agri/> .


###  https://saref.etsi.org/saref4agri/receives
saref4agri:receives a owl:ObjectProperty ;
          rdfs:subPropertyOf saref:hasProperty ;
          rdfs:comment "A relation to represent the intake/consumption of certain substances in a Crop." ;
          rdfs:label "receives" ;
          rdfs:isDefinedBy <https://saref.etsi.org/saref4agri/> .

### http://foodie-cloud.com/model/foodie#cropArea
foodie:cropArea  a      owl:ObjectProperty ;
        rdfs:range      geo:Geometry ;
        skos:prefLabel  "cropArea"@en ;
        rdfs:comment "The geometry defining the spatial extent of the CropSpecies on the Plot" ;
        rdfs:label "cropArea" ;
        rdfs:isDefinedBy <http://foodie-cloud.com/model/foodie> .

### http://foodie-cloud.com/model/foodie#cropSpecies
foodie:cropSpecies  a   owl:ObjectProperty ;
        rdfs:range      foodie:CropType ;
        skos:prefLabel  "cropSpecies"@en ;
        rdfs:comment "Relation to the designation under which the CropSpecies is commonly known; such designation is expressed as a CropType" ;
        rdfs:label "cropSpecies" ;
        rdfs:isDefinedBy <http://foodie-cloud.com/model/foodie> .

### http://foodie-cloud.com/model/foodie#production
foodie:production  a    owl:ObjectProperty ;
        rdfs:range      foodie:ProductionType ;
        skos:prefLabel  "production"@en ;
        rdfs:comment "Relation to entity containing relevant production-related data, that is defined as a ProductionType" ;
        rdfs:label "production" ;
        rdfs:isDefinedBy <http://foodie-cloud.com/model/foodie> .

### http://foodie-cloud.com/model/foodie#productionAmount
foodie:productionAmount	a	owl:ObjectProperty ;
        rdfs:range      iso19103:Measure ;
        skos:prefLabel  "productionAmount"@en ;
        rdfs:comment "The value of a physical quantity of produced variety, together with its unit" ;
        rdfs:label "productionAmount" ;
        rdfs:isDefinedBy <http://foodie-cloud.com/model/foodie> .

### https://smartdatamodels.org/dataModel.Agrifood/hasAgriSoil
fiware-agrifood:hasAgriSoil	a	owl:ObjectProperty ;
        rdfs:label   		"cropHasAgriSoil"@en ;
        rdfs:comment		"Reference to the recommended types of soil suitable for growing this crop" ;
        rdfs:isDefinedBy <https://github.com/smart-data-models/dataModel.Agrifood/blob/master/AgriCrop/schema.json> .

### https://smartdatamodels.org/dataModel.Agrifood/hasAgriFertiliser
fiware-agrifood:hasAgriFertiliser	a	owl:ObjectProperty ;
        rdfs:label   		"hasAgriFertiliser"@en ;
        rdfs:comment		"Reference to the recommended types of fertiliser suitable for growing this crop" ;
        rdfs:isDefinedBy <https://github.com/smart-data-models/dataModel.Agrifood/blob/master/AgriCrop/schema.json> .

### https://smartdatamodels.org/dataModel.Agrifood/hasAgriPest
fiware-agrifood:hasAgriPest	a		owl:ObjectProperty ;
        rdfs:label   		"hasAgriPest"@en ;
        rdfs:comment		"Reference to the pests known to attack this crop." ;
        rdfs:isDefinedBy <https://github.com/smart-data-models/dataModel.Agrifood/blob/master/AgriCrop/schema.json> .


#################################################################
#    Data properties
#################################################################

###  https://w3id.org/demeter/agri/agriCrop#expectedBloomingStart
demeterAgriCrop:expectedBloomingStart a owl:DatatypeProperty ;
         rdfs:range xsd:dateTime ;
         rdfs:label "Expected Blooming Start" ;
         rdfs:comment "Expected Blooming Start" ;
         rdfs:isDefinedBy <https://w3id.org/demeter/agri/agriCrop#> .

###  https://w3id.org/demeter/agri/agriCrop#expectedBloomingEnd
demeterAgriCrop:expectedBloomingEnd a owl:DatatypeProperty ;
         rdfs:range xsd:dateTime ;
         rdfs:label "Expected Blooming End" ;
         rdfs:comment "Expected Blooming End" ;
         rdfs:isDefinedBy <https://w3id.org/demeter/agri/agriCrop#> .

###  https://w3id.org/demeter/agri/agriCrop#numberOfHivesNeeded
demeterAgriCrop:numberOfHivesNeeded a owl:DatatypeProperty ;
         rdfs:range xsd:dateTime ;
         rdfs:label "Number Of Hives Needed" ;
         rdfs:comment "Number Of Hives Needed" ;
         rdfs:isDefinedBy <https://w3id.org/demeter/agri/agriCrop#> .

###  https://saref.etsi.org/saref4agri/hasHarvestDate
saref4agri:hasHarvestDate a owl:DatatypeProperty ;
                rdfs:subPropertyOf owl:topDataProperty ;
                rdfs:range xsd:dateTime ;
                rdfs:comment "A relation to express the day the crop is harvested." ;
                rdfs:label "has harvest date" ;
                rdfs:isDefinedBy <https://saref.etsi.org/saref4agri/> .

###  https://saref.etsi.org/saref4agri/hasPlantDate
saref4agri:hasPlantDate a owl:DatatypeProperty ;
              rdfs:subPropertyOf owl:topDataProperty ;
              rdfs:range xsd:dateTime ;
              rdfs:comment "A relation to express the day the crop is planted." ;
              rdfs:label "has plant date" ;
              rdfs:isDefinedBy <https://saref.etsi.org/saref4agri/> .

### http://foodie-cloud.com/model/foodie#variety
foodie:variety  a       owl:DatatypeProperty ;
        rdfs:range      xsd:string ;
        skos:prefLabel  "variety"@en ;
        rdfs:comment "a taxonomic category that ranks below subspecies (where present) or species, its mem-bers differing from others of the same subspecies or species in minor but permanent or heritable characteristics" ;
        rdfs:label "variety" ;
        rdfs:isDefinedBy <http://foodie-cloud.com/model/foodie> .

### http://foodie-cloud.com/model/foodie#family
foodie:family  a        owl:DatatypeProperty ;
        rdfs:range      xsd:string ;
        skos:prefLabel  "family"@en ;
        rdfs:comment "a principal taxonomic category that ranks above genus and below order" ;
        rdfs:label "family" ;
        rdfs:isDefinedBy <http://foodie-cloud.com/model/foodie> .

### http://foodie-cloud.com/model/foodie#species
foodie:species  a       owl:DatatypeProperty ;
        rdfs:range      xsd:string ;
        skos:prefLabel  "species"@en ;
        rdfs:comment "a group of living organisms consisting of similar individuals capable of exchanging genes or interbreeding" ;
        rdfs:label "species" ;
        rdfs:isDefinedBy <http://foodie-cloud.com/model/foodie> .

### http://foodie-cloud.com/model/foodie#genus
foodie:genus  a         owl:DatatypeProperty ;
        rdfs:range      xsd:string ;
        skos:prefLabel  "genus"@en ;
         rdfs:comment "a principal taxonomic category that ranks above species and below family" ;
        rdfs:label "genus" ;
        rdfs:isDefinedBy <http://foodie-cloud.com/model/foodie> .

### http://foodie-cloud.com/model/foodie#productionDate
foodie:productionDate	a	owl:DatatypeProperty ;
        rdfs:range 			xsd:dateTime ;
        skos:prefLabel  "productionDate"@en ;
         rdfs:comment "date and time of production, e.g., when it was inserted or changed in the database" ;
        rdfs:label "productionDate" ;
        rdfs:isDefinedBy <http://foodie-cloud.com/model/foodie> .

### https://smartdatamodels.org/dataModel.Agrifood/plantingFrom
fiware-agrifood:plantingFrom	a		owl:DatatypeProperty ;
        rdfs:label   		"plantingFrom"@en ;
        rdfs:comment		"""A list of the recommended planting interval date(s) for this crop. Specified using ISO8601 repeating date intervals:
interval, description
Where interval is in the form of start date/end date
--MM-DD/--MM-DD
Meaning repeat each year from this start date to this end date.""" ;
        rdfs:isDefinedBy <https://github.com/smart-data-models/dataModel.Agrifood/blob/master/AgriCrop/schema.json> .

### https://smartdatamodels.org/dataModel.Agrifood/harvestingInterval
fiware-agrifood:harvestingInterval	a	owl:DatatypeProperty ;
        rdfs:label   		"harvestingInterval"@en ;
        rdfs:comment		"""A list of the recommended harvesting interval date(s) for this crop. Specified using ISO8601 repeating date intervals:
interval, description
Where interval is in the form of start date/end date
--MM-DD/--MM-DD
Meaning repeat each year from this start date to this end date.""" ;
        rdfs:isDefinedBy <https://github.com/smart-data-models/dataModel.Agrifood/blob/master/AgriCrop/schema.json> .

#################################################################
#    Classes
#################################################################


###  https://saref.etsi.org/saref4agri/Crop
saref4agri:Crop a owl:Class ;
      rdfs:subClassOf saref:FeatureOfInterest ,
                      [ a owl:Restriction ;
                        owl:onProperty <http://purl.obolibrary.org/obo/TAXRANK_1000000> ;
                        owl:someValuesFrom <http://purl.obolibrary.org/obo/TAXRANK_0000000>
                      ] ,
                      [ a owl:Restriction ;
                        owl:onProperty saref4agri:hasHarvestDate ;
                        owl:someValuesFrom xsd:dateTime
                      ] ,
                      [ a owl:Restriction ;
                        owl:onProperty saref4agri:hasPlantDate ;
                        owl:someValuesFrom xsd:dateTime
                      ] ;
      rdfs:comment "A collection of cultivated plants that is grown on a large scale commercially, especially a cereal, fruit, or vegetable."@en ;
      rdfs:label "Crop" ;
      rdfs:isDefinedBy <https://saref.etsi.org/saref4agri/> .

### http://foodie-cloud.com/model/foodie#CropSpecies
foodie:CropSpecies  a    owl:Class ;
        rdfs:subClassOf  geo:Feature;
        rdfs:subClassOf  [ a                   owl:Restriction ;
                           owl:minCardinality  "1"^^xsd:int ;
                           owl:onProperty      foodie:cropArea
                         ] ;
        rdfs:subClassOf  [ a                owl:Restriction ;
                           owl:cardinality  "1"^^xsd:int ;
                           owl:onProperty   foodie:cropSpecies
                         ] ;
        rdfs:subClassOf  [ a                   owl:Restriction ;
                           owl:maxCardinality  "1"^^xsd:int ;
                           owl:onProperty      prov:invalidatedAtTime
                         ] ;
        rdfs:subClassOf  [ a                owl:Restriction ;
                           owl:maxCardinality  "1"^^xsd:int ;
                           owl:onProperty   prov:generatedAtTime
                         ] ;
        rdfs:subClassOf  [ a                owl:Restriction ;
                           owl:cardinality  "1"^^xsd:int ;
                           owl:onProperty   common:validFrom
                         ] ;
        rdfs:subClassOf  [ a                   owl:Restriction ;
                           owl:maxCardinality  "1"^^xsd:int ;
                           owl:onProperty      common:validTo
                         ] ;
        skos:prefLabel   "CropSpecies"@en ;
        rdfs:comment "An entity for the species of the Crops grown in a plot. The planted crop species"@en ;
        rdfs:label "CropSpecies" ;
        rdfs:isDefinedBy <http://foodie-cloud.com/model/foodie> .

### http://foodie-cloud.com/model/foodie#CropType
foodie:CropType  a       owl:Class ;
        rdfs:subClassOf  [ a                   owl:Restriction ;
                           owl:maxCardinality  "1"^^xsd:int ;
                           owl:onProperty      foodie:code
                         ] ;
        rdfs:subClassOf  [ a                   owl:Restriction ;
                           owl:maxCardinality  "1"^^xsd:int ;
                           owl:onProperty      foodie:notes
                         ] ;
        rdfs:subClassOf  [ a                   owl:Restriction ;
                           owl:maxCardinality  "1"^^xsd:int ;
                           owl:onProperty      foodie:variety
                         ] ;
        rdfs:subClassOf  [ a                   owl:Restriction ;
                           owl:maxCardinality  "1"^^xsd:int ;
                           owl:onProperty      foodie:description
                         ] ;
        rdfs:subClassOf  [ a                   owl:Restriction ;
                           owl:maxCardinality  "1"^^xsd:int ;
                           owl:onProperty      foodie:family
                         ] ;
        rdfs:subClassOf  [ a                   owl:Restriction ;
                           owl:maxCardinality  "1"^^xsd:int ;
                           owl:onProperty      foodie:species
                         ] ;
        rdfs:subClassOf  [ a                   owl:Restriction ;
                           owl:maxCardinality  "1"^^xsd:int ;
                           owl:onProperty      foodie:genus
                         ] ;
        skos:prefLabel   "CropType"@en ;
        rdfs:comment "Designation under which the CropSpecies is commonly known"@en ;
        rdfs:label "CropType" ;
        rdfs:isDefinedBy <http://foodie-cloud.com/model/foodie> .

### http://foodie-cloud.com/model/foodie#ProductionType
foodie:ProductionType
        a                owl:Class ;
        rdfs:subClassOf  [ a                owl:Restriction ;
                           owl:cardinality  "1"^^xsd:int ;
                           owl:onProperty   foodie:variety
                         ] ;
        rdfs:subClassOf  [ a                owl:Restriction ;
                           owl:cardinality  "1"^^xsd:int ;
                           owl:onProperty   foodie:productionDate
                         ] ;
        rdfs:subClassOf  [ a                   owl:Restriction ;
                           owl:maxCardinality  "1"^^xsd:int ;
                           owl:onProperty      foodie:productionAmount
                         ] ;
        skos:prefLabel   "ProductionType"@en ;
        rdfs:comment "An entity containing relevant production-related data"@en ;
        rdfs:label "ProductionType" ;
        rdfs:isDefinedBy <http://foodie-cloud.com/model/foodie> .


### https://smartdatamodels.org/dataModel.Agrifood/AgriCrop
fiware-agrifood:AgriCrop	a owl:Class ;
			rdfs:label "Agri Crop" ;
			rdfs:comment "This entity contains a harmonised description of a generic crop. This entity is primarily associated with the agricultural vertical and related IoT applications." ;
			rdfs:isDefinedBy <https://github.com/smart-data-models/dataModel.Agrifood/blob/master/AgriCrop/schema.json> .



#################################################################
#    Alignments
#################################################################

saref4agri:Crop owl:equivalentClass foodie:CropSpecies .
saref4agri:Crop owl:equivalentClass fiware-agrifood:AgriCrop .
saref4agri:hasHarvestDate owl:equivalentProperty foodie:productionDate .

#################################################################
#    Individuals
#################################################################
