@prefix : <https://w3id.org/cybele/> .
@prefix qb: <http://purl.org/linked-data/cube#> .
@prefix dct: <http://purl.org/dc/terms/> .
@prefix owl: <http://www.w3.org/2002/07/owl#> .
@prefix rdf: <http://www.w3.org/1999/02/22-rdf-syntax-ns#> .
@prefix xml: <http://www.w3.org/XML/1998/namespace> .
@prefix xsd: <http://www.w3.org/2001/XMLSchema#> .
@prefix dcat: <http://www.w3.org/ns/dcat#> .
@prefix foaf: <http://xmlns.com/foaf/0.1/> .
@prefix prov: <http://www.w3.org/ns/prov#> .
@prefix rdfs: <http://www.w3.org/2000/01/rdf-schema#> .
@prefix skos: <http://www.w3.org/2004/02/skos/core#> .
@prefix stat: <http://data.europa.eu/m8g/> .
@prefix schema: <https://schema.org/> .
@prefix af-inspire:	<http://inspire.ec.europa.eu/schemas/af/3.0#> .
@prefix act-inspire:	<http://inspire.ec.europa.eu/schemas/act-core/3.0#> .
@prefix foodie: <http://foodie-cloud.com/model/foodie#> .
@prefix saref4agri: <https://saref.etsi.org/saref4agri/> .
@prefix common: <http://portele.de/ont/inspire/baseInspire#> .
@prefix fiware: <https://smartdatamodels.org/> .
@prefix fiware-agrifood: <https://smartdatamodels.org/dataModel.Agrifood/> .
@prefix fiware-weather: <https://smartdatamodels.org/dataModel.Weather/> .
@prefix ngsi-ld: <https://uri.etsi.org/ngsi-ld/> .
@prefix iso19109: <http://def.seegrid.csiro.au/isotc211/iso19109/2005/feature#> .
@prefix iso19150-2: <http://def.seegrid.csiro.au/isotc211/iso19150/-2/2012/basic#> .
@prefix iso19103: <http://def.seegrid.csiro.au/isotc211/iso19103/2005/basic#> .
@prefix geo:   <http://www.opengis.net/ont/geosparql#> .
@prefix ssn: <http://www.w3.org/ns/ssn/> .
@prefix sosa: <http://www.w3.org/ns/sosa/> .
@prefix saref: <https://saref.etsi.org/core/> .
@base <https://w3id.org/demeter/> .

<https://w3id.org/demeter/agri/agriAlert> a owl:Ontology ;
                            owl:versionIRI <https://w3id.org/demeter/agri/agriAlert/2.0> ;
                            dct:contributor [ schema:affiliation [ foaf:name "OGC"
                                                                 ] ;
                                              foaf:name "Rob Atkinson"
                                            ] ,
                                            [ schema:affiliation [ foaf:name "ICCS"
                                                                 ] ;
                                              foaf:name "Ioanna Roussaki"
                                            ] ;
                            dct:creator [ schema:affiliation [ foaf:name "PSNC"
                                                             ] ;
                                          rdfs:seeAlso <http://orcid.org/0000-0003-4289-4922> ;
                                          foaf:name "Raul Palma"
                                        ] ;
                            owl:imports <https://w3id.org/demeter/agri/agriCommon/2.0> ;
                            dct:description "The DEMETER AgriAlert is one of the agri profiles of DEMETER AIM. This profile was created by reusing and aligning well-known ontologies and vocabularies"@en ;
                            dct:rights "This vocabulary is distributed under Creative Commons Attribution 4.0 License - http://creativecommons.org/licenses/by/4.0"@en ;
                            dct:title "DEMETER AgriAlert"@en ;
                            rdfs:label "DEMETER AgriAlert" ;
                            rdfs:comment "The DEMETER Agriculture Information Model (AIM) is the common vocabulary in DEMETER project providing the basis for semantic interoperability across smart farming solutions"@en ;
                            owl:versionInfo "2.0" ;
                            foaf:maker [ foaf:homepage <https://h2020-demeter.eu/> ;
                                         foaf:name "DEMETER project"
                                       ] .

#################################################################
#    Annotation properties
#################################################################


#################################################################
#    Datatypes
#################################################################


#################################################################
#    Object Properties
#################################################################

###  http://foodie-cloud.com/model/foodie#alertGeometry
foodie:alertGeometry  a  owl:ObjectProperty ;
        rdfs:range      geo:Geometry ;
        skos:prefLabel  "alertGeometry"@en ;
        rdfs:label "alertGeometry" ;
        rdfs:comment "A relation between Geometry entity and Alert" ;
        rdfs:isDefinedBy <http://foodie-cloud.com/model/foodie> .

###  http://foodie-cloud.com/model/foodie#plotAlert
foodie:plotAlert
	a owl:ObjectProperty ;
        rdfs:range      foodie:Alert ;
        skos:prefLabel  "plotAlert"@en ;
        rdfs:label "plotAlert" ;
        rdfs:comment "A relation from Plot to Alert" ;
        rdfs:isDefinedBy <http://foodie-cloud.com/model/foodie> .

###  http://foodie-cloud.com/model/foodie#alertPlot
foodie:alertPlot  a     owl:ObjectProperty ;
        rdfs:range      foodie:Plot ;
        owl:inverseOf   foodie:plotAlert ;
        skos:prefLabel  "alertPlot"@en ;
        rdfs:label "plotAlert" ;
        rdfs:comment "A relation inverse of plotAlert directing from Alert to Plot class" ;
        rdfs:isDefinedBy <http://foodie-cloud.com/model/foodie> .

###  http://foodie-cloud.com/model/foodie#speciesAlert
foodie:speciesAlert  a  owl:ObjectProperty ;
        rdfs:range      foodie:Alert ;
        skos:prefLabel  "speciesAlert"@en ;
        rdfs:label "plotAlert" ;
        rdfs:comment "A relation inverse of plotAlert directing from Alert to Plot class" ;
        rdfs:isDefinedBy <http://foodie-cloud.com/model/foodie> .

###  http://foodie-cloud.com/model/foodie#alertSpecies
foodie:alertSpecies  a  owl:ObjectProperty ;
        rdfs:range      foodie:CropSpecies ;
        owl:inverseOf   foodie:speciesAlert ;
        skos:prefLabel  "alertSpecies"@en ;
        rdfs:label "alertSpecies" ;
        rdfs:comment "A relation between crop species and alert." ;
        rdfs:isDefinedBy <http://foodie-cloud.com/model/foodie> .

###  http://foodie-cloud.com/model/foodie#alertZone
foodie:alertZone  a     owl:ObjectProperty ;
        rdfs:range      foodie:ManagementZone ;
        owl:inverseOf   foodie:zoneAlert ;
        skos:prefLabel  "alertZone"@en ;
        rdfs:label "alertSpecies" ;
        rdfs:comment "A relation between management zone and alert." ;
        rdfs:isDefinedBy <http://foodie-cloud.com/model/foodie> .

###  http://foodie-cloud.com/model/foodie#zoneAlert
foodie:zoneAlert  a     owl:ObjectProperty ;
        rdfs:range      foodie:Alert ;
        skos:prefLabel  "zoneAlert"@en ;
        rdfs:label "zoneAlert" ;
        rdfs:comment "A relation between management zone and alert, inverse of alertZone" ;
        rdfs:isDefinedBy <http://foodie-cloud.com/model/foodie> .   

### https://uri.etsi.org/ngsi-ld/data
ngsi-ld:data	a      owl:ObjectProperty ;
        rdfs:label   		"data"@en ;
        rdfs:comment		"Payload containing the data retrieved" ;
        rdfs:isDefinedBy <https://uri.etsi.org/ngsi-ld/v1/ngsi-ld-core-context-v1.6.jsonld> .

#################################################################
#    Data properties
#################################################################

###  http://foodie-cloud.com/model/foodie#alertDate
foodie:alertDate  a     owl:DatatypeProperty ;
        rdfs:range      xsd:dateTime ;
        skos:prefLabel  "alertDate"@en ;
         rdfs:label "alertDate" ;
        rdfs:comment "The date/time of the generated alert" ;
        rdfs:isDefinedBy <http://foodie-cloud.com/model/foodie> .

### https://smartdatamodels.org/dataModel.Weather/subCategory
fiware-weather:subCategory	a      owl:DatatypeProperty ;
        rdfs:label   		"subCategory"@en ;
        rdfs:comment		"Describe the sub category of alert, i.e., Weather categories, e.g., avalanches,coastalEvent, coldWave, flood, fog, forestFire, heatWave, highTemperature, hurricane, ice, lowTemperature, rainfall, rain_flood, snow, snow_ice, thunderstorms, tornado, tropicalCyclone, tsunami, wind" ;
        rdfs:isDefinedBy <https://github.com/smart-data-models/dataModel.Weather/blob/master/WeatherAlert/schema.json> .

### https://smartdatamodels.org/dataModel.Weather/dateIssued
fiware-weather:dateIssued	a      owl:DatatypeProperty ;
        rdfs:range      xsd:dateTime ;
        rdfs:label   		"dateIssued"@en ;
        rdfs:comment		"The date and time the item was issued in ISO8601 UTC format" ;
        rdfs:isDefinedBy <https://github.com/smart-data-models/dataModel.Weather/blob/master/WeatherAlert/schema.json> .

### https://smartdatamodels.org/dataModel.Weather/validFrom
fiware-weather:validFrom	a      owl:DatatypeProperty ;
        rdfs:range      xsd:dateTime ;
        rdfs:label   		"validFrom"@en ;
        rdfs:comment		"The start of the validity period for this weather alert as a ISO8601 format" ;
        rdfs:isDefinedBy <https://github.com/smart-data-models/dataModel.Weather/blob/master/WeatherAlert/doc/spec.md> .

### https://smartdatamodels.org/dataModel.Weather/validTo
fiware-weather:validTo	a      owl:DatatypeProperty ;
        rdfs:range      xsd:dateTime ;
        rdfs:label   		"validTo"@en ;
        rdfs:comment		"The end of the validity period for this weather alert as a ISO8601 format " ;
        rdfs:isDefinedBy <https://github.com/smart-data-models/dataModel.Weather/blob/master/WeatherAlert/doc/spec.md> .

### https://smartdatamodels.org/dataModel.Weather/alertSource
fiware-weather:alertSource	a      owl:DatatypeProperty ;
        rdfs:label   		"alertSource"@en ;
        rdfs:comment		"reference to the source of the alert. For example, it could be a user of an application, a device, or a service" ;
        rdfs:isDefinedBy <https://github.com/smart-data-models/dataModel.Weather/blob/master/WeatherAlert/schema.json> .

### https://smartdatamodels.org/dataModel.Weather/severity
fiware-weather:severity	a      owl:DatatypeProperty ;
        rdfs:label   		"severity"@en ;
        rdfs:comment		"define the level of gravity of a given alert" ;
        rdfs:isDefinedBy <https://smart-data-models.github.io/data-models/terms.jsonld#/definitions/severity> .

#################################################################
#    Classes
#################################################################

### http://foodie-cloud.com/model/foodie#Alert
foodie:Alert  a          owl:Class ;
        rdfs:subClassOf  geo:Feature ;
        rdfs:subClassOf  [ a                   owl:Restriction ;
                           owl:minCardinality  "1"^^xsd:int ;
                           owl:onProperty      foodie:alertGeometry
                         ] ;
        rdfs:subClassOf  [ a                owl:Restriction ;
                           owl:cardinality  "1"^^xsd:int ;
                           owl:onProperty   foodie:code
                         ] ;
        rdfs:subClassOf  [ a                owl:Restriction ;
                           owl:cardinality  "1"^^xsd:int ;
                           owl:onProperty   foodie:alertDate
                         ] ;
        rdfs:subClassOf  [ a                   owl:Restriction ;
                           owl:minCardinality  "1"^^xsd:int ;
                           owl:onProperty      foodie:type
                         ] ;
        rdfs:subClassOf  [ a                   owl:Restriction ;
                           owl:maxCardinality  "1"^^xsd:int ;
                           owl:onProperty      foodie:description
                         ] ;
        skos:prefLabel   "Alert"@en ;
        rdfs:label "Alert" ;
	rdfs:comment "Alerts automatically generated" ;
        rdfs:isDefinedBy <http://foodie-cloud.com/model/foodie> .

### https://smartdatamodels.org/dataModel.Weather/WeatherAlert
fiware-weather:Alert	a owl:Class ;
			rdfs:label "Alert" ;
			rdfs:comment "A weather alert generated by a user or device in a given location" ;
			rdfs:isDefinedBy <https://github.com/smart-data-models/dataModel.Weather/blob/master/WeatherAlert/schema.json> .

#################################################################
#    Alignments
#################################################################
foodie:Alert owl:equivalentClass fiware-weather:WeatherAlert .
fiware-weather:validFrom rdfs:subPropertyOf common:validFrom .
fiware-weather:validTo rdfs:subPropertyOf common:validTo .
foodie:alertGeometry rdfs:subPropertyOf geo:hasGeometry .


#################################################################
#    Individuals
#################################################################
