<?xml version="1.0"?>
<rdf:RDF xmlns="https://w3id.org/demeter/agri/agriProperty#"
     xml:base="https://w3id.org/demeter/agri/agriProperty"
     xmlns:obo="http://purl.obolibrary.org/obo/"
     xmlns:owl="http://www.w3.org/2002/07/owl#"
     xmlns:rdf="http://www.w3.org/1999/02/22-rdf-syntax-ns#"
     xmlns:ssn="http://www.w3.org/ns/ssn/"
     xmlns:xml="http://www.w3.org/XML/1998/namespace"
     xmlns:xsd="http://www.w3.org/2001/XMLSchema#"
     xmlns:foaf="http://xmlns.com/foaf/0.1/"
     xmlns:rdfs="http://www.w3.org/2000/01/rdf-schema#"
     xmlns:skos="http://www.w3.org/2004/02/skos/core#"
     xmlns:terms="http://purl.org/dc/terms/"
     xmlns:schema="https://schema.org/"
     xmlns:agriCommon="https://w3id.org/demeter/agri/agriCommon#"
     xmlns:smartdatamodels="https://smartdatamodels.org/">
    <owl:Ontology rdf:about="https://w3id.org/demeter/agri/agriProperty">
        <owl:versionIRI rdf:resource="https://w3id.org/demeter/agri/agriProperty/2.0"/>
        <owl:imports rdf:resource="https://w3id.org/demeter/agri/agriCommon"/>
        <terms:contributor rdf:resource="_:genid-nodeid-node1grit1nc2x3"/>
        <terms:contributor rdf:resource="_:genid-nodeid-node1grit1nc2x5"/>
        <terms:contributor rdf:nodeID="genid1"/>
        <terms:contributor rdf:nodeID="genid3"/>
        <terms:contributor rdf:nodeID="genid5"/>
        <terms:creator rdf:nodeID="genid7"/>
        <terms:description xml:lang="en">The DEMETER AgriProperty is one of the agri profiles of DEMETER AIM. This profile was created by reusing and aligning well-known ontologies and vocabularies</terms:description>
        <terms:rights xml:lang="en">This vocabulary is distributed under Creative Commons Attribution 4.0 License - http://creativecommons.org/licenses/by/4.0</terms:rights>
        <terms:title xml:lang="en">DEMETER AgriProperty</terms:title>
        <rdfs:comment xml:lang="en">The DEMETER Agriculture Information Model (AIM) is the common vocabulary in DEMETER project providing the basis for semantic interoperability across smart farming solutions</rdfs:comment>
        <rdfs:label>DEMETER AgriProperty</rdfs:label>
        <owl:versionInfo>2.0</owl:versionInfo>
        <foaf:maker rdf:nodeID="genid9"/>
    </owl:Ontology>
    <rdf:Description rdf:nodeID="genid1">
        <foaf:name>Rob Atkinson</foaf:name>
        <schema:affiliation>
            <rdf:Description>
                <foaf:name>OGC</foaf:name>
            </rdf:Description>
        </schema:affiliation>
    </rdf:Description>
    <rdf:Description rdf:nodeID="genid3">
        <foaf:name>Ioanna Roussaki</foaf:name>
        <schema:affiliation>
            <rdf:Description>
                <foaf:name>ICCS</foaf:name>
            </rdf:Description>
        </schema:affiliation>
    </rdf:Description>
    <rdf:Description rdf:nodeID="genid5">
        <foaf:name>George Routis</foaf:name>
        <schema:affiliation>
            <rdf:Description>
                <foaf:name>ICCS</foaf:name>
            </rdf:Description>
        </schema:affiliation>
    </rdf:Description>
    <rdf:Description rdf:nodeID="genid7">
        <rdfs:seeAlso rdf:resource="http://orcid.org/0000-0003-4289-4922"/>
        <foaf:name>Raul Palma</foaf:name>
        <schema:affiliation>
            <rdf:Description>
                <foaf:name>PSNC</foaf:name>
            </rdf:Description>
        </schema:affiliation>
    </rdf:Description>
    <rdf:Description rdf:nodeID="genid9">
        <foaf:homepage rdf:resource="https://h2020-demeter.eu/"/>
        <foaf:name>DEMETER project</foaf:name>
    </rdf:Description>
    


    <!-- 
    ///////////////////////////////////////////////////////////////////////////////////////
    //
    // Object Properties
    //
    ///////////////////////////////////////////////////////////////////////////////////////
     -->


    


    <!-- http://foodie-cloud.com/model/foodie#productionAmount -->


    <owl:ObjectProperty rdf:about="http://foodie-cloud.com/model/foodie#productionAmount">
        <rdfs:subPropertyOf rdf:resource="http://www.w3.org/ns/sosa/hasResult"/>
    </owl:ObjectProperty>
    


    <!-- http://foodie-cloud.com/model/foodie#productionProperty -->


    <owl:ObjectProperty rdf:about="http://foodie-cloud.com/model/foodie#productionProperty">
        <rdfs:range rdf:resource="http://foodie-cloud.com/model/foodie#PropertyType"/>
        <rdfs:comment>Relation between a ProductionType and PropertyType</rdfs:comment>
        <rdfs:isDefinedBy rdf:resource="http://foodie-cloud.com/model/foodie"/>
        <rdfs:label>productionProperty</rdfs:label>
        <skos:prefLabel xml:lang="en">productionProperty</skos:prefLabel>
    </owl:ObjectProperty>
    


    <!-- http://foodie-cloud.com/model/foodie#propertyType -->


    <owl:ObjectProperty rdf:about="http://foodie-cloud.com/model/foodie#propertyType">
        <owl:equivalentProperty rdf:resource="https://saref.etsi.org/core/relatesToProperty"/>
        <rdfs:range rdf:resource="http://foodie-cloud.com/model/foodie#PropertyTypeValue"/>
        <rdfs:comment>Relation between a PropertyType and PropertyTypeValue</rdfs:comment>
        <rdfs:isDefinedBy rdf:resource="http://foodie-cloud.com/model/foodie"/>
        <rdfs:label>propertyType</rdfs:label>
        <skos:prefLabel xml:lang="en">propertyType</skos:prefLabel>
    </owl:ObjectProperty>
    


    <!-- http://foodie-cloud.com/model/foodie#quantitativeProperty -->


    <owl:ObjectProperty rdf:about="http://foodie-cloud.com/model/foodie#quantitativeProperty">
        <owl:equivalentProperty rdf:resource="http://www.w3.org/ns/sosa/hasResult"/>
        <rdfs:range rdf:resource="http://def.seegrid.csiro.au/isotc211/iso19103/2005/basic#Measure"/>
        <rdfs:comment>Relation between a PropertyType and Measure</rdfs:comment>
        <rdfs:isDefinedBy rdf:resource="http://foodie-cloud.com/model/foodie"/>
        <rdfs:label>quantitativeProperty</rdfs:label>
        <skos:prefLabel xml:lang="en">quantitativeProperty</skos:prefLabel>
    </owl:ObjectProperty>
    


    <!-- http://foodie-cloud.com/model/foodie#soilProperty -->


    <owl:ObjectProperty rdf:about="http://foodie-cloud.com/model/foodie#soilProperty">
        <rdfs:range rdf:resource="http://foodie-cloud.com/model/foodie#PropertyType"/>
        <rdfs:comment>Relation between a ManagementZone and PropertyType</rdfs:comment>
        <rdfs:isDefinedBy rdf:resource="http://foodie-cloud.com/model/foodie"/>
        <rdfs:label>soilProperty</rdfs:label>
        <skos:prefLabel xml:lang="en">soilProperty</skos:prefLabel>
    </owl:ObjectProperty>
    


    <!-- http://qudt.org/schema/qudt/unit -->


    <rdf:Description rdf:about="http://qudt.org/schema/qudt/unit">
        <owl:equivalentProperty rdf:resource="https://saref.etsi.org/core/isMeasuredIn"/>
    </rdf:Description>
    


    <!-- http://www.w3.org/ns/sosa/hasFeatureOfInterest -->


    <rdf:Description rdf:about="http://www.w3.org/ns/sosa/hasFeatureOfInterest">
        <owl:equivalentProperty rdf:resource="https://saref.etsi.org/core/hasFeatureOfInterest"/>
    </rdf:Description>
    


    <!-- http://www.w3.org/ns/sosa/isFeatureOfInterestOf -->


    <rdf:Description rdf:about="http://www.w3.org/ns/sosa/isFeatureOfInterestOf">
        <owl:equivalentProperty rdf:resource="https://saref.etsi.org/core/isFeatureOfInterestOf"/>
    </rdf:Description>
    


    <!-- http://www.w3.org/ns/sosa/madeBySensor -->


    <rdf:Description rdf:about="http://www.w3.org/ns/sosa/madeBySensor">
        <owl:equivalentProperty rdf:resource="https://saref.etsi.org/core/measurementMadeBy"/>
    </rdf:Description>
    


    <!-- http://www.w3.org/ns/sosa/madeObservation -->


    <rdf:Description rdf:about="http://www.w3.org/ns/sosa/madeObservation">
        <owl:equivalentProperty rdf:resource="https://saref.etsi.org/core/makesMeasurement"/>
    </rdf:Description>
    


    <!-- http://www.w3.org/ns/sosa/observedProperty -->


    <rdf:Description rdf:about="http://www.w3.org/ns/sosa/observedProperty">
        <owl:equivalentProperty rdf:resource="https://saref.etsi.org/core/relatesToProperty"/>
    </rdf:Description>
    


    <!-- http://www.w3.org/ns/ssn/hasProperty -->


    <rdf:Description rdf:about="http://www.w3.org/ns/ssn/hasProperty">
        <owl:equivalentProperty rdf:resource="https://saref.etsi.org/core/hasProperty"/>
    </rdf:Description>
    


    <!-- http://www.w3.org/ns/ssn/isPropertyOf -->


    <rdf:Description rdf:about="http://www.w3.org/ns/ssn/isPropertyOf">
        <owl:equivalentProperty rdf:resource="https://saref.etsi.org/core/isPropertyOf"/>
    </rdf:Description>
    


    <!-- https://saref.etsi.org/core/controlsProperty -->


    <owl:ObjectProperty rdf:about="https://saref.etsi.org/core/controlsProperty">
        <rdfs:comment>A relationship specifying the Property that can be controlled by a certain Device</rdfs:comment>
        <rdfs:isDefinedBy rdf:resource="https://saref.etsi.org/core/"/>
        <rdfs:label xml:lang="en">controls property</rdfs:label>
    </owl:ObjectProperty>
    


    <!-- https://saref.etsi.org/core/hasFeatureOfInterest -->


    <owl:ObjectProperty rdf:about="https://saref.etsi.org/core/hasFeatureOfInterest">
        <owl:inverseOf rdf:resource="https://saref.etsi.org/core/isFeatureOfInterestOf"/>
        <rdfs:comment xml:lang="en">Relation between a measurement and the feature of interest being measured.</rdfs:comment>
        <rdfs:isDefinedBy rdf:resource="https://saref.etsi.org/core/"/>
        <rdfs:label xml:lang="en">has feature of interest</rdfs:label>
    </owl:ObjectProperty>
    


    <!-- https://saref.etsi.org/core/hasProperty -->


    <owl:ObjectProperty rdf:about="https://saref.etsi.org/core/hasProperty">
        <owl:inverseOf rdf:resource="https://saref.etsi.org/core/isPropertyOf"/>
        <rdfs:comment xml:lang="en">Relation between a feature of interest and its properties.</rdfs:comment>
        <rdfs:isDefinedBy rdf:resource="https://saref.etsi.org/core/"/>
        <rdfs:label xml:lang="en">has property</rdfs:label>
    </owl:ObjectProperty>
    


    <!-- https://saref.etsi.org/core/isControlledByDevice -->


    <owl:ObjectProperty rdf:about="https://saref.etsi.org/core/isControlledByDevice">
        <rdfs:comment>A relationship specifying the devices that can control a certain property</rdfs:comment>
        <rdfs:isDefinedBy rdf:resource="https://saref.etsi.org/core/"/>
        <rdfs:label xml:lang="en">is controlled by device</rdfs:label>
    </owl:ObjectProperty>
    


    <!-- https://saref.etsi.org/core/isFeatureOfInterestOf -->


    <owl:ObjectProperty rdf:about="https://saref.etsi.org/core/isFeatureOfInterestOf">
        <rdfs:comment xml:lang="en">Relation betwwen a feature of interest and the measurments that are about it.</rdfs:comment>
        <rdfs:isDefinedBy rdf:resource="https://saref.etsi.org/core/"/>
        <rdfs:label xml:lang="en">is feature of interest of</rdfs:label>
    </owl:ObjectProperty>
    


    <!-- https://saref.etsi.org/core/isMeasuredByDevice -->


    <owl:ObjectProperty rdf:about="https://saref.etsi.org/core/isMeasuredByDevice">
        <rdfs:comment>A relationship specifying the devices that can measure a certain property</rdfs:comment>
        <rdfs:isDefinedBy rdf:resource="https://saref.etsi.org/core/"/>
        <rdfs:label xml:lang="en">is measured by device</rdfs:label>
    </owl:ObjectProperty>
    


    <!-- https://saref.etsi.org/core/isMeasuredIn -->


    <owl:ObjectProperty rdf:about="https://saref.etsi.org/core/isMeasuredIn">
        <rdfs:comment>A relationship identifying the unit of measure used for a certain entity.</rdfs:comment>
        <rdfs:isDefinedBy rdf:resource="https://saref.etsi.org/core/"/>
        <rdfs:label xml:lang="en">is measured in</rdfs:label>
    </owl:ObjectProperty>
    


    <!-- https://saref.etsi.org/core/isPropertyOf -->


    <owl:ObjectProperty rdf:about="https://saref.etsi.org/core/isPropertyOf">
        <rdfs:comment xml:lang="en">Relation between a property and a feature of interest in which such property appears.</rdfs:comment>
        <rdfs:isDefinedBy rdf:resource="https://saref.etsi.org/core/"/>
        <rdfs:label xml:lang="en">is property of</rdfs:label>
    </owl:ObjectProperty>
    


    <!-- https://saref.etsi.org/core/makesMeasurement -->


    <owl:ObjectProperty rdf:about="https://saref.etsi.org/core/makesMeasurement">
        <owl:inverseOf rdf:resource="https://saref.etsi.org/core/measurementMadeBy"/>
        <rdfs:comment>A relation between a device and the measurements it makes. Such measurement will link together the value of the measurement, its unit of measure and the property to which it relates.</rdfs:comment>
        <rdfs:isDefinedBy rdf:resource="https://saref.etsi.org/core/"/>
        <rdfs:label xml:lang="en">makes measurement</rdfs:label>
    </owl:ObjectProperty>
    


    <!-- https://saref.etsi.org/core/measurementMadeBy -->


    <owl:ObjectProperty rdf:about="https://saref.etsi.org/core/measurementMadeBy">
        <owl:equivalentProperty rdf:resource="https://smartdatamodels.org/dataModel.Weather/refDevice"/>
        <rdfs:comment xml:lang="en">Relation between a measurement and the device that made it.</rdfs:comment>
        <rdfs:isDefinedBy rdf:resource="https://saref.etsi.org/core/"/>
        <rdfs:label xml:lang="en">measurement made by</rdfs:label>
    </owl:ObjectProperty>
    


    <!-- https://saref.etsi.org/core/measuresProperty -->


    <owl:ObjectProperty rdf:about="https://saref.etsi.org/core/measuresProperty">
        <rdfs:comment>A relationship specifying the Property that can be measured by a certain Device</rdfs:comment>
        <rdfs:isDefinedBy rdf:resource="https://saref.etsi.org/core/"/>
        <rdfs:label xml:lang="en">measures property</rdfs:label>
    </owl:ObjectProperty>
    


    <!-- https://saref.etsi.org/core/relatesToMeasurement -->


    <owl:ObjectProperty rdf:about="https://saref.etsi.org/core/relatesToMeasurement">
        <rdfs:comment>A relationship between a property and the measurements it relates to</rdfs:comment>
        <rdfs:isDefinedBy rdf:resource="https://saref.etsi.org/core/"/>
        <rdfs:label xml:lang="en">relates to measurement</rdfs:label>
    </owl:ObjectProperty>
    


    <!-- https://saref.etsi.org/core/relatesToProperty -->


    <owl:ObjectProperty rdf:about="https://saref.etsi.org/core/relatesToProperty">
        <rdfs:comment>A relationship between a measurement and the property it relates to</rdfs:comment>
        <rdfs:isDefinedBy rdf:resource="https://saref.etsi.org/core/"/>
        <rdfs:label xml:lang="en">relates to property</rdfs:label>
    </owl:ObjectProperty>
    


    <!-- https://smartdatamodels.org/dataModel.Agrifood/hasAgriParcel -->


    <owl:ObjectProperty rdf:about="https://smartdatamodels.org/dataModel.Agrifood/hasAgriParcel">
        <rdfs:comment>A reference to the AgriParcel</rdfs:comment>
        <rdfs:isDefinedBy rdf:resource="https://github.com/smart-data-models/dataModel.Agrifood/blob/master/AgriParcelRecord/schema.json"/>
        <rdfs:label xml:lang="en">hasAgriParcel</rdfs:label>
    </owl:ObjectProperty>
    


    <!-- https://smartdatamodels.org/dataModel.Agrifood/hasDevice -->


    <owl:ObjectProperty rdf:about="https://smartdatamodels.org/dataModel.Agrifood/hasDevice">
        <rdfs:comment>Reference to the IoT devices associated with this [entity] i.e. sensors, controls.</rdfs:comment>
        <rdfs:isDefinedBy rdf:resource="https://github.com/GSMADeveloper/NGSI-LD-Entities/blob/master/definitions/Agri-Parcel.md"/>
        <rdfs:isDefinedBy rdf:resource="https://github.com/smart-data-models/dataModel.Agrifood/blob/master/AgriParcelRecord/schema.json"/>
        <rdfs:label xml:lang="en">hasDevice</rdfs:label>
    </owl:ObjectProperty>
    


    <!-- https://smartdatamodels.org/dataModel.Weather/refDevice -->


    <owl:ObjectProperty rdf:about="https://smartdatamodels.org/dataModel.Weather/refDevice">
        <rdfs:comment>A reference to the device(s) which captured this observation.</rdfs:comment>
        <rdfs:isDefinedBy rdf:resource="https://github.com/smart-data-models/dataModel.Weather/blob/master/WeatherObserved/schema.json"/>
        <rdfs:label xml:lang="en">refDevice</rdfs:label>
    </owl:ObjectProperty>
    


    <!-- https://smartdatamodels.org/dataModel.Weather/refPointOfInterest -->


    <owl:ObjectProperty rdf:about="https://smartdatamodels.org/dataModel.Weather/refPointOfInterest">
        <rdfs:comment>Point of interest related to the item</rdfs:comment>
        <rdfs:isDefinedBy rdf:resource="https://github.com/smart-data-models/dataModel.Weather/blob/master/weather-schema.json"/>
        <rdfs:label xml:lang="en">refPointOfInterest</rdfs:label>
    </owl:ObjectProperty>
    


    <!-- 
    ///////////////////////////////////////////////////////////////////////////////////////
    //
    // Data properties
    //
    ///////////////////////////////////////////////////////////////////////////////////////
     -->


    


    <!-- http://foodie-cloud.com/model/foodie#analysisDate -->


    <owl:DatatypeProperty rdf:about="http://foodie-cloud.com/model/foodie#analysisDate">
        <rdfs:subPropertyOf rdf:resource="https://saref.etsi.org/core/hasTimestamp"/>
        <rdfs:range rdf:resource="http://www.w3.org/2001/XMLSchema#dateTime"/>
        <rdfs:comment>The date/time of a recorded analysis</rdfs:comment>
        <rdfs:isDefinedBy rdf:resource="http://foodie-cloud.com/model/foodie"/>
        <rdfs:label>analysisDate</rdfs:label>
        <skos:prefLabel xml:lang="en">analysisDate</skos:prefLabel>
    </owl:DatatypeProperty>
    


    <!-- http://foodie-cloud.com/model/foodie#nonQuantitativeProperty -->


    <owl:DatatypeProperty rdf:about="http://foodie-cloud.com/model/foodie#nonQuantitativeProperty">
        <rdfs:subPropertyOf rdf:resource="https://saref.etsi.org/core/hasValue"/>
        <rdfs:range rdf:resource="http://www.w3.org/2001/XMLSchema#string"/>
        <rdfs:comment>The name of a non quantitative property </rdfs:comment>
        <rdfs:isDefinedBy rdf:resource="http://foodie-cloud.com/model/foodie"/>
        <rdfs:label>nonQuantitativeProperty</rdfs:label>
        <skos:prefLabel xml:lang="en">nonQuantitativeProperty</skos:prefLabel>
    </owl:DatatypeProperty>
    


    <!-- http://foodie-cloud.com/model/foodie#propertyName -->


    <owl:DatatypeProperty rdf:about="http://foodie-cloud.com/model/foodie#propertyName">
        <rdfs:subPropertyOf rdf:resource="https://smartdatamodels.org/name"/>
        <rdfs:range rdf:resource="http://www.w3.org/2001/XMLSchema#string"/>
        <rdfs:comment>The name of an agricultural property</rdfs:comment>
        <rdfs:isDefinedBy rdf:resource="http://foodie-cloud.com/model/foodie"/>
        <rdfs:label>propertyName</rdfs:label>
        <skos:prefLabel xml:lang="en">propertyName</skos:prefLabel>
    </owl:DatatypeProperty>
    


    <!-- http://www.w3.org/ns/sosa/hasSimpleResult -->


    <rdf:Description rdf:about="http://www.w3.org/ns/sosa/hasSimpleResult">
        <owl:equivalentProperty rdf:resource="https://saref.etsi.org/core/hasValue"/>
    </rdf:Description>
    


    <!-- http://www.w3.org/ns/sosa/resultTime -->


    <rdf:Description rdf:about="http://www.w3.org/ns/sosa/resultTime">
        <owl:equivalentProperty rdf:resource="https://saref.etsi.org/core/hasTimestamp"/>
    </rdf:Description>
    


    <!-- https://saref.etsi.org/core/hasValue -->


    <owl:DatatypeProperty rdf:about="https://saref.etsi.org/core/hasValue">
        <rdfs:comment>A relationship defining the value of a certain property, e.g., energy or power</rdfs:comment>
        <rdfs:isDefinedBy rdf:resource="https://saref.etsi.org/core/"/>
        <rdfs:label xml:lang="en">has value</rdfs:label>
    </owl:DatatypeProperty>
    


    <!-- https://smartdatamodels.org/dateObserved -->


    <owl:DatatypeProperty rdf:about="https://smartdatamodels.org/dateObserved">
        <rdfs:subPropertyOf rdf:resource="https://saref.etsi.org/core/hasTimestamp"/>
    </owl:DatatypeProperty>
    


    <!-- https://smartdatamodels.org/observedAt -->


    <owl:DatatypeProperty rdf:about="https://smartdatamodels.org/observedAt">
        <rdfs:range rdf:resource="http://www.w3.org/2001/XMLSchema#dateTime"/>
        <rdfs:comment>Date of the observed entity defined by the user</rdfs:comment>
        <rdfs:isDefinedBy rdf:resource="https://smart-data-models.github.io/data-models/common-schema.json#/definitions/dateObserved"/>
        <rdfs:label xml:lang="en">date observed</rdfs:label>
    </owl:DatatypeProperty>
    


    <!-- https://smartdatamodels.org/dataModel.Agrifood/relativeHumidity -->


    <owl:DatatypeProperty rdf:about="https://smartdatamodels.org/dataModel.Agrifood/relativeHumidity">
        <rdfs:subPropertyOf rdf:resource="https://saref.etsi.org/core/hasValue"/>
        <rdfs:comment>Relative Humidity a number between 0 and 1 representing the range of 0% to 100%. 0 ≤ relativeHumidity ≤ 1</rdfs:comment>
        <rdfs:isDefinedBy rdf:resource="https://github.com/smart-data-models/dataModel.Agrifood/blob/master/AgriParcelRecord/schema.json"/>
        <rdfs:label xml:lang="en">relativeHumidity</rdfs:label>
    </owl:DatatypeProperty>
    


    <!-- https://smartdatamodels.org/dataModel.Agrifood/soilMoistureEC -->


    <owl:DatatypeProperty rdf:about="https://smartdatamodels.org/dataModel.Agrifood/soilMoistureEC">
        <rdfs:subPropertyOf rdf:resource="https://saref.etsi.org/core/hasValue"/>
    </owl:DatatypeProperty>
    


    <!-- https://smartdatamodels.org/dataModel.Agrifood/soilMoistureEc -->


    <owl:DatatypeProperty rdf:about="https://smartdatamodels.org/dataModel.Agrifood/soilMoistureEc">
        <rdfs:comment>Measured as Electrical Conductivity, EC nominally in units of Siemens per meter. Units:&apos;siemens / m&apos;</rdfs:comment>
        <rdfs:isDefinedBy rdf:resource="https://github.com/smart-data-models/dataModel.Agrifood/blob/master/AgriParcelRecord/schema.json"/>
        <rdfs:label xml:lang="en">soilMoistureEC</rdfs:label>
    </owl:DatatypeProperty>
    


    <!-- https://smartdatamodels.org/dataModel.Agrifood/soilMoistureVwc -->


    <owl:DatatypeProperty rdf:about="https://smartdatamodels.org/dataModel.Agrifood/soilMoistureVwc">
        <rdfs:subPropertyOf rdf:resource="https://saref.etsi.org/core/hasValue"/>
        <rdfs:comment>Measured as Volumetric Water Content, VWC as a percentage. 0 ≤soilMoistureVwc ≤ 1</rdfs:comment>
        <rdfs:isDefinedBy rdf:resource="https://github.com/smart-data-models/dataModel.Agrifood/blob/master/AgriParcelRecord/schema.json"/>
        <rdfs:label xml:lang="en">soilMoistureVwc</rdfs:label>
    </owl:DatatypeProperty>
    


    <!-- https://smartdatamodels.org/dataModel.Agrifood/soilTemperature -->


    <owl:DatatypeProperty rdf:about="https://smartdatamodels.org/dataModel.Agrifood/soilTemperature">
        <rdfs:subPropertyOf rdf:resource="https://saref.etsi.org/core/hasValue"/>
        <rdfs:comment>TThe observed soil temperature nominally in degrees centigrade. Units:&apos;degrees centigrade&apos;</rdfs:comment>
        <rdfs:isDefinedBy rdf:resource="https://github.com/smart-data-models/dataModel.Agrifood/blob/master/AgriParcelRecord/schema.json"/>
        <rdfs:label xml:lang="en">soilTemperature</rdfs:label>
    </owl:DatatypeProperty>
    


    <!-- https://smartdatamodels.org/dataModel.Agrifood/solarRadiation -->


    <owl:DatatypeProperty rdf:about="https://smartdatamodels.org/dataModel.Agrifood/solarRadiation">
        <rdfs:subPropertyOf rdf:resource="https://saref.etsi.org/core/hasValue"/>
        <rdfs:comment>Instantaneous solar radiation measured in kW/m2. Units:&apos;kW/m2&apos;</rdfs:comment>
        <rdfs:isDefinedBy rdf:resource="https://github.com/smart-data-models/dataModel.Agrifood/blob/master/AgriParcelRecord/schema.json"/>
        <rdfs:label xml:lang="en">solarRadiation</rdfs:label>
    </owl:DatatypeProperty>
    


    <!-- https://smartdatamodels.org/dataModel.Weather/airTemperatureForecast -->


    <owl:DatatypeProperty rdf:about="https://smartdatamodels.org/dataModel.Weather/airTemperatureForecast">
        <rdfs:subPropertyOf rdf:resource="https://saref.etsi.org/core/hasValue"/>
        <rdfs:comment>Forecasted value of air temperature over a certain duration in future</rdfs:comment>
        <rdfs:isDefinedBy rdf:resource="https://github.com/smart-data-models/dataModel.Weather/blob/master/WeatherObserved/schema.json"/>
        <rdfs:label xml:lang="en">airTemperatureForecast</rdfs:label>
    </owl:DatatypeProperty>
    


    <!-- https://smartdatamodels.org/dataModel.Weather/atmosphericPressure -->


    <owl:DatatypeProperty rdf:about="https://smartdatamodels.org/dataModel.Weather/atmosphericPressure">
        <rdfs:subPropertyOf rdf:resource="https://saref.etsi.org/core/hasValue"/>
        <rdfs:comment>The atmospheric pressure observed measured in Hecto Pascals. Units:&apos;Hecto pascals&apos;</rdfs:comment>
        <rdfs:isDefinedBy rdf:resource="https://github.com/smart-data-models/dataModel.Weather/blob/master/weather-schema.json"/>
        <rdfs:label xml:lang="en">atmosphericPressure</rdfs:label>
    </owl:DatatypeProperty>
    


    <!-- https://smartdatamodels.org/dataModel.Weather/dewPoint -->


    <owl:DatatypeProperty rdf:about="https://smartdatamodels.org/dataModel.Weather/dewPoint">
        <rdfs:subPropertyOf rdf:resource="https://saref.etsi.org/core/hasValue"/>
        <rdfs:comment>The dew point encoded as a number. Observed temperature to which air must be cooled to become saturated with water vapor</rdfs:comment>
        <rdfs:isDefinedBy rdf:resource="https://github.com/smart-data-models/dataModel.Weather/blob/master/WeatherObserved/schema.json"/>
        <rdfs:label xml:lang="en">dewPoint</rdfs:label>
    </owl:DatatypeProperty>
    


    <!-- https://smartdatamodels.org/dataModel.Weather/illuminance -->


    <owl:DatatypeProperty rdf:about="https://smartdatamodels.org/dataModel.Weather/illuminance">
        <rdfs:subPropertyOf rdf:resource="https://saref.etsi.org/core/hasValue"/>
        <rdfs:comment>The illumninance observed measured in lux (lx) or lumens per square metre (cd·sr·m−2)</rdfs:comment>
        <rdfs:isDefinedBy rdf:resource="https://github.com/smart-data-models/dataModel.Weather/blob/master/weather-schema.json"/>
        <rdfs:label xml:lang="en">illuminance</rdfs:label>
    </owl:DatatypeProperty>
    


    <!-- https://smartdatamodels.org/dataModel.Weather/precipitation -->


    <owl:DatatypeProperty rdf:about="https://smartdatamodels.org/dataModel.Weather/precipitation">
        <rdfs:subPropertyOf rdf:resource="https://saref.etsi.org/core/hasValue"/>
        <rdfs:comment>Amount of water rain registered. Units:&apos;Liters per square meter&apos;</rdfs:comment>
        <rdfs:isDefinedBy rdf:resource="https://github.com/smart-data-models/dataModel.Weather/blob/master/WeatherObserved/schema.json"/>
        <rdfs:label xml:lang="en">precipitation</rdfs:label>
    </owl:DatatypeProperty>
    


    <!-- https://smartdatamodels.org/dataModel.Weather/pressureTendency -->


    <owl:DatatypeProperty rdf:about="https://smartdatamodels.org/dataModel.Weather/pressureTendency">
        <rdfs:subPropertyOf rdf:resource="https://saref.etsi.org/core/hasValue"/>
        <rdfs:comment>Is the pressure rising or falling? It can be expressed in quantitative terms or qualitative terms (raising, falling, steady)</rdfs:comment>
        <rdfs:isDefinedBy rdf:resource="https://github.com/smart-data-models/dataModel.Weather/blob/master/WeatherObserved/schema.json"/>
        <rdfs:label xml:lang="en">pressureTendency</rdfs:label>
    </owl:DatatypeProperty>
    


    <!-- https://smartdatamodels.org/dataModel.Weather/relativeHumidity -->


    <owl:DatatypeProperty rdf:about="https://smartdatamodels.org/dataModel.Weather/relativeHumidity">
        <rdfs:subPropertyOf rdf:resource="https://saref.etsi.org/core/hasValue"/>
        <rdfs:comment>Humidity in the Air. Observed instantaneous relative humidity (water vapour in air)</rdfs:comment>
        <rdfs:isDefinedBy rdf:resource="https://github.com/smart-data-models/dataModel.Weather/blob/master/weather-schema.json"/>
        <rdfs:label xml:lang="en">relativeHumidity</rdfs:label>
    </owl:DatatypeProperty>
    


    <!-- https://smartdatamodels.org/dataModel.Weather/snowHeight -->


    <owl:DatatypeProperty rdf:about="https://smartdatamodels.org/dataModel.Weather/snowHeight">
        <rdfs:subPropertyOf rdf:resource="https://saref.etsi.org/core/hasValue"/>
        <rdfs:comment>The snow height observed by generic snow depth measurement sensors, expressed in centimeters. Units:&apos;centimeters&apos;</rdfs:comment>
        <rdfs:isDefinedBy rdf:resource="https://github.com/smart-data-models/dataModel.Weather/blob/master/WeatherObserved/schema.json"/>
        <rdfs:label xml:lang="en">snowHeight</rdfs:label>
    </owl:DatatypeProperty>
    


    <!-- https://smartdatamodels.org/dataModel.Weather/solarRadiation -->


    <owl:DatatypeProperty rdf:about="https://smartdatamodels.org/dataModel.Weather/solarRadiation">
        <rdfs:subPropertyOf rdf:resource="https://saref.etsi.org/core/hasValue"/>
        <rdfs:comment>The solar radiation observed measured in Watts per square. Units:&apos;w/m2&apos;</rdfs:comment>
        <rdfs:isDefinedBy rdf:resource="https://github.com/smart-data-models/dataModel.Weather/blob/master/WeatherObserved/schema.json"/>
        <rdfs:label xml:lang="en">solarRadiation</rdfs:label>
    </owl:DatatypeProperty>
    


    <!-- https://smartdatamodels.org/dataModel.Weather/streamGauge -->


    <owl:DatatypeProperty rdf:about="https://smartdatamodels.org/dataModel.Weather/streamGauge">
        <rdfs:subPropertyOf rdf:resource="https://saref.etsi.org/core/hasValue"/>
        <rdfs:comment>The water level surface elevation observed by Hydrometric measurement sensors, namely a Stream Gauge expressed in centimeters. Units:&apos;centimeters&apos;</rdfs:comment>
        <rdfs:isDefinedBy rdf:resource="https://github.com/smart-data-models/dataModel.Weather/blob/master/WeatherObserved/schema.json"/>
        <rdfs:label xml:lang="en">streamGauge</rdfs:label>
    </owl:DatatypeProperty>
    


    <!-- https://smartdatamodels.org/dataModel.Weather/temperature -->


    <owl:DatatypeProperty rdf:about="https://smartdatamodels.org/dataModel.Weather/temperature">
        <rdfs:subPropertyOf rdf:resource="https://saref.etsi.org/core/hasValue"/>
        <rdfs:comment>Temperature of the item. Prev: The observed air temperature (in the shade) nominally in degrees centigrade.</rdfs:comment>
        <rdfs:isDefinedBy rdf:resource="https://github.com/smart-data-models/dataModel.Weather/blob/master/WeatherObserved/schema.json"/>
        <rdfs:label xml:lang="en">temperature</rdfs:label>
    </owl:DatatypeProperty>
    


    <!-- https://smartdatamodels.org/dataModel.Weather/visibility -->


    <owl:DatatypeProperty rdf:about="https://smartdatamodels.org/dataModel.Weather/visibility">
        <rdfs:subPropertyOf rdf:resource="https://saref.etsi.org/core/hasValue"/>
        <rdfs:comment>Categories of visibility. Prev: Visibility reported (veryPoor, poor, moderate, good, veryGood, excellent)</rdfs:comment>
        <rdfs:isDefinedBy rdf:resource="https://github.com/smart-data-models/dataModel.Weather/blob/master/weather-schema.json"/>
        <rdfs:label xml:lang="en">visibility</rdfs:label>
    </owl:DatatypeProperty>
    


    <!-- https://smartdatamodels.org/dataModel.Weather/weatherType -->


    <owl:DatatypeProperty rdf:about="https://smartdatamodels.org/dataModel.Weather/weatherType">
        <rdfs:comment>Text description of the weather. Prev: The observed weather type. It is represented by a comma separated list of weather statuses, for instance overcast, lightRain.</rdfs:comment>
        <rdfs:isDefinedBy rdf:resource="https://github.com/smart-data-models/dataModel.Weather/blob/master/weather-schema.json"/>
        <rdfs:label xml:lang="en">weatherType</rdfs:label>
    </owl:DatatypeProperty>
    


    <!-- https://smartdatamodels.org/dataModel.Weather/windDirection -->


    <owl:DatatypeProperty rdf:about="https://smartdatamodels.org/dataModel.Weather/windDirection">
        <rdfs:subPropertyOf rdf:resource="https://saref.etsi.org/core/hasValue"/>
        <rdfs:comment>Direction of the wind bet</rdfs:comment>
        <rdfs:isDefinedBy rdf:resource="https://github.com/smart-data-models/dataModel.Weather/blob/master/weather-schema.json"/>
        <rdfs:label xml:lang="en">windDirection</rdfs:label>
    </owl:DatatypeProperty>
    


    <!-- https://smartdatamodels.org/dataModel.Weather/windSpeed -->


    <owl:DatatypeProperty rdf:about="https://smartdatamodels.org/dataModel.Weather/windSpeed">
        <rdfs:subPropertyOf rdf:resource="https://saref.etsi.org/core/hasValue"/>
        <rdfs:comment>Intensity of the wind.</rdfs:comment>
        <rdfs:isDefinedBy rdf:resource="https://github.com/smart-data-models/dataModel.Weather/blob/master/weather-schema.json"/>
        <rdfs:label xml:lang="en">windSpeed</rdfs:label>
    </owl:DatatypeProperty>
    


    <!-- 
    ///////////////////////////////////////////////////////////////////////////////////////
    //
    // Classes
    //
    ///////////////////////////////////////////////////////////////////////////////////////
     -->


    


    <!-- http://foodie-cloud.com/model/foodie#PropertyType -->


    <owl:Class rdf:about="http://foodie-cloud.com/model/foodie#PropertyType">
        <rdfs:subClassOf>
            <owl:Restriction>
                <owl:onProperty rdf:resource="http://foodie-cloud.com/model/foodie#propertyType"/>
                <owl:maxCardinality rdf:datatype="http://www.w3.org/2001/XMLSchema#nonNegativeInteger">1</owl:maxCardinality>
            </owl:Restriction>
        </rdfs:subClassOf>
        <rdfs:subClassOf>
            <owl:Restriction>
                <owl:onProperty rdf:resource="http://foodie-cloud.com/model/foodie#quantitativeProperty"/>
                <owl:maxCardinality rdf:datatype="http://www.w3.org/2001/XMLSchema#nonNegativeInteger">1</owl:maxCardinality>
            </owl:Restriction>
        </rdfs:subClassOf>
        <rdfs:subClassOf>
            <owl:Restriction>
                <owl:onProperty rdf:resource="http://foodie-cloud.com/model/foodie#analysisDate"/>
                <owl:cardinality rdf:datatype="http://www.w3.org/2001/XMLSchema#nonNegativeInteger">1</owl:cardinality>
            </owl:Restriction>
        </rdfs:subClassOf>
        <rdfs:subClassOf>
            <owl:Restriction>
                <owl:onProperty rdf:resource="http://foodie-cloud.com/model/foodie#propertyName"/>
                <owl:cardinality rdf:datatype="http://www.w3.org/2001/XMLSchema#nonNegativeInteger">1</owl:cardinality>
            </owl:Restriction>
        </rdfs:subClassOf>
        <rdfs:subClassOf>
            <owl:Restriction>
                <owl:onProperty rdf:resource="http://foodie-cloud.com/model/foodie#nonQuantitativeProperty"/>
                <owl:maxCardinality rdf:datatype="http://www.w3.org/2001/XMLSchema#nonNegativeInteger">1</owl:maxCardinality>
            </owl:Restriction>
        </rdfs:subClassOf>
        <rdfs:comment>An entity class for the Measured Properties</rdfs:comment>
        <rdfs:isDefinedBy rdf:resource="http://foodie-cloud.com/model/foodie"/>
        <rdfs:label>PropertyType</rdfs:label>
        <skos:prefLabel xml:lang="en">PropertyType</skos:prefLabel>
    </owl:Class>
    


    <!-- http://foodie-cloud.com/model/foodie#PropertyTypeValue -->


    <owl:Class rdf:about="http://foodie-cloud.com/model/foodie#PropertyTypeValue">
        <owl:equivalentClass rdf:resource="https://saref.etsi.org/core/Property"/>
        <rdfs:subClassOf rdf:resource="http://www.w3.org/2004/02/skos/core#Concept"/>
        <rdfs:comment>An entity class for the values of the measured properties</rdfs:comment>
        <rdfs:isDefinedBy rdf:resource="http://foodie-cloud.com/model/foodie"/>
        <rdfs:label>PropertyTypeValue</rdfs:label>
        <skos:prefLabel xml:lang="en">PropertyTypeValue</skos:prefLabel>
    </owl:Class>
    


    <!-- http://purl.oclc.org/NET/ssnx/cf/cf-feature#Layer -->


    <owl:Class rdf:about="http://purl.oclc.org/NET/ssnx/cf/cf-feature#Layer">
        <rdfs:subClassOf rdf:resource="http://www.w3.org/ns/sosa/FeatureOfInterest"/>
        <rdfs:comment>A cf-feature:Layer is something that is a ssn:FeatureOfInterest</rdfs:comment>
        <rdfs:isDefinedBy rdf:resource="http://purl.oclc.org/NET/ssnx/cf/cf-feature"/>
        <rdfs:label>Layer</rdfs:label>
    </owl:Class>
    


    <!-- http://purl.oclc.org/NET/ssnx/cf/cf-feature#Medium -->


    <owl:Class rdf:about="http://purl.oclc.org/NET/ssnx/cf/cf-feature#Medium">
        <rdfs:subClassOf rdf:resource="http://www.w3.org/ns/sosa/FeatureOfInterest"/>
        <rdfs:comment>A cf-feature:Medium is something that is a ssn:FeatureOfInterest</rdfs:comment>
        <rdfs:isDefinedBy rdf:resource="http://purl.oclc.org/NET/ssnx/cf/cf-feature"/>
        <rdfs:label>Medium</rdfs:label>
    </owl:Class>
    


    <!-- http://purl.oclc.org/NET/ssnx/cf/cf-feature#Precipitation -->


    <owl:Class rdf:about="http://purl.oclc.org/NET/ssnx/cf/cf-feature#Precipitation">
        <rdfs:subClassOf rdf:resource="http://www.w3.org/ns/sosa/FeatureOfInterest"/>
        <rdfs:comment>A cf-feature:Precipitation is something that is a ssn:FeatureOfInterest</rdfs:comment>
        <rdfs:isDefinedBy rdf:resource="http://purl.oclc.org/NET/ssnx/cf/cf-feature"/>
        <rdfs:label>Precipitation</rdfs:label>
    </owl:Class>
    


    <!-- http://purl.oclc.org/NET/ssnx/cf/cf-feature#Surface -->


    <owl:Class rdf:about="http://purl.oclc.org/NET/ssnx/cf/cf-feature#Surface">
        <rdfs:subClassOf rdf:resource="http://www.w3.org/ns/sosa/FeatureOfInterest"/>
        <rdfs:comment>A cf-feature:Surface is something that is a ssn:FeatureOfInterest</rdfs:comment>
        <rdfs:isDefinedBy rdf:resource="http://purl.oclc.org/NET/ssnx/cf/cf-feature"/>
        <rdfs:label>Surface</rdfs:label>
    </owl:Class>
    


    <!-- http://purl.oclc.org/NET/ssnx/cf/cf-feature#SurfaceLayer -->


    <owl:Class rdf:about="http://purl.oclc.org/NET/ssnx/cf/cf-feature#SurfaceLayer">
        <rdfs:subClassOf rdf:resource="http://www.w3.org/ns/sosa/FeatureOfInterest"/>
        <rdfs:comment>A cf-feature:SurfaceLayer is something that is a ssn:FeatureOfInterest</rdfs:comment>
        <rdfs:isDefinedBy rdf:resource="http://purl.oclc.org/NET/ssnx/cf/cf-feature"/>
        <rdfs:label>Surface Layer</rdfs:label>
    </owl:Class>
    


    <!-- http://purl.oclc.org/NET/ssnx/cf/cf-feature#Wind -->


    <owl:Class rdf:about="http://purl.oclc.org/NET/ssnx/cf/cf-feature#Wind">
        <rdfs:subClassOf rdf:resource="http://www.w3.org/ns/sosa/FeatureOfInterest"/>
        <rdfs:comment>A cf-feature:Wind is something that is a ssn:FeatureOfInterest</rdfs:comment>
        <rdfs:isDefinedBy rdf:resource="http://purl.oclc.org/NET/ssnx/cf/cf-feature"/>
        <rdfs:label>Wind</rdfs:label>
    </owl:Class>
    


    <!-- http://purl.oclc.org/NET/ssnx/qu/dim#Temperature -->


    <rdf:Description rdf:about="http://purl.oclc.org/NET/ssnx/qu/dim#Temperature">
        <owl:equivalentClass rdf:resource="https://saref.etsi.org/core/Temperature"/>
    </rdf:Description>
    


    <!-- http://purl.oclc.org/NET/ssnx/qu/qu#QuantityKind -->


    <rdf:Description rdf:about="http://purl.oclc.org/NET/ssnx/qu/qu#QuantityKind">
        <owl:equivalentClass rdf:resource="https://saref.etsi.org/core/Property"/>
    </rdf:Description>
    


    <!-- http://qudt.org/schema/qudt/Unit -->


    <rdf:Description rdf:about="http://qudt.org/schema/qudt/Unit">
        <owl:equivalentClass rdf:resource="https://saref.etsi.org/core/UnitOfMeasure"/>
    </rdf:Description>
    


    <!-- http://www.w3.org/ns/sosa/FeatureOfInterest -->


    <rdf:Description rdf:about="http://www.w3.org/ns/sosa/FeatureOfInterest">
        <owl:equivalentClass rdf:resource="https://saref.etsi.org/core/FeatureOfInterest"/>
    </rdf:Description>
    


    <!-- http://www.w3.org/ns/sosa/ObservableProperty -->


    <rdf:Description rdf:about="http://www.w3.org/ns/sosa/ObservableProperty">
        <owl:equivalentClass rdf:resource="https://saref.etsi.org/core/Property"/>
    </rdf:Description>
    


    <!-- http://www.w3.org/ns/sosa/Observation -->


    <rdf:Description rdf:about="http://www.w3.org/ns/sosa/Observation">
        <owl:equivalentClass rdf:resource="https://saref.etsi.org/core/Measurement"/>
    </rdf:Description>
    


    <!-- https://saref.etsi.org/core/Device -->


    <owl:Class rdf:about="https://saref.etsi.org/core/Device"/>
    


    <!-- https://saref.etsi.org/core/FeatureOfInterest -->


    <owl:Class rdf:about="https://saref.etsi.org/core/FeatureOfInterest">
        <rdfs:subClassOf>
            <owl:Restriction>
                <owl:onProperty rdf:resource="https://saref.etsi.org/core/hasProperty"/>
                <owl:allValuesFrom rdf:resource="https://saref.etsi.org/core/Property"/>
            </owl:Restriction>
        </rdfs:subClassOf>
        <rdfs:subClassOf>
            <owl:Restriction>
                <owl:onProperty rdf:resource="https://saref.etsi.org/core/isFeatureOfInterestOf"/>
                <owl:allValuesFrom rdf:resource="https://saref.etsi.org/core/Measurement"/>
            </owl:Restriction>
        </rdfs:subClassOf>
        <rdfs:comment>A feature of interest represents any real world entity from which a property is measured</rdfs:comment>
        <rdfs:isDefinedBy rdf:resource="https://saref.etsi.org/core/"/>
        <rdfs:label xml:lang="en">Feature of interest</rdfs:label>
    </owl:Class>
    


    <!-- https://saref.etsi.org/core/Humidity -->


    <owl:Class rdf:about="https://saref.etsi.org/core/Humidity">
        <rdfs:subClassOf rdf:resource="https://saref.etsi.org/core/Property"/>
        <rdfs:comment>A saref:Property related to some measurements that are characterized by a certain value that is measured in a humidity unit</rdfs:comment>
        <rdfs:isDefinedBy rdf:resource="https://saref.etsi.org/core/"/>
        <rdfs:label xml:lang="en">Humidity</rdfs:label>
    </owl:Class>
    


    <!-- https://saref.etsi.org/core/Measurement -->


    <owl:Class rdf:about="https://saref.etsi.org/core/Measurement">
        <rdfs:subClassOf>
            <owl:Restriction>
                <owl:onProperty rdf:resource="https://saref.etsi.org/core/hasFeatureOfInterest"/>
                <owl:allValuesFrom rdf:resource="https://saref.etsi.org/core/FeatureOfInterest"/>
            </owl:Restriction>
        </rdfs:subClassOf>
        <rdfs:subClassOf>
            <owl:Restriction>
                <owl:onProperty rdf:resource="https://saref.etsi.org/core/isMeasuredIn"/>
                <owl:allValuesFrom rdf:resource="https://saref.etsi.org/core/UnitOfMeasure"/>
            </owl:Restriction>
        </rdfs:subClassOf>
        <rdfs:subClassOf>
            <owl:Restriction>
                <owl:onProperty rdf:resource="https://saref.etsi.org/core/relatesToProperty"/>
                <owl:allValuesFrom rdf:resource="https://saref.etsi.org/core/Property"/>
            </owl:Restriction>
        </rdfs:subClassOf>
        <rdfs:subClassOf>
            <owl:Restriction>
                <owl:onProperty rdf:resource="https://saref.etsi.org/core/isMeasuredIn"/>
                <owl:qualifiedCardinality rdf:datatype="http://www.w3.org/2001/XMLSchema#nonNegativeInteger">1</owl:qualifiedCardinality>
                <owl:onClass rdf:resource="https://saref.etsi.org/core/UnitOfMeasure"/>
            </owl:Restriction>
        </rdfs:subClassOf>
        <rdfs:subClassOf>
            <owl:Restriction>
                <owl:onProperty rdf:resource="https://saref.etsi.org/core/relatesToProperty"/>
                <owl:qualifiedCardinality rdf:datatype="http://www.w3.org/2001/XMLSchema#nonNegativeInteger">1</owl:qualifiedCardinality>
                <owl:onClass rdf:resource="https://saref.etsi.org/core/Property"/>
            </owl:Restriction>
        </rdfs:subClassOf>
        <rdfs:subClassOf>
            <owl:Restriction>
                <owl:onProperty rdf:resource="https://saref.etsi.org/core/hasTimestamp"/>
                <owl:allValuesFrom rdf:resource="http://www.w3.org/2001/XMLSchema#dateTime"/>
            </owl:Restriction>
        </rdfs:subClassOf>
        <rdfs:subClassOf>
            <owl:Restriction>
                <owl:onProperty rdf:resource="https://saref.etsi.org/core/hasValue"/>
                <owl:cardinality rdf:datatype="http://www.w3.org/2001/XMLSchema#nonNegativeInteger">1</owl:cardinality>
            </owl:Restriction>
        </rdfs:subClassOf>
        <rdfs:subClassOf>
            <owl:Restriction>
                <owl:onProperty rdf:resource="https://saref.etsi.org/core/hasValue"/>
                <owl:qualifiedCardinality rdf:datatype="http://www.w3.org/2001/XMLSchema#nonNegativeInteger">1</owl:qualifiedCardinality>
                <owl:onDataRange rdf:resource="http://www.w3.org/2001/XMLSchema#float"/>
            </owl:Restriction>
        </rdfs:subClassOf>
        <owl:disjointWith rdf:resource="https://saref.etsi.org/core/Property"/>
        <owl:disjointWith rdf:resource="https://saref.etsi.org/core/UnitOfMeasure"/>
        <rdfs:comment xml:lang="en">Represents the measured value made over a property. It is also linked to the unit of measure in which the value is expressed and the timestamp of the measurement.</rdfs:comment>
        <rdfs:isDefinedBy rdf:resource="https://saref.etsi.org/core/"/>
        <rdfs:label xml:lang="en">Measurement</rdfs:label>
    </owl:Class>
    


    <!-- https://saref.etsi.org/core/Property -->


    <owl:Class rdf:about="https://saref.etsi.org/core/Property">
        <rdfs:subClassOf>
            <owl:Restriction>
                <owl:onProperty rdf:resource="https://saref.etsi.org/core/isControlledByDevice"/>
                <owl:allValuesFrom rdf:resource="https://saref.etsi.org/core/Device"/>
            </owl:Restriction>
        </rdfs:subClassOf>
        <rdfs:subClassOf>
            <owl:Restriction>
                <owl:onProperty rdf:resource="https://saref.etsi.org/core/isMeasuredByDevice"/>
                <owl:allValuesFrom rdf:resource="https://saref.etsi.org/core/Device"/>
            </owl:Restriction>
        </rdfs:subClassOf>
        <rdfs:subClassOf>
            <owl:Restriction>
                <owl:onProperty rdf:resource="https://saref.etsi.org/core/isPropertyOf"/>
                <owl:allValuesFrom rdf:resource="https://saref.etsi.org/core/FeatureOfInterest"/>
            </owl:Restriction>
        </rdfs:subClassOf>
        <rdfs:subClassOf>
            <owl:Restriction>
                <owl:onProperty rdf:resource="https://saref.etsi.org/core/relatesToMeasurement"/>
                <owl:allValuesFrom rdf:resource="https://saref.etsi.org/core/Measurement"/>
            </owl:Restriction>
        </rdfs:subClassOf>
        <owl:disjointWith rdf:resource="https://saref.etsi.org/core/UnitOfMeasure"/>
        <rdfs:comment xml:lang="en">An aspect of an entity that can be observable by a sensor.</rdfs:comment>
        <rdfs:comment>Anything that can be sensed, measured or controlled in households, common public buildings or offices. We propose here a list of properties that are relevant for the purpose of SAREF, but this list can be extended.</rdfs:comment>
        <rdfs:isDefinedBy rdf:resource="https://saref.etsi.org/core/"/>
        <rdfs:label xml:lang="en">Property</rdfs:label>
        <rdfs:label>Property</rdfs:label>
    </owl:Class>
    


    <!-- https://saref.etsi.org/core/Temperature -->


    <owl:Class rdf:about="https://saref.etsi.org/core/Temperature">
        <rdfs:subClassOf rdf:resource="https://saref.etsi.org/core/Property"/>
        <rdfs:comment>A saref:Property related to some measurements that are characterized by a certain value that is measured in a temperature unit (degree_Celsius, degree_Fahrenheit, or degree_kelvin)</rdfs:comment>
        <rdfs:isDefinedBy rdf:resource="https://saref.etsi.org/core/"/>
        <rdfs:label xml:lang="en">Temperature</rdfs:label>
    </owl:Class>
    


    <!-- https://saref.etsi.org/core/UnitOfMeasure -->


    <owl:Class rdf:about="https://saref.etsi.org/core/UnitOfMeasure">
        <rdfs:comment xml:lang="en">The unit of measure is a standard for measurement of a quantity, such as a Property. For example,  Power is a property and Watt is a unit of power that represents a definite predetermined power: when we say 10 Watt, we actually mean 10 times the definite predetermined power called &quot;watt&quot;. Our definition is based on the definition of unit of measure in the Ontology of units of Measure (OM). We propose here a list of some units of measure that are relevant for the purpose of the Smart Appliances ontology, but this list can be extended.</rdfs:comment>
        <rdfs:comment>The unit of measure is a standard for measurement of a quantity, such as a Property. For example,  Power is a property and Watt is a unit of power that represents a definite predetermined power: when we say 10 Watt, we actually mean 10 times the definite predetermined power called &quot;watt&quot;. Our definition is based on the definition of unit of measure in the Ontology of units of Measure (OM). We propose here a list of some units of measure that are relevant for the purpose of SAREF, but this list can be extended, also using some other ontologies rather than the Ontology of units of Measure (OM).</rdfs:comment>
        <rdfs:isDefinedBy rdf:resource="http://www.wurvoc.org/vocabularies/om-1.6/Unit_of_measure"/>
        <rdfs:isDefinedBy rdf:resource="https://saref.etsi.org/core/"/>
        <rdfs:label xml:lang="en">Unit of measure</rdfs:label>
    </owl:Class>
    


    <!-- https://saref.etsi.org/saref4agri/Soil -->


    <owl:Class rdf:about="https://saref.etsi.org/saref4agri/Soil">
        <rdfs:subClassOf rdf:resource="https://saref.etsi.org/core/FeatureOfInterest"/>
        <rdfs:comment>Upper layer of the earth in which plants grow.</rdfs:comment>
        <rdfs:isDefinedBy rdf:resource="https://saref.etsi.org/saref4agri/"/>
        <rdfs:label>Soil</rdfs:label>
    </owl:Class>
    


    <!-- https://smartdatamodels.org/dataModel.Agrifood/AgriParcelRecord -->


    <owl:Class rdf:about="https://smartdatamodels.org/dataModel.Agrifood/AgriParcelRecord">
        <rdfs:comment>This entity contains a harmonised description of the conditions recorded on a generic parcel of land. This entity is primarily associated with the agricultural vertical and related IoT applications.</rdfs:comment>
        <rdfs:isDefinedBy rdf:resource="https://github.com/smart-data-models/dataModel.Agrifood/blob/master/AgriParcelRecord/schema.json"/>
        <rdfs:label>AgriParcelRecord</rdfs:label>
    </owl:Class>
    


    <!-- https://smartdatamodels.org/dataModel.Weather/WeatherForecast -->


    <owl:Class rdf:about="https://smartdatamodels.org/dataModel.Weather/WeatherForecast">
        <rdfs:subClassOf rdf:resource="https://saref.etsi.org/core/FeatureOfInterest"/>
        <rdfs:comment>A harmonised description of a Weather Forecast</rdfs:comment>
        <rdfs:isDefinedBy rdf:resource="https://github.com/smart-data-models/dataModel.Weather/blob/master/WeatherForecast/schema.json"/>
        <rdfs:label>WeatherForecast</rdfs:label>
    </owl:Class>
    


    <!-- https://smartdatamodels.org/dataModel.Weather/WeatherObserved -->


    <owl:Class rdf:about="https://smartdatamodels.org/dataModel.Weather/WeatherObserved">
        <rdfs:subClassOf rdf:resource="https://saref.etsi.org/core/FeatureOfInterest"/>
        <rdfs:comment>An observation of weather conditions at a certain place and time</rdfs:comment>
        <rdfs:isDefinedBy rdf:resource="https://github.com/smart-data-models/dataModel.Weather/blob/master/WeatherObserved/schema.json"/>
        <rdfs:label>WeatherObserved</rdfs:label>
    </owl:Class>
    


    <!-- 
    ///////////////////////////////////////////////////////////////////////////////////////
    //
    // Individuals
    //
    ///////////////////////////////////////////////////////////////////////////////////////
     -->


    


    <!-- http://dbpedia.org/resource/DBM -->


    <owl:NamedIndividual rdf:about="http://dbpedia.org/resource/DBM">
        <rdf:type rdf:resource="https://saref.etsi.org/core/UnitOfMeasure"/>
        <rdfs:comment>a unit for power measurement</rdfs:comment>
        <rdfs:isDefinedBy rdf:resource="https://en.wikipedia.org/wiki/DBm"/>
        <rdfs:label xml:lang="en">decibel-milliwatts</rdfs:label>
    </owl:NamedIndividual>
    


    <!-- http://foodie-cloud.com/model/foodie/code/PropertyTypeValue/electricConductivity -->


    <owl:NamedIndividual rdf:about="http://foodie-cloud.com/model/foodie/code/PropertyTypeValue/electricConductivity">
        <rdf:type rdf:resource="http://www.w3.org/2004/02/skos/core#Concept"/>
        <rdf:type rdf:resource="https://saref.etsi.org/core/Property"/>
        <rdfs:comment>Electric conductivity is a physical property of any material (e.g. Soil).</rdfs:comment>
        <rdfs:isDefinedBy rdf:resource="http://foodie-cloud.com/model/foodie"/>
        <rdfs:label xml:lang="en">electricConductivity</rdfs:label>
        <skos:inScheme rdf:resource="http://foodie-cloud.com/model/foodie/code/PropertyTypeValue"/>
        <skos:prefLabel xml:lang="en">electricConductivity</skos:prefLabel>
    </owl:NamedIndividual>
    


    <!-- http://foodie-cloud.com/model/foodie/code/PropertyTypeValue/organicMatter -->


    <owl:NamedIndividual rdf:about="http://foodie-cloud.com/model/foodie/code/PropertyTypeValue/organicMatter">
        <rdf:type rdf:resource="http://www.w3.org/2004/02/skos/core#Concept"/>
        <rdf:type rdf:resource="https://saref.etsi.org/core/Property"/>
        <rdfs:comment>An organic matter in the components of soil.</rdfs:comment>
        <rdfs:isDefinedBy rdf:resource="http://foodie-cloud.com/model/foodie"/>
        <rdfs:label xml:lang="en">organicMatter</rdfs:label>
        <skos:inScheme rdf:resource="http://foodie-cloud.com/model/foodie/code/PropertyTypeValue"/>
        <skos:prefLabel xml:lang="en">organicMatter</skos:prefLabel>
    </owl:NamedIndividual>
    


    <!-- http://foodie-cloud.com/model/foodie/code/PropertyTypeValue/pH -->


    <owl:NamedIndividual rdf:about="http://foodie-cloud.com/model/foodie/code/PropertyTypeValue/pH">
        <rdf:type rdf:resource="http://www.w3.org/2004/02/skos/core#Concept"/>
        <rdf:type rdf:resource="https://saref.etsi.org/core/Property"/>
        <rdfs:comment>Hydrogen potential of soil</rdfs:comment>
        <rdfs:isDefinedBy rdf:resource="http://foodie-cloud.com/model/foodie"/>
        <rdfs:label xml:lang="en">pH</rdfs:label>
        <skos:inScheme rdf:resource="http://foodie-cloud.com/model/foodie/code/PropertyTypeValue"/>
        <skos:prefLabel xml:lang="en">pH</skos:prefLabel>
    </owl:NamedIndividual>
    


    <!-- http://foodie-cloud.com/model/foodie/code/PropertyTypeValue/soilTexture -->


    <owl:NamedIndividual rdf:about="http://foodie-cloud.com/model/foodie/code/PropertyTypeValue/soilTexture">
        <rdf:type rdf:resource="http://www.w3.org/2004/02/skos/core#Concept"/>
        <rdf:type rdf:resource="https://saref.etsi.org/core/Property"/>
        <rdfs:comment>Defines the texture of soil</rdfs:comment>
        <rdfs:isDefinedBy rdf:resource="http://foodie-cloud.com/model/foodie"/>
        <rdfs:label xml:lang="en">soilTexture</rdfs:label>
        <skos:inScheme rdf:resource="http://foodie-cloud.com/model/foodie/code/PropertyTypeValue"/>
        <skos:prefLabel xml:lang="en">soilTexture</skos:prefLabel>
    </owl:NamedIndividual>
    


    <!-- http://foodie-cloud.com/model/foodie/code/PropertyTypeValue/soilType -->


    <owl:NamedIndividual rdf:about="http://foodie-cloud.com/model/foodie/code/PropertyTypeValue/soilType">
        <rdf:type rdf:resource="http://www.w3.org/2004/02/skos/core#Concept"/>
        <rdf:type rdf:resource="https://saref.etsi.org/core/Property"/>
        <rdfs:comment>Defines the type of soil</rdfs:comment>
        <rdfs:isDefinedBy rdf:resource="http://foodie-cloud.com/model/foodie"/>
        <rdfs:label xml:lang="en">soilType</rdfs:label>
        <skos:inScheme rdf:resource="http://foodie-cloud.com/model/foodie/code/PropertyTypeValue"/>
        <skos:prefLabel xml:lang="en">soilType</skos:prefLabel>
    </owl:NamedIndividual>
    


    <!-- http://purl.oclc.org/NET/ssnx/cf/cf-feature#snowfall -->


    <owl:NamedIndividual rdf:about="http://purl.oclc.org/NET/ssnx/cf/cf-feature#snowfall">
        <rdf:type rdf:resource="http://purl.oclc.org/NET/ssnx/cf/cf-feature#Precipitation"/>
        <ssn:hasProperty rdf:resource="http://purl.oclc.org/NET/ssnx/cf/cf-property#convective_snowfall_amount"/>
        <ssn:hasProperty rdf:resource="http://purl.oclc.org/NET/ssnx/cf/cf-property#convective_snowfall_flux"/>
        <ssn:hasProperty rdf:resource="http://purl.oclc.org/NET/ssnx/cf/cf-property#large_scale_snowfall_amount"/>
        <ssn:hasProperty rdf:resource="http://purl.oclc.org/NET/ssnx/cf/cf-property#large_scale_snowfall_flux"/>
        <ssn:hasProperty rdf:resource="http://purl.oclc.org/NET/ssnx/cf/cf-property#lwe_convective_snowfall_rate"/>
        <ssn:hasProperty rdf:resource="http://purl.oclc.org/NET/ssnx/cf/cf-property#lwe_large_scale_snowfall_rate"/>
        <ssn:hasProperty rdf:resource="http://purl.oclc.org/NET/ssnx/cf/cf-property#lwe_snowfall_rate"/>
        <ssn:hasProperty rdf:resource="http://purl.oclc.org/NET/ssnx/cf/cf-property#lwe_thickness_of_convective_snowfall_amount"/>
        <ssn:hasProperty rdf:resource="http://purl.oclc.org/NET/ssnx/cf/cf-property#lwe_thickness_of_large_scale_snowfall_amount"/>
        <ssn:hasProperty rdf:resource="http://purl.oclc.org/NET/ssnx/cf/cf-property#lwe_thickness_of_snowfall_amount"/>
        <ssn:hasProperty rdf:resource="http://purl.oclc.org/NET/ssnx/cf/cf-property#snowfall_amount"/>
        <ssn:hasProperty rdf:resource="http://purl.oclc.org/NET/ssnx/cf/cf-property#snowfall_flux"/>
        <ssn:hasProperty rdf:resource="http://purl.oclc.org/NET/ssnx/cf/cf-property#thickness_of_convective_snowfall_amount"/>
        <ssn:hasProperty rdf:resource="http://purl.oclc.org/NET/ssnx/cf/cf-property#thickness_of_large_scale_snowfall_amount"/>
        <ssn:hasProperty rdf:resource="http://purl.oclc.org/NET/ssnx/cf/cf-property#thickness_of_snowfall_amount"/>
        <rdfs:comment>Snowfall at a definite scale e.g. cm</rdfs:comment>
        <rdfs:isDefinedBy rdf:resource="http://purl.oclc.org/NET/ssnx/cf/cf-feature"/>
        <rdfs:label>snowfall</rdfs:label>
    </owl:NamedIndividual>
    


    <!-- http://purl.oclc.org/NET/ssnx/cf/cf-feature#soil -->


    <owl:NamedIndividual rdf:about="http://purl.oclc.org/NET/ssnx/cf/cf-feature#soil">
        <rdf:type rdf:resource="http://purl.oclc.org/NET/ssnx/cf/cf-feature#Medium"/>
        <ssn:hasProperty rdf:resource="http://purl.oclc.org/NET/ssnx/cf/cf-property#downward_heat_flux_in_soil"/>
        <ssn:hasProperty rdf:resource="http://purl.oclc.org/NET/ssnx/cf/cf-property#lwe_thickness_of_soil_moisture_content"/>
        <ssn:hasProperty rdf:resource="http://purl.oclc.org/NET/ssnx/cf/cf-property#mass_concentration_of_condensed_water_in_soil"/>
        <ssn:hasProperty rdf:resource="http://purl.oclc.org/NET/ssnx/cf/cf-property#soil_albedo"/>
        <ssn:hasProperty rdf:resource="http://purl.oclc.org/NET/ssnx/cf/cf-property#soil_carbon_content"/>
        <ssn:hasProperty rdf:resource="http://purl.oclc.org/NET/ssnx/cf/cf-property#soil_frozen_water_content"/>
        <ssn:hasProperty rdf:resource="http://purl.oclc.org/NET/ssnx/cf/cf-property#soil_hydraulic_conductivity_at_saturation"/>
        <ssn:hasProperty rdf:resource="http://purl.oclc.org/NET/ssnx/cf/cf-property#soil_moisture_content"/>
        <ssn:hasProperty rdf:resource="http://purl.oclc.org/NET/ssnx/cf/cf-property#soil_moisture_content_at_field_capacity"/>
        <ssn:hasProperty rdf:resource="http://purl.oclc.org/NET/ssnx/cf/cf-property#soil_porosity"/>
        <ssn:hasProperty rdf:resource="http://purl.oclc.org/NET/ssnx/cf/cf-property#soil_suction_at_saturation"/>
        <ssn:hasProperty rdf:resource="http://purl.oclc.org/NET/ssnx/cf/cf-property#soil_temperature"/>
        <ssn:hasProperty rdf:resource="http://purl.oclc.org/NET/ssnx/cf/cf-property#soil_thermal_capacity"/>
        <ssn:hasProperty rdf:resource="http://purl.oclc.org/NET/ssnx/cf/cf-property#soil_thermal_conductivity"/>
        <ssn:hasProperty rdf:resource="http://purl.oclc.org/NET/ssnx/cf/cf-property#soil_type"/>
        <ssn:hasProperty rdf:resource="http://purl.oclc.org/NET/ssnx/cf/cf-property#volume_fraction_of_clay_in_soil"/>
        <ssn:hasProperty rdf:resource="http://purl.oclc.org/NET/ssnx/cf/cf-property#volume_fraction_of_condensed_water_in_soil"/>
        <ssn:hasProperty rdf:resource="http://purl.oclc.org/NET/ssnx/cf/cf-property#volume_fraction_of_condensed_water_in_soil_at_critical_point"/>
        <ssn:hasProperty rdf:resource="http://purl.oclc.org/NET/ssnx/cf/cf-property#volume_fraction_of_condensed_water_in_soil_at_field_capacity"/>
        <ssn:hasProperty rdf:resource="http://purl.oclc.org/NET/ssnx/cf/cf-property#volume_fraction_of_condensed_water_in_soil_at_wilting_point"/>
        <ssn:hasProperty rdf:resource="http://purl.oclc.org/NET/ssnx/cf/cf-property#volume_fraction_of_frozen_water_in_soil"/>
        <ssn:hasProperty rdf:resource="http://purl.oclc.org/NET/ssnx/cf/cf-property#volume_fraction_of_sand_in_soil"/>
        <ssn:hasProperty rdf:resource="http://purl.oclc.org/NET/ssnx/cf/cf-property#volume_fraction_of_silt_in_soil"/>
        <ssn:hasProperty rdf:resource="http://purl.oclc.org/NET/ssnx/cf/cf-property#water_evaporation_flux_from_soil"/>
        <rdfs:comment>The top layer of earth&apos;s crust</rdfs:comment>
        <rdfs:isDefinedBy rdf:resource="http://purl.oclc.org/NET/ssnx/cf/cf-feature"/>
        <rdfs:label>soil</rdfs:label>
    </owl:NamedIndividual>
    


    <!-- http://purl.oclc.org/NET/ssnx/cf/cf-feature#soil_layer -->


    <owl:NamedIndividual rdf:about="http://purl.oclc.org/NET/ssnx/cf/cf-feature#soil_layer">
        <rdf:type rdf:resource="http://purl.oclc.org/NET/ssnx/cf/cf-feature#Layer"/>
        <ssn:hasProperty rdf:resource="http://purl.oclc.org/NET/ssnx/cf/cf-property#frozen_water_content_of_soil_layer"/>
        <ssn:hasProperty rdf:resource="http://purl.oclc.org/NET/ssnx/cf/cf-property#liquid_water_content_of_soil_layer"/>
        <ssn:hasProperty rdf:resource="http://purl.oclc.org/NET/ssnx/cf/cf-property#lwe_thickness_of_frozen_water_content_of_soil_layer"/>
        <ssn:hasProperty rdf:resource="http://purl.oclc.org/NET/ssnx/cf/cf-property#lwe_thickness_of_moisture_content_of_soil_layer"/>
        <ssn:hasProperty rdf:resource="http://purl.oclc.org/NET/ssnx/cf/cf-property#moisture_content_of_soil_layer"/>
        <ssn:hasProperty rdf:resource="http://purl.oclc.org/NET/ssnx/cf/cf-property#moisture_content_of_soil_layer_at_field_capacity"/>
        <rdfs:comment>The top layer of soil</rdfs:comment>
        <rdfs:isDefinedBy rdf:resource="http://purl.oclc.org/NET/ssnx/cf/cf-feature"/>
        <rdfs:label>soil layer</rdfs:label>
    </owl:NamedIndividual>
    


    <!-- http://purl.oclc.org/NET/ssnx/cf/cf-feature#soil_pores -->


    <owl:NamedIndividual rdf:about="http://purl.oclc.org/NET/ssnx/cf/cf-feature#soil_pores">
        <rdf:type rdf:resource="http://purl.oclc.org/NET/ssnx/cf/cf-feature#Medium"/>
        <ssn:hasProperty rdf:resource="http://purl.oclc.org/NET/ssnx/cf/cf-property#volume_fraction_of_condensed_water_in_soil_pores"/>
        <rdfs:comment>the pores on the layer of soil for water to pass</rdfs:comment>
        <rdfs:isDefinedBy rdf:resource="http://purl.oclc.org/NET/ssnx/cf/cf-feature"/>
        <rdfs:label>soil pores</rdfs:label>
    </owl:NamedIndividual>
    


    <!-- http://purl.oclc.org/NET/ssnx/cf/cf-feature#vegetation -->


    <owl:NamedIndividual rdf:about="http://purl.oclc.org/NET/ssnx/cf/cf-feature#vegetation">
        <rdf:type rdf:resource="http://purl.oclc.org/NET/ssnx/cf/cf-feature#Layer"/>
        <ssn:hasProperty rdf:resource="http://purl.oclc.org/NET/ssnx/cf/cf-property#vegetation_area_fraction"/>
        <ssn:hasProperty rdf:resource="http://purl.oclc.org/NET/ssnx/cf/cf-property#vegetation_carbon_content"/>
        <rdfs:comment>The collective species of plants on a given area</rdfs:comment>
        <rdfs:isDefinedBy rdf:resource="http://purl.oclc.org/NET/ssnx/cf/cf-feature"/>
        <rdfs:label>vegetation</rdfs:label>
    </owl:NamedIndividual>
    


    <!-- http://purl.oclc.org/NET/ssnx/cf/cf-feature#water -->


    <owl:NamedIndividual rdf:about="http://purl.oclc.org/NET/ssnx/cf/cf-feature#water">
        <rdf:type rdf:resource="http://purl.oclc.org/NET/ssnx/cf/cf-feature#Medium"/>
        <rdfs:comment>water</rdfs:comment>
        <rdfs:isDefinedBy rdf:resource="http://purl.oclc.org/NET/ssnx/cf/cf-feature"/>
        <rdfs:label>water</rdfs:label>
    </owl:NamedIndividual>
    


    <!-- http://purl.oclc.org/NET/ssnx/cf/cf-property#air_density -->


    <owl:NamedIndividual rdf:about="http://purl.oclc.org/NET/ssnx/cf/cf-property#air_density">
        <rdf:type rdf:resource="http://purl.oclc.org/NET/ssnx/qu/dim#Density"/>
        <rdfs:comment>The amount of air in per cubic volume</rdfs:comment>
        <rdfs:isDefinedBy rdf:resource="http://purl.oclc.org/NET/ssnx/cf/cf-property"/>
        <rdfs:label>air density</rdfs:label>
    </owl:NamedIndividual>
    


    <!-- http://purl.oclc.org/NET/ssnx/cf/cf-property#air_temperature -->


    <owl:NamedIndividual rdf:about="http://purl.oclc.org/NET/ssnx/cf/cf-property#air_temperature">
        <rdf:type rdf:resource="http://purl.oclc.org/NET/ssnx/qu/dim#Temperature"/>
        <rdfs:comment>Air temperature is the bulk temperature of the air, not the surface (skin) temperature</rdfs:comment>
        <rdfs:isDefinedBy rdf:resource="http://purl.oclc.org/NET/ssnx/cf/cf-property"/>
        <rdfs:label>air temperature</rdfs:label>
    </owl:NamedIndividual>
    


    <!-- http://purl.oclc.org/NET/ssnx/cf/cf-property#atmosphere_mass_content_of_carbon_dioxide -->


    <owl:NamedIndividual rdf:about="http://purl.oclc.org/NET/ssnx/cf/cf-property#atmosphere_mass_content_of_carbon_dioxide">
        <rdf:type rdf:resource="http://purl.oclc.org/NET/ssnx/qu/dim#SurfaceDensity"/>
        <rdfs:comment>&quot;Content&quot; indicates a quantity per unit area.  The &quot;atmosphere content&quot; of a quantity refers to the vertical integral from the surface to the top of the atmosphere. For the content between specified levels in the atmosphere, standard names including content_of_atmosphere_layer are used.  The chemical formula for carbon dioxide is CO2</rdfs:comment>
        <rdfs:isDefinedBy rdf:resource="http://purl.oclc.org/NET/ssnx/cf/cf-property"/>
        <rdfs:label>atmosphere mass content of carbon dioxide</rdfs:label>
    </owl:NamedIndividual>
    


    <!-- http://purl.oclc.org/NET/ssnx/cf/cf-property#atmosphere_mass_content_of_carbon_monoxide -->


    <owl:NamedIndividual rdf:about="http://purl.oclc.org/NET/ssnx/cf/cf-property#atmosphere_mass_content_of_carbon_monoxide">
        <rdf:type rdf:resource="http://purl.oclc.org/NET/ssnx/qu/dim#SurfaceDensity"/>
        <rdfs:comment>&quot;Content&quot; indicates a quantity per unit area.  The &quot;atmosphere content&quot; of a quantity refers to the vertical integral from the surface to the top of the atmosphere. For the content between specified levels in the atmosphere, standard names including content_of_atmosphere_layer are used.  The chemical formula of carbon monoxide is CO</rdfs:comment>
        <rdfs:isDefinedBy rdf:resource="http://purl.oclc.org/NET/ssnx/cf/cf-property"/>
        <rdfs:label>atmosphere mass content of carbon monoxide</rdfs:label>
    </owl:NamedIndividual>
    


    <!-- http://purl.oclc.org/NET/ssnx/cf/cf-property#atmosphere_water_vapor_content -->


    <owl:NamedIndividual rdf:about="http://purl.oclc.org/NET/ssnx/cf/cf-property#atmosphere_water_vapor_content">
        <rdf:type rdf:resource="http://purl.oclc.org/NET/ssnx/qu/dim#SurfaceDensity"/>
        <rdfs:comment>&quot;Content&quot; indicates a quantity per unit area. The &quot;atmosphere content&quot; of a quantity refers to the vertical integral from the surface to the top of the atmosphere. For the content between specified levels in the atmosphere, standard names including content_of_atmosphere_layer are used. Atmosphere water vapor content is sometimes referred to as &quot;precipitable water&quot;, although this term does not imply the water could all be precipitated</rdfs:comment>
        <rdfs:isDefinedBy rdf:resource="http://purl.oclc.org/NET/ssnx/cf/cf-property"/>
        <rdfs:label>atmosphere water vapor content</rdfs:label>
    </owl:NamedIndividual>
    


    <!-- http://purl.oclc.org/NET/ssnx/cf/cf-property#convective_snowfall_amount -->


    <owl:NamedIndividual rdf:about="http://purl.oclc.org/NET/ssnx/cf/cf-property#convective_snowfall_amount">
        <rdf:type rdf:resource="http://purl.oclc.org/NET/ssnx/qu/dim#SurfaceDensity"/>
        <rdfs:comment>&quot;Amount&quot; means mass per unit area. Convective snow bands develop in response to a cold air outbreak from the continent or the frozen sea over the open water surface of lakes or seas.</rdfs:comment>
        <rdfs:isDefinedBy rdf:resource="http://purl.oclc.org/NET/ssnx/cf/cf-property"/>
        <rdfs:label>convective snowfall amount</rdfs:label>
    </owl:NamedIndividual>
    


    <!-- http://purl.oclc.org/NET/ssnx/cf/cf-property#convective_snowfall_flux -->


    <owl:NamedIndividual rdf:about="http://purl.oclc.org/NET/ssnx/cf/cf-property#convective_snowfall_flux">
        <rdf:type rdf:resource="http://purl.oclc.org/NET/ssnx/qu/dim#MassPerTimePerArea"/>
        <rdfs:comment>In accordance with common usage in geophysical disciplines, &quot;flux&quot; implies per unit area, called &quot;flux density&quot; in physics</rdfs:comment>
        <rdfs:isDefinedBy rdf:resource="http://purl.oclc.org/NET/ssnx/cf/cf-property"/>
        <rdfs:label>convective snowfall flux</rdfs:label>
    </owl:NamedIndividual>
    


    <!-- http://purl.oclc.org/NET/ssnx/cf/cf-property#downward_heat_flux_in_soil -->


    <owl:NamedIndividual rdf:about="http://purl.oclc.org/NET/ssnx/cf/cf-property#downward_heat_flux_in_soil">
        <rdf:type rdf:resource="http://purl.oclc.org/NET/ssnx/qu/dim#EnergyFlux"/>
        <rdfs:comment>&quot;Downward&quot; indicates a vector component which is positive when directed downward (negative upward). In accordance with common usage in geophysical disciplines, &quot;flux&quot; implies per unit area, called &quot;flux density&quot; in physics</rdfs:comment>
        <rdfs:isDefinedBy rdf:resource="http://purl.oclc.org/NET/ssnx/cf/cf-property"/>
        <rdfs:label>downward heat flux in soil</rdfs:label>
    </owl:NamedIndividual>
    


    <!-- http://purl.oclc.org/NET/ssnx/cf/cf-property#frozen_water_content_of_soil_layer -->


    <owl:NamedIndividual rdf:about="http://purl.oclc.org/NET/ssnx/cf/cf-property#frozen_water_content_of_soil_layer">
        <rdf:type rdf:resource="http://purl.oclc.org/NET/ssnx/qu/dim#SurfaceDensity"/>
        <rdfs:comment>&quot;frozen_water&quot; means ice. &quot;Content&quot; indicates a quantity per unit area. &quot;Layer&quot; means any layer with upper and lower boundaries that have constant values in some vertical coordinate. There must be a vertical coordinate variable indicating the extent of the layer(s). If the layers are model layers, the vertical coordinate can be model_level_number, but it is recommended to specify a physical coordinate (in a scalar or auxiliary coordinate variable) as well. Quantities defined for a soil layer must have a vertical coordinate variable with boundaries indicating the extent of the layer(s).</rdfs:comment>
        <rdfs:isDefinedBy rdf:resource="http://purl.oclc.org/NET/ssnx/cf/cf-property"/>
        <rdfs:label>frozen water content of soil layer</rdfs:label>
    </owl:NamedIndividual>
    


    <!-- http://purl.oclc.org/NET/ssnx/cf/cf-property#large_scale_snowfall_amount -->


    <owl:NamedIndividual rdf:about="http://purl.oclc.org/NET/ssnx/cf/cf-property#large_scale_snowfall_amount">
        <rdf:type rdf:resource="http://purl.oclc.org/NET/ssnx/qu/dim#SurfaceDensity"/>
        <rdfs:comment>&quot;Amount&quot; means mass per unit area</rdfs:comment>
        <rdfs:isDefinedBy rdf:resource="http://purl.oclc.org/NET/ssnx/cf/cf-property"/>
        <rdfs:label>large scale snowfall amount</rdfs:label>
    </owl:NamedIndividual>
    


    <!-- http://purl.oclc.org/NET/ssnx/cf/cf-property#large_scale_snowfall_flux -->


    <owl:NamedIndividual rdf:about="http://purl.oclc.org/NET/ssnx/cf/cf-property#large_scale_snowfall_flux">
        <rdf:type rdf:resource="http://purl.oclc.org/NET/ssnx/qu/dim#MassPerTimePerArea"/>
        <rdfs:comment>In accordance with common usage in geophysical disciplines, &quot;flux&quot; implies per unit area, called &quot;flux density&quot; in physics.</rdfs:comment>
        <rdfs:isDefinedBy rdf:resource="http://purl.oclc.org/NET/ssnx/cf/cf-property"/>
        <rdfs:label>large scale snowfall flux</rdfs:label>
    </owl:NamedIndividual>
    


    <!-- http://purl.oclc.org/NET/ssnx/cf/cf-property#liquid_water_content_of_soil_layer -->


    <owl:NamedIndividual rdf:about="http://purl.oclc.org/NET/ssnx/cf/cf-property#liquid_water_content_of_soil_layer">
        <rdf:type rdf:resource="http://purl.oclc.org/NET/ssnx/qu/dim#SurfaceDensity"/>
        <rdfs:comment>&quot;Content&quot; indicates a quantity per unit area. &quot;Layer&quot; means any layer with upper and lower boundaries that have constant values in some vertical coordinate. There must be a vertical coordinate variable indicating the extent of the layer(s). If the layers are model layers, the vertical coordinate can be model_level_number, but it is recommended to specify a physical coordinate (in a scalar or auxiliary coordinate variable) as well. Quantities defined for a soil layer must have a vertical coordinate variable with boundaries indicating the extent of the layer(s).</rdfs:comment>
        <rdfs:isDefinedBy rdf:resource="http://purl.oclc.org/NET/ssnx/cf/cf-property"/>
        <rdfs:label>liquid water content of soil layer</rdfs:label>
    </owl:NamedIndividual>
    


    <!-- http://purl.oclc.org/NET/ssnx/cf/cf-property#lwe_convective_snowfall_rate -->


    <owl:NamedIndividual rdf:about="http://purl.oclc.org/NET/ssnx/cf/cf-property#lwe_convective_snowfall_rate">
        <rdf:type rdf:resource="http://purl.oclc.org/NET/ssnx/qu/dim#VelocityOrSpeed"/>
        <rdfs:comment>&quot;lwe&quot; means liquid water equivalent</rdfs:comment>
        <rdfs:isDefinedBy rdf:resource="http://purl.oclc.org/NET/ssnx/cf/cf-property"/>
        <rdfs:label>lwe convective snowfall rate</rdfs:label>
    </owl:NamedIndividual>
    


    <!-- http://purl.oclc.org/NET/ssnx/cf/cf-property#lwe_large_scale_snowfall_rate -->


    <owl:NamedIndividual rdf:about="http://purl.oclc.org/NET/ssnx/cf/cf-property#lwe_large_scale_snowfall_rate">
        <rdf:type rdf:resource="http://purl.oclc.org/NET/ssnx/qu/dim#VelocityOrSpeed"/>
        <rdfs:comment>&quot;lwe&quot; means liquid water equivalent</rdfs:comment>
        <rdfs:isDefinedBy rdf:resource="http://purl.oclc.org/NET/ssnx/cf/cf-property"/>
        <rdfs:label>lwe large scale snowfall rate</rdfs:label>
    </owl:NamedIndividual>
    


    <!-- http://purl.oclc.org/NET/ssnx/cf/cf-property#lwe_snowfall_rate -->


    <owl:NamedIndividual rdf:about="http://purl.oclc.org/NET/ssnx/cf/cf-property#lwe_snowfall_rate">
        <rdf:type rdf:resource="http://purl.oclc.org/NET/ssnx/qu/dim#VelocityOrSpeed"/>
        <rdfs:comment>&quot;lwe&quot; means liquid water equivalent</rdfs:comment>
        <rdfs:isDefinedBy rdf:resource="http://purl.oclc.org/NET/ssnx/cf/cf-property"/>
        <rdfs:label>lwe snowfall rate</rdfs:label>
    </owl:NamedIndividual>
    


    <!-- http://purl.oclc.org/NET/ssnx/cf/cf-property#lwe_thickness_of_convective_snowfall_amount -->


    <owl:NamedIndividual rdf:about="http://purl.oclc.org/NET/ssnx/cf/cf-property#lwe_thickness_of_convective_snowfall_amount">
        <rdf:type rdf:resource="http://purl.oclc.org/NET/ssnx/qu/dim#Distance"/>
        <rdfs:comment>&quot;lwe&quot; means liquid water equivalent. &quot;Amount&quot; means mass per unit area. The construction lwe_thickness_of_X_amount or _content means the vertical extent of a layer of liquid water having the same mass per unit area.</rdfs:comment>
        <rdfs:isDefinedBy rdf:resource="http://purl.oclc.org/NET/ssnx/cf/cf-property"/>
        <rdfs:label>lwe thickness of convective snowfall amount</rdfs:label>
    </owl:NamedIndividual>
    


    <!-- http://purl.oclc.org/NET/ssnx/cf/cf-property#lwe_thickness_of_frozen_water_content_of_soil_layer -->


    <owl:NamedIndividual rdf:about="http://purl.oclc.org/NET/ssnx/cf/cf-property#lwe_thickness_of_frozen_water_content_of_soil_layer">
        <rdf:type rdf:resource="http://purl.oclc.org/NET/ssnx/qu/dim#Distance"/>
        <rdfs:comment>&quot;frozen_water&quot; means ice. &quot;lwe&quot; means liquid water equivalent. The construction lwe_thickness_of_X_amount or _content means the vertical extent of a layer of liquid water having the same mass per unit area. &quot;Content&quot; indicates a quantity per unit area. &quot;Layer&quot; means any layer with upper and lower boundaries that have constant values in some vertical coordinate. There must be a vertical coordinate variable indicating the extent of the layer(s). If the layers are model layers, the vertical coordinate can be model_level_number, but it is recommended to specify a physical coordinate (in a scalar or auxiliary coordinate variable) as well. Quantities defined for a soil layer must have a vertical coordinate variable with boundaries indicating the extent of the layer(s)</rdfs:comment>
        <rdfs:isDefinedBy rdf:resource="http://purl.oclc.org/NET/ssnx/cf/cf-property"/>
        <rdfs:label>lwe thickness of frozen water content of soil layer</rdfs:label>
    </owl:NamedIndividual>
    


    <!-- http://purl.oclc.org/NET/ssnx/cf/cf-property#lwe_thickness_of_large_scale_snowfall_amount -->


    <owl:NamedIndividual rdf:about="http://purl.oclc.org/NET/ssnx/cf/cf-property#lwe_thickness_of_large_scale_snowfall_amount">
        <rdf:type rdf:resource="http://purl.oclc.org/NET/ssnx/qu/dim#Distance"/>
        <rdfs:comment>&quot;lwe&quot; means liquid water equivalent. &quot;Amount&quot; means mass per unit area. The construction lwe_thickness_of_X_amount or _content means the vertical extent of a layer of liquid water having the same mass per unit area.</rdfs:comment>
        <rdfs:isDefinedBy rdf:resource="http://purl.oclc.org/NET/ssnx/cf/cf-property"/>
        <rdfs:label>lwe thickness of large scale snowfall amount</rdfs:label>
    </owl:NamedIndividual>
    


    <!-- http://purl.oclc.org/NET/ssnx/cf/cf-property#lwe_thickness_of_moisture_content_of_soil_layer -->


    <owl:NamedIndividual rdf:about="http://purl.oclc.org/NET/ssnx/cf/cf-property#lwe_thickness_of_moisture_content_of_soil_layer">
        <rdf:type rdf:resource="http://purl.oclc.org/NET/ssnx/qu/dim#Distance"/>
        <rdfs:comment>&quot;lwe&quot; means liquid water equivalent. &quot;moisture&quot; means water in all phases contained in soil. The construction lwe_thickness_of_X_amount or _content means the vertical extent of a layer of liquid water having the same mass per unit area. &quot;Content&quot; indicates a quantity per unit area. &quot;Layer&quot; means any layer with upper and lower boundaries that have constant values in some vertical coordinate. There must be a vertical coordinate variable indicating the extent of the layer(s). If the layers are model layers, the vertical coordinate can be model_level_number, but it is recommended to specify a physical coordinate (in a scalar or auxiliary coordinate variable) as well. Quantities defined for a soil layer must have a vertical coordinate variable with boundaries indicating the extent of the layer(s)</rdfs:comment>
        <rdfs:isDefinedBy rdf:resource="http://purl.oclc.org/NET/ssnx/cf/cf-property"/>
        <rdfs:label>lwe thickness of moisture content of soil layer</rdfs:label>
    </owl:NamedIndividual>
    


    <!-- http://purl.oclc.org/NET/ssnx/cf/cf-property#lwe_thickness_of_snowfall_amount -->


    <owl:NamedIndividual rdf:about="http://purl.oclc.org/NET/ssnx/cf/cf-property#lwe_thickness_of_snowfall_amount">
        <rdf:type rdf:resource="http://purl.oclc.org/NET/ssnx/qu/dim#Distance"/>
        <rdfs:comment>&quot;lwe&quot; means liquid water equivalent. &quot;Amount&quot; means mass per unit area. The construction lwe_thickness_of_X_amount or _content means the vertical extent of a layer of liquid water having the same mass per unit area</rdfs:comment>
        <rdfs:isDefinedBy rdf:resource="http://purl.oclc.org/NET/ssnx/cf/cf-property"/>
        <rdfs:label>lwe thickness of snowfall amount</rdfs:label>
    </owl:NamedIndividual>
    


    <!-- http://purl.oclc.org/NET/ssnx/cf/cf-property#lwe_thickness_of_soil_moisture_content -->


    <owl:NamedIndividual rdf:about="http://purl.oclc.org/NET/ssnx/cf/cf-property#lwe_thickness_of_soil_moisture_content">
        <rdf:type rdf:resource="http://purl.oclc.org/NET/ssnx/qu/dim#Distance"/>
        <rdfs:comment>&quot;lwe&quot; means liquid water equivalent. &quot;moisture&quot; means water in all phases contained in soil. The construction lwe_thickness_of_X_amount or _content means the vertical extent of a layer of liquid water having the same mass per unit area. &quot;Content&quot; indicates a quantity per unit area. The &quot;soil content&quot; of a quantity refers to the vertical integral from the surface down to the bottom of the soil model. For the content between specified levels in the soil, standard names including content_of_soil_layer are used</rdfs:comment>
        <rdfs:isDefinedBy rdf:resource="http://purl.oclc.org/NET/ssnx/cf/cf-property"/>
        <rdfs:label>lwe thickness of soil moisture content</rdfs:label>
    </owl:NamedIndividual>
    


    <!-- http://purl.oclc.org/NET/ssnx/cf/cf-property#mass_concentration_of_condensed_water_in_soil -->


    <owl:NamedIndividual rdf:about="http://purl.oclc.org/NET/ssnx/cf/cf-property#mass_concentration_of_condensed_water_in_soil">
        <rdf:type rdf:resource="http://purl.oclc.org/NET/ssnx/qu/dim#Density"/>
        <rdfs:comment>Mass concentration means mass per unit volume and is used in the construction mass_concentration_of_X_in_Y, where X is a material constituent of Y.  Condensed water means liquid and ice</rdfs:comment>
        <rdfs:isDefinedBy rdf:resource="http://purl.oclc.org/NET/ssnx/cf/cf-property"/>
        <rdfs:label>mass concentration of condensed water in soil</rdfs:label>
    </owl:NamedIndividual>
    


    <!-- http://purl.oclc.org/NET/ssnx/cf/cf-property#moisture_content_of_soil_layer -->


    <owl:NamedIndividual rdf:about="http://purl.oclc.org/NET/ssnx/cf/cf-property#moisture_content_of_soil_layer">
        <rdf:type rdf:resource="http://purl.oclc.org/NET/ssnx/qu/dim#SurfaceDensity"/>
        <rdfs:comment>&quot;moisture&quot; means water in all phases contained in soil. &quot;Content&quot; indicates a quantity per unit area. &quot;Layer&quot; means any layer with upper and lower boundaries that have constant values in some vertical coordinate. There must be a vertical coordinate variable indicating the extent of the layer(s). If the layers are model layers, the vertical coordinate can be model_level_number, but it is recommended to specify a physical coordinate (in a scalar or auxiliary coordinate variable) as well. Quantities defined for a soil layer must have a vertical coordinate variable with boundaries indicating the extent of the layer(s)</rdfs:comment>
        <rdfs:isDefinedBy rdf:resource="http://purl.oclc.org/NET/ssnx/cf/cf-property"/>
        <rdfs:label>moisture content of soil layer</rdfs:label>
    </owl:NamedIndividual>
    


    <!-- http://purl.oclc.org/NET/ssnx/cf/cf-property#moisture_content_of_soil_layer_at_field_capacity -->


    <owl:NamedIndividual rdf:about="http://purl.oclc.org/NET/ssnx/cf/cf-property#moisture_content_of_soil_layer_at_field_capacity">
        <rdf:type rdf:resource="http://purl.oclc.org/NET/ssnx/qu/dim#SurfaceDensity"/>
        <rdfs:comment>&quot;moisture&quot; means water in all phases contained in soil. &quot;Content&quot; indicates a quantity per unit area. &quot;Layer&quot; means any layer with upper and lower boundaries that have constant values in some vertical coordinate. There must be a vertical coordinate variable indicating the extent of the layer(s). If the layers are model layers, the vertical coordinate can be model_level_number, but it is recommended to specify a physical coordinate (in a scalar or auxiliary coordinate variable) as well. Quantities defined for a soil layer must have a vertical coordinate variable with boundaries indicating the extent of the layer(s). The field capacity of soil is the maximum content of water it can retain against gravitational drainage</rdfs:comment>
        <rdfs:isDefinedBy rdf:resource="http://purl.oclc.org/NET/ssnx/cf/cf-property"/>
        <rdfs:label>moisture content of soil layer at field capacity</rdfs:label>
    </owl:NamedIndividual>
    


    <!-- http://purl.oclc.org/NET/ssnx/cf/cf-property#normalized_difference_vegetation_index -->


    <owl:NamedIndividual rdf:about="http://purl.oclc.org/NET/ssnx/cf/cf-property#normalized_difference_vegetation_index">
        <rdf:type rdf:resource="http://purl.oclc.org/NET/ssnx/qu/dim#Dimensionless"/>
        <rdfs:comment>&quot;Normalized_difference_vegetation_index&quot;, usually abbreviated to NDVI, is an index calculated from reflectances measured in the visible and near infrared channels.  It is calculated as NDVI = (NIR - R) / (NIR + R) where NIR is the reflectance in the near-infrared band and R is the reflectance in the red visible band.  Reflectance is the ratio of the reflected over the incoming radiation in each spectral band.  The calculated value of NDVI depends on the precise definitions of the spectral bands and these definitions may vary between different models and remote sensing instruments</rdfs:comment>
        <rdfs:isDefinedBy rdf:resource="http://purl.oclc.org/NET/ssnx/cf/cf-property"/>
        <rdfs:label>normalized difference vegetation index</rdfs:label>
    </owl:NamedIndividual>
    


    <!-- http://purl.oclc.org/NET/ssnx/cf/cf-property#precipitation_amount -->


    <owl:NamedIndividual rdf:about="http://purl.oclc.org/NET/ssnx/cf/cf-property#precipitation_amount">
        <rdf:type rdf:resource="http://purl.oclc.org/NET/ssnx/qu/dim#SurfaceDensity"/>
        <rdfs:comment>&quot;Amount&quot; means mass per unit area</rdfs:comment>
        <rdfs:isDefinedBy rdf:resource="http://purl.oclc.org/NET/ssnx/cf/cf-property"/>
        <rdfs:label>precipitation amount</rdfs:label>
    </owl:NamedIndividual>
    


    <!-- http://purl.oclc.org/NET/ssnx/cf/cf-property#snow_density -->


    <owl:NamedIndividual rdf:about="http://purl.oclc.org/NET/ssnx/cf/cf-property#snow_density">
        <rdf:type rdf:resource="http://purl.oclc.org/NET/ssnx/qu/dim#Density"/>
        <rdfs:comment>the amount of snow in per meter cube</rdfs:comment>
        <rdfs:isDefinedBy rdf:resource="http://purl.oclc.org/NET/ssnx/cf/cf-property"/>
        <rdfs:label>snow density</rdfs:label>
    </owl:NamedIndividual>
    


    <!-- http://purl.oclc.org/NET/ssnx/cf/cf-property#snow_grain_size -->


    <owl:NamedIndividual rdf:about="http://purl.oclc.org/NET/ssnx/cf/cf-property#snow_grain_size">
        <rdf:type rdf:resource="http://purl.oclc.org/NET/ssnx/qu/dim#Distance"/>
        <rdfs:comment>the size of a snow grain </rdfs:comment>
        <rdfs:isDefinedBy rdf:resource="http://purl.oclc.org/NET/ssnx/cf/cf-property"/>
        <rdfs:label>snow grain size</rdfs:label>
    </owl:NamedIndividual>
    


    <!-- http://purl.oclc.org/NET/ssnx/cf/cf-property#snow_soot_content -->


    <owl:NamedIndividual rdf:about="http://purl.oclc.org/NET/ssnx/cf/cf-property#snow_soot_content">
        <rdf:type rdf:resource="http://purl.oclc.org/NET/ssnx/qu/dim#SurfaceDensity"/>
        <rdfs:comment>&quot;Content&quot; indicates a quantity per unit area</rdfs:comment>
        <rdfs:isDefinedBy rdf:resource="http://purl.oclc.org/NET/ssnx/cf/cf-property"/>
        <rdfs:label>snow soot content</rdfs:label>
    </owl:NamedIndividual>
    


    <!-- http://purl.oclc.org/NET/ssnx/cf/cf-property#snow_temperature -->


    <owl:NamedIndividual rdf:about="http://purl.oclc.org/NET/ssnx/cf/cf-property#snow_temperature">
        <rdf:type rdf:resource="http://purl.oclc.org/NET/ssnx/qu/dim#Temperature"/>
        <rdfs:comment>Snow temperature is the bulk temperature of the snow, not the surface (skin) temperature</rdfs:comment>
        <rdfs:isDefinedBy rdf:resource="http://purl.oclc.org/NET/ssnx/cf/cf-property"/>
        <rdfs:label>snow temperature</rdfs:label>
    </owl:NamedIndividual>
    


    <!-- http://purl.oclc.org/NET/ssnx/cf/cf-property#snowfall_amount -->


    <owl:NamedIndividual rdf:about="http://purl.oclc.org/NET/ssnx/cf/cf-property#snowfall_amount">
        <rdf:type rdf:resource="http://purl.oclc.org/NET/ssnx/qu/dim#SurfaceDensity"/>
        <rdfs:comment>&quot;Amount&quot; means mass per unit area</rdfs:comment>
        <rdfs:isDefinedBy rdf:resource="http://purl.oclc.org/NET/ssnx/cf/cf-property"/>
        <rdfs:label>snowfall amount</rdfs:label>
    </owl:NamedIndividual>
    


    <!-- http://purl.oclc.org/NET/ssnx/cf/cf-property#snowfall_flux -->


    <owl:NamedIndividual rdf:about="http://purl.oclc.org/NET/ssnx/cf/cf-property#snowfall_flux">
        <rdf:type rdf:resource="http://purl.oclc.org/NET/ssnx/qu/dim#MassPerTimePerArea"/>
        <rdfs:comment>In accordance with common usage in geophysical disciplines, &quot;flux&quot; implies per unit area, called &quot;flux density&quot; in physics</rdfs:comment>
        <rdfs:isDefinedBy rdf:resource="http://purl.oclc.org/NET/ssnx/cf/cf-property"/>
        <rdfs:label>snowfall flux</rdfs:label>
    </owl:NamedIndividual>
    


    <!-- http://purl.oclc.org/NET/ssnx/cf/cf-property#soil_albedo -->


    <owl:NamedIndividual rdf:about="http://purl.oclc.org/NET/ssnx/cf/cf-property#soil_albedo">
        <rdf:type rdf:resource="http://purl.oclc.org/NET/ssnx/qu/dim#Dimensionless"/>
        <rdfs:comment>Soil albedo is the albedo of the soil surface assuming no snow</rdfs:comment>
        <rdfs:isDefinedBy rdf:resource="http://purl.oclc.org/NET/ssnx/cf/cf-property"/>
        <rdfs:label>soil albedo</rdfs:label>
    </owl:NamedIndividual>
    


    <!-- http://purl.oclc.org/NET/ssnx/cf/cf-property#soil_carbon_content -->


    <owl:NamedIndividual rdf:about="http://purl.oclc.org/NET/ssnx/cf/cf-property#soil_carbon_content">
        <rdf:type rdf:resource="http://purl.oclc.org/NET/ssnx/qu/dim#SurfaceDensity"/>
        <rdfs:comment>&quot;Content&quot; indicates a quantity per unit area. The &quot;soil content&quot; of a quantity refers to the vertical integral from the surface down to the bottom of the soil model. For the content between specified levels in the soil, standard names including content_of_soil_layer are used</rdfs:comment>
        <rdfs:isDefinedBy rdf:resource="http://purl.oclc.org/NET/ssnx/cf/cf-property"/>
        <rdfs:label>soil carbon content</rdfs:label>
    </owl:NamedIndividual>
    


    <!-- http://purl.oclc.org/NET/ssnx/cf/cf-property#soil_frozen_water_content -->


    <owl:NamedIndividual rdf:about="http://purl.oclc.org/NET/ssnx/cf/cf-property#soil_frozen_water_content">
        <rdf:type rdf:resource="http://purl.oclc.org/NET/ssnx/qu/dim#SurfaceDensity"/>
        <rdfs:comment>&quot;frozen_water&quot; means ice. &quot;Content&quot; indicates a quantity per unit area. The &quot;soil content&quot; of a quantity refers to the vertical integral from the surface down to the bottom of the soil model. For the content between specified levels in the soil, standard names including content_of_soil_layer are used</rdfs:comment>
        <rdfs:isDefinedBy rdf:resource="http://purl.oclc.org/NET/ssnx/cf/cf-property"/>
        <rdfs:label>soil frozen water content</rdfs:label>
    </owl:NamedIndividual>
    


    <!-- http://purl.oclc.org/NET/ssnx/cf/cf-property#soil_hydraulic_conductivity_at_saturation -->


    <owl:NamedIndividual rdf:about="http://purl.oclc.org/NET/ssnx/cf/cf-property#soil_hydraulic_conductivity_at_saturation">
        <rdf:type rdf:resource="http://purl.oclc.org/NET/ssnx/qu/dim#VelocityOrSpeed"/>
        <rdfs:comment>Hydraulic conductivity is the constant k in Darcy&apos;s Law q=-k grad h for fluid flow q (volume transport per unit area i.e. velocity) through a porous medium, where h is the hydraulic head (pressure expressed as an equivalent depth of water)</rdfs:comment>
        <rdfs:isDefinedBy rdf:resource="http://purl.oclc.org/NET/ssnx/cf/cf-property"/>
        <rdfs:label>soil hydraulic conductivity at saturation</rdfs:label>
    </owl:NamedIndividual>
    


    <!-- http://purl.oclc.org/NET/ssnx/cf/cf-property#soil_moisture_content -->


    <owl:NamedIndividual rdf:about="http://purl.oclc.org/NET/ssnx/cf/cf-property#soil_moisture_content">
        <rdf:type rdf:resource="http://purl.oclc.org/NET/ssnx/qu/dim#SurfaceDensity"/>
        <rdfs:comment>&quot;moisture&quot; means water in all phases contained in soil. &quot;Content&quot; indicates a quantity per unit area. The &quot;soil content&quot; of a quantity refers to the vertical integral from the surface down to the bottom of the soil model. For the content between specified levels in the soil, standard names including content_of_soil_layer are used</rdfs:comment>
        <rdfs:isDefinedBy rdf:resource="http://purl.oclc.org/NET/ssnx/cf/cf-property"/>
        <rdfs:label>soil moisture content</rdfs:label>
    </owl:NamedIndividual>
    


    <!-- http://purl.oclc.org/NET/ssnx/cf/cf-property#soil_moisture_content_at_field_capacity -->


    <owl:NamedIndividual rdf:about="http://purl.oclc.org/NET/ssnx/cf/cf-property#soil_moisture_content_at_field_capacity">
        <rdf:type rdf:resource="http://purl.oclc.org/NET/ssnx/qu/dim#SurfaceDensity"/>
        <rdfs:comment>&quot;moisture&quot; means water in all phases contained in soil. &quot;Content&quot; indicates a quantity per unit area. The &quot;soil content&quot; of a quantity refers to the vertical integral from the surface down to the bottom of the soil model. For the content between specified levels in the soil, standard names including content_of_soil_layer are used. The field capacity of soil is the maximum content of water it can retain against gravitational drainage</rdfs:comment>
        <rdfs:isDefinedBy rdf:resource="http://purl.oclc.org/NET/ssnx/cf/cf-property"/>
        <rdfs:label>soil moisture content at field capacity</rdfs:label>
    </owl:NamedIndividual>
    


    <!-- http://purl.oclc.org/NET/ssnx/cf/cf-property#soil_porosity -->


    <owl:NamedIndividual rdf:about="http://purl.oclc.org/NET/ssnx/cf/cf-property#soil_porosity">
        <rdf:type rdf:resource="http://purl.oclc.org/NET/ssnx/qu/dim#Dimensionless"/>
        <rdfs:comment>The soil porosity is the proportion of its total volume not occupied by soil solids</rdfs:comment>
        <rdfs:isDefinedBy rdf:resource="http://purl.oclc.org/NET/ssnx/cf/cf-property"/>
        <rdfs:label>soil porosity</rdfs:label>
    </owl:NamedIndividual>
    


    <!-- http://purl.oclc.org/NET/ssnx/cf/cf-property#soil_respiration_carbon_flux -->


    <owl:NamedIndividual rdf:about="http://purl.oclc.org/NET/ssnx/cf/cf-property#soil_respiration_carbon_flux">
        <rdf:type rdf:resource="http://purl.oclc.org/NET/ssnx/qu/dim#MassPerTimePerArea"/>
        <rdfs:comment>&quot;Respiration carbon&quot; refers to the rate at which biomass is respired expressed as the mass of carbon which it contains. Soil respiration is the sum of respiration in the soil by animals and decomposers of litter (heterotrophs or &quot;consumers&quot;), which have not produced the biomass they respire, and respiration by the roots of plants (autotrophs or &quot;producers&quot;), which have themselves produced the biomass they respire. In accordance with common usage in geophysical disciplines, &quot;flux&quot; implies per unit area, called &quot;flux density&quot; in physics</rdfs:comment>
        <rdfs:isDefinedBy rdf:resource="http://purl.oclc.org/NET/ssnx/cf/cf-property"/>
        <rdfs:label>soil respiration carbon flux</rdfs:label>
    </owl:NamedIndividual>
    


    <!-- http://purl.oclc.org/NET/ssnx/cf/cf-property#soil_suction_at_saturation -->


    <owl:NamedIndividual rdf:about="http://purl.oclc.org/NET/ssnx/cf/cf-property#soil_suction_at_saturation">
        <rdf:type rdf:resource="http://purl.oclc.org/NET/ssnx/qu/dim#StressOrPressure"/>
        <rdfs:comment>Soil suction is the tensile stress on water in soil due to molecular forces acting at the water-soil particle boundary. The forces may cause water to be drawn into the spaces within the soil matrix or cause it to be held in the soil without draining. Soil suction occurs in soil above the water table</rdfs:comment>
        <rdfs:isDefinedBy rdf:resource="http://purl.oclc.org/NET/ssnx/cf/cf-property"/>
        <rdfs:label>soil suction at saturation</rdfs:label>
    </owl:NamedIndividual>
    


    <!-- http://purl.oclc.org/NET/ssnx/cf/cf-property#soil_temperature -->


    <owl:NamedIndividual rdf:about="http://purl.oclc.org/NET/ssnx/cf/cf-property#soil_temperature">
        <rdf:type rdf:resource="http://purl.oclc.org/NET/ssnx/qu/dim#Temperature"/>
        <owl:sameAs rdf:resource="https://saref.etsi.org/saref4agri/SoilTemperature"/>
        <rdfs:comment>Soil temperature is the bulk temperature of the soil, not the surface (skin) temperature</rdfs:comment>
        <rdfs:isDefinedBy rdf:resource="http://purl.oclc.org/NET/ssnx/cf/cf-property"/>
        <rdfs:label>soil temperature</rdfs:label>
    </owl:NamedIndividual>
    


    <!-- https://saref.etsi.org/saref4agri/SoilTemperature -->


    <rdf:Description rdf:about="https://saref.etsi.org/saref4agri/SoilTemperature"/>
    


    <!-- http://purl.oclc.org/NET/ssnx/cf/cf-property#soil_thermal_capacity -->


    <owl:NamedIndividual rdf:about="http://purl.oclc.org/NET/ssnx/cf/cf-property#soil_thermal_capacity">
        <rdf:type rdf:resource="http://purl.oclc.org/NET/ssnx/qu/dim#SpecificEntropy"/>
        <rdfs:comment>Thermal capacity, or heat capacity, is the amount of heat energy required to increase the temperature of 1 kg of material by 1 K. It is a property of the material</rdfs:comment>
        <rdfs:isDefinedBy rdf:resource="http://purl.oclc.org/NET/ssnx/cf/cf-property"/>
        <rdfs:label>soil thermal capacity</rdfs:label>
    </owl:NamedIndividual>
    


    <!-- http://purl.oclc.org/NET/ssnx/cf/cf-property#soil_thermal_conductivity -->


    <owl:NamedIndividual rdf:about="http://purl.oclc.org/NET/ssnx/cf/cf-property#soil_thermal_conductivity">
        <rdf:type rdf:resource="http://purl.oclc.org/NET/ssnx/qu/dim#ThermalConductivity"/>
        <rdfs:comment>Thermal conductivity is the constant k in the formula q = -k grad T where q is the heat transfer per unit time per unit area of a surface normal to the direction of transfer and grad T is the temperature gradient. Thermal conductivity is a property of the material</rdfs:comment>
        <rdfs:isDefinedBy rdf:resource="http://purl.oclc.org/NET/ssnx/cf/cf-property"/>
        <rdfs:label>soil thermal conductivity</rdfs:label>
    </owl:NamedIndividual>
    


    <!-- http://purl.oclc.org/NET/ssnx/cf/cf-property#soil_type -->


    <owl:NamedIndividual rdf:about="http://purl.oclc.org/NET/ssnx/cf/cf-property#soil_type">
        <rdf:type rdf:resource="http://purl.oclc.org/NET/ssnx/qu/dim#Dimensionless"/>
        <rdfs:comment>A variable with the standard name of soil_type contains strings which indicate the character of the soil e.g. clay. These strings have not yet been standardised. Alternatively, the data variable may contain integers which can be translated to strings using flag_values and flag_meanings attributes</rdfs:comment>
        <rdfs:isDefinedBy rdf:resource="http://purl.oclc.org/NET/ssnx/cf/cf-property"/>
        <rdfs:label>soil type</rdfs:label>
    </owl:NamedIndividual>
    


    <!-- http://purl.oclc.org/NET/ssnx/cf/cf-property#sound_intensity_in_air -->


    <owl:NamedIndividual rdf:about="http://purl.oclc.org/NET/ssnx/cf/cf-property#sound_intensity_in_air">
        <rdf:type rdf:resource="http://purl.oclc.org/NET/ssnx/qu/dim#EnergyFlux"/>
        <rdfs:comment>Sound intensity is the sound energy per unit time per unit area</rdfs:comment>
        <rdfs:isDefinedBy rdf:resource="http://purl.oclc.org/NET/ssnx/cf/cf-property"/>
        <rdfs:label>sound intensity in air</rdfs:label>
    </owl:NamedIndividual>
    


    <!-- http://purl.oclc.org/NET/ssnx/cf/cf-property#sound_pressure_in_air -->


    <owl:NamedIndividual rdf:about="http://purl.oclc.org/NET/ssnx/cf/cf-property#sound_pressure_in_air">
        <rdf:type rdf:resource="http://purl.oclc.org/NET/ssnx/qu/dim#StressOrPressure"/>
        <rdfs:comment>Sound pressure is the difference from the local ambient pressure caused by a sound wave at a particular location and time</rdfs:comment>
        <rdfs:isDefinedBy rdf:resource="http://purl.oclc.org/NET/ssnx/cf/cf-property"/>
        <rdfs:label>sound pressure in air</rdfs:label>
    </owl:NamedIndividual>
    


    <!-- http://purl.oclc.org/NET/ssnx/cf/cf-property#thickness_of_convective_snowfall_amount -->


    <owl:NamedIndividual rdf:about="http://purl.oclc.org/NET/ssnx/cf/cf-property#thickness_of_convective_snowfall_amount">
        <rdf:type rdf:resource="http://purl.oclc.org/NET/ssnx/qu/dim#Distance"/>
        <rdfs:comment>&quot;Amount&quot; means mass per unit area. The construction thickness_of_[X_]snowfall_amount means the accumulated &quot;depth&quot; of snow which fell i.e. the thickness of the layer of snow at its own density. There are corresponding standard names for liquid water equivalent (lwe) thickness</rdfs:comment>
        <rdfs:isDefinedBy rdf:resource="http://purl.oclc.org/NET/ssnx/cf/cf-property"/>
        <rdfs:label>thickness of convective snowfall amount</rdfs:label>
    </owl:NamedIndividual>
    


    <!-- http://purl.oclc.org/NET/ssnx/cf/cf-property#thickness_of_large_scale_rainfall_amount -->


    <owl:NamedIndividual rdf:about="http://purl.oclc.org/NET/ssnx/cf/cf-property#thickness_of_large_scale_rainfall_amount">
        <rdf:type rdf:resource="http://purl.oclc.org/NET/ssnx/qu/dim#Distance"/>
        <rdfs:comment>&quot;Amount&quot; means mass per unit area. The construction thickness_of_[X_]rainfall_amount means the accumulated &quot;depth&quot; of rainfall i.e. the thickness of a layer of liquid water having the same mass per unit area as the rainfall amount</rdfs:comment>
        <rdfs:isDefinedBy rdf:resource="http://purl.oclc.org/NET/ssnx/cf/cf-property"/>
        <rdfs:label>thickness of large scale rainfall amount</rdfs:label>
    </owl:NamedIndividual>
    


    <!-- http://purl.oclc.org/NET/ssnx/cf/cf-property#thickness_of_large_scale_snowfall_amount -->


    <owl:NamedIndividual rdf:about="http://purl.oclc.org/NET/ssnx/cf/cf-property#thickness_of_large_scale_snowfall_amount">
        <rdf:type rdf:resource="http://purl.oclc.org/NET/ssnx/qu/dim#Distance"/>
        <rdfs:comment>&quot;Amount&quot; means mass per unit area. The construction thickness_of_[X_]snowfall_amount means the accumulated &quot;depth&quot; of snow which fell i.e. the thickness of the layer of snow at its own density. There are corresponding standard names for liquid water equivalent (lwe) thickness</rdfs:comment>
        <rdfs:isDefinedBy rdf:resource="http://purl.oclc.org/NET/ssnx/cf/cf-property"/>
        <rdfs:label>thickness of large scale snowfall amount</rdfs:label>
    </owl:NamedIndividual>
    


    <!-- http://purl.oclc.org/NET/ssnx/cf/cf-property#thickness_of_rainfall_amount -->


    <owl:NamedIndividual rdf:about="http://purl.oclc.org/NET/ssnx/cf/cf-property#thickness_of_rainfall_amount">
        <rdf:type rdf:resource="http://purl.oclc.org/NET/ssnx/qu/dim#Distance"/>
        <rdfs:comment>&quot;Amount&quot; means mass per unit area. The construction thickness_of_[X_]rainfall_amount means the accumulated &quot;depth&quot; of rainfall i.e. the thickness of a layer of liquid water having the same mass per unit area as the rainfall amount</rdfs:comment>
        <rdfs:isDefinedBy rdf:resource="http://purl.oclc.org/NET/ssnx/cf/cf-property"/>
        <rdfs:label>thickness of rainfall amount</rdfs:label>
    </owl:NamedIndividual>
    


    <!-- http://purl.oclc.org/NET/ssnx/cf/cf-property#thickness_of_snowfall_amount -->


    <owl:NamedIndividual rdf:about="http://purl.oclc.org/NET/ssnx/cf/cf-property#thickness_of_snowfall_amount">
        <rdf:type rdf:resource="http://purl.oclc.org/NET/ssnx/qu/dim#Distance"/>
        <rdfs:comment>&quot;Amount&quot; means mass per unit area. The construction thickness_of_[X_]snowfall_amount means the accumulated &quot;depth&quot; of snow which fell i.e. the thickness of the layer of snow at its own density. There are corresponding standard names for liquid water equivalent (lwe) thickness</rdfs:comment>
        <rdfs:isDefinedBy rdf:resource="http://purl.oclc.org/NET/ssnx/cf/cf-property"/>
        <rdfs:label>thickness of snowfall amount</rdfs:label>
    </owl:NamedIndividual>
    


    <!-- http://purl.oclc.org/NET/ssnx/cf/cf-property#vegetation_area_fraction -->


    <owl:NamedIndividual rdf:about="http://purl.oclc.org/NET/ssnx/cf/cf-property#vegetation_area_fraction">
        <rdf:type rdf:resource="http://purl.oclc.org/NET/ssnx/qu/dim#Dimensionless"/>
        <rdfs:comment>&quot;X_area_fraction&quot; means the fraction of horizontal area occupied by X. &quot;X_area&quot; means the horizontal area occupied by X within the grid cell. &quot;Vegetation&quot; means any plants e.g. trees, shrubs, grass</rdfs:comment>
        <rdfs:isDefinedBy rdf:resource="http://purl.oclc.org/NET/ssnx/cf/cf-property"/>
        <rdfs:label>vegetation area fraction</rdfs:label>
    </owl:NamedIndividual>
    


    <!-- http://purl.oclc.org/NET/ssnx/cf/cf-property#vegetation_carbon_content -->


    <owl:NamedIndividual rdf:about="http://purl.oclc.org/NET/ssnx/cf/cf-property#vegetation_carbon_content">
        <rdf:type rdf:resource="http://purl.oclc.org/NET/ssnx/qu/dim#SurfaceDensity"/>
        <rdfs:comment>&quot;Content&quot; indicates a quantity per unit area. &quot;Vegetation&quot; means any plants e.g. trees, shrubs, grass</rdfs:comment>
        <rdfs:isDefinedBy rdf:resource="http://purl.oclc.org/NET/ssnx/cf/cf-property"/>
        <rdfs:label>vegetation carbon content</rdfs:label>
    </owl:NamedIndividual>
    


    <!-- http://purl.oclc.org/NET/ssnx/cf/cf-property#volume_fraction_of_clay_in_soil -->


    <owl:NamedIndividual rdf:about="http://purl.oclc.org/NET/ssnx/cf/cf-property#volume_fraction_of_clay_in_soil">
        <rdf:type rdf:resource="http://purl.oclc.org/NET/ssnx/qu/dim#Dimensionless"/>
        <rdfs:comment>&quot;Volume fraction&quot; is used in the construction volume_fraction_of_X_in_Y, where X is a material constituent of Y</rdfs:comment>
        <rdfs:isDefinedBy rdf:resource="http://purl.oclc.org/NET/ssnx/cf/cf-property"/>
        <rdfs:label>volume fraction of clay in soil</rdfs:label>
    </owl:NamedIndividual>
    


    <!-- http://purl.oclc.org/NET/ssnx/cf/cf-property#volume_fraction_of_condensed_water_in_soil -->


    <owl:NamedIndividual rdf:about="http://purl.oclc.org/NET/ssnx/cf/cf-property#volume_fraction_of_condensed_water_in_soil">
        <rdf:type rdf:resource="http://purl.oclc.org/NET/ssnx/qu/dim#Dimensionless"/>
        <rdfs:comment>&quot;Condensed water&quot; means liquid and ice. &quot;Volume fraction&quot; is used in the construction volume_fraction_of_X_in_Y, where X is a material constituent of Y</rdfs:comment>
        <rdfs:isDefinedBy rdf:resource="http://purl.oclc.org/NET/ssnx/cf/cf-property"/>
        <rdfs:label>volume fraction of condensed water in soil</rdfs:label>
    </owl:NamedIndividual>
    


    <!-- http://purl.oclc.org/NET/ssnx/cf/cf-property#volume_fraction_of_condensed_water_in_soil_at_critical_point -->


    <owl:NamedIndividual rdf:about="http://purl.oclc.org/NET/ssnx/cf/cf-property#volume_fraction_of_condensed_water_in_soil_at_critical_point">
        <rdf:type rdf:resource="http://purl.oclc.org/NET/ssnx/qu/dim#Dimensionless"/>
        <rdfs:comment>&quot;Condensed water&quot; means liquid and ice. &quot;Volume fraction&quot; is used in the construction volume_fraction_of_X_in_Y, where X is a material constituent of Y.  When soil moisture equals or exceeds the critical point evapotranspiration takes place at the potential rate and is controlled by the ambient meteorological conditions (temperature, wind, relative humidity).  Evapotranspiration is the sum of evaporation and plant transpiration.  Potential evapotranspiration is the rate at which evapotranspiration would occur under ambient conditions from a uniformly vegetated area when the water supply is not limiting</rdfs:comment>
        <rdfs:isDefinedBy rdf:resource="http://purl.oclc.org/NET/ssnx/cf/cf-property"/>
        <rdfs:label>volume fraction of condensed water in soil at critical point</rdfs:label>
    </owl:NamedIndividual>
    


    <!-- http://purl.oclc.org/NET/ssnx/cf/cf-property#volume_fraction_of_condensed_water_in_soil_at_field_capacity -->


    <owl:NamedIndividual rdf:about="http://purl.oclc.org/NET/ssnx/cf/cf-property#volume_fraction_of_condensed_water_in_soil_at_field_capacity">
        <rdf:type rdf:resource="http://purl.oclc.org/NET/ssnx/qu/dim#Dimensionless"/>
        <rdfs:comment>&quot;Condensed water&quot; means liquid and ice. &quot;Volume fraction&quot; is used in the construction volume_fraction_of_X_in_Y, where X is a material constituent of Y. The field capacity of soil is the maximum content of water it can retain against gravitational drainage</rdfs:comment>
        <rdfs:isDefinedBy rdf:resource="http://purl.oclc.org/NET/ssnx/cf/cf-property"/>
        <rdfs:label>volume fraction of condensed water in soil at field capacity</rdfs:label>
    </owl:NamedIndividual>
    


    <!-- http://purl.oclc.org/NET/ssnx/cf/cf-property#volume_fraction_of_condensed_water_in_soil_at_wilting_point -->


    <owl:NamedIndividual rdf:about="http://purl.oclc.org/NET/ssnx/cf/cf-property#volume_fraction_of_condensed_water_in_soil_at_wilting_point">
        <rdf:type rdf:resource="http://purl.oclc.org/NET/ssnx/qu/dim#Dimensionless"/>
        <rdfs:comment>&quot;Condensed water&quot; means liquid and ice. &quot;Volume fraction&quot; is used in the construction volume_fraction_of_X_in_Y, where X is a material constituent of Y. The wilting point of soil is the water content below which plants cannot extract sufficient water to balance their loss through transpiration</rdfs:comment>
        <rdfs:isDefinedBy rdf:resource="http://purl.oclc.org/NET/ssnx/cf/cf-property"/>
        <rdfs:label>volume fraction of condensed water in soil at wilting point</rdfs:label>
    </owl:NamedIndividual>
    


    <!-- http://purl.oclc.org/NET/ssnx/cf/cf-property#volume_fraction_of_condensed_water_in_soil_pores -->


    <owl:NamedIndividual rdf:about="http://purl.oclc.org/NET/ssnx/cf/cf-property#volume_fraction_of_condensed_water_in_soil_pores">
        <rdf:type rdf:resource="http://purl.oclc.org/NET/ssnx/qu/dim#Dimensionless"/>
        <rdfs:comment>&quot;Volume fraction&quot; is used in the construction volume_fraction_of_X_in_Y, where X is a material constituent of Y.  &quot;Condensed water&quot; means liquid and ice.  &quot;Volume_fraction_of_condensed_water_in_soil_pores&quot; is the ratio of the volume of condensed water in soil pores to the volume of the pores themselves</rdfs:comment>
        <rdfs:isDefinedBy rdf:resource="http://purl.oclc.org/NET/ssnx/cf/cf-property"/>
        <rdfs:label>volume fraction of condensed water in soil pores</rdfs:label>
    </owl:NamedIndividual>
    


    <!-- http://purl.oclc.org/NET/ssnx/cf/cf-property#volume_fraction_of_frozen_water_in_soil -->


    <owl:NamedIndividual rdf:about="http://purl.oclc.org/NET/ssnx/cf/cf-property#volume_fraction_of_frozen_water_in_soil">
        <rdf:type rdf:resource="http://purl.oclc.org/NET/ssnx/qu/dim#Dimensionless"/>
        <rdfs:comment>&quot;frozen_water&quot; means ice. &quot;Volume fraction&quot; is used in the construction volume_fraction_of_X_in_Y, where X is a material constituent of Y</rdfs:comment>
        <rdfs:isDefinedBy rdf:resource="http://purl.oclc.org/NET/ssnx/cf/cf-property"/>
        <rdfs:label>volume fraction of frozen water in soil</rdfs:label>
    </owl:NamedIndividual>
    


    <!-- http://purl.oclc.org/NET/ssnx/cf/cf-property#volume_fraction_of_sand_in_soil -->


    <owl:NamedIndividual rdf:about="http://purl.oclc.org/NET/ssnx/cf/cf-property#volume_fraction_of_sand_in_soil">
        <rdf:type rdf:resource="http://purl.oclc.org/NET/ssnx/qu/dim#Dimensionless"/>
        <rdfs:comment>&quot;Volume fraction&quot; is used in the construction volume_fraction_of_X_in_Y, where X is a material constituent of Y</rdfs:comment>
        <rdfs:isDefinedBy rdf:resource="http://purl.oclc.org/NET/ssnx/cf/cf-property"/>
        <rdfs:label>volume fraction of sand in soil</rdfs:label>
    </owl:NamedIndividual>
    


    <!-- http://purl.oclc.org/NET/ssnx/cf/cf-property#volume_fraction_of_silt_in_soil -->


    <owl:NamedIndividual rdf:about="http://purl.oclc.org/NET/ssnx/cf/cf-property#volume_fraction_of_silt_in_soil">
        <rdf:type rdf:resource="http://purl.oclc.org/NET/ssnx/qu/dim#Dimensionless"/>
        <rdfs:comment>&quot;Volume fraction&quot; is used in the construction volume_fraction_of_X_in_Y, where X is a material constituent of Y</rdfs:comment>
        <rdfs:isDefinedBy rdf:resource="http://purl.oclc.org/NET/ssnx/cf/cf-property"/>
        <rdfs:label>volume fraction of silt in soil</rdfs:label>
    </owl:NamedIndividual>
    


    <!-- http://purl.oclc.org/NET/ssnx/cf/cf-property#water_evaporation_flux_from_soil -->


    <owl:NamedIndividual rdf:about="http://purl.oclc.org/NET/ssnx/cf/cf-property#water_evaporation_flux_from_soil">
        <rdf:type rdf:resource="http://purl.oclc.org/NET/ssnx/qu/dim#MassPerTimePerArea"/>
        <rdfs:comment>&quot;Water&quot; means water in all phases. Evaporation is the conversion of liquid or solid into vapor. (The conversion of solid alone into vapor is called &quot;sublimation&quot;.) In accordance with common usage in geophysical disciplines, &quot;flux&quot; implies per unit area, called &quot;flux density&quot; in physics</rdfs:comment>
        <rdfs:isDefinedBy rdf:resource="http://purl.oclc.org/NET/ssnx/cf/cf-property"/>
        <rdfs:label>water evaporation flux from soil</rdfs:label>
    </owl:NamedIndividual>
    


    <!-- http://purl.oclc.org/NET/ssnx/cf/cf-property#wind_speed -->


    <owl:NamedIndividual rdf:about="http://purl.oclc.org/NET/ssnx/cf/cf-property#wind_speed">
        <rdf:type rdf:resource="http://purl.oclc.org/NET/ssnx/qu/dim#VelocityOrSpeed"/>
        <rdfs:comment>Speed is the magnitude of velocity. Wind is defined as a two-dimensional (horizontal) air velocity vector, with no vertical component. (Vertical motion in the atmosphere has the standard name upward_air_velocity.) The wind speed is the magnitude of the wind velocity</rdfs:comment>
        <rdfs:isDefinedBy rdf:resource="http://purl.oclc.org/NET/ssnx/cf/cf-property"/>
        <rdfs:label>wind speed</rdfs:label>
    </owl:NamedIndividual>
    


    <!-- http://www.ontology-of-units-of-measure.org/resource/om-2/degreeCelsius -->


    <owl:NamedIndividual rdf:about="http://www.ontology-of-units-of-measure.org/resource/om-2/degreeCelsius">
        <rdf:type rdf:resource="https://saref.etsi.org/core/UnitOfMeasure"/>
        <rdfs:comment>The degree Celsius is a unit of temperature defined as 1 kelvin.</rdfs:comment>
        <rdfs:isDefinedBy rdf:resource="http://www.ontology-of-units-of-measure.org/resource/om-2/degreeCelsius"/>
        <rdfs:label xml:lang="en">degree Celsius</rdfs:label>
    </owl:NamedIndividual>
    


    <!-- http://www.ontology-of-units-of-measure.org/resource/om-2/millibar -->


    <owl:NamedIndividual rdf:about="http://www.ontology-of-units-of-measure.org/resource/om-2/millibar">
        <rdf:type rdf:resource="https://saref.etsi.org/core/UnitOfMeasure"/>
        <rdfs:comment>The millibar is a unit of pressure defined as 1.0e-3 bar.</rdfs:comment>
        <rdfs:isDefinedBy rdf:resource="http://www.ontology-of-units-of-measure.org/resource/om-2/millibar"/>
        <rdfs:label xml:lang="en">millibar</rdfs:label>
    </owl:NamedIndividual>
    


    <!-- http://www.ontology-of-units-of-measure.org/resource/om-2/millimetre -->


    <owl:NamedIndividual rdf:about="http://www.ontology-of-units-of-measure.org/resource/om-2/millimetre">
        <rdf:type rdf:resource="https://saref.etsi.org/core/UnitOfMeasure"/>
        <rdfs:comment>The millimetre is a unit of length defined as 1.0e-3 metre.</rdfs:comment>
        <rdfs:isDefinedBy rdf:resource="http://www.ontology-of-units-of-measure.org/resource/om-2/millimetre"/>
        <rdfs:label xml:lang="en">millimetre</rdfs:label>
    </owl:NamedIndividual>
    


    <!-- http://www.ontology-of-units-of-measure.org/resource/om-2/millivolt -->


    <owl:NamedIndividual rdf:about="http://www.ontology-of-units-of-measure.org/resource/om-2/millivolt">
        <rdf:type rdf:resource="https://saref.etsi.org/core/UnitOfMeasure"/>
        <rdfs:comment>The millivolt is a unit of Voltage</rdfs:comment>
        <rdfs:isDefinedBy rdf:resource="http://www.ontology-of-units-of-measure.org/resource/om-2/millivolt"/>
        <rdfs:label xml:lang="en">millivolt</rdfs:label>
    </owl:NamedIndividual>
    


    <!-- https://saref.etsi.org/saref4agri/AirTemperature -->


    <owl:NamedIndividual rdf:about="https://saref.etsi.org/saref4agri/AirTemperature">
        <rdf:type rdf:resource="https://saref.etsi.org/core/Temperature"/>
        <rdfs:comment>The degree or intensity of heat present in the air.</rdfs:comment>
        <rdfs:isDefinedBy rdf:resource="https://saref.etsi.org/saref4agri/"/>
        <rdfs:label xml:lang="en">Air temperature</rdfs:label>
    </owl:NamedIndividual>
    


    <!-- https://saref.etsi.org/saref4agri/AmbientHumidity -->


    <owl:NamedIndividual rdf:about="https://saref.etsi.org/saref4agri/AmbientHumidity">
        <rdf:type rdf:resource="https://saref.etsi.org/core/Humidity"/>
        <rdfs:comment>The amount of water vapour in the air.</rdfs:comment>
        <rdfs:isDefinedBy rdf:resource="https://saref.etsi.org/saref4agri/"/>
        <rdfs:label xml:lang="en">Ambient huidity</rdfs:label>
    </owl:NamedIndividual>
    


    <!-- https://saref.etsi.org/saref4agri/IrrigationWater -->


    <owl:NamedIndividual rdf:about="https://saref.etsi.org/saref4agri/IrrigationWater">
        <rdf:type rdf:resource="https://saref.etsi.org/core/Property"/>
        <rdfs:comment>The amount of water falling in the soil by irrigation methods.</rdfs:comment>
        <rdfs:isDefinedBy rdf:resource="https://saref.etsi.org/saref4agri/"/>
        <rdfs:label xml:lang="en">Irrigation water</rdfs:label>
    </owl:NamedIndividual>
    


    <!-- https://saref.etsi.org/saref4agri/PlantGrowthStage -->


    <owl:NamedIndividual rdf:about="https://saref.etsi.org/saref4agri/PlantGrowthStage">
        <rdf:type rdf:resource="https://saref.etsi.org/core/Property"/>
        <rdfs:comment>The level or stage of growth of the plant.</rdfs:comment>
        <rdfs:isDefinedBy rdf:resource="https://saref.etsi.org/saref4agri/"/>
        <rdfs:label xml:lang="en">Plant growth stage</rdfs:label>
    </owl:NamedIndividual>
    


    <!-- https://saref.etsi.org/saref4agri/Precipitation -->


    <owl:NamedIndividual rdf:about="https://saref.etsi.org/saref4agri/Precipitation">
        <rdf:type rdf:resource="https://saref.etsi.org/core/Property"/>
        <rdfs:comment>The amount of water falling in the soil by natural process (e.g. rain).</rdfs:comment>
        <rdfs:isDefinedBy rdf:resource="https://saref.etsi.org/saref4agri/"/>
        <rdfs:label xml:lang="en">Precipitation</rdfs:label>
    </owl:NamedIndividual>
    


    <!-- https://saref.etsi.org/saref4agri/SoilMoisture -->


    <owl:NamedIndividual rdf:about="https://saref.etsi.org/saref4agri/SoilMoisture">
        <rdf:type rdf:resource="https://saref.etsi.org/core/Property"/>
        <rdfs:comment>The amount of water or humidity contained in the soil.</rdfs:comment>
        <rdfs:isDefinedBy rdf:resource="https://saref.etsi.org/saref4agri/"/>
        <rdfs:label xml:lang="en">Soil moisture</rdfs:label>
    </owl:NamedIndividual>
    


    <!-- https://saref.etsi.org/saref4agri/SoilTemperature -->


    <owl:NamedIndividual rdf:about="https://saref.etsi.org/saref4agri/SoilTemperature">
        <rdf:type rdf:resource="https://saref.etsi.org/core/Temperature"/>
        <rdfs:comment>The degree or intensity of heat present in the soil.</rdfs:comment>
        <rdfs:isDefinedBy rdf:resource="https://saref.etsi.org/saref4agri/"/>
        <rdfs:label xml:lang="en">Soil temperature</rdfs:label>
    </owl:NamedIndividual>
</rdf:RDF>



<!-- Generated by the OWL API (version 5.1.18) https://github.com/owlcs/owlapi/ -->


