@prefix : <https://w3id.org/cybele/> .
@prefix qb: <http://purl.org/linked-data/cube#> .
@prefix dct: <http://purl.org/dc/terms/> .
@prefix owl: <http://www.w3.org/2002/07/owl#> .
@prefix rdf: <http://www.w3.org/1999/02/22-rdf-syntax-ns#> .
@prefix xml: <http://www.w3.org/XML/1998/namespace> .
@prefix xsd: <http://www.w3.org/2001/XMLSchema#> .
@prefix dcat: <http://www.w3.org/ns/dcat#> .
@prefix foaf: <http://xmlns.com/foaf/0.1/> .
@prefix prov: <http://www.w3.org/ns/prov#> .
@prefix rdfs: <http://www.w3.org/2000/01/rdf-schema#> .
@prefix skos: <http://www.w3.org/2004/02/skos/core#> .
@prefix stat: <http://data.europa.eu/m8g/> .
@prefix schema: <https://schema.org/> .
@prefix af-inspire:	<http://inspire.ec.europa.eu/schemas/af/3.0#> .
@prefix act-inspire:	<http://inspire.ec.europa.eu/schemas/act-core/3.0#> .
@prefix foodie: <http://foodie-cloud.com/model/foodie#> .
@prefix saref4agri: <https://w3id.org/def/saref4agri#> .
@prefix common: <http://portele.de/ont/inspire/baseInspire#> .
@prefix fiware: <https://smartdatamodels.org/> .
@prefix fiware-agrifood: <https://smartdatamodels.org/dataModel.Agrifood/> .
@prefix fiware-weather: <https://smartdatamodels.org/dataModel.Weather/> .
@prefix ngsi-ld: <https://uri.etsi.org/ngsi-ld/> .
@prefix iso19109: <http://def.seegrid.csiro.au/isotc211/iso19109/2005/feature#> .
@prefix iso19150-2: <http://def.seegrid.csiro.au/isotc211/iso19150/-2/2012/basic#> .
@prefix iso19103: <http://def.seegrid.csiro.au/isotc211/iso19103/2005/basic#> .
@prefix geo:   <http://www.opengis.net/ont/geosparql#> .
@prefix ssn: <http://www.w3.org/ns/ssn/> .
@prefix sosa: <http://www.w3.org/ns/sosa/> .
@prefix saref: <https://w3id.org/saref#> .
@base <https://w3id.org/demeter/> .

<https://w3id.org/demeter/agri/agriAlert> a owl:Ontology ;
                            owl:versionIRI <https://w3id.org/demeter/agri/agriAlert/2.0> ;
                            dct:contributor [ schema:affiliation [ foaf:name "OGC"
                                                                 ] ;
                                              foaf:name "Rob Atkinson"
                                            ] ,
                                            [ schema:affiliation [ foaf:name "ICCS"
                                                                 ] ;
                                              foaf:name "Ioanna Roussaki"
                                            ] ;
                            dct:creator [ schema:affiliation [ foaf:name "PSNC"
                                                             ] ;
                                          rdfs:seeAlso <http://orcid.org/0000-0003-4289-4922> ;
                                          foaf:name "Raul Palma"
                                        ] ;
                            owl:imports <https://w3id.org/demeter/agri/agriCommon> ;
                            dct:description "The DEMETER AgriAlert is one of the agri profiles of DEMETER AIM. This profile was created by reusing and aligning well-known ontologies and vocabularies"@en ;
                            dct:rights "This vocabulary is distributed under Creative Commons Attribution 4.0 License - http://creativecommons.org/licenses/by/4.0"@en ;
                            dct:title "DEMETER AgriAlert"@en ;
                            rdfs:label "DEMETER AgriAlert" ;
                            rdfs:comment "The DEMETER Agriculture Information Model (AIM) is the common vocabulary in DEMETER project providing the basis for semantic interoperability across smart farming solutions"@en ;
                            owl:versionInfo "2.0" ;
                            foaf:maker [ foaf:homepage <https://h2020-demeter.eu/> ;
                                         foaf:name "DEMETER project"
                                       ] .

#################################################################
#    Annotation properties
#################################################################


#################################################################
#    Datatypes
#################################################################


#################################################################
#    Object Properties
#################################################################

###  http://foodie-cloud.com/model/foodie#alertGeometry
foodie:alertGeometry  a  owl:ObjectProperty ;
        rdfs:range      geo:Geometry ;
        skos:prefLabel  "alertGeometry"@en ;
        rdfs:label "alertGeometry" ;
        rdfs:comment "A relation between Geometry entity and Alert" ;
        rdfs:isDefinedBy <http://foodie-cloud.com/model/foodie> .

###  http://foodie-cloud.com/model/foodie#plotAlert
foodie:plotAlert
				a owl:ObjectProperty ;
        rdfs:range      foodie:Alert ;
        skos:prefLabel  "plotAlert"@en ;
        rdfs:label "plotAlert" ;
        rdfs:comment "A relation from Plot to Alert" ;
        rdfs:isDefinedBy <http://foodie-cloud.com/model/foodie> .

###  http://foodie-cloud.com/model/foodie#alertPlot
foodie:alertPlot  a     owl:ObjectProperty ;
        rdfs:range      foodie:Plot ;
        owl:inverseOf   foodie:plotAlert ;
        skos:prefLabel  "alertPlot"@en ;
        rdfs:label "plotAlert" ;
        rdfs:comment "A relation inverse of plotAlert directing from Alert to Plot class" ;
        rdfs:isDefinedBy <http://foodie-cloud.com/model/foodie> .

###  http://foodie-cloud.com/model/foodie#speciesAlert
foodie:speciesAlert  a  owl:ObjectProperty ;
        rdfs:range      foodie:Alert ;
        skos:prefLabel  "speciesAlert"@en ;
        rdfs:label "plotAlert" ;
        rdfs:comment "A relation inverse of plotAlert directing from Alert to Plot class" ;
        rdfs:isDefinedBy <http://foodie-cloud.com/model/foodie> .

###  http://foodie-cloud.com/model/foodie#alertSpecies
foodie:alertSpecies  a  owl:ObjectProperty ;
        rdfs:range      foodie:CropSpecies ;
        owl:inverseOf   foodie:speciesAlert ;
        skos:prefLabel  "alertSpecies"@en ;
        rdfs:label "alertSpecies" ;
        rdfs:comment "A relation between crop species and alert." ;
        rdfs:isDefinedBy <http://foodie-cloud.com/model/foodie> .

###  http://foodie-cloud.com/model/foodie#alertZone
foodie:alertZone  a     owl:ObjectProperty ;
        rdfs:range      foodie:ManagementZone ;
        owl:inverseOf   foodie:zoneAlert ;
        skos:prefLabel  "alertZone"@en ;
        rdfs:label "alertSpecies" ;
        rdfs:comment "A relation between management zone and alert." ;
        rdfs:isDefinedBy <http://foodie-cloud.com/model/foodie> .

###  http://foodie-cloud.com/model/foodie#zoneAlert
foodie:zoneAlert  a     owl:ObjectProperty ;
        rdfs:range      foodie:Alert ;
        skos:prefLabel  "zoneAlert"@en ;
        rdfs:label "zoneAlert" ;
        rdfs:comment "A relation between management zone and alert, inverse of alertZone" ;
        rdfs:isDefinedBy <http://foodie-cloud.com/model/foodie> .

#################################################################
#    Data properties
#################################################################

###  http://foodie-cloud.com/model/foodie#alertDate
foodie:alertDate  a     owl:DatatypeProperty ;
        rdfs:range      xsd:dateTime ;
        skos:prefLabel  "alertDate"@en ;
         rdfs:label "alertDate" ;
        rdfs:comment "The date/time of the generated alert" ;
        rdfs:isDefinedBy <http://foodie-cloud.com/model/foodie> .

### https://smartdatamodels.org/dataModel.Weather/subCategory
fiware-weather:subCategory	a      owl:DatatypeProperty ;
        rdfs:label   		"subCategory"@en ;
        rdfs:comment		"Describe the sub category of alert" ;
        rdfs:isDefinedBy <https://github.com/smart-data-models/dataModel.Weather/blob/master/WeatherAlert/schema.json> .

### https://smartdatamodels.org/address
fiware:address	a      owl:DatatypeProperty ;
        rdfs:label   		"address"@en ;
        rdfs:comment		"Civic address of Alert" ;
        rdfs:isDefinedBy <https://github.com/smart-data-models/dataModel.Agrifood/blob/master/AgriApp/schemaDTDL.json> .

### https://smartdatamodels.org/dataModel.Weather/dateIssued
fiware-weather:dateIssued	a      owl:DatatypeProperty ;
        rdfs:range      xsd:dateTime ;
        rdfs:label   		"dateIssued"@en ;
        rdfs:comment		"The date and time the forecast was issued by the meteorological bureau in ISO8601 UTC format" ;
        rdfs:isDefinedBy <https://github.com/smart-data-models/dataModel.Weather/blob/master/WeatherForecast/schemaDTDL.json> .

### https://smartdatamodels.org/dataModel.Weather/validFrom
fiware-weather:validFrom	a      owl:DatatypeProperty ;
        rdfs:range      xsd:dateTime ;
        rdfs:label   		"validFrom"@en ;
        rdfs:comment		"The start date of validity of the alert in ISO8601 UTC format." ;
        rdfs:isDefinedBy <https://github.com/smart-data-models/dataModel.Weather/blob/master/WeatherForecast/schemaDTDL.json> .

### https://smartdatamodels.org/dataModel.Weather/validTo
fiware-weather:validTo	a      owl:DatatypeProperty ;
        rdfs:range      xsd:dateTime ;
        rdfs:label   		"validTo"@en ;
        rdfs:comment		"The end date of validity of the alert in ISO8601 UTC format." ;
        rdfs:isDefinedBy <https://github.com/smart-data-models/dataModel.Weather/blob/master/WeatherForecast/schemaDTDL.json> .

### https://smartdatamodels.org/dataModel.Weather/alertSource
fiware-weather:alertSource	a      owl:DatatypeProperty ;
        rdfs:label   		"alertSource"@en ;
        rdfs:comment		"reference to the source of the alert. For example, it could be a user of an application, a device, or a service" ;
        rdfs:isDefinedBy <https://github.com/smart-data-models/dataModel.Weather/blob/master/WeatherAlert/schema.json> .

### https://uri.etsi.org/ngsi-ld/data
ngsi-ld:data	a      owl:DatatypeProperty ;
        rdfs:label   		"data"@en ;
        rdfs:comment		"used to carry additional data for the alert." ;
        rdfs:isDefinedBy <https://uri.etsi.org/ngsi-ld/v1/ngsi-ld-core-context-v1.6.jsonld> .

### https://smartdatamodels.org/dataModel.Weather/severity
fiware-weather:severity	a      owl:DatatypeProperty ;
        rdfs:label   		"severity"@en ;
        rdfs:comment		"define the level of gravity of a given alert" ;
        rdfs:isDefinedBy <https://smart-data-models.github.io/data-models/terms.jsonld#/definitions/severity> .

#################################################################
#    Classes
#################################################################

### http://foodie-cloud.com/model/foodie#Alert
foodie:Alert  a          owl:Class ;
        rdfs:subClassOf  geo:Feature ;
        rdfs:subClassOf  [ a                   owl:Restriction ;
                           owl:minCardinality  "1"^^xsd:int ;
                           owl:onProperty      foodie:alertGeometry
                         ] ;
        rdfs:subClassOf  [ a                owl:Restriction ;
                           owl:cardinality  "1"^^xsd:int ;
                           owl:onProperty   foodie:code
                         ] ;
        rdfs:subClassOf  [ a                owl:Restriction ;
                           owl:cardinality  "1"^^xsd:int ;
                           owl:onProperty   foodie:alertDate
                         ] ;
        rdfs:subClassOf  [ a                   owl:Restriction ;
                           owl:minCardinality  "1"^^xsd:int ;
                           owl:onProperty      foodie:type
                         ] ;
        rdfs:subClassOf  [ a                   owl:Restriction ;
                           owl:maxCardinality  "1"^^xsd:int ;
                           owl:onProperty      foodie:description
                         ] ;
        skos:prefLabel   "Alert"@en ;
        rdfs:isDefinedBy <http://foodie-cloud.com/model/foodie> .

### https://smartdatamodels.org/dataModel.Weather/WeatherAlert
fiware-weather:Alert	a owl:Class ;
			rdfs:label "Alert" ;
			rdfs:comment "This entity models an alert and could be used to send alerts related to traffic jam, accidents, weather conditions, high level of pollutants and so on. The purpose of the model is to support the generation of notifications for a user or trigger other actions, based on such alerts. An alert is generated by a specific situation. The main features of an alert is that it is not predictable and it is not a recurrent data. That means that an alert could be an accident or a high level of pollutants measure, additionally it could be the fall down of a patient or a car driving in the opposite direction." ;
			rdfs:isDefinedBy <https://github.com/smart-data-models/dataModel.Weather/blob/master/WeatherAlert/schema.json> .

#################################################################
#    Alignments
#################################################################
foodie:Alert owl:equivalentClass fiware-weather:WeatherAlert .
fiware-weather:validFrom rdfs:subPropertyOf common:validFrom .
fiware-weather:validTo rdfs:subPropertyOf common:validTo .
foodie:alertGeometry rdfs:subPropertyOf geo:hasGeometry .


#################################################################
#    Individuals
#################################################################
