@prefix : <https://w3id.org/cybele/> .
@prefix qb: <http://purl.org/linked-data/cube#> .
@prefix dct: <http://purl.org/dc/terms/> .
@prefix owl: <http://www.w3.org/2002/07/owl#> .
@prefix rdf: <http://www.w3.org/1999/02/22-rdf-syntax-ns#> .
@prefix xml: <http://www.w3.org/XML/1998/namespace> .
@prefix xsd: <http://www.w3.org/2001/XMLSchema#> .
@prefix dcat: <http://www.w3.org/ns/dcat#> .
@prefix foaf: <http://xmlns.com/foaf/0.1/> .
@prefix prov: <http://www.w3.org/ns/prov#> .
@prefix rdfs: <http://www.w3.org/2000/01/rdf-schema#> .
@prefix skos: <http://www.w3.org/2004/02/skos/core#> .
@prefix stat: <http://data.europa.eu/m8g/> .
@prefix schema: <https://schema.org/> .
@prefix af-inspire:	<http://inspire.ec.europa.eu/schemas/af/3.0#> .
@prefix act-inspire:	<http://inspire.ec.europa.eu/schemas/act-core/3.0#> .
@prefix foodie: <http://foodie-cloud.com/model/foodie#> .
@prefix saref4agri: <https://w3id.org/def/saref4agri#> .
@prefix common: <http://portele.de/ont/inspire/baseInspire#> .
@prefix fiware: <https://smartdatamodels.org/> .
@prefix iso19109: <http://def.seegrid.csiro.au/isotc211/iso19109/2005/feature#> .
@prefix iso19150-2: <http://def.seegrid.csiro.au/isotc211/iso19150/-2/2012/basic#> .
@prefix geo:   <http://www.opengis.net/ont/geosparql#> .
@prefix ssn: <http://www.w3.org/ns/ssn/> .
@prefix sosa: <http://www.w3.org/ns/sosa/> .
@prefix saref: <https://w3id.org/saref#> .
@prefix cf-feature: <http://purl.oclc.org/NET/ssnx/cf/cf-feature#> .
@prefix quantity: <http://purl.oclc.org/NET/ssnx/qu/quantity#> .
@prefix cf: <http://purl.oclc.org/NET/ssnx/cf/cf-property#> .
@prefix qu: <http://purl.oclc.org/NET/ssnx/qu/qu#> .
@prefix dim: <http://purl.oclc.org/NET/ssnx/qu/dim#> .
@base <https://w3id.org/demeter/> .

<https://w3id.org/demeter/agri/agriSystem> a owl:Ontology ;
                            owl:versionIRI <https://w3id.org/demeter/agri/agriSystem/2.0> ;
                            dct:contributor [ schema:affiliation [ foaf:name "OGC"
                                                                 ] ;
                                              foaf:name "Rob Atkinson"
                                            ] ,
                                            [ schema:affiliation [ foaf:name "ICCS"
                                                                 ] ;
                                              foaf:name "Ioanna Roussaki"
                                            ] ,
                                            [ schema:affiliation [ foaf:name "ICCS"
                                                                 ] ;
                                              foaf:name "George Routis"
                                            ] ;
                            dct:creator [ schema:affiliation [ foaf:name "PSNC"
                                                             ] ;
                                          rdfs:seeAlso <http://orcid.org/0000-0003-4289-4922> ;
                                          foaf:name "Raul Palma"
                                        ] ;
                            owl:imports <https://w3id.org/demeter/agri/agriCommon> ;
                            dct:description "The DEMETER AgriSystem is one of the agri profiles of DEMETER AIM. This profile was created by reusing and aligning well-known ontologies and vocabularies"@en ;
                            dct:rights "This vocabulary is distributed under Creative Commons Attribution 4.0 License - http://creativecommons.org/licenses/by/4.0"@en ;
                            dct:title "DEMETER AgriSystem"@en ;
                            rdfs:label "DEMETER AgriSystem"@en ;
                            rdfs:comment "The DEMETER Agriculture Information Model (AIM) is the common vocabulary in DEMETER project providing the basis for semantic interoperability across smart farming solutions"@en ;
                            owl:versionInfo "2.0" ;
                            foaf:maker [ foaf:homepage <https://h2020-demeter.eu/> ;
                                         foaf:name "DEMETER project"
                                       ] .

#################################################################
#    Annotation properties
#################################################################


#################################################################
#    Datatypes
#################################################################


#################################################################
#    Object Properties
#################################################################



#################################################################
#    Data properties
#################################################################



#################################################################
#    Classes
#################################################################

###  https://w3id.org/saref#Device
<https://w3id.org/saref#Device> a owl:Class ;
                                rdfs:subClassOf <http://www.w3.org/ns/ssn/System> ;
                                rdfs:comment "A tangible object designed to accomplish a particular task in households, common public buildings or offices. In order to accomplish this task, the device performs one or more functions. For example, a washing machine is designed to wash (task) and to accomplish this task it performs a start and stop function. Devices can be structured in categories (subclasses) that reflect the different domain in which a device is used, e.g., smart appliances domain (subclass FunctionRelated) vs. building domain (subclass BuildingRelated) vs. smart grid domain (subclass EnergyRelated). New categories can be defined,if needed, to reflect other differences, for example different points of view, such as the point of view of the device's user vs. the point of view of the device's manufacturer. We propose a list of devices that are relevant for the purpose of SAREF, but this list can be extended" ;
                                rdfs:isDefinedBy <https://w3id.org/saref#> ;
                                rdfs:label "Device"@en .

###  https://w3id.org/saref#Sensor
<https://w3id.org/saref#Sensor> a owl:Class ;
                                rdfs:subClassOf <https://w3id.org/saref#Device> ;
                                rdfs:comment "A device that detects and responds to events or changes in the physical environment such as light, motion, or temperature changes. Further, a device of category saref:Sensor that performs a saref:SensingFunction." ;
                                rdfs:isDefinedBy <https://w3id.org/saref#> ;
                                rdfs:label "Sensor"@en .

###  https://w3id.org/saref#Actuator
<https://w3id.org/saref#Actuator> a owl:Class ;
                                  rdfs:subClassOf <https://w3id.org/saref#Device> ;
                                  rdfs:comment "A device responsible for moving or controlling a mechanism or system by performing an actuating function" ;
                                  rdfs:isDefinedBy <https://w3id.org/saref#> ;
                                  rdfs:label "Actuator"@en .

###  https://w3id.org/def/saref4agri#SoilTensiometer
saref4agri:SoilTensiometer a owl:Class ;
                 rdfs:subClassOf <https://w3id.org/saref#Sensor> ;
                 rdfs:comment "A sensor that measures the soil moisture."@en ;
                 rdfs:label "Soil tensiometer"@en ;
                 rdfs:isDefinedBy <https://w3id.org/def/saref4agri#> .


###  https://w3id.org/def/saref4agri#Thermometer
saref4agri:Thermometer a owl:Class ;
             rdfs:subClassOf <https://w3id.org/saref#Sensor> ;
             rdfs:label "Thermometer"@en ;
             rdfs:comment "A device that measures the temperature (e.g. soil temperature)." ;
             rdfs:isDefinedBy <https://w3id.org/def/saref4agri#> .


###  https://w3id.org/def/saref4agri#WateringGun
saref4agri:WateringGun a owl:Class ;
             rdfs:subClassOf <https://w3id.org/saref#Actuator> ;
             rdfs:comment "An actuator to irrigate an space."@en ;
             rdfs:label "Watering gun"@en ;
             rdfs:isDefinedBy <https://w3id.org/def/saref4agri#> .


###  https://w3id.org/def/saref4agri#WateringSystem
saref4agri:WateringSystem a owl:Class ;
                rdfs:subClassOf <http://www.w3.org/ns/ssn/System> ;
                rdfs:label "Watering system"@en ;
                rdfs:comment "Watering system" ;
                rdfs:isDefinedBy <https://w3id.org/def/saref4agri#> .


###  https://w3id.org/def/saref4agri#WateringValve
saref4agri:WateringValve a owl:Class ;
               rdfs:subClassOf <https://w3id.org/saref#Actuator> ;
               rdfs:label "Watering valve"@en ;
               rdfs:comment "Watering valve" ;
               rdfs:isDefinedBy <https://w3id.org/def/saref4agri#> .


###  https://w3id.org/def/saref4agri#WeatherStation
saref4agri:WeatherStation a owl:Class ;
                rdfs:subClassOf <http://www.w3.org/ns/ssn/System> ,
                                <https://w3id.org/saref#Sensor> ;
                rdfs:comment "A sensor or system that measure weather conditions."@en ;
                rdfs:label "Weather station"@en ;
                rdfs:isDefinedBy <https://w3id.org/def/saref4agri#> .

###  https://w3id.org/def/saref4agri#WeightSensor
saref4agri:WeightSensor a owl:Class ;
              rdfs:subClassOf <https://w3id.org/saref#Sensor> ;
              rdfs:label "Weight sensor"@en ;
              rdfs:comment "Weight sensor" ;
              rdfs:isDefinedBy <https://w3id.org/def/saref4agri#> .

###  https://w3id.org/def/saref4agri#Pluviometer
saref4agri:Pluviometer a owl:Class ;
             rdfs:subClassOf <https://w3id.org/saref#Sensor> ;
             rdfs:comment "A sensor that measures the rain fall."@en ;
             rdfs:label "Pluviometer"@en ;
             rdfs:isDefinedBy <https://w3id.org/def/saref4agri#> .

###  https://w3id.org/def/saref4agri#EatingActivitySensor
saref4agri:EatingActivitySensor a owl:Class ;
                      rdfs:subClassOf <https://w3id.org/saref#Sensor> ;
                      rdfs:label "Eating activity sensor"@en ;
                      rdfs:comment "Eating activity sensor" ;
                      rdfs:isDefinedBy <https://w3id.org/def/saref4agri#> .

###  https://w3id.org/def/saref4agri#MilkingSensor
saref4agri:MilkingSensor a owl:Class ;
               rdfs:subClassOf <https://w3id.org/saref#Sensor> ;
               rdfs:label "Milking sensor"@en ;
               rdfs:comment "Milking sensor" ;
               rdfs:isDefinedBy <https://w3id.org/def/saref4agri#> .

###  https://w3id.org/def/saref4agri#MovementActivitySensor
saref4agri:MovementActivitySensor a owl:Class ;
                        rdfs:subClassOf <https://w3id.org/saref#Sensor> ;
                        rdfs:label "Movement activity sensor"@en ;
                        rdfs:comment "Movement activity sensor" ;
                        rdfs:isDefinedBy <https://w3id.org/def/saref4agri#> .

### http://foodie-cloud.com/model/foodie#MachineType
foodie:MachineType  a       owl:Class ;
        rdfs:subClassOf  [ a                   owl:Restriction ;
                           owl:cardinality  "1"^^xsd:int ;
                           owl:onProperty      foodie:code
                         ] ;
        skos:prefLabel   "MachineType"@en ;
        rdfs:label "Machine type" ;
        rdfs:comment "Identification of a machine applying the agricultural treatment" ;
        rdfs:isDefinedBy <http://foodie-cloud.com/model/foodie> .

### http://foodie-cloud.com/model/foodie#TractorType
foodie:TractorType  a       owl:Class ;
        rdfs:subClassOf  [ a                   owl:Restriction ;
                           owl:cardinality  "1"^^xsd:int ;
                           owl:onProperty      foodie:code
                         ] ;
        skos:prefLabel   "TractorType"@en ;
        rdfs:label "Tractor type" ;
        rdfs:comment "identification of a tractive vehicle for the machine applying the agricultural treatment" ;
        rdfs:isDefinedBy <http://foodie-cloud.com/model/foodie> .



#################################################################
#    Alignments
#################################################################

foodie:MachineType rdfs:subClassOf sosa:Platform .
foodie:TractorType rdfs:subClassOf sosa:Platform .
saref:Sensor owl:equivalentClass sosa:Sensor .


#################################################################
#    Individuals
#################################################################
