@prefix : <https://w3id.org/cybele/> .
@prefix qb: <http://purl.org/linked-data/cube#> .
@prefix dct: <http://purl.org/dc/terms/> .
@prefix owl: <http://www.w3.org/2002/07/owl#> .
@prefix rdf: <http://www.w3.org/1999/02/22-rdf-syntax-ns#> .
@prefix xml: <http://www.w3.org/XML/1998/namespace> .
@prefix xsd: <http://www.w3.org/2001/XMLSchema#> .
@prefix dcat: <http://www.w3.org/ns/dcat#> .
@prefix foaf: <http://xmlns.com/foaf/0.1/> .
@prefix prov: <http://www.w3.org/ns/prov#> .
@prefix rdfs: <http://www.w3.org/2000/01/rdf-schema#> .
@prefix skos: <http://www.w3.org/2004/02/skos/core#> .
@prefix stat: <http://data.europa.eu/m8g/> .
@prefix schema: <https://schema.org/> .
@prefix af-inspire:	<http://inspire.ec.europa.eu/schemas/af/3.0#> .
@prefix act-inspire:	<http://inspire.ec.europa.eu/schemas/act-core/3.0#> .
@prefix foodie: <http://foodie-cloud.com/model/foodie#> .
@prefix saref4agri: <https://saref.etsi.org/saref4agri/> .
@prefix common: <http://portele.de/ont/inspire/baseInspire#> .
@prefix fiware: <https://smartdatamodels.org/> .
@prefix fiware-agrifood: <https://smartdatamodels.org/dataModel.Agrifood/> .
@prefix iso19109: <http://def.seegrid.csiro.au/isotc211/iso19109/2005/feature#> .
@prefix iso19150-2: <http://def.seegrid.csiro.au/isotc211/iso19150/-2/2012/basic#> .
@prefix iso19103: <http://def.seegrid.csiro.au/isotc211/iso19103/2005/basic#> .
@prefix iso19115-citation: <http://def.seegrid.csiro.au/isotc211/iso19115/2003/citation#> .
@prefix iso19108: <http://def.seegrid.csiro.au/isotc211/iso19108/2002/temporal#> .
@prefix geo:   <http://www.opengis.net/ont/geosparql#> .
@prefix ssn: <http://www.w3.org/ns/ssn/> .
@prefix sosa: <http://www.w3.org/ns/sosa/> .
@prefix saref: <https://saref.etsi.org/core/> .
@prefix obo: <http://purl.obolibrary.org/obo/> .
@base <https://w3id.org/demeter/> .

<https://w3id.org/demeter/agri/agriProduct> a owl:Ontology ;
                            owl:versionIRI <https://w3id.org/demeter/agri/agriProduct/3.0> ;
                            dct:contributor [ schema:affiliation [ foaf:name "OGC"
                                                                 ] ;
                                              foaf:name "Rob Atkinson"
                                            ] ,
                                            [ schema:affiliation [ foaf:name "ICCS"
                                                                 ] ;
                                              foaf:name "Ioanna Roussaki"
                                            ] ;
                            dct:creator [ schema:affiliation [ foaf:name "PSNC"
                                                             ] ;
                                          rdfs:seeAlso <http://orcid.org/0000-0003-4289-4922> ;
                                          foaf:name "Raul Palma"
                                        ] ;
                            owl:imports <https://w3id.org/demeter/agri/agriCommon> ;
                            dct:description "The DEMETER AgriProduct is one of the agri profiles of DEMETER AIM. This profile was created by reusing and aligning well-known ontologies and vocabularies"@en ;
                            dct:rights "This vocabulary is distributed under Creative Commons Attribution 4.0 License - http://creativecommons.org/licenses/by/4.0"@en ;
                            dct:title "DEMETER AgriProduct"@en ;
                            rdfs:label "DEMETER AgriProduct"@en ;
                            rdfs:comment "The DEMETER Agriculture Information Model (AIM) is the common vocabulary in DEMETER project providing the basis for semantic interoperability across smart farming solutions"@en ;
                            owl:versionInfo "3.0" ;
                            foaf:maker [ foaf:homepage <https://h2020-demeter.eu/> ;
                                         foaf:name "DEMETER project"
                                       ] .

#################################################################
#    Annotation properties
#################################################################


#################################################################
#    Datatypes
#################################################################


#################################################################
#    Object Properties
#################################################################

###  http://foodie-cloud.com/model/foodie#productKind
foodie:productKind  a   owl:ObjectProperty ;
        rdfs:range      foodie:ProductKindValue ;
        skos:prefLabel  "productKind"@en ;
        rdfs:label "productKind" ;
        rdfs:comment "Reference to the product kind value entity related to a product entity" ;
        rdfs:isDefinedBy <http://foodie-cloud.com/model/foodie> .

###  http://foodie-cloud.com/model/foodie#manufacturer
foodie:manufacturer  a  owl:ObjectProperty ;
        rdfs:range      iso19115-citation:ResponsibleParty ;
        skos:prefLabel  "manufacturer"@en ;
        rdfs:label "manufacturer" ;
        rdfs:comment "Reference to the responsible party entity related to a product entity defining the manufacturer relationship" ;
        rdfs:isDefinedBy <http://foodie-cloud.com/model/foodie> .

###  http://foodie-cloud.com/model/foodie#nutrient
foodie:nutrient  a      owl:ObjectProperty ;
        rdfs:range      foodie:ProductNutrients ;
        skos:prefLabel  "nutrient"@en ;
        rdfs:label "nutrient" ;
        rdfs:comment "Reference to the Product Nutrients entity related to a product entity" ;
        rdfs:isDefinedBy <http://foodie-cloud.com/model/foodie> .

###  http://foodie-cloud.com/model/foodie#nutrientProduct
foodie:nutrientProduct  a	owl:ObjectProperty ;
        rdfs:range      foodie:Product ;
        skos:prefLabel  "nutrientProduct"@en ;
        rdfs:label "nutrientProduct" ;
        rdfs:comment "Reference to the Product entity from  product nutrients entity" ;
        rdfs:isDefinedBy <http://foodie-cloud.com/model/foodie> .

###  http://foodie-cloud.com/model/foodie#solventQuantity
foodie:solventQuantity
        a               owl:ObjectProperty ;
        rdfs:range      iso19103:Measure ;
        skos:prefLabel  "solventQuantity"@en ;
        rdfs:label "solventQuantity" ;
        rdfs:comment "Reference to denote the quantity of measure (e.g. solvent) in the product prepartion entity" ;
        rdfs:isDefinedBy <http://foodie-cloud.com/model/foodie> .

###  http://foodie-cloud.com/model/foodie#safetyPeriod
foodie:safetyPeriod  a  owl:ObjectProperty ;
        rdfs:range      iso19108:Period ;
        skos:prefLabel  "safetyPeriod"@en ;
        rdfs:label "safetyPeriod" ;
        rdfs:comment "Reference to denote the time period for an element in the product prepartion entity" ;
        rdfs:isDefinedBy <http://foodie-cloud.com/model/foodie> .

###  http://foodie-cloud.com/model/foodie#productQuantity
foodie:productQuantity
        a               owl:ObjectProperty ;
        rdfs:range      iso19103:Measure ;
        skos:prefLabel  "productQuantity"@en ;
        rdfs:label "productQuantity" ;
        rdfs:comment "Reference to denote the measured quantity of an ingredient in the product prepartion entity" ;
        rdfs:isDefinedBy <http://foodie-cloud.com/model/foodie> .

###  http://foodie-cloud.com/model/foodie#ingredientAmount
foodie:ingredientAmount
        a               owl:ObjectProperty ;
        rdfs:range      iso19103:Measure ;
        skos:prefLabel  "ingredientAmount"@en ;
        rdfs:label "ingredientAmount" ;
        rdfs:comment "Reference to product nutrients entity to denote the measured amount of an specific ingredient" ;
        rdfs:isDefinedBy <http://foodie-cloud.com/model/foodie> .

###  http://foodie-cloud.com/model/foodie#nutrientAmount
foodie:nutrientAmount
        a               owl:ObjectProperty ;
        rdfs:range      iso19103:Measure ;
        skos:prefLabel  "nutrientAmount"@en ;
        rdfs:label "nutrientAmount" ;
        rdfs:comment "Reference to product nutrients entity to denote the measured amount of an specific nutrient" ;
        rdfs:isDefinedBy <http://foodie-cloud.com/model/foodie> .

### https://smartdatamodels.org/dataModel.Agrifood/hasAgriProductTypeParent
fiware-agrifood:hasAgriProductTypeParent	a	owl:ObjectProperty ;
        rdfs:label   		"hasAgriProductTypeParent"@en ;
        rdfs:comment		"Reference to the parent product type i.e. immediately above the entity in the hierarchy." ;
        rdfs:isDefinedBy <https://github.com/smart-data-models/dataModel.Agrifood/blob/master/AgriProductType/schema.json> .

### https://smartdatamodels.org/dataModel.Agrifood/hasAgriProductTypeChildren
fiware-agrifood:hasAgriProductTypeChildren	a	owl:ObjectProperty ;
        rdfs:label   		"hasAgriProductTypeChildren"@en ;
        rdfs:comment		"Reference to child product types i.e. immediately below this entity in the hierarchy." ;
        rdfs:isDefinedBy <https://github.com/smart-data-models/dataModel.Agrifood/blob/master/AgriProductType/schema.json> .

### https://smartdatamodels.org/dataModel.Agrifood/hasAgriProductType
fiware-agrifood:hasAgriProductType	a      owl:ObjectProperty ;
        rdfs:label   		"hasAgriProductType"@en ;
        rdfs:comment		"Reference to the AgriProductType used/ applied." ;
        rdfs:isDefinedBy <https://github.com/smart-data-models/dataModel.Agrifood/blob/master/AgriParcelOperation/schema.json> .

###  http://purl.obolibrary.org/obo/HANCESTRO_0308
obo:HANCESTRO_0308 a      owl:ObjectProperty ;
        rdfs:label "hasCountryOfOrigin" ;
        rdfs:comment "has country of origin" ;
        rdfs:isDefinedBy <http://purl.obolibrary.org/obo/> .

###  http://purl.obolibrary.org/obo/RO_0002473
obo:RO_0002473 a      owl:ObjectProperty ;
        rdfs:label "composedPrimarilyOf" ;
        rdfs:comment "composed_primarily_of y if and only if more than half of the mass of x is made from y or units of the same type as y" ;
        rdfs:isDefinedBy <http://purl.obolibrary.org/obo/> .

###  http://purl.obolibrary.org/obo/RO_0002180
obo:RO_0002180 a      owl:ObjectProperty ;
        rdfs:label "hasComponent" ;
        rdfs:comment "w 'has component' p if w 'has part' p and w is such that it can be directly disassembled into into n parts p, p2, p3, ..., pn, where these parts are of similar type." ;
        rdfs:isDefinedBy <http://purl.obolibrary.org/obo/> .

###  http://purl.obolibrary.org/obo/FOODON_00001301
obo:FOODON_00001301 a      owl:ObjectProperty ;
        rdfs:label "hasFoodSubstanceAnalog" ;
        rdfs:comment "has food substance analog" ;
        rdfs:isDefinedBy <http://purl.obolibrary.org/obo/> .

#################################################################
#    Data properties
#################################################################

###  http://foodie-cloud.com/model/foodie#productType
foodie:productType  a   owl:DatatypeProperty ;
        rdfs:range      xsd:string ;
        skos:prefLabel  "productType"@en ;
        rdfs:label "productType" ;
        rdfs:comment "Type of the Product, e.g. pesticide, as a free text. The types of Product vary from country to country as well as from farmer to farmer" ;
        rdfs:isDefinedBy <http://foodie-cloud.com/model/foodie> .

###  http://foodie-cloud.com/model/foodie#productSubType
foodie:productSubType
        a               owl:DatatypeProperty ;
        rdfs:range      xsd:string ;
        skos:prefLabel  "productSubType"@en ;
        rdfs:label "productSubType" ;
        rdfs:comment "More detailed classification of a type of the Product, e.g. biochemical insecticide, as a free text. The sub-types of Product vary from country to country as well as from farmer to farmer" ;
        rdfs:isDefinedBy <http://foodie-cloud.com/model/foodie> .

###  http://foodie-cloud.com/model/foodie#storageHandling
foodie:storageHandling
        a               owl:DatatypeProperty ;
        rdfs:range      xsd:string ;
        skos:prefLabel  "storageHandling"@en ;
        rdfs:label "storageHandling" ;
        rdfs:comment "The property defines the information on the safe storage of the Product" ;
        rdfs:isDefinedBy <http://foodie-cloud.com/model/foodie> .

###  http://foodie-cloud.com/model/foodie#productName
foodie:productName  a   owl:DatatypeProperty ;
        rdfs:range      xsd:string ;
        skos:prefLabel  "productName"@en ;
        rdfs:label "productName" ;
        rdfs:comment "The property defines the designation under which the Product is commonly known" ;
        rdfs:isDefinedBy <http://foodie-cloud.com/model/foodie> .

###  http://foodie-cloud.com/model/foodie#safetyInstructions
foodie:safetyInstructions
        a               owl:DatatypeProperty ;
        rdfs:range      xsd:string ;
        skos:prefLabel  "safetyInstructions"@en ;
        rdfs:label "safetyInstructions" ;
        rdfs:comment "The property defines the information on safe manipulation of the Product" ;
        rdfs:isDefinedBy <http://foodie-cloud.com/model/foodie> .

###  http://foodie-cloud.com/model/foodie#productCode
foodie:productCode  a   owl:DatatypeProperty ;
        rdfs:range      xsd:string ;
        skos:prefLabel  "productCode"@en ;
        rdfs:label "productCode" ;
        rdfs:comment "Indentifing code of a product. Unique identification of the Product." ;
        rdfs:isDefinedBy <http://foodie-cloud.com/model/foodie> .

###  http://foodie-cloud.com/model/foodie#registrationCode
foodie:registrationCode
        a               owl:DatatypeProperty ;
        rdfs:range      xsd:string ;
        skos:prefLabel  "registrationCode"@en ;
        rdfs:label "registrationCode" ;
        rdfs:comment "Indentifing the registration code of a product. Unique identification of a Product according to the national or any other relevant registration scheme." ;
        rdfs:isDefinedBy <http://foodie-cloud.com/model/foodie> .

###  http://foodie-cloud.com/model/foodie#registerUrl
foodie:registerUrl  a   owl:DatatypeProperty ;
        rdfs:range      xsd:anyURI ;
        skos:prefLabel  "registerUrl"@en ;
        rdfs:label "registerUrl" ;
        rdfs:comment "Link to the national or any other relevant register where the Product was registered" ;
        rdfs:isDefinedBy <http://foodie-cloud.com/model/foodie> .

###  http://foodie-cloud.com/model/foodie#ingredientName
foodie:ingredientName
        a               owl:DatatypeProperty ;
        rdfs:range      xsd:string ;
        skos:prefLabel  "ingredientName"@en ;
        rdfs:label "ingredientName" ;
        rdfs:comment "Designation under which the Ingredient is commonly known" ;
        rdfs:isDefinedBy <http://foodie-cloud.com/model/foodie> .

###  http://foodie-cloud.com/model/foodie#nutrientName
foodie:nutrientName  a  owl:DatatypeProperty ;
        rdfs:range      xsd:string ;
        skos:prefLabel  "nutrientName"@en ;
        rdfs:label "ingredientName" ;
        rdfs:comment "Designation under which the nutrient is commonly known" ;
        rdfs:isDefinedBy <http://foodie-cloud.com/model/foodie> .

###  http://foodie-cloud.com/model/foodie#nutrientMeasure
foodie:nutrientMeasure
        a               owl:DatatypeProperty ;
        rdfs:range      xsd:string ;
        skos:prefLabel  "nutrientMeasure"@en ;
        rdfs:label "nutrientMeasure" ;
        rdfs:comment "Textual description of a method for an estimation of the nutrient amount in the Product" ;
        rdfs:isDefinedBy <http://foodie-cloud.com/model/foodie> .

### https://smartdatamodels.org/dataModel.Agrifood/root
fiware-agrifood:root	a      owl:DatatypeProperty ;
        rdfs:label   		"root"@en ;
        rdfs:comment		"A logical indicator that this product is the root of an AgriProductType hierarchy. Logical true indicates it is the root." ;
        rdfs:isDefinedBy <https://github.com/smart-data-models/dataModel.Agrifood/blob/master/AgriProductType/schema.json> .


#################################################################
#    Classes
#################################################################

### http://foodie-cloud.com/model/foodie#Product
foodie:Product  a        owl:Class ;
        rdfs:subClassOf  geo:Feature ;
        rdfs:subClassOf  [ a                   owl:Restriction ;
                           owl:maxCardinality  "1"^^xsd:int ;
                           owl:onProperty      foodie:description
                         ] ;
        rdfs:subClassOf  [ a                owl:Restriction ;
                           owl:cardinality  "1"^^xsd:int ;
                           owl:onProperty   foodie:productKind
                         ] ;
        rdfs:subClassOf  [ a                   owl:Restriction ;
                           owl:maxCardinality  "1"^^xsd:int ;
                           owl:onProperty      foodie:price
                         ] ;
        rdfs:subClassOf  [ a                owl:Restriction ;
                           owl:cardinality  "1"^^xsd:int ;
                           owl:onProperty   foodie:productType
                         ] ;
        rdfs:subClassOf  [ a                   owl:Restriction ;
                           owl:maxCardinality  "1"^^xsd:int ;
                           owl:onProperty      foodie:storageHandling
                         ] ;
        rdfs:subClassOf  [ a                   owl:Restriction ;
                           owl:minCardinality  "1"^^xsd:int ;
                           owl:onProperty      foodie:productName
                         ] ;
        rdfs:subClassOf  [ a                   owl:Restriction ;
                           owl:maxCardinality  "1"^^xsd:int ;
                           owl:onProperty      foodie:safetyInstructions
                         ] ;
        rdfs:subClassOf  [ a                   owl:Restriction ;
                           owl:minCardinality  "1"^^xsd:int ;
                           owl:onProperty      foodie:manufacturer
                         ] ;
        skos:prefLabel   "Product"@en ;
        rdfs:label "Product" ;
        rdfs:comment "This entity defines a product" ;
        rdfs:isDefinedBy <http://foodie-cloud.com/model/foodie> .

### http://foodie-cloud.com/model/foodie#ProductPreparation
foodie:ProductPreparation
        a                owl:Class ;
        rdfs:subClassOf  geo:Feature ;
        rdfs:subClassOf  [ a                   owl:Restriction ;
                           owl:maxCardinality  "1"^^xsd:int ;
                           owl:onProperty      foodie:solventQuantity
                         ] ;
        rdfs:subClassOf  [ a                owl:Restriction ;
                           owl:cardinality  "1"^^xsd:int ;
                           owl:onProperty   foodie:safetyPeriod
                         ] ;
        rdfs:subClassOf  [ a                owl:Restriction ;
                           owl:cardinality  "1"^^xsd:int ;
                           owl:onProperty   foodie:productQuantity
                         ] ;
        skos:prefLabel   "ProductPreparation"@en ;
        rdfs:label "ProductPreparation" ;
        rdfs:comment "This entity defines the preparation of a product (e.g. quantities of the ingredients)" ;
        rdfs:isDefinedBy <http://foodie-cloud.com/model/foodie> .

### http://foodie-cloud.com/model/foodie#ActiveIngredients
foodie:ActiveIngredients
        a                owl:Class ;
        rdfs:subClassOf  [ a                owl:Restriction ;
                           owl:cardinality  "1"^^xsd:int ;
                           owl:onProperty   foodie:ingredientName
                         ] ;
        rdfs:subClassOf  [ a                   owl:Restriction ;
                           owl:maxCardinality  "1"^^xsd:int ;
                           owl:onProperty      foodie:ingredientAmount
                         ] ;
        rdfs:subClassOf  [ a                   owl:Restriction ;
                           owl:maxCardinality  "1"^^xsd:int ;
                           owl:onProperty      foodie:code
                         ] ;
        skos:prefLabel   "ActiveIngredients"@en ;
        rdfs:label "ActiveIngredients" ;
        rdfs:comment "This entity holds the information of the active ingredients (e.g. incredient name, ingredient code, ingredient amount) for a product" ;
        rdfs:isDefinedBy <http://foodie-cloud.com/model/foodie> .

### http://foodie-cloud.com/model/foodie#ProductNutrients
foodie:ProductNutrients
        a                owl:Class ;
        rdfs:subClassOf  geo:Feature ;
        rdfs:subClassOf  [ a                owl:Restriction ;
                           owl:cardinality  "1"^^xsd:int ;
                           owl:onProperty   foodie:nutrientName
                         ] ;
        rdfs:subClassOf  [ a                   owl:Restriction ;
                           owl:maxCardinality  "1"^^xsd:int ;
                           owl:onProperty      foodie:nutrientMeasure
                         ] ;
        rdfs:subClassOf  [ a                   owl:Restriction ;
                           owl:maxCardinality  "1"^^xsd:int ;
                           owl:onProperty      foodie:nutrientAmount
                         ] ;
        rdfs:subClassOf  [ a                   owl:Restriction ;
                           owl:cardinality  "1"^^xsd:int ;
                           owl:onProperty      foodie:nutrientProduct
                         ] ;
        skos:prefLabel   "ProductNutrients"@en ;
        rdfs:label "ProductNutrients" ;
        rdfs:comment "This entity holds the information of the nutrients (e.g. nutrient name, nutrient measure, nutrient amount) used for a product" ;
        rdfs:isDefinedBy <http://foodie-cloud.com/model/foodie> .

### http://foodie-cloud.com/model/foodie#ProductKindValue
foodie:ProductKindValue
        a                owl:Class ;
        rdfs:subClassOf  skos:Concept ;
        skos:prefLabel   "ProductKindValue"@en ;
        rdfs:label "ProductNutrients" ;
        rdfs:comment "This entity holds the information of the kind/type of product (e.g. oragnic, mineral) as codelist" ;
        rdfs:isDefinedBy <http://foodie-cloud.com/model/foodie> .

### https://uri.fiware.org/ns/data-models#AgriProductType
fiware-agrifood:AgriProductType	a owl:Class ;
			rdfs:label "AgriProductType" ;
			rdfs:comment "This entity contains a harmonised description of a generic agricultural product type. This entity is primarily associated with the agricultural vertical and related IoT applications. The AgriProductType includes a hierarchical structure that allows product types to be grouped in a flexible way." ;
			rdfs:isDefinedBy <https://github.com/smart-data-models/dataModel.Agrifood/blob/master/AgriProductType/schema.json> .

#################################################################
#    Alignments
#################################################################

foodie:Product owl:equivalentClass fiware-agrifood:AgriProductType .
foodie:productName rdfs:subPropertyOf fiware:name .
foodie:nutrientName rdfs:subPropertyOf fiware:name .
foodie:ingredientName rdfs:subPropertyOf fiware:name .
fiware-agrifood:hasAgriProductTypeParent rdfs:subPropertyOf fiware-agrifood:hasAgriProductType .
fiware-agrifood:hasAgriProductTypeChildren rdfs:subPropertyOf fiware-agrifood:hasAgriProductType .

#################################################################
#    Individuals
#################################################################
