@prefix : <https://w3id.org/demeter/> .
@prefix qb: <http://purl.org/linked-data/cube#> .
@prefix dct: <http://purl.org/dc/terms/> .
@prefix owl: <http://www.w3.org/2002/07/owl#> .
@prefix rdf: <http://www.w3.org/1999/02/22-rdf-syntax-ns#> .
@prefix xml: <http://www.w3.org/XML/1998/namespace> .
@prefix xsd: <http://www.w3.org/2001/XMLSchema#> .
@prefix dcat: <http://www.w3.org/ns/dcat#> .
@prefix foaf: <http://xmlns.com/foaf/0.1/> .
@prefix prov: <http://www.w3.org/ns/prov#> .
@prefix rdfs: <http://www.w3.org/2000/01/rdf-schema#> .
@prefix skos: <http://www.w3.org/2004/02/skos/core#> .
@prefix stat: <http://data.europa.eu/m8g/> .
@prefix schema: <https://schema.org/> .
@prefix af-inspire:	<http://inspire.ec.europa.eu/schemas/af/3.0#> .
@prefix act-inspire:	<http://inspire.ec.europa.eu/schemas/act-core/3.0#> .
@prefix foodie: <http://foodie-cloud.com/model/foodie#> .
@prefix saref4agri: <https://w3id.org/def/saref4agri#> .
@prefix common: <http://portele.de/ont/inspire/baseInspire#> .
@prefix fiware-agrifood: <https://smartdatamodels.org/dataModel.Agrifood/> .
@prefix fiware: <https://smartdatamodels.org/> .
@prefix iso19109: <http://def.seegrid.csiro.au/isotc211/iso19109/2005/feature#> .
@prefix iso19150-2: <http://def.seegrid.csiro.au/isotc211/iso19150/-2/2012/basic#> .
@prefix iso19103: <http://def.seegrid.csiro.au/isotc211/iso19103/2005/basic#> .
@prefix iso19115-citation: <http://def.seegrid.csiro.au/isotc211/iso19115/2003/citation#> .
@prefix geo:   <http://www.opengis.net/ont/geosparql#> .
@prefix ssn: <http://www.w3.org/ns/ssn/> .
@prefix sosa: <http://www.w3.org/ns/sosa/> .
@prefix saref: <https://w3id.org/saref#> .
@prefix obo: <http://purl.obolibrary.org/obo/> .
@prefix demeterAgriCommon: <https://w3id.org/demeter/agri/agriCommon#> .
@prefix qudt: <http://qudt.org/schema/qudt/> .
@prefix ecrop: <https://w3id.org/demeter/agri/ecrop/> .
@base <https://w3id.org/demeter/> .

<https://w3id.org/demeter/agri/agriCommon> a owl:Ontology ;
                            owl:versionIRI <https://w3id.org/demeter/agri/agriCommon/2.0> ;
                            dct:contributor [ schema:affiliation [ foaf:name "OGC"
                                                                 ] ;
                                              foaf:name "Rob Atkinson"
                                            ] ,
                                            [ schema:affiliation [ foaf:name "ICCS"
                                                                 ] ;
                                              foaf:name "Ioanna Roussaki"
                                            ] ;
                            dct:creator [ schema:affiliation [ foaf:name "PSNC"
                                                             ] ;
                                          rdfs:seeAlso <http://orcid.org/0000-0003-4289-4922> ;
                                          foaf:name "Raul Palma"
                                        ] ;
                            owl:imports <https://w3id.org/demeter/crossDomain> ;
                            dct:description "AgriCommon is one of the agri profiles of the Agriculture Information Model (AIM). This profile was created by reusing and aligning well-known ontologies and vocabularies"@en ;
                            dct:rights "This vocabulary is distributed under Creative Commons Attribution 4.0 License - http://creativecommons.org/licenses/by/4.0"@en ;
                            dct:title "AIM AgriCommon"@en ;
                            rdfs:label "AIM AgriCommon"@en ;
                            rdfs:comment "The Agriculture Information Model (AIM) is the common vocabulary in DEMETER project providing the basis for semantic interoperability across smart farming solutions"@en ;
                            owl:versionInfo "2.0" ;
                            foaf:maker [ foaf:homepage <https://h2020-demeter.eu/> ;
                                         foaf:name "DEMETER project"
                                       ] .

#################################################################
#    Annotation properties
#################################################################


###  http://purl.obolibrary.org/obo/TAXRANK_1000000
<http://purl.obolibrary.org/obo/TAXRANK_1000000> a owl:AnnotationProperty ;
                                                 rdfs:label "has_rank"@en ;
                                                 rdfs:comment "has rank annotation property from obo namespace taxonomic rank"@en ;
                                                 rdfs:isDefinedBy <http://purl.obolibrary.org/obo/> . 


#################################################################
#    Datatypes
#################################################################

#################################################################
#    Object Properties
#################################################################

###  https://w3id.org/def/saref4agri#managesFarm
saref4agri:managesFarm a owl:ObjectProperty ;
             rdfs:label "manages farm"@en ;
             rdfs:comment "manages farm"@en ;
             rdfs:isDefinedBy <https://w3id.org/def/saref4agri> .  

### https://smartdatamodels.org/dataModel.Agrifood/agroVocConcept
fiware-agrifood:agroVocConcept	a      owl:ObjectProperty ;
        rdfs:label   		"agroVocConcept"@en ;
        rdfs:comment		"The link with the defined concept into the AgroVoc vocabulary" ;
        rdfs:isDefinedBy <https://github.com/smart-data-models/dataModel.Agrifood/blob/master/AgriCrop/schema.json> .  

###  https://w3id.org/demeter/agri/agriCommon#eppoConcept
demeterAgriCommon:eppoConcept	a      owl:ObjectProperty ;
        rdfs:label   		"eppoConcept"@en ;
        rdfs:comment		"The link with the defined concept into the EPPO vocabulary" ;
        rdfs:isDefinedBy <https://w3id.org/demeter/agri/agriCommon#> .

###  https://w3id.org/demeter/agri/ecrop/contractBuyer
ecrop:contractBuyer a      owl:ObjectProperty ;
        rdfs:label "contractBuyer" ;
        rdfs:comment "The buyer party for an agricultural contract" ;
        rdfs:isDefinedBy <https://unece.org/fileadmin/DAM/cefact/brs/BRS_eCROP_v1.pdf> .

###  https://w3id.org/demeter/agri/ecrop/contractSeller
ecrop:contractSeller a      owl:ObjectProperty ;
        rdfs:label "contractSeller" ;
        rdfs:comment "The seller party for an agricultural contract" ;
        rdfs:isDefinedBy <https://unece.org/fileadmin/DAM/cefact/brs/BRS_eCROP_v1.pdf> .


#################################################################
#    Data properties
#################################################################

###  https://w3id.org/demeter/agri/agriCommon#userName
demeterAgriCommon:userName a owl:DatatypeProperty ;
         rdfs:range xsd:string ;
         rdfs:label "User Name" ;
         rdfs:comment "User Name" ;
         rdfs:isDefinedBy <https://w3id.org/demeter/agri/agriCommon#> .

###  https://w3id.org/demeter/agri/agriCommon#password
demeterAgriCommon:password a owl:DatatypeProperty ;
         rdfs:range xsd:string ;
         rdfs:label "Password" ;
         rdfs:comment "Password" ;
         rdfs:isDefinedBy <https://w3id.org/demeter/agri/agriCommon#> .

###  https://w3id.org/def/saref4agri#hasName
saref4agri:hasName a owl:DatatypeProperty ;
         rdfs:range xsd:string ;
         rdfs:comment "A relation to express the name of an entity (e.g.,animal)." ;
         rdfs:label "has name" ;
         rdfs:isDefinedBy <https://w3id.org/def/saref4agri> .  

###  https://w3id.org/saref#hasDescription
<https://w3id.org/saref#hasDescription> a owl:DatatypeProperty ;
                                        rdfs:range xsd:string ;
                                        rdfs:comment "A relationship providing a description of an entity (e.g., device)" ;
                                        rdfs:isDefinedBy <https://w3id.org/saref> ;
                                        rdfs:label "has description"@en .

###  https://w3id.org/saref#hasTimestamp
<https://w3id.org/saref#hasTimestamp> a owl:DatatypeProperty ;
                                      rdfs:range      xsd:dateTime ;  
                                      rdfs:comment "A relationship stating the timestamp of an entity (e.g. a measurement)" ;
                                      rdfs:isDefinedBy <https://w3id.org/saref> ;
                                      rdfs:label "has timestamp"@en .                                                           
				
###  http://foodie-cloud.com/model/foodie#code
foodie:code  a          owl:DatatypeProperty ;
        rdfs:range      xsd:string ;
        skos:prefLabel  "code"@en ;
        rdfs:label      "code" ;
        rdfs:comment    "Unique identification of an entity, e.g., ActiveIngredient" ;
        rdfs:isDefinedBy <http://foodie-cloud.com/model/foodie> .

###  http://foodie-cloud.com/model/foodie#description        
foodie:description  a   owl:DatatypeProperty ;
        rdfs:range      xsd:string ;
        skos:prefLabel  "description"@en ;
        rdfs:label      "description" ;
        rdfs:comment    "Any further information related to an entity that may help for a better understanding" ;
        rdfs:isDefinedBy <http://foodie-cloud.com/model/foodie> .

###  http://foodie-cloud.com/model/foodie#notes        
foodie:notes  a         owl:DatatypeProperty ;
        rdfs:range      xsd:string ;
        skos:prefLabel  "notes"@en ;
        rdfs:label      "notes" ;
        rdfs:comment    "Relation depicting additional information for a recource or entity" ;
        rdfs:isDefinedBy <http://foodie-cloud.com/model/foodie> .        

###  http://foodie-cloud.com/model/foodie#price                
foodie:price  a         owl:DatatypeProperty ;
        rdfs:range      xsd:string ;
        skos:prefLabel  "price"@en ;
        rdfs:label      "price" ;
        rdfs:comment    "Relation depicting price of a any resource e.g. Product, Treatment etc" ;
        rdfs:isDefinedBy <http://foodie-cloud.com/model/foodie> .
        
###  http://foodie-cloud.com/model/foodie#type        
foodie:type  a          owl:DatatypeProperty ;
        rdfs:range      xsd:string ;
        skos:prefLabel  "type"@en ;
        rdfs:label      "type" ;
        rdfs:comment    "Relation specifying the type of an enity, e.g., Intervention" ;
        rdfs:isDefinedBy <http://foodie-cloud.com/model/foodie> .
        				
###  <http://portele.de/ont/inspire/baseInspire#validFrom> 
common:validFrom	a      owl:DatatypeProperty ;
        rdfs:range       xsd:dateTime ;
        skos:prefLabel   "valid from"@en ;
        rdfs:label      "valid from" ;
        rdfs:comment    "begin of real-world phenomenon" ;
        rdfs:isDefinedBy <http://portele.de/ont/inspire/baseInspire#> .

###  <http://portele.de/ont/inspire/baseInspire#validTo> 
common:validTo	a        owl:DatatypeProperty ;
        rdfs:range       xsd:dateTime ;        
        skos:prefLabel   "valid to"@en ;
        rdfs:label       "valid to" ;
        rdfs:comment     "end of real-world phenomenon" ;
        rdfs:isDefinedBy <http://portele.de/ont/inspire/baseInspire#> .
        
### https://smartdatamodels.org/dateCreated
fiware:dateCreated	a      owl:DatatypeProperty ;
        rdfs:range      xsd:dateTime ;  
        rdfs:label   	"dateCreated"@en ;
        rdfs:comment	"Entity creation timestamp. This will usually be allocated by the storage platform" ;
        rdfs:isDefinedBy <https://github.com/smart-data-models/dataModel.Agrifood/blob/master/AgriApp/schemaDTDL.json> .

### https://smartdatamodels.org/dateModified
fiware:dateModified	a      owl:DatatypeProperty ;
        rdfs:range      xsd:dateTime ;  
        rdfs:label   	"dateModified"@en ;
        rdfs:comment	"Timestamp of the last modification of the entity. This will usually be allocated by the storage platform" ;
        rdfs:isDefinedBy <https://github.com/smart-data-models/dataModel.Agrifood/blob/master/AgriApp/schemaDTDL.json> .

### https://smartdatamodels.org/source
fiware:source	a      owl:DatatypeProperty ;
        rdfs:label   	"source"@en ;
        rdfs:comment	"A sequence of characters giving the original source of the entity data as a URL. Recommended to be the fully qualified domain name of the source provider, or the URL to the source object." ;
        rdfs:isDefinedBy <https://github.com/smart-data-models/dataModel.Agrifood/blob/master/AgriApp/schemaDTDL.json> .
                       
### https://smartdatamodels.org/dataProvider
fiware:dataProvider	a      owl:DatatypeProperty ;
        rdfs:label   	"dataProvider"@en ;
        rdfs:comment	"A sequence of characters identifying the provider of the harmonised data entity" ;
        rdfs:isDefinedBy <https://github.com/smart-data-models/dataModel.Agrifood/blob/master/AgriApp/schemaDTDL.json> .

### https://smartdatamodels.org/dataModel.Agrifood/version
fiware-agrifood:version	a      owl:DatatypeProperty ;
        rdfs:label   	"version"@en ;
        rdfs:comment	"The version of the App" ;
        rdfs:isDefinedBy <https://github.com/smart-data-models/dataModel.Agrifood/blob/master/AgriApp/schema.json> .

### https://smartdatamodels.org/name
fiware:name	a      owl:DatatypeProperty ;
        rdfs:label   	"name"@en ;
        rdfs:comment	"The name of this item" ;
        rdfs:isDefinedBy <https://github.com/smart-data-models/dataModel.Agrifood/blob/master/AgriApp/schemaDTDL.json> .
        
### https://smartdatamodels.org/alternateName
fiware:alternateName	a      owl:DatatypeProperty ;
        rdfs:label   	"alternateName"@en ;
        rdfs:comment	"An alternative name for this item" ;
        rdfs:isDefinedBy <https://github.com/smart-data-models/dataModel.Agrifood/blob/master/AgriApp/schemaDTDL.json> .
                
### https://smartdatamodels.org/dataModel.Agrifood/category
fiware-agrifood:category	a      owl:DatatypeProperty ;     
        rdfs:label   	"category"@en ;
        rdfs:comment	"The category of the entity, e.g., parcel of land e.g.: **arable, grassland, vineyard, orchard, mixed crop, lowland, upland, set-aside, forestry, wetland.**, alert (traffic, naturalDisaster, weather, environment, health, security, agriculture)." ;
        rdfs:isDefinedBy <https://github.com/smart-data-models/dataModel.Agrifood/blob/master/AgriParcel/schema.json> .                        

###  https://w3id.org/demeter/agri/agriCommon#imageURL
demeterAgriCommon:imageURL a owl:DatatypeProperty ;
        rdfs:subPropertyOf <https://schema.org/contentUrl> ;
        rdfs:range  xsd:anyURI ;
        rdfs:domain  demeterAgriCommon:Image ;
        rdfs:label "imageURL" ;
        rdfs:comment "Actual bytes of the image object, i.e., image file" ;
        rdfs:isDefinedBy <https://w3id.org/demeter/agri/agriCommon#> .

###  https://w3id.org/demeter/agri/agriCommon#imageHeight
demeterAgriCommon:imageHeight a owl:DatatypeProperty ;
        rdfs:subPropertyOf <https://schema.org/height> , saref:hasValue ;
        rdfs:domain  demeterAgriCommon:Image ;
        rdfs:label "imageHeight" ;
        rdfs:comment "The height of the image, e.g., 3 or 3 cm^^cdt:ucum" ;
        rdfs:isDefinedBy <https://w3id.org/demeter/agri/agriCommon#> .

###  https://w3id.org/demeter/agri/agriCommon#imageWidth
demeterAgriCommon:imageWidth a owl:DatatypeProperty ;
        rdfs:subPropertyOf <https://schema.org/width> , saref:hasValue ;   
        rdfs:domain  demeterAgriCommon:Image ;     
        rdfs:label "imageWidth" ;
        rdfs:comment "The width of the image, e.g., 3 or 3 cm^^cdt:ucum" ;
        rdfs:isDefinedBy <https://w3id.org/demeter/agri/agriCommon#> .

###  https://w3id.org/demeter/agri/agriCommon#imageDataType
demeterAgriCommon:imageDataType a owl:DatatypeProperty ;
        rdfs:domain  demeterAgriCommon:Image ;
        rdfs:label "imageDataType" ;
        rdfs:comment "The data type of the image, e.g., NDVI" ;
        rdfs:isDefinedBy <https://w3id.org/demeter/agri/agriCommon#> .        

###  https://w3id.org/demeter/agri/agriCommon#imageFormat
demeterAgriCommon:imageFormat a owl:DatatypeProperty ;
        rdfs:subPropertyOf <https://schema.org/encodingFormat> ;   
        rdfs:domain  demeterAgriCommon:Image ;     
        rdfs:label "imageFormat" ;
        rdfs:comment "The format of the image, e.g., tiff, jpg" ;
        rdfs:isDefinedBy <https://w3id.org/demeter/agri/agriCommon#> .

#################################################################
#    Classes
#################################################################
                                  
                                  
###  https://w3id.org/def/saref4agri#FarmHolding
saref4agri:FarmHolding a owl:Class ;
             rdfs:subClassOf <https://schema.org/Organization> ,
                             [ a owl:Restriction ;
                               owl:onProperty saref4agri:managesFarm ;
                               owl:someValuesFrom saref4agri:Farm
                             ] ,
                             [ a owl:Restriction ;
                               owl:onProperty saref4agri:hasName ;
                               owl:allValuesFrom xsd:string
                             ] ;
             rdfs:comment "A class to decsribe a saref4agri farm holding as subcass of an org:Organization" ;
             rdfs:label "Farm holding"@en ;
             rdfs:isDefinedBy <https://w3id.org/def/saref4agri> .


###  https://w3id.org/def/saref4agri#Farmer
saref4agri:Farmer a owl:Class ;
        rdfs:subClassOf <http://xmlns.com/foaf/0.1/Person> ,
                        [ a owl:Restriction ;
                          owl:onProperty saref4agri:managesFarm ;
                          owl:someValuesFrom saref4agri:Farm
                        ] ,
                        [ a owl:Restriction ;
                          owl:onProperty saref4agri:hasName ;
                          owl:allValuesFrom xsd:string
                        ] ;
        rdfs:comment "A class to decsribe a saref4agri farmer as subcass of a foaf:Person" ;
        rdfs:label "Farmer"@en ;
        rdfs:isDefinedBy <https://w3id.org/def/saref4agri> .

###  http://purl.obolibrary.org/obo/TAXRANK_0000000
<http://purl.obolibrary.org/obo/TAXRANK_0000000> a owl:Class ;
                                                 rdfs:label "taxonomic_rank"@en ;
                                                 rdfs:isDefinedBy <http://purl.obolibrary.org/obo/> .

###  https://w3id.org/demeter/agri/agriCommon#Image
demeterAgriCommon:Image a owl:Class ;
        rdfs:subClassOf <https://schema.org/ImageObject> ;
        rdfs:label "Image" ;
        rdfs:comment "An image object" ;
        rdfs:isDefinedBy <https://w3id.org/demeter/agri/agriCommon#> .

###  https://w3id.org/demeter/agri/ecrop/AgriculturalCertificate
ecrop:AgriculturalCertificate a owl:Class ;
        rdfs:label "AgriculturalCertificate" ;
        rdfs:comment "A legal proof of ownership, worthiness or qualification to operate an agricultural item" ;
        rdfs:isDefinedBy <https://unece.org/fileadmin/DAM/cefact/brs/BRS_eCROP_v1.pdf> .

###  https://w3id.org/demeter/agri/ecrop/AgriculturalContract
ecrop:AgriculturalCertificate a owl:Class ;
        rdfs:label "AgriculturalContract" ;
        rdfs:comment "The written or spoken contract between two or more parties for the expressed purpose of specifying the required agricultural produce, products or services" ;
        rdfs:isDefinedBy <https://unece.org/fileadmin/DAM/cefact/brs/BRS_eCROP_v1.pdf> .


#################################################################
#    Alignments
#################################################################

fiware:name rdfs:subPropertyOf schema:name .
saref4agri:hasName owl:equivalentProperty fiware:name .
fiware:alternateName rdfs:subPropertyOf fiware:name .
saref:hasDescription owl:equivalentProperty foodie:description .
prov:generatedAtTime rdfs:subPropertyOf saref:hasTimestamp .
fiware:dateCreated rdfs:subPropertyOf saref:hasTimestamp .
iso19115-citation:ResponsibleParty owl:equivalentClass foaf:Agent .
fiware-agrifood:category owl:equivalentProperty foodie:type .

#################################################################
#    Individuals
#################################################################

